_:genid1 <http://xmlns.com/foaf/0.1/homepage> <https://csiro.au> .
_:genid1 <http://xmlns.com/foaf/0.1/name> "Commonwealth Scientific and Industrial Research Organisation" .
_:genid2 <http://www.w3.org/1999/02/22-rdf-syntax-ns#type> <http://xmlns.com/foaf/0.1/Person> .
_:genid2 <http://schema.org/affiliation> _:genid1 .
_:genid2 <http://www.w3.org/2000/01/rdf-schema#seeAlso> <https://orcid.org/0000-0002-3884-3420> .
_:genid2 <http://xmlns.com/foaf/0.1/name> "Simon J D Cox" .
_:genid2 <http://xmlns.com/foaf/0.1/workInfoHomepage> <http://people.csiro.au/Simon-Cox> .
_:genid3 <http://schema.org/affiliation> <http://www.w3.org/data#W3C> .
_:genid3 <http://www.w3.org/2000/01/rdf-schema#seeAlso> <http://philarcher.org/foaf.rdf#me> .
_:genid3 <http://xmlns.com/foaf/0.1/homepage> <http://www.w3.org/People/all#phila> .
_:genid3 <http://xmlns.com/foaf/0.1/name> "Phil Archer" .
_:genid4 <http://xmlns.com/foaf/0.1/homepage> <http://ec.europa.eu/dgs/informatics/> .
_:genid4 <http://xmlns.com/foaf/0.1/name> "European Commission, DG DIGIT" .
_:genid5 <http://schema.org/affiliation> _:genid4 .
_:genid5 <http://xmlns.com/foaf/0.1/name> "Vassilios Peristeras" .
_:genid6 <http://xmlns.com/foaf/0.1/homepage> <http://okfn.org> .
_:genid6 <http://xmlns.com/foaf/0.1/name> "Open Knowledge Foundation" .
_:genid7 <http://schema.org/affiliation> _:genid6 .
_:genid7 <http://xmlns.com/foaf/0.1/name> "Rufus Pollock" .
_:genid8 <http://xmlns.com/foaf/0.1/homepage> <http://stfc.ac.uk> .
_:genid8 <http://xmlns.com/foaf/0.1/name> "Science and Technology Facilities Council, UK" .
_:genid9 <http://schema.org/affiliation> _:genid8 .
_:genid9 <http://www.w3.org/2000/01/rdf-schema#seeAlso> <https://orcid.org/0000-0003-3499-8262> .
_:genid9 <http://xmlns.com/foaf/0.1/homepage> <https://agbeltran.github.io> .
_:genid9 <http://xmlns.com/foaf/0.1/name> "Alejandra Gonzalez-Beltran" .
_:genid10 <http://xmlns.com/foaf/0.1/homepage> <http://www.refinitiv.com> .
_:genid10 <http://xmlns.com/foaf/0.1/name> "Refinitiv" .
_:genid11 <http://schema.org/affiliation> _:genid10 .
_:genid11 <http://xmlns.com/foaf/0.1/name> "David Browning" .
_:genid12 <http://www.w3.org/2000/01/rdf-schema#seeAlso> <http://makxdekkers.com/makxdekkers.rdf#me> .
_:genid12 <http://xmlns.com/foaf/0.1/homepage> <http://makxdekkers.com/> .
_:genid12 <http://xmlns.com/foaf/0.1/name> "Makx Dekkers" .
_:genid13 <http://www.w3.org/2000/01/rdf-schema#seeAlso> <http://www.eurecom.fr/~atemezin/gatemezing-foaf.rdf> .
_:genid13 <http://xmlns.com/foaf/0.1/name> "Ghislain Auguste Atemezing" .
_:genid14 <http://www.w3.org/2000/01/rdf-schema#seeAlso> <https://jakub.kl\u00EDmek.com/#me> .
_:genid14 <http://xmlns.com/foaf/0.1/homepage> <https://jakub.kl\u00EDmek.com/> .
_:genid14 <http://xmlns.com/foaf/0.1/name> "Jakub Kl\u00EDmek" .
_:genid15 <http://www.w3.org/2000/01/rdf-schema#seeAlso> <https://orcid.org/0000-0001-5648-2713> .
_:genid15 <http://xmlns.com/foaf/0.1/homepage> <http://www.imati.cnr.it/index.php/people/8-curricula/178-riccardo-albertoni> .
_:genid15 <http://xmlns.com/foaf/0.1/homepage> <https://w3id.org/people/ralbertoni/> .
_:genid15 <http://xmlns.com/foaf/0.1/name> "Riccardo Albertoni" .
_:genid16 <http://www.w3.org/2000/01/rdf-schema#seeAlso> <https://orcid.org/0000-0001-9300-2694> .
_:genid16 <http://xmlns.com/foaf/0.1/homepage> <http://www.andrea-perego.name/foaf/#me> .
_:genid16 <http://xmlns.com/foaf/0.1/name> "Andrea Perego" .
_:genid17 <http://xmlns.com/foaf/0.1/homepage> <http://www.asahi-net.or.jp/~ax2s-kmtn/> .
_:genid17 <http://xmlns.com/foaf/0.1/name> "Shuji Kamitsuna" .
_:genid18 <http://xmlns.com/foaf/0.1/name> "Boris Villaz\u00F3n-Terrazas" .
_:genid19 <http://xmlns.com/foaf/0.1/name> "Marios Meimaris" .
_:genid20 <http://xmlns.com/foaf/0.1/name> "Martin Alvarez-Espinar" .
_:genid21 <http://xmlns.com/foaf/0.1/name> "Richard Cyganiak" .
_:genid22 <http://www.w3.org/2000/01/rdf-schema#seeAlso> <http://fadmaa.me/foaf.ttl> .
_:genid22 <http://xmlns.com/foaf/0.1/name> "Fadi Maali" .
_:genid23 <http://xmlns.com/foaf/0.1/name> "John Erickson" .
_:genid24 <http://xmlns.com/foaf/0.1/homepage> <http://www.w3.org/2011/gld/> .
_:genid24 <http://xmlns.com/foaf/0.1/name> "Government Linked Data WG" .
<http://www.w3.org/ns/dcat> <http://www.w3.org/1999/02/22-rdf-syntax-ns#type> <http://www.w3.org/2002/07/owl#Ontology> .
<http://www.w3.org/ns/dcat> <http://purl.org/dc/terms/contributor> _:genid2 .
<http://www.w3.org/ns/dcat> <http://purl.org/dc/terms/contributor> _:genid3 .
<http://www.w3.org/ns/dcat> <http://purl.org/dc/terms/contributor> _:genid5 .
<http://www.w3.org/ns/dcat> <http://purl.org/dc/terms/contributor> _:genid7 .
<http://www.w3.org/ns/dcat> <http://purl.org/dc/terms/contributor> _:genid9 .
<http://www.w3.org/ns/dcat> <http://purl.org/dc/terms/contributor> _:genid11 .
<http://www.w3.org/ns/dcat> <http://purl.org/dc/terms/contributor> _:genid12 .
<http://www.w3.org/ns/dcat> <http://purl.org/dc/terms/contributor> _:genid13 .
<http://www.w3.org/ns/dcat> <http://purl.org/dc/terms/contributor> _:genid14 .
<http://www.w3.org/ns/dcat> <http://purl.org/dc/terms/contributor> _:genid15 .
<http://www.w3.org/ns/dcat> <http://purl.org/dc/terms/contributor> _:genid16 .
<http://www.w3.org/ns/dcat> <http://purl.org/dc/terms/contributor> _:genid17 .
<http://www.w3.org/ns/dcat> <http://purl.org/dc/terms/contributor> _:genid18 .
<http://www.w3.org/ns/dcat> <http://purl.org/dc/terms/contributor> _:genid19 .
<http://www.w3.org/ns/dcat> <http://purl.org/dc/terms/contributor> _:genid20 .
<http://www.w3.org/ns/dcat> <http://purl.org/dc/terms/contributor> _:genid21 .
<http://www.w3.org/ns/dcat> <http://purl.org/dc/terms/creator> _:genid22 .
<http://www.w3.org/ns/dcat> <http://purl.org/dc/terms/creator> _:genid23 .
<http://www.w3.org/ns/dcat> <http://purl.org/dc/terms/license> <https://creativecommons.org/licenses/by/4.0/> .
<http://www.w3.org/ns/dcat> <http://purl.org/dc/terms/modified> "2012-04-24"^^<http://www.w3.org/2001/XMLSchema#date> .
<http://www.w3.org/ns/dcat> <http://purl.org/dc/terms/modified> "2013-09-20"^^<http://www.w3.org/2001/XMLSchema#date> .
<http://www.w3.org/ns/dcat> <http://purl.org/dc/terms/modified> "2013-11-28"^^<http://www.w3.org/2001/XMLSchema#date> .
<http://www.w3.org/ns/dcat> <http://purl.org/dc/terms/modified> "2017-12-19"^^<http://www.w3.org/2001/XMLSchema#date> .
<http://www.w3.org/ns/dcat> <http://purl.org/dc/terms/modified> "2019" .
<http://www.w3.org/ns/dcat> <http://www.w3.org/2000/01/rdf-schema#comment> "DCAT es un vocabulario RDF dise\u00F1ado para facilitar la interoperabilidad entre cat\u00E1logos de datos publicados en la Web. Utilizando DCAT para describir datos disponibles en cat\u00E1logos se aumenta la posibilidad de que sean descubiertos y se permite que las aplicaciones consuman f\u00E1cilmente los metadatos de varios cat\u00E1logos."@es .
<http://www.w3.org/ns/dcat> <http://www.w3.org/2000/01/rdf-schema#comment> "DCAT est un vocabulaire d\u00E9velopp\u00E9 pour faciliter l'interop\u00E9rabilit\u00E9 entre les jeux de donn\u00E9es publi\u00E9es sur le Web. En utilisant DCAT pour d\u00E9crire les jeux de donn\u00E9es dans les catalogues de donn\u00E9es, les fournisseurs de donn\u00E9es augmentent leur d\u00E9couverte et permettent que les applications facilement les m\u00E9tadonn\u00E9es de plusieurs catalogues. Il permet en plus la publication d\u00E9centralis\u00E9e des catalogues et facilitent la recherche f\u00E9d\u00E9r\u00E9e des donn\u00E9es entre plusieurs sites. Les m\u00E9tadonn\u00E9es DCAT aggr\u00E9g\u00E9es peuvent servir comme un manifeste pour faciliter la pr\u00E9servation digitale des ressources. DCAT est d\u00E9finie \u00E0 l'adresse http://www.w3.org/TR/vocab-dcat/. Une quelconque version de ce document normatif et ce vocabulaire est une erreur dans ce vocabulaire."@fr .
<http://www.w3.org/ns/dcat> <http://www.w3.org/2000/01/rdf-schema#comment> "DCAT is an RDF vocabulary designed to facilitate interoperability between data catalogs published on the Web. By using DCAT to describe datasets in data catalogs, publishers increase discoverability and enable applications easily to consume metadata from multiple catalogs. It further enables decentralized publishing of catalogs and facilitates federated dataset search across sites. Aggregated DCAT metadata can serve as a manifest file to facilitate digital preservation. DCAT is defined at http://www.w3.org/TR/vocab-dcat/. Any variance between that normative document and this schema is an error in this schema."@en .
<http://www.w3.org/ns/dcat> <http://www.w3.org/2000/01/rdf-schema#comment> "DCAT je RDF slovn\u00EDk navr\u017Een\u00FD pro zprost\u0159edkov\u00E1n\u00ED interoperability mezi datov\u00FDmi katalogy publikovan\u00FDmi na Webu. Poskytovatel\u00E9 dat pou\u017E\u00EDv\u00E1n\u00EDm slovn\u00EDku DCAT pro popis datov\u00FDch sad v datov\u00FDch kataloz\u00EDch zvy\u0161uj\u00ED jejich dohledatelnost a umo\u017E\u0148uj\u00ED aplikac\u00EDm konzumovat metadata z v\u00EDce katalog\u016F. D\u00E1le je umo\u017E\u0148ena decentralizovan\u00E1 publikace katalog\u016F a federovan\u00E9 dotazov\u00E1n\u00ED na datov\u00E9 sady nap\u0159\u00ED\u010D katalogy. Agregovan\u00E1 DCAT metadata mohou tak\u00E9 slou\u017Eit jako pr\u016Fvodka umo\u017E\u0148uj\u00EDc\u00ED digit\u00E1ln\u00ED uchov\u00E1n\u00ED informace. DCAT je definov\u00E1n na http://www.w3.org/TR/vocab-dcat/. Jak\u00FDkoliv nesoulad mezi odkazovan\u00FDm dokumentem a t\u00EDmto sch\u00E9matem je chybou v tomto sch\u00E9matu."@cs .
<http://www.w3.org/ns/dcat> <http://www.w3.org/2000/01/rdf-schema#comment> "DCAT \u00E8 un vocabolario RDF progettato per facilitare l'interoperabilit\u00E0 tra i cataloghi di dati pubblicati nel Web. Utilizzando DCAT per descrivere i dataset nei cataloghi di dati, i fornitori migliorano la capacit\u00E0 di individuazione dei dati e abilitano le  applicazioni al consumo di dati provenienti da cataloghi differenti. DCAT permette di decentralizzare la pubblicazione di cataloghi e facilita la ricerca federata dei dataset. L'aggregazione dei metadati federati pu\u00F2 fungere da file manifesto per facilitare la conservazione digitale. DCAT \u00E8 definito all'indirizzo http://www.w3.org/TR/vocab-dcat/. Qualsiasi scostamento tra tale definizione normativa e questo schema \u00E8 da considerarsi un errore di questo schema."@it .
<http://www.w3.org/ns/dcat> <http://www.w3.org/2000/01/rdf-schema#comment> "DCAT\u306F\u3001\u30A6\u30A7\u30D6\u4E0A\u3067\u516C\u958B\u3055\u308C\u305F\u30C7\u30FC\u30BF\u30FB\u30AB\u30BF\u30ED\u30B0\u9593\u306E\u76F8\u4E92\u904B\u7528\u6027\u306E\u4FC3\u9032\u3092\u76EE\u7684\u3068\u3059\u308BRDF\u306E\u8A9E\u5F59\u3067\u3059\u3002\u3053\u306E\u30C9\u30AD\u30E5\u30E1\u30F3\u30C8\u3067\u306F\u3001\u305D\u306E\u5229\u7528\u306E\u305F\u3081\u306B\u3001\u30B9\u30AD\u30FC\u30DE\u3092\u5B9A\u7FA9\u3057\u3001\u4F8B\u3092\u63D0\u4F9B\u3057\u307E\u3059\u3002\u30C7\u30FC\u30BF\u30FB\u30AB\u30BF\u30ED\u30B0\u5185\u306E\u30C7\u30FC\u30BF\u30BB\u30C3\u30C8\u3092\u8A18\u8FF0\u3059\u308B\u305F\u3081\u306BDCAT\u3092\u7528\u3044\u308B\u3068\u3001\u516C\u958B\u8005\u304C\u3001\u767A\u898B\u53EF\u80FD\u6027\u3092\u5897\u52A0\u3055\u305B\u3001\u30A2\u30D7\u30EA\u30B1\u30FC\u30B7\u30E7\u30F3\u304C\u8907\u6570\u306E\u30AB\u30BF\u30ED\u30B0\u306E\u30E1\u30BF\u30C7\u30FC\u30BF\u3092\u5BB9\u6613\u306B\u5229\u7528\u3067\u304D\u308B\u3088\u3046\u306B\u306A\u308A\u307E\u3059\u3002\u3055\u3089\u306B\u3001\u30AB\u30BF\u30ED\u30B0\u306E\u5206\u6563\u516C\u958B\u3092\u53EF\u80FD\u306B\u3057\u3001\u8907\u6570\u306E\u30B5\u30A4\u30C8\u306B\u307E\u305F\u304C\u308B\u30C7\u30FC\u30BF\u30BB\u30C3\u30C8\u306E\u7D71\u5408\u691C\u7D22\u3092\u4FC3\u9032\u3057\u307E\u3059\u3002\u96C6\u7D04\u3055\u308C\u305FDCAT\u30E1\u30BF\u30C7\u30FC\u30BF\u306F\u3001\u30C7\u30A3\u30B8\u30BF\u30EB\u4FDD\u5B58\u3092\u4FC3\u9032\u3059\u308B\u305F\u3081\u306E\u30DE\u30CB\u30D5\u30A7\u30B9\u30C8\u30FB\u30D5\u30A1\u30A4\u30EB\u3068\u3057\u3066\u4F7F\u7528\u3067\u304D\u307E\u3059\u3002"@ja .
<http://www.w3.org/ns/dcat> <http://www.w3.org/2000/01/rdf-schema#comment> "\u03A4\u03BF DCAT \u03B5\u03AF\u03BD\u03B1\u03B9 \u03AD\u03BD\u03B1 RDF \u03BB\u03B5\u03BE\u03B9\u03BB\u03CC\u03B3\u03B9\u03BF \u03C0\u03BF\u03C5 \u03C3\u03C7\u03B5\u03B4\u03B9\u03AC\u03C3\u03B8\u03B7\u03BA\u03B5 \u03B3\u03B9\u03B1 \u03BD\u03B1 \u03BA\u03AC\u03BD\u03B5\u03B9 \u03B5\u03C6\u03B9\u03BA\u03C4\u03AE \u03C4\u03B7 \u03B4\u03B9\u03B1\u03BB\u03B5\u03B9\u03C4\u03BF\u03C5\u03C1\u03B3\u03B9\u03BA\u03CC\u03C4\u03B7\u03C4\u03B1 \u03BC\u03B5\u03C4\u03B1\u03BE\u03CD \u03BA\u03B1\u03C4\u03B1\u03BB\u03CC\u03B3\u03C9\u03BD \u03B4\u03B5\u03B4\u03BF\u03BC\u03AD\u03BD\u03C9\u03BD \u03C3\u03C4\u03BF\u03BD \u03A0\u03B1\u03B3\u03BA\u03CC\u03C3\u03BC\u03B9\u03BF \u0399\u03C3\u03C4\u03CC. \u03A7\u03C1\u03B7\u03C3\u03B9\u03BC\u03BF\u03C0\u03BF\u03B9\u03CE\u03BD\u03C4\u03B1\u03C2 \u03C4\u03BF DCAT \u03B3\u03B9\u03B1 \u03C4\u03B7\u03BD \u03C0\u03B5\u03C1\u03B9\u03B3\u03C1\u03B1\u03C6\u03AE \u03C3\u03C5\u03BD\u03CC\u03BB\u03C9\u03BD \u03B4\u03B5\u03B4\u03BF\u03BC\u03AD\u03BD\u03C9\u03BD, \u03BF\u03B9 \u03B5\u03BA\u03B4\u03CC\u03C4\u03B5\u03C2 \u03B1\u03C5\u03C4\u03CE\u03BD \u03B1\u03C5\u03BE\u03AC\u03BD\u03BF\u03C5\u03BD \u03C4\u03B7\u03BD \u03B1\u03BD\u03B1\u03BA\u03B1\u03BB\u03C5\u03C8\u03B9\u03BC\u03CC\u03C4\u03B7\u03C4\u03B1 \u03BA\u03B1\u03B9 \u03B5\u03C0\u03B9\u03C4\u03C1\u03AD\u03C0\u03BF\u03C5\u03BD \u03C3\u03C4\u03B9\u03C2 \u03B5\u03C6\u03B1\u03C1\u03BC\u03BF\u03B3\u03AD\u03C2 \u03C4\u03B7\u03BD \u03B5\u03CD\u03BA\u03BF\u03BB\u03B7 \u03BA\u03B1\u03C4\u03B1\u03BD\u03AC\u03BB\u03C9\u03C3\u03B7 \u03BC\u03B5\u03C4\u03B1\u03B4\u03B5\u03B4\u03BF\u03BC\u03AD\u03BD\u03C9\u03BD \u03B1\u03C0\u03CC \u03C0\u03BF\u03BB\u03BB\u03B1\u03C0\u03BB\u03BF\u03CD\u03C2 \u03BA\u03B1\u03C4\u03B1\u03BB\u03CC\u03B3\u03BF\u03C5\u03C2. \u0395\u03C0\u03B9\u03C0\u03BB\u03AD\u03BF\u03BD, \u03B4\u03AF\u03BD\u03B5\u03B9 \u03C4\u03B7 \u03B4\u03C5\u03BD\u03B1\u03C4\u03CC\u03C4\u03B7\u03C4\u03B1 \u03B3\u03B9\u03B1 \u03B1\u03C0\u03BF\u03BA\u03B5\u03BD\u03C4\u03C1\u03C9\u03BC\u03AD\u03BD\u03B7 \u03AD\u03BA\u03B4\u03BF\u03C3\u03B7 \u03BA\u03B1\u03B9 \u03B4\u03B9\u03AC\u03B8\u03B5\u03C3\u03B7 \u03BA\u03B1\u03C4\u03B1\u03BB\u03CC\u03B3\u03C9\u03BD \u03BA\u03B1\u03B9 \u03B5\u03C0\u03B9\u03C4\u03C1\u03AD\u03C0\u03B5\u03B9 \u03B4\u03C5\u03BD\u03B1\u03C4\u03CC\u03C4\u03B7\u03C4\u03B5\u03C2 \u03B5\u03BD\u03BF\u03C0\u03BF\u03B9\u03B7\u03BC\u03AD\u03BD\u03B7\u03C2 \u03B1\u03BD\u03B1\u03B6\u03AE\u03C4\u03B7\u03C3\u03B7\u03C2 \u03BC\u03B5\u03C4\u03B1\u03BE\u03CD \u03B4\u03B9\u03B1\u03C6\u03BF\u03C1\u03B5\u03C4\u03B9\u03BA\u03CE\u03BD \u03C0\u03B7\u03B3\u03CE\u03BD. \u03A3\u03C5\u03B3\u03BA\u03B5\u03BD\u03C4\u03C1\u03C9\u03C4\u03B9\u03BA\u03AC \u03BC\u03B5\u03C4\u03B1\u03B4\u03B5\u03B4\u03BF\u03BC\u03AD\u03BD\u03B1 \u03C0\u03BF\u03C5 \u03AD\u03C7\u03BF\u03C5\u03BD \u03C0\u03B5\u03C1\u03B9\u03B3\u03C1\u03B1\u03C6\u03B5\u03AF \u03BC\u03B5 \u03C4\u03BF DCAT \u03BC\u03C0\u03BF\u03C1\u03BF\u03CD\u03BD \u03BD\u03B1 \u03C7\u03C1\u03B7\u03C3\u03B9\u03BC\u03BF\u03C0\u03BF\u03B9\u03B7\u03B8\u03BF\u03CD\u03BD \u03C3\u03B1\u03BD \u03AD\u03BD\u03B1 \u03B4\u03B7\u03BB\u03C9\u03C4\u03B9\u03BA\u03CC \u03B1\u03C1\u03C7\u03B5\u03AF\u03BF (manifest file) \u03CE\u03C3\u03C4\u03B5 \u03BD\u03B1 \u03B4\u03B9\u03B5\u03C5\u03BA\u03BF\u03BB\u03CD\u03BD\u03BF\u03C5\u03BD \u03C4\u03B7\u03BD \u03C8\u03B7\u03C6\u03B9\u03B1\u03BA\u03AE \u03C3\u03C5\u03BD\u03C4\u03AE\u03C1\u03B7\u03C3\u03B7."@el .
<http://www.w3.org/ns/dcat> <http://www.w3.org/2000/01/rdf-schema#comment> "\u0647\u064A \u0623\u0646\u0637\u0648\u0644\u0648\u062C\u064A\u0629 \u062A\u0633\u0647\u0644 \u062A\u0628\u0627\u062F\u0644 \u0627\u0644\u0628\u064A\u0627\u0646\u0627\u062A \u0628\u064A\u0646 \u0645\u062E\u062A\u0644\u0641 \u0627\u0644\u0641\u0647\u0627\u0631\u0633 \u0639\u0644\u0649 \u0627\u0644\u0648\u0628. \u0627\u0633\u062A\u062E\u062F\u0627\u0645 \u0647\u0630\u0647 \u0627\u0644\u0623\u0646\u0637\u0648\u0644\u0648\u062C\u064A\u0629 \u064A\u0633\u0627\u0639\u062F \u0639\u0644\u0649 \u0627\u0643\u062A\u0634\u0627\u0641 \u0642\u0648\u0627\u0626\u0645  \u0627\u0644\u0628\u064A\u0627\u0646\u0627\u062A \u0627\u0644\u0645\u0646\u0634\u0648\u0631\u0629 \u0639\u0644\u0649 \u0627\u0644\u0648\u0628 \u0648 \u064A\u0645\u0643\u0646 \u0627\u0644\u062A\u0637\u0628\u064A\u0642\u0627\u062A \u0627\u0644\u0645\u062E\u062A\u0644\u0641\u0629 \u0645\u0646 \u0627\u0644\u0627\u0633\u062A\u0641\u0627\u062F\u0629 \u0623\u062A\u0648\u0645\u0627\u062A\u064A\u0643\u064A\u0627 \u0645\u0646 \u0627\u0644\u0628\u064A\u0627\u0646\u0627\u062A \u0627\u0644\u0645\u062A\u0627\u062D\u0629 \u0645\u0646 \u0645\u062E\u062A\u0644\u0641 \u0627\u0644\u0641\u0647\u0627\u0631\u0633."@ar .
<http://www.w3.org/ns/dcat> <http://www.w3.org/2000/01/rdf-schema#label> "El vocabulario de cat\u00E1logo de datos"@es .
<http://www.w3.org/ns/dcat> <http://www.w3.org/2000/01/rdf-schema#label> "Il vocabolario del catalogo dei dati"@it .
<http://www.w3.org/ns/dcat> <http://www.w3.org/2000/01/rdf-schema#label> "Le vocabulaire des jeux de donn\u00E9es"@fr .
<http://www.w3.org/ns/dcat> <http://www.w3.org/2000/01/rdf-schema#label> "Slovn\u00EDk pro datov\u00E9 katalogy"@cs .
<http://www.w3.org/ns/dcat> <http://www.w3.org/2000/01/rdf-schema#label> "The data catalog vocabulary"@en .
<http://www.w3.org/ns/dcat> <http://www.w3.org/2000/01/rdf-schema#label> "\u03A4\u03BF \u03BB\u03B5\u03BE\u03B9\u03BB\u03CC\u03B3\u03B9\u03BF \u03C4\u03C9\u03BD \u03BA\u03B1\u03C4\u03B1\u03BB\u03CC\u03B3\u03C9\u03BD \u03B4\u03B5\u03B4\u03BF\u03BC\u03AD\u03BD\u03C9\u03BD"@el .
<http://www.w3.org/ns/dcat> <http://www.w3.org/2000/01/rdf-schema#label> "\u0623\u0646\u0637\u0648\u0644\u0648\u062C\u064A\u0629 \u0641\u0647\u0627\u0631\u0633 \u0642\u0648\u0627\u0626\u0645 \u0627\u0644\u0628\u064A\u0627\u0646\u0627\u062A"@ar .
<http://www.w3.org/ns/dcat> <http://www.w3.org/2000/01/rdf-schema#label> "\u30C7\u30FC\u30BF\u30FB\u30AB\u30BF\u30ED\u30B0\u8A9E\u5F59\uFF08DCAT\uFF09"@ja .
<http://www.w3.org/ns/dcat> <http://www.w3.org/2002/07/owl#imports> <http://purl.org/dc/terms/> .
<http://www.w3.org/ns/dcat> <http://www.w3.org/2002/07/owl#imports> <http://www.w3.org/2004/02/skos/core> .
<http://www.w3.org/ns/dcat> <http://www.w3.org/2002/07/owl#imports> <http://www.w3.org/ns/prov-o#> .
<http://www.w3.org/ns/dcat> <http://www.w3.org/2002/07/owl#versionInfo> "Esta es una copia del vocabulario DCAT v2.0 disponible en https://www.w3.org/ns/dcat.ttl"@es .
<http://www.w3.org/ns/dcat> <http://www.w3.org/2002/07/owl#versionInfo> "This is an updated copy of v2.0 of the DCAT vocabulary, taken from https://www.w3.org/ns/dcat.ttl"@en .
<http://www.w3.org/ns/dcat> <http://www.w3.org/2002/07/owl#versionInfo> "Questa \u00E8 una copia aggiornata del vocabolario DCAT v2.0 disponibile in https://www.w3.org/ns/dcat.ttl"@en .
<http://www.w3.org/ns/dcat> <http://www.w3.org/2002/07/owl#versionInfo> "Toto je aktualizovan\u00E1 kopie slovn\u00EDku DCAT verze 2.0, p\u0159evzat\u00E1 z https://www.w3.org/ns/dcat.ttl"@cs .
<http://www.w3.org/ns/dcat> <http://www.w3.org/2004/02/skos/core#editorialNote> "English language definitions updated in this revision in line with ED. Multilingual text unevenly updated."@en .
<http://www.w3.org/ns/dcat> <http://xmlns.com/foaf/0.1/maker> _:genid24 .
_:genid25 <http://www.w3.org/1999/02/22-rdf-syntax-ns#type> <http://www.w3.org/2002/07/owl#Restriction> .
_:genid25 <http://www.w3.org/2002/07/owl#allValuesFrom> <http://www.w3.org/ns/dcat#Resource> .
_:genid25 <http://www.w3.org/2002/07/owl#onProperty> <http://purl.org/dc/terms/hasPart> .
<http://www.w3.org/ns/dcat#Catalog> <http://www.w3.org/1999/02/22-rdf-syntax-ns#type> <http://www.w3.org/2000/01/rdf-schema#Class> .
<http://www.w3.org/ns/dcat#Catalog> <http://www.w3.org/1999/02/22-rdf-syntax-ns#type> <http://www.w3.org/2002/07/owl#Class> .
<http://www.w3.org/ns/dcat#Catalog> <http://www.w3.org/2000/01/rdf-schema#comment> "A curated collection of metadata about resources (e.g., datasets and data services in the context of a data catalog)."@en .
<http://www.w3.org/ns/dcat#Catalog> <http://www.w3.org/2000/01/rdf-schema#comment> "Una colecci\u00F3n curada de metadatos sobre recursos (por ejemplo, conjuntos de datos y servicios de datos en el contexto de un cat\u00E1logo de datos)."@es .
<http://www.w3.org/ns/dcat#Catalog> <http://www.w3.org/2000/01/rdf-schema#comment> "Una raccolta curata di metadati sulle risorse (ad es. sui dataset e relativi servizi nel contesto di cataloghi di dati)."@it .
<http://www.w3.org/ns/dcat#Catalog> <http://www.w3.org/2000/01/rdf-schema#comment> "Une collection \u00E9labor\u00E9e de m\u00E9tadonn\u00E9es sur les jeux de donn\u00E9es"@fr .
<http://www.w3.org/ns/dcat#Catalog> <http://www.w3.org/2000/01/rdf-schema#comment> "\u0158\u00EDzen\u00E1 kolekce metadat o datov\u00FDch sad\u00E1ch a datov\u00FDch slu\u017Eb\u00E1ch"@cs .
<http://www.w3.org/ns/dcat#Catalog> <http://www.w3.org/2000/01/rdf-schema#comment> "\u039C\u03B9\u03B1 \u03B5\u03C0\u03B9\u03BC\u03B5\u03BB\u03B7\u03BC\u03AD\u03BD\u03B7 \u03C3\u03C5\u03BB\u03BB\u03BF\u03B3\u03AE \u03BC\u03B5\u03C4\u03B1\u03B4\u03B5\u03B4\u03BF\u03BC\u03AD\u03BD\u03C9\u03BD \u03C0\u03B5\u03C1\u03AF \u03C3\u03C5\u03BD\u03CC\u03BB\u03C9\u03BD \u03B4\u03B5\u03B4\u03BF\u03BC\u03AD\u03BD\u03C9\u03BD"@el .
<http://www.w3.org/ns/dcat#Catalog> <http://www.w3.org/2000/01/rdf-schema#comment> "\u0645\u062C\u0645\u0648\u0639\u0629 \u0645\u0646 \u062A\u0648\u0635\u064A\u0641\u0627\u062A \u0642\u0648\u0627\u0626\u0645 \u0627\u0644\u0628\u064A\u0627\u0646\u0627\u062A"@ar .
<http://www.w3.org/ns/dcat#Catalog> <http://www.w3.org/2000/01/rdf-schema#comment> "\u30C7\u30FC\u30BF\u30FB\u30AB\u30BF\u30ED\u30B0\u306F\u3001\u30C7\u30FC\u30BF\u30BB\u30C3\u30C8\u306B\u95A2\u3059\u308B\u30AD\u30E5\u30EC\u30FC\u30C8\u3055\u308C\u305F\u30E1\u30BF\u30C7\u30FC\u30BF\u306E\u96C6\u5408\u3067\u3059\u3002"@ja .
<http://www.w3.org/ns/dcat#Catalog> <http://www.w3.org/2000/01/rdf-schema#isDefinedBy> <http://www.w3.org/TR/vocab-dcat/> .
<http://www.w3.org/ns/dcat#Catalog> <http://www.w3.org/2000/01/rdf-schema#label> "Catalog"@en .
<http://www.w3.org/ns/dcat#Catalog> <http://www.w3.org/2000/01/rdf-schema#label> "Catalogo"@it .
<http://www.w3.org/ns/dcat#Catalog> <http://www.w3.org/2000/01/rdf-schema#label> "Catalogue"@fr .
<http://www.w3.org/ns/dcat#Catalog> <http://www.w3.org/2000/01/rdf-schema#label> "Cat\u00E1logo"@es .
<http://www.w3.org/ns/dcat#Catalog> <http://www.w3.org/2000/01/rdf-schema#label> "Katalog"@cs .
<http://www.w3.org/ns/dcat#Catalog> <http://www.w3.org/2000/01/rdf-schema#label> "\u039A\u03B1\u03C4\u03AC\u03BB\u03BF\u03B3\u03BF\u03C2"@el .
<http://www.w3.org/ns/dcat#Catalog> <http://www.w3.org/2000/01/rdf-schema#label> "\u0641\u0647\u0631\u0633 \u0642\u0648\u0627\u0626\u0645 \u0627\u0644\u0628\u064A\u0627\u0646\u0627\u062A"@ar .
<http://www.w3.org/ns/dcat#Catalog> <http://www.w3.org/2000/01/rdf-schema#label> "\u30AB\u30BF\u30ED\u30B0"@ja .
<http://www.w3.org/ns/dcat#Catalog> <http://www.w3.org/2000/01/rdf-schema#subClassOf> <http://www.w3.org/ns/dcat#Dataset> .
<http://www.w3.org/ns/dcat#Catalog> <http://www.w3.org/2000/01/rdf-schema#subClassOf> _:genid25 .
<http://www.w3.org/ns/dcat#Catalog> <http://www.w3.org/2004/02/skos/core#definition> "A curated collection of metadata about resources (e.g., datasets and data services in the context of a data catalog)."@en .
<http://www.w3.org/ns/dcat#Catalog> <http://www.w3.org/2004/02/skos/core#definition> "Una colecci\u00F3n curada de metadatos sobre recursos (por ejemplo, conjuntos de datos y servicios de datos en el contexto de un cat\u00E1logo de datos)."@es .
<http://www.w3.org/ns/dcat#Catalog> <http://www.w3.org/2004/02/skos/core#definition> "Una raccolta curata di metadati sulle risorse (ad es. sui dataset e relativi servizi nel contesto di cataloghi di dati)."@it .
<http://www.w3.org/ns/dcat#Catalog> <http://www.w3.org/2004/02/skos/core#definition> "Une collection \u00E9labor\u00E9e de m\u00E9tadonn\u00E9es sur les jeux de donn\u00E9es."@fr .
<http://www.w3.org/ns/dcat#Catalog> <http://www.w3.org/2004/02/skos/core#definition> "\u0158\u00EDzen\u00E1 kolekce metadat o datov\u00FDch sad\u00E1ch a datov\u00FDch slu\u017Eb\u00E1ch."@cs .
<http://www.w3.org/ns/dcat#Catalog> <http://www.w3.org/2004/02/skos/core#definition> "\u039C\u03B9\u03B1 \u03B5\u03C0\u03B9\u03BC\u03B5\u03BB\u03B7\u03BC\u03AD\u03BD\u03B7 \u03C3\u03C5\u03BB\u03BB\u03BF\u03B3\u03AE \u03BC\u03B5\u03C4\u03B1\u03B4\u03B5\u03B4\u03BF\u03BC\u03AD\u03BD\u03C9\u03BD \u03C0\u03B5\u03C1\u03AF \u03C3\u03C5\u03BD\u03CC\u03BB\u03C9\u03BD \u03B4\u03B5\u03B4\u03BF\u03BC\u03AD\u03BD\u03C9\u03BD."@el .
<http://www.w3.org/ns/dcat#Catalog> <http://www.w3.org/2004/02/skos/core#definition> "\u0645\u062C\u0645\u0648\u0639\u0629 \u0645\u0646 \u062A\u0648\u0635\u064A\u0641\u0627\u062A \u0642\u0648\u0627\u0626\u0645 \u0627\u0644\u0628\u064A\u0627\u0646\u0627\u062A"@ar .
<http://www.w3.org/ns/dcat#Catalog> <http://www.w3.org/2004/02/skos/core#definition> "\u30C7\u30FC\u30BF\u30FB\u30AB\u30BF\u30ED\u30B0\u306F\u3001\u30C7\u30FC\u30BF\u30BB\u30C3\u30C8\u306B\u95A2\u3059\u308B\u30AD\u30E5\u30EC\u30FC\u30C8\u3055\u308C\u305F\u30E1\u30BF\u30C7\u30FC\u30BF\u306E\u96C6\u5408\u3067\u3059\u3002"@ja .
<http://www.w3.org/ns/dcat#Catalog> <http://www.w3.org/2004/02/skos/core#editorialNote> "English, Italian, Spanish definitions updated in this revision. Multilingual text not yet updated."@en .
<http://www.w3.org/ns/dcat#Catalog> <http://www.w3.org/2004/02/skos/core#scopeNote> "A web-based data catalog is typically represented as a single instance of this class."@en .
<http://www.w3.org/ns/dcat#Catalog> <http://www.w3.org/2004/02/skos/core#scopeNote> "Normalmente, un catalogo di dati nel web viene rappresentato come una singola istanza di questa classe."@it .
<http://www.w3.org/ns/dcat#Catalog> <http://www.w3.org/2004/02/skos/core#scopeNote> "Normalmente, un cat\u00E1logo de datos disponible en la web se representa como una \u00FAnica instancia de esta clase."@es .
<http://www.w3.org/ns/dcat#Catalog> <http://www.w3.org/2004/02/skos/core#scopeNote> "Webov\u00FD datov\u00FD katalog je typicky reprezentov\u00E1n jako jedna instance t\u00E9to t\u0159\u00EDdy."@cs .
<http://www.w3.org/ns/dcat#Catalog> <http://www.w3.org/2004/02/skos/core#scopeNote> "\u03A3\u03C5\u03BD\u03AE\u03B8\u03C9\u03C2, \u03AD\u03BD\u03B1\u03C2 \u03BA\u03B1\u03C4\u03AC\u03BB\u03BF\u03B3\u03BF\u03C2 \u03B4\u03B5\u03B4\u03BF\u03BC\u03AD\u03BD\u03C9\u03BD \u03C3\u03C4\u03BF\u03BD \u03A0\u03B1\u03B3\u03BA\u03CC\u03C3\u03BC\u03B9\u03BF \u0399\u03C3\u03C4\u03CC \u03B1\u03BD\u03B1\u03C0\u03B1\u03C1\u03AF\u03C3\u03C4\u03B1\u03C4\u03B1\u03B9 \u03C9\u03C2 \u03AD\u03BD\u03B1 \u03C3\u03C4\u03B9\u03B3\u03BC\u03B9\u03CC\u03C4\u03C5\u03C0\u03BF \u03B1\u03C5\u03C4\u03AE\u03C2 \u03C4\u03B7\u03C2 \u03BA\u03BB\u03AC\u03C3\u03B7\u03C2."@el .
<http://www.w3.org/ns/dcat#Catalog> <http://www.w3.org/2004/02/skos/core#scopeNote> "\u901A\u5E38\u3001\u30A6\u30A7\u30D6\u30FB\u30D9\u30FC\u30B9\u306E\u30C7\u30FC\u30BF\u30FB\u30AB\u30BF\u30ED\u30B0\u306F\u3001\u3053\u306E\u30AF\u30E9\u30B9\u306E1\u3064\u306E\u30A4\u30F3\u30B9\u30BF\u30F3\u30B9\u3068\u3057\u3066\u8868\u308F\u3055\u308C\u307E\u3059\u3002"@ja .
_:genid26 <http://www.w3.org/1999/02/22-rdf-syntax-ns#type> <http://www.w3.org/2002/07/owl#Restriction> .
_:genid26 <http://www.w3.org/2002/07/owl#allValuesFrom> <http://www.w3.org/ns/dcat#Resource> .
_:genid26 <http://www.w3.org/2002/07/owl#onProperty> <http://xmlns.com/foaf/0.1/primaryTopic> .
_:genid27 <http://www.w3.org/1999/02/22-rdf-syntax-ns#type> <http://www.w3.org/2002/07/owl#Restriction> .
_:genid27 <http://www.w3.org/2002/07/owl#cardinality> "1"^^<http://www.w3.org/2001/XMLSchema#nonNegativeInteger> .
_:genid27 <http://www.w3.org/2002/07/owl#onProperty> <http://xmlns.com/foaf/0.1/primaryTopic> .
<http://www.w3.org/ns/dcat#CatalogRecord> <http://www.w3.org/1999/02/22-rdf-syntax-ns#type> <http://www.w3.org/2000/01/rdf-schema#Class> .
<http://www.w3.org/ns/dcat#CatalogRecord> <http://www.w3.org/1999/02/22-rdf-syntax-ns#type> <http://www.w3.org/2002/07/owl#Class> .
<http://www.w3.org/ns/dcat#CatalogRecord> <http://www.w3.org/2000/01/rdf-schema#comment> "1\u3064\u306E\u30C7\u30FC\u30BF\u30BB\u30C3\u30C8\u3092\u8A18\u8FF0\u3057\u305F\u30C7\u30FC\u30BF\u30FB\u30AB\u30BF\u30ED\u30B0\u5185\u306E\u30EC\u30B3\u30FC\u30C9\u3002"@ja .
<http://www.w3.org/ns/dcat#CatalogRecord> <http://www.w3.org/2000/01/rdf-schema#comment> "A record in a data catalog, describing the registration of a single dataset or data service."@en .
<http://www.w3.org/ns/dcat#CatalogRecord> <http://www.w3.org/2000/01/rdf-schema#comment> "Un record in un catalogo di dati che descrive un singolo dataset o servizio di dati."@it .
<http://www.w3.org/ns/dcat#CatalogRecord> <http://www.w3.org/2000/01/rdf-schema#comment> "Un registre du catalogue ou une entr\u00E9e du catalogue, d\u00E9crivant un seul jeu de donn\u00E9es."@fr .
<http://www.w3.org/ns/dcat#CatalogRecord> <http://www.w3.org/2000/01/rdf-schema#comment> "Un registro en un cat\u00E1logo de datos que describe un solo conjunto de datos o un servicio de datos."@es .
<http://www.w3.org/ns/dcat#CatalogRecord> <http://www.w3.org/2000/01/rdf-schema#comment> "Z\u00E1znam v datov\u00E9m katalogu popisuj\u00EDc\u00ED jednu datovou sadu \u010Di datovou slu\u017Ebu."@cs .
<http://www.w3.org/ns/dcat#CatalogRecord> <http://www.w3.org/2000/01/rdf-schema#comment> "\u039C\u03AF\u03B1 \u03BA\u03B1\u03C4\u03B1\u03B3\u03C1\u03B1\u03C6\u03AE \u03B5\u03BD\u03CC\u03C2 \u03BA\u03B1\u03C4\u03B1\u03BB\u03CC\u03B3\u03BF\u03C5, \u03B7 \u03BF\u03C0\u03BF\u03AF\u03B1 \u03C0\u03B5\u03C1\u03B9\u03B3\u03C1\u03AC\u03C6\u03B5\u03B9 \u03AD\u03BD\u03B1 \u03C3\u03C5\u03B3\u03BA\u03B5\u03BA\u03C1\u03B9\u03BC\u03AD\u03BD\u03BF \u03C3\u03CD\u03BD\u03BF\u03BB\u03BF \u03B4\u03B5\u03B4\u03BF\u03BC\u03AD\u03BD\u03C9\u03BD."@el .
<http://www.w3.org/ns/dcat#CatalogRecord> <http://www.w3.org/2000/01/rdf-schema#isDefinedBy> <http://www.w3.org/TR/vocab-dcat/> .
<http://www.w3.org/ns/dcat#CatalogRecord> <http://www.w3.org/2000/01/rdf-schema#label> "Catalog Record"@en .
<http://www.w3.org/ns/dcat#CatalogRecord> <http://www.w3.org/2000/01/rdf-schema#label> "Katalogiza\u010Dn\u00ED z\u00E1znam"@cs .
<http://www.w3.org/ns/dcat#CatalogRecord> <http://www.w3.org/2000/01/rdf-schema#label> "Record di catalogo"@it .
<http://www.w3.org/ns/dcat#CatalogRecord> <http://www.w3.org/2000/01/rdf-schema#label> "Registre du catalogue"@fr .
<http://www.w3.org/ns/dcat#CatalogRecord> <http://www.w3.org/2000/01/rdf-schema#label> "Registro del cat\u00E1logo"@es .
<http://www.w3.org/ns/dcat#CatalogRecord> <http://www.w3.org/2000/01/rdf-schema#label> "\u039A\u03B1\u03C4\u03B1\u03B3\u03C1\u03B1\u03C6\u03AE \u03BA\u03B1\u03C4\u03B1\u03BB\u03CC\u03B3\u03BF\u03C5"@el .
<http://www.w3.org/ns/dcat#CatalogRecord> <http://www.w3.org/2000/01/rdf-schema#label> "\u0633\u062C\u0644"@ar .
<http://www.w3.org/ns/dcat#CatalogRecord> <http://www.w3.org/2000/01/rdf-schema#label> "\u30AB\u30BF\u30ED\u30B0\u30FB\u30EC\u30B3\u30FC\u30C9"@ja .
<http://www.w3.org/ns/dcat#CatalogRecord> <http://www.w3.org/2000/01/rdf-schema#subClassOf> _:genid26 .
<http://www.w3.org/ns/dcat#CatalogRecord> <http://www.w3.org/2000/01/rdf-schema#subClassOf> _:genid27 .
<http://www.w3.org/ns/dcat#CatalogRecord> <http://www.w3.org/2004/02/skos/core#definition> "1\u3064\u306E\u30C7\u30FC\u30BF\u30BB\u30C3\u30C8\u3092\u8A18\u8FF0\u3057\u305F\u30C7\u30FC\u30BF\u30FB\u30AB\u30BF\u30ED\u30B0\u5185\u306E\u30EC\u30B3\u30FC\u30C9\u3002"@ja .
<http://www.w3.org/ns/dcat#CatalogRecord> <http://www.w3.org/2004/02/skos/core#definition> "A record in a data catalog, describing the registration of a single dataset or data service."@en .
<http://www.w3.org/ns/dcat#CatalogRecord> <http://www.w3.org/2004/02/skos/core#definition> "Un record in un catalogo di dati che descrive un singolo dataset o servizio di dati."@it .
<http://www.w3.org/ns/dcat#CatalogRecord> <http://www.w3.org/2004/02/skos/core#definition> "Un registre du catalogue ou une entr\u00E9e du catalogue, d\u00E9crivant un seul jeu de donn\u00E9es."@fr .
<http://www.w3.org/ns/dcat#CatalogRecord> <http://www.w3.org/2004/02/skos/core#definition> "Un registro en un cat\u00E1logo de datos que describe un solo conjunto de datos o un servicio de datos."@es .
<http://www.w3.org/ns/dcat#CatalogRecord> <http://www.w3.org/2004/02/skos/core#definition> "Z\u00E1znam v datov\u00E9m katalogu popisuj\u00EDc\u00ED jednu datovou sadu \u010Di datovou slu\u017Ebu."@cs .
<http://www.w3.org/ns/dcat#CatalogRecord> <http://www.w3.org/2004/02/skos/core#definition> "\u039C\u03AF\u03B1 \u03BA\u03B1\u03C4\u03B1\u03B3\u03C1\u03B1\u03C6\u03AE \u03B5\u03BD\u03CC\u03C2 \u03BA\u03B1\u03C4\u03B1\u03BB\u03CC\u03B3\u03BF\u03C5, \u03B7 \u03BF\u03C0\u03BF\u03AF\u03B1 \u03C0\u03B5\u03C1\u03B9\u03B3\u03C1\u03AC\u03C6\u03B5\u03B9 \u03AD\u03BD\u03B1 \u03C3\u03C5\u03B3\u03BA\u03B5\u03BA\u03C1\u03B9\u03BC\u03AD\u03BD\u03BF \u03C3\u03CD\u03BD\u03BF\u03BB\u03BF \u03B4\u03B5\u03B4\u03BF\u03BC\u03AD\u03BD\u03C9\u03BD."@el .
<http://www.w3.org/ns/dcat#CatalogRecord> <http://www.w3.org/2004/02/skos/core#editorialNote> "English definition updated in this revision. Multilingual text not yet updated except the Spanish one and the Czech one and Italian one."@en .
<http://www.w3.org/ns/dcat#CatalogRecord> <http://www.w3.org/2004/02/skos/core#scopeNote> "C'est une classe facultative et tous les catalogues ne l'utiliseront pas. Cette classe existe pour les catalogues\tayant une distinction entre les m\u00E9tadonn\u00E9es sur le jeu de donn\u00E9es et les m\u00E9tadonn\u00E9es sur une entr\u00E9e du jeu de donn\u00E9es dans le catalogue."@fr .
<http://www.w3.org/ns/dcat#CatalogRecord> <http://www.w3.org/2004/02/skos/core#scopeNote> "Esta clase es opcional y no todos los cat\u00E1logos la utilizar\u00E1n. Esta clase existe para cat\u00E1logos que hacen una distinci\u00F3n entre los metadatos acerca de un conjunto de datos o un servicio de datos y los metadatos acerca de una entrada en ese conjunto de datos en el cat\u00E1logo. Por ejemplo, la propiedad sobre la fecha de la publicaci\u00F3n de los datos refleja la fecha en que la informaci\u00F3n fue originalmente publicada, mientras que la fecha de publicaci\u00F3n del registro del cat\u00E1logo es la fecha en que los datos se agregaron al mismo. En caso en que ambas fechas fueran diferentes, o en que s\u00F3lo la fecha de publicaci\u00F3n del registro del cat\u00E1logo estuviera disponible, s\u00F3lo debe especificarse en el registro del cat\u00E1logo. Tengan en cuenta que la ontolog\u00EDa PROV de W3C permite describir otra informaci\u00F3n sobre la proveniencia de los datos, como por ejemplo detalles del proceso y de los agentes involucrados en alg\u00FAn cambio espec\u00EDfico a los datos."@es .
<http://www.w3.org/ns/dcat#CatalogRecord> <http://www.w3.org/2004/02/skos/core#scopeNote> "Questa classe \u00E8 opzionale e non tutti i cataloghi la utilizzeranno. Esiste per cataloghi in cui si opera una distinzione tra i metadati relativi al dataset ed i metadati relativi alla gestione del dataset nel catalogo. Ad esempio, la  propriet\u00E0 per indicare la data di pubblicazione del dataset rifletter\u00E0 la data in cui l'informazione \u00E8 stata originariamente messa a disposizione dalla casa editrice, mentre la data di pubblicazione per il record nel catalogo rifletter\u00E0 la data in cui il dataset \u00E8 stato aggiunto al catalogo. Nei casi dove solo quest'ultima sia nota, si utilizzer\u00E0 esclusivamente la data di  pubblicazione relativa al record del catalogo. Si noti che l'Ontologia W3C PROV permette di descrivere ulteriori informazioni sulla provenienza, quali i dettagli del processo, la procedura e l'agente coinvolto in una particolare modifica di un dataset."@it .
<http://www.w3.org/ns/dcat#CatalogRecord> <http://www.w3.org/2004/02/skos/core#scopeNote> "Tato t\u0159\u00EDda je voliteln\u00E1 a ne v\u0161echny katalogy ji vyu\u017Eij\u00ED. Existuje pro katalogy, ve kter\u00FDch se rozli\u0161uj\u00ED metadata datov\u00E9 sady \u010Di datov\u00E9 slu\u017Eby a metadata o z\u00E1znamu o datov\u00E9 sad\u011B \u010Di datov\u00E9 slu\u017Eb\u011B v katalogu. Nap\u0159\u00EDklad datum publikace datov\u00E9 sady odr\u00E1\u017E\u00ED datum, kdy byla datov\u00E1 sada p\u016Fvodn\u011B zve\u0159ejn\u011Bna poskytovatelem dat, zat\u00EDmco datum publikace katalogiza\u010Dn\u00EDho z\u00E1znamu je datum zanesen\u00ED datov\u00E9 sady do katalogu. V p\u0159\u00EDpadech kdy se ob\u011B data li\u0161\u00ED, nebo je zn\u00E1mo jen to druh\u00E9, by m\u011Blo b\u00FDt specifikov\u00E1no jen datum publikace katalogiza\u010Dn\u00EDho z\u00E1znamu. V\u0161imn\u011Bte si, \u017Ee ontologie W3C PROV umo\u017E\u0148uje popsat dal\u0161\u00ED informace o p\u016Fvodu jako nap\u0159\u00EDklad podrobnosti o procesu konkr\u00E9tn\u00ED zm\u011Bny datov\u00E9 sady a jeho \u00FA\u010Dastn\u00EDc\u00EDch."@cs .
<http://www.w3.org/ns/dcat#CatalogRecord> <http://www.w3.org/2004/02/skos/core#scopeNote> "This class is optional and not all catalogs will use it. It exists for catalogs where a distinction is made between metadata about a dataset or data service and metadata about the entry for the dataset or data service in the catalog. For example, the publication date property of the dataset reflects the date when the information was originally made available by the publishing agency, while the publication date of the catalog record is the date when the dataset was added to the catalog. In cases where both dates differ, or where only the latter is known, the publication date should only be specified for the catalog record. Notice that the W3C PROV Ontology allows describing further provenance information such as the details of the process and the agent involved in a particular change to a dataset."@en .
<http://www.w3.org/ns/dcat#CatalogRecord> <http://www.w3.org/2004/02/skos/core#scopeNote> "\u0391\u03C5\u03C4\u03AE \u03B7 \u03BA\u03BB\u03AC\u03C3\u03B7 \u03B5\u03AF\u03BD\u03B1\u03B9 \u03C0\u03C1\u03BF\u03B1\u03B9\u03C1\u03B5\u03C4\u03B9\u03BA\u03AE \u03BA\u03B1\u03B9 \u03B4\u03B5\u03BD \u03C7\u03C1\u03B7\u03C3\u03B9\u03BC\u03BF\u03C0\u03BF\u03B9\u03B5\u03AF\u03C4\u03B1\u03B9 \u03B1\u03C0\u03CC \u03CC\u03BB\u03BF\u03C5\u03C2 \u03C4\u03BF\u03C5\u03C2 \u03BA\u03B1\u03C4\u03B1\u03BB\u03CC\u03B3\u03BF\u03C5\u03C2. \u03A5\u03C0\u03AC\u03C1\u03C7\u03B5\u03B9 \u03B3\u03B9\u03B1 \u03C4\u03B9\u03C2 \u03C0\u03B5\u03C1\u03B9\u03C0\u03C4\u03CE\u03C3\u03B5\u03B9\u03C2 \u03BA\u03B1\u03C4\u03B1\u03BB\u03CC\u03B3\u03C9\u03BD \u03CC\u03C0\u03BF\u03C5 \u03B3\u03AF\u03BD\u03B5\u03C4\u03B1\u03B9 \u03B4\u03B9\u03B1\u03C7\u03C9\u03C1\u03B9\u03C3\u03BC\u03CC\u03C2 \u03BC\u03B5\u03C4\u03B1\u03BE\u03CD \u03C4\u03C9\u03BD \u03BC\u03B5\u03C4\u03B1\u03B4\u03B5\u03B4\u03BF\u03BC\u03AD\u03BD\u03C9\u03BD \u03B3\u03B9\u03B1 \u03C4\u03BF \u03C3\u03CD\u03BD\u03BF\u03BB\u03BF \u03C4\u03C9\u03BD \u03B4\u03B5\u03B4\u03BF\u03BC\u03AD\u03BD\u03C9\u03BD \u03BA\u03B1\u03B9 \u03C4\u03C9\u03BD \u03BC\u03B5\u03C4\u03B1\u03B4\u03B5\u03B4\u03BF\u03BC\u03AD\u03BD\u03C9\u03BD \u03B3\u03B9\u03B1 \u03C4\u03B7\u03BD \u03BA\u03B1\u03C4\u03B1\u03B3\u03C1\u03B1\u03C6\u03AE \u03C4\u03BF\u03C5 \u03C3\u03C5\u03BD\u03CC\u03BB\u03BF\u03C5 \u03B4\u03B5\u03B4\u03BF\u03BC\u03AD\u03BD\u03C9\u03BD \u03B5\u03BD\u03C4\u03CC\u03C2 \u03C4\u03BF\u03C5 \u03BA\u03B1\u03C4\u03B1\u03BB\u03CC\u03B3\u03BF\u03C5. \u0393\u03B9\u03B1 \u03C0\u03B1\u03C1\u03AC\u03B4\u03B5\u03B9\u03B3\u03BC\u03B1, \u03B7 \u03B9\u03B4\u03B9\u03CC\u03C4\u03B7\u03C4\u03B1 \u03C4\u03B7\u03C2 \u03B7\u03BC\u03B5\u03C1\u03BF\u03BC\u03B7\u03BD\u03AF\u03B1\u03C2 \u03B4\u03B7\u03BC\u03BF\u03C3\u03AF\u03B5\u03C5\u03C3\u03B7\u03C2 \u03C4\u03BF\u03C5 \u03C3\u03C5\u03BD\u03CC\u03BB\u03BF\u03C5 \u03B4\u03B5\u03B4\u03BF\u03BC\u03AD\u03BD\u03C9\u03BD \u03B4\u03B5\u03AF\u03C7\u03BD\u03B5\u03B9 \u03C4\u03B7\u03BD \u03B7\u03BC\u03B5\u03C1\u03BF\u03BC\u03B7\u03BD\u03AF\u03B1 \u03BA\u03B1\u03C4\u03AC \u03C4\u03B7\u03BD \u03BF\u03C0\u03BF\u03AF\u03B1 \u03BF\u03B9 \u03C0\u03BB\u03B7\u03C1\u03BF\u03C6\u03BF\u03C1\u03AF\u03B5\u03C2 \u03AD\u03B3\u03B9\u03BD\u03B1\u03BD \u03B4\u03B9\u03B1\u03B8\u03AD\u03C3\u03B9\u03BC\u03B5\u03C2 \u03B1\u03C0\u03CC \u03C4\u03BF\u03BD \u03C6\u03BF\u03C1\u03AD\u03B1 \u03B4\u03B7\u03BC\u03BF\u03C3\u03AF\u03B5\u03C5\u03C3\u03B7\u03C2, \u03B5\u03BD\u03CE \u03B7 \u03B7\u03BC\u03B5\u03C1\u03BF\u03BC\u03B7\u03BD\u03AF\u03B1 \u03B4\u03B7\u03BC\u03BF\u03C3\u03AF\u03B5\u03C5\u03C3\u03B7\u03C2 \u03C4\u03B7\u03C2 \u03BA\u03B1\u03C4\u03B1\u03B3\u03C1\u03B1\u03C6\u03AE\u03C2 \u03C4\u03BF\u03C5 \u03BA\u03B1\u03C4\u03B1\u03BB\u03CC\u03B3\u03BF\u03C5 \u03B4\u03B5\u03AF\u03C7\u03BD\u03B5\u03B9 \u03C4\u03B7\u03BD \u03B7\u03BC\u03B5\u03C1\u03BF\u03BC\u03B7\u03BD\u03AF\u03B1 \u03C0\u03BF\u03C5 \u03C4\u03BF \u03C3\u03CD\u03BD\u03BF\u03BB\u03BF \u03B4\u03B5\u03B4\u03BF\u03BC\u03AD\u03BD\u03C9\u03BD \u03C0\u03C1\u03BF\u03C3\u03C4\u03AD\u03B8\u03B7\u03BA\u03B5 \u03C3\u03C4\u03BF\u03BD \u03BA\u03B1\u03C4\u03AC\u03BB\u03BF\u03B3\u03BF. \u03A3\u03B5 \u03C0\u03B5\u03C1\u03B9\u03C0\u03C4\u03CE\u03C3\u03B5\u03B9\u03C2 \u03C0\u03BF\u03C5 \u03BF\u03B9 \u03B4\u03CD\u03BF \u03B7\u03BC\u03B5\u03C1\u03BF\u03BC\u03B7\u03BD\u03AF\u03B5\u03C2 \u03B4\u03B9\u03B1\u03C6\u03AD\u03C1\u03BF\u03C5\u03BD, \u03AE \u03C0\u03BF\u03C5 \u03BC\u03CC\u03BD\u03BF \u03B7 \u03C4\u03B5\u03BB\u03B5\u03C5\u03C4\u03B1\u03AF\u03B1 \u03B5\u03AF\u03BD\u03B1\u03B9 \u03B3\u03BD\u03C9\u03C3\u03C4\u03AE, \u03B7 \u03B7\u03BC\u03B5\u03C1\u03BF\u03BC\u03B7\u03BD\u03AF\u03B1 \u03B4\u03B7\u03BC\u03BF\u03C3\u03AF\u03B5\u03C5\u03C3\u03B7\u03C2 \u03B8\u03B1 \u03C0\u03C1\u03AD\u03C0\u03B5\u03B9 \u03BD\u03B1 \u03B4\u03AF\u03BD\u03B5\u03C4\u03B1\u03B9 \u03B3\u03B9\u03B1 \u03C4\u03B7\u03BD \u03BA\u03B1\u03C4\u03B1\u03B3\u03C1\u03B1\u03C6\u03AE \u03C4\u03BF\u03C5 \u03BA\u03B1\u03C4\u03B1\u03BB\u03CC\u03B3\u03BF\u03C5. \u039D\u03B1 \u03C3\u03B7\u03BC\u03B5\u03B9\u03C9\u03B8\u03B5\u03AF \u03C0\u03C9\u03C2 \u03B7 \u03BF\u03BD\u03C4\u03BF\u03BB\u03BF\u03B3\u03AF\u03B1 W3C PROV \u03B5\u03C0\u03B9\u03C4\u03C1\u03AD\u03C0\u03B5\u03B9 \u03C4\u03B7\u03BD \u03C0\u03B5\u03C1\u03B9\u03B3\u03C1\u03B1\u03C6\u03AE \u03B5\u03C0\u03B9\u03C0\u03BB\u03AD\u03BF\u03BD \u03C0\u03BB\u03B7\u03C1\u03BF\u03C6\u03BF\u03C1\u03B9\u03CE\u03BD \u03B9\u03C3\u03C4\u03BF\u03C1\u03B9\u03BA\u03BF\u03CD \u03CC\u03C0\u03C9\u03C2 \u03BB\u03B5\u03C0\u03C4\u03BF\u03BC\u03AD\u03C1\u03B5\u03B9\u03B5\u03C2 \u03B3\u03B9\u03B1 \u03C4\u03B7 \u03B4\u03B9\u03B1\u03B4\u03B9\u03BA\u03B1\u03C3\u03AF\u03B1 \u03BA\u03B1\u03B9 \u03C4\u03BF\u03BD \u03B4\u03C1\u03AC\u03C3\u03C4\u03B7 \u03C0\u03BF\u03C5 \u03B5\u03BC\u03C0\u03BB\u03AD\u03BA\u03BF\u03BD\u03C4\u03B1\u03B9 \u03C3\u03B5 \u03BC\u03AF\u03B1 \u03C3\u03C5\u03B3\u03BA\u03B5\u03BA\u03C1\u03B9\u03BC\u03AD\u03BD\u03B7 \u03B1\u03BB\u03BB\u03B1\u03B3\u03AE \u03B5\u03BD\u03C4\u03CC\u03C2 \u03C4\u03BF\u03C5 \u03C3\u03C5\u03BD\u03CC\u03BB\u03BF\u03C5 \u03B4\u03B5\u03B4\u03BF\u03BC\u03AD\u03BD\u03C9\u03BD."@el .
<http://www.w3.org/ns/dcat#CatalogRecord> <http://www.w3.org/2004/02/skos/core#scopeNote> "\u3053\u306E\u30AF\u30E9\u30B9\u306F\u30AA\u30D7\u30B7\u30E7\u30F3\u3067\u3001\u3059\u3079\u3066\u306E\u30AB\u30BF\u30ED\u30B0\u304C\u305D\u308C\u3092\u7528\u3044\u308B\u3068\u306F\u9650\u308A\u307E\u305B\u3093\u3002\u3053\u308C\u306F\u3001\u30C7\u30FC\u30BF\u30BB\u30C3\u30C8\u306B\u95A2\u3059\u308B\u30E1\u30BF\u30C7\u30FC\u30BF\u3068\u30AB\u30BF\u30ED\u30B0\u5185\u306E\u30C7\u30FC\u30BF\u30BB\u30C3\u30C8\u306E\u30A8\u30F3\u30C8\u30EA\u30FC\u306B\u95A2\u3059\u308B\u30E1\u30BF\u30C7\u30FC\u30BF\u3068\u3067\u533A\u5225\u304C\u884C\u308F\u308C\u308B\u30AB\u30BF\u30ED\u30B0\u306E\u305F\u3081\u306B\u5B58\u5728\u3057\u3066\u3044\u307E\u3059\u3002\u4F8B\u3048\u3070\u3001\u30C7\u30FC\u30BF\u30BB\u30C3\u30C8\u306E\u516C\u958B\u65E5\u30D7\u30ED\u30D1\u30C6\u30A3\u30FC\u306F\u3001\u516C\u958B\u6A5F\u95A2\u304C\u60C5\u5831\u3092\u6700\u521D\u306B\u5229\u7528\u53EF\u80FD\u3068\u3057\u305F\u65E5\u4ED8\u3092\u793A\u3057\u307E\u3059\u304C\u3001\u30AB\u30BF\u30ED\u30B0\u30FB\u30EC\u30B3\u30FC\u30C9\u306E\u516C\u958B\u65E5\u306F\u3001\u30C7\u30FC\u30BF\u30BB\u30C3\u30C8\u304C\u30AB\u30BF\u30ED\u30B0\u306B\u8FFD\u52A0\u3055\u308C\u305F\u65E5\u4ED8\u3067\u3059\u3002\u4E21\u65B9\u306E\u65E5\u4ED8\u304C\u7570\u3063\u3066\u3044\u305F\u308A\u3001\u5F8C\u8005\u3060\u3051\u304C\u5206\u304B\u3063\u3066\u3044\u308B\u5834\u5408\u306F\u3001\u30AB\u30BF\u30ED\u30B0\u30FB\u30EC\u30B3\u30FC\u30C9\u306B\u5BFE\u3057\u3066\u306E\u307F\u516C\u958B\u65E5\u3092\u6307\u5B9A\u3059\u3079\u304D\u3067\u3059\u3002W3C\u306EPROV\u30AA\u30F3\u30C8\u30ED\u30B8\u30FC[prov-o]\u3092\u7528\u3044\u308C\u3070\u3001\u30C7\u30FC\u30BF\u30BB\u30C3\u30C8\u306B\u5BFE\u3059\u308B\u7279\u5B9A\u306E\u5909\u66F4\u306B\u95A2\u9023\u3059\u308B\u30D7\u30ED\u30BB\u30B9\u3084\u30A8\u30FC\u30B8\u30A7\u30F3\u30C8\u306E\u8A73\u7D30\u306A\u3069\u306E\u3001\u3055\u3089\u306B\u8A73\u3057\u3044\u6765\u6B74\u60C5\u5831\u306E\u8A18\u8FF0\u304C\u53EF\u80FD\u3068\u306A\u308B\u3053\u3068\u306B\u6CE8\u610F\u3057\u3066\u304F\u3060\u3055\u3044\u3002"@ja .
_:genid28 <http://www.w3.org/1999/02/22-rdf-syntax-ns#type> <http://www.w3.org/2002/07/owl#Restriction> .
_:genid28 <http://www.w3.org/2002/07/owl#maxCardinality> "1"^^<http://www.w3.org/2001/XMLSchema#nonNegativeInteger> .
_:genid28 <http://www.w3.org/2002/07/owl#onProperty> <http://www.w3.org/ns/dcat#endpointURL> .
<http://www.w3.org/ns/dcat#DataService> <http://www.w3.org/1999/02/22-rdf-syntax-ns#type> <http://www.w3.org/2002/07/owl#Class> .
<http://www.w3.org/ns/dcat#DataService> <http://www.w3.org/2000/01/rdf-schema#comment> "A site or end-point providing operations related to the discovery of, access to, or processing functions on, data or related resources."@en .
<http://www.w3.org/ns/dcat#DataService> <http://www.w3.org/2000/01/rdf-schema#comment> "Um\u00EDst\u011Bn\u00ED \u010Di p\u0159\u00EDstupov\u00FD bod poskytuj\u00EDc\u00ED operace souvisej\u00EDc\u00ED s hled\u00E1n\u00EDm, p\u0159istupem k, \u010Di v\u00FDkonem funkc\u00ED na datech \u010Di souvisej\u00EDc\u00EDch zdroj\u00EDch."@cs .
<http://www.w3.org/ns/dcat#DataService> <http://www.w3.org/2000/01/rdf-schema#comment> "Un sitio o end-point que provee operaciones relacionadas a funciones de descubrimiento, acceso, o procesamiento de datos o recursos relacionados."@es .
<http://www.w3.org/ns/dcat#DataService> <http://www.w3.org/2000/01/rdf-schema#comment> "Un sito o end-point che fornisce operazioni relative alla scoperta, all'accesso o all'elaborazione di funzioni su dati o risorse correlate."@it .
<http://www.w3.org/ns/dcat#DataService> <http://www.w3.org/2000/01/rdf-schema#label> "Data service"@en .
<http://www.w3.org/ns/dcat#DataService> <http://www.w3.org/2000/01/rdf-schema#label> "Servizio di dati"@it .
<http://www.w3.org/ns/dcat#DataService> <http://www.w3.org/2000/01/rdf-schema#label> "Servicio de datos"@es .
<http://www.w3.org/ns/dcat#DataService> <http://www.w3.org/2000/01/rdf-schema#subClassOf> <http://purl.org/dc/dcmitype/Service> .
<http://www.w3.org/ns/dcat#DataService> <http://www.w3.org/2000/01/rdf-schema#subClassOf> <http://www.w3.org/ns/dcat#Resource> .
<http://www.w3.org/ns/dcat#DataService> <http://www.w3.org/2000/01/rdf-schema#subClassOf> _:genid28 .
<http://www.w3.org/ns/dcat#DataService> <http://www.w3.org/2004/02/skos/core#changeNote> "New class added in DCAT 2.0."@en .
<http://www.w3.org/ns/dcat#DataService> <http://www.w3.org/2004/02/skos/core#changeNote> "Nov\u00E1 t\u0159\u00EDda p\u0159idan\u00E1 ve verzi DCAT 2.0."@cs .
<http://www.w3.org/ns/dcat#DataService> <http://www.w3.org/2004/02/skos/core#changeNote> "Nueva clase a\u00F1adida en DCAT 2.0."@es .
<http://www.w3.org/ns/dcat#DataService> <http://www.w3.org/2004/02/skos/core#changeNote> "Nuova classe aggiunta in DCAT 2.0."@it .
<http://www.w3.org/ns/dcat#DataService> <http://www.w3.org/2004/02/skos/core#definition> "A site or end-point providing operations related to the discovery of, access to, or processing functions on, data or related resources."@en .
<http://www.w3.org/ns/dcat#DataService> <http://www.w3.org/2004/02/skos/core#definition> "Um\u00EDst\u011Bn\u00ED \u010Di p\u0159\u00EDstupov\u00FD bod poskytuj\u00EDc\u00ED operace souvisej\u00EDc\u00ED s hled\u00E1n\u00EDm, p\u0159istupem k, \u010Di v\u00FDkonem funkc\u00ED na datech \u010Di souvisej\u00EDc\u00EDch zdroj\u00EDch."@cs .
<http://www.w3.org/ns/dcat#DataService> <http://www.w3.org/2004/02/skos/core#definition> "Un sitio o end-point que provee operaciones relacionadas a funciones de descubrimiento, acceso, o procesamiento de datos o recursos relacionados."@es .
<http://www.w3.org/ns/dcat#DataService> <http://www.w3.org/2004/02/skos/core#definition> "Un sito o end-point che fornisce operazioni relative alla scoperta, all'accesso o all'elaborazione di funzioni su dati o risorse correlate."@it .
<http://www.w3.org/ns/dcat#DataService> <http://www.w3.org/2004/02/skos/core#scopeNote> "Druh slu\u017Eby m\u016F\u017Ee b\u00FDt indikov\u00E1n vlastnost\u00ED dct:type. Jej\u00ED hodnota m\u016F\u017Ee b\u00FDt z \u0159\u00EDzen\u00E9ho slovn\u00EDku, kter\u00FDm je nap\u0159\u00EDklad slovn\u00EDk typ\u016F prostorov\u00FDch datov\u00FDch slu\u017Eeb INSPIRE."@cs .
<http://www.w3.org/ns/dcat#DataService> <http://www.w3.org/2004/02/skos/core#scopeNote> "El tipo de servicio puede indicarse usando la propiedad dct:type. Su valor puede provenir de un vocabulario controlado, como por ejemplo el vocabulario de servicios de datos espaciales de INSPIRE."@es .
<http://www.w3.org/ns/dcat#DataService> <http://www.w3.org/2004/02/skos/core#scopeNote> "If a dcat:DataService is bound to one or more specified Datasets, they are indicated by the dcat:servesDataset property."@en .
<http://www.w3.org/ns/dcat#DataService> <http://www.w3.org/2004/02/skos/core#scopeNote> "Il tipo di servizio pu\u00F2 essere indicato usando la propriet\u00E0 dct:type. Il suo valore pu\u00F2 essere preso da un vocabolario controllato come il vocabolario dei tipi di servizi per dati spaziali di INSPIRE."@it .
<http://www.w3.org/ns/dcat#DataService> <http://www.w3.org/2004/02/skos/core#scopeNote> "Pokud je dcat:DataService nav\u00E1z\u00E1na na jednu \u010Di v\u00EDce Datov\u00FDch sad, jsou tyto indikov\u00E1ny vlstnost\u00ED dcat:servesDataset."@cs .
<http://www.w3.org/ns/dcat#DataService> <http://www.w3.org/2004/02/skos/core#scopeNote> "Se un dcat:DataService \u00E8 associato a uno o pi\u00F9 Dataset specificati, questi sono indicati dalla propriet\u00E0 dcat:serveDataset."@it .
<http://www.w3.org/ns/dcat#DataService> <http://www.w3.org/2004/02/skos/core#scopeNote> "Si un dcat:DataService est\u00E1 asociado con uno o m\u00E1s conjuntos de datos especificados, dichos conjuntos de datos pueden indicarse con la propiedad dcat:servesDataset."@es .
<http://www.w3.org/ns/dcat#DataService> <http://www.w3.org/2004/02/skos/core#scopeNote> "The kind of service can be indicated using the dct:type property. Its value may be taken from a controlled vocabulary such as the INSPIRE spatial data service type vocabulary."@en .
<http://www.w3.org/ns/dcat#Dataset> <http://www.w3.org/1999/02/22-rdf-syntax-ns#type> <http://www.w3.org/2000/01/rdf-schema#Class> .
<http://www.w3.org/ns/dcat#Dataset> <http://www.w3.org/1999/02/22-rdf-syntax-ns#type> <http://www.w3.org/2002/07/owl#Class> .
<http://www.w3.org/ns/dcat#Dataset> <http://www.w3.org/2000/01/rdf-schema#comment> "1\u3064\u306E\u30A8\u30FC\u30B8\u30A7\u30F3\u30C8\u306B\u3088\u3063\u3066\u516C\u958B\u307E\u305F\u306F\u30AD\u30E5\u30EC\u30FC\u30C8\u3055\u308C\u30011\u3064\u4EE5\u4E0A\u306E\u5F62\u5F0F\u3067\u30A2\u30AF\u30BB\u30B9\u307E\u305F\u306F\u30C0\u30A6\u30F3\u30ED\u30FC\u30C9\u3067\u304D\u308B\u30C7\u30FC\u30BF\u306E\u96C6\u5408\u3002"@ja .
<http://www.w3.org/ns/dcat#Dataset> <http://www.w3.org/2000/01/rdf-schema#comment> "A collection of data, published or curated by a single source, and available for access or download in one or more represenations."@en .
<http://www.w3.org/ns/dcat#Dataset> <http://www.w3.org/2000/01/rdf-schema#comment> "Kolekce dat poskytovan\u00E1 \u010Di \u0159\u00EDzen\u00E1 jedn\u00EDm zdrojem, kter\u00E1 je k dispozici pro p\u0159\u00EDstup \u010Di sta\u017Een\u00ED v jednom \u010Di v\u00EDce form\u00E1tech."@cs .
<http://www.w3.org/ns/dcat#Dataset> <http://www.w3.org/2000/01/rdf-schema#comment> "Raccolta di dati, pubblicati o curati da un'unica fonte, disponibili per l'accesso o il download in uno o pi\u00F9 formati."@it .
<http://www.w3.org/ns/dcat#Dataset> <http://www.w3.org/2000/01/rdf-schema#comment> "Una colecci\u00F3n de datos, publicados o conservados por una \u00FAnica fuente, y disponibles para ser accedidos o descargados en uno o m\u00E1s formatos."@es .
<http://www.w3.org/ns/dcat#Dataset> <http://www.w3.org/2000/01/rdf-schema#comment> "Une collection de donn\u00E9es, publi\u00E9e ou \u00E9labor\u00E9e par une seule source, et disponible pour acc\u00E8s ou t\u00E9l\u00E9chargement dans un ou plusieurs formats."@fr .
<http://www.w3.org/ns/dcat#Dataset> <http://www.w3.org/2000/01/rdf-schema#comment> "\u039C\u03AF\u03B1 \u03C3\u03C5\u03BB\u03BB\u03BF\u03B3\u03AE \u03B1\u03C0\u03CC \u03B4\u03B5\u03B4\u03BF\u03BC\u03AD\u03BD\u03B1, \u03B4\u03B7\u03BC\u03BF\u03C3\u03B9\u03B5\u03C5\u03BC\u03AD\u03BD\u03B7 \u03AE \u03B5\u03C0\u03B9\u03BC\u03B5\u03BB\u03B7\u03BC\u03AD\u03BD\u03B7 \u03B1\u03C0\u03CC \u03BC\u03AF\u03B1 \u03BA\u03B1\u03B9 \u03BC\u03CC\u03BD\u03BF \u03C0\u03B7\u03B3\u03AE, \u03B4\u03B9\u03B1\u03B8\u03AD\u03C3\u03B9\u03BC\u03B7 \u03B4\u03B5 \u03C0\u03C1\u03BF\u03C2 \u03C0\u03C1\u03CC\u03C3\u03B2\u03B1\u03C3\u03B7 \u03AE \u03BC\u03B5\u03C4\u03B1\u03C6\u03CC\u03C1\u03C4\u03C9\u03C3\u03B7 \u03C3\u03B5 \u03BC\u03AF\u03B1 \u03AE \u03C0\u03B5\u03C1\u03B9\u03C3\u03C3\u03CC\u03C4\u03B5\u03C1\u03B5\u03C2 \u03BC\u03BF\u03C1\u03C6\u03AD\u03C2."@el .
<http://www.w3.org/ns/dcat#Dataset> <http://www.w3.org/2000/01/rdf-schema#comment> "\u0642\u0627\u0626\u0645\u0629 \u0628\u064A\u0627\u0646\u0627\u062A \u0645\u0646\u0634\u0648\u0631\u0629 \u0623\u0648 \u0645\u062C\u0645\u0648\u0639\u0629 \u0645\u0646 \u0642\u0628\u0644 \u0645\u0635\u062F\u0631 \u0645\u0627 \u0648 \u0645\u062A\u0627\u062D \u0627\u0644\u0648\u0635\u0648\u0644 \u0625\u0644\u064A\u0647\u0627 \u0623\u0648 \u062A\u062D\u0645\u064A\u0644\u0647\u0627"@ar .
<http://www.w3.org/ns/dcat#Dataset> <http://www.w3.org/2000/01/rdf-schema#isDefinedBy> <http://www.w3.org/TR/vocab-dcat/> .
<http://www.w3.org/ns/dcat#Dataset> <http://www.w3.org/2000/01/rdf-schema#label> "Conjunto de datos"@es .
<http://www.w3.org/ns/dcat#Dataset> <http://www.w3.org/2000/01/rdf-schema#label> "Dataset"@en .
<http://www.w3.org/ns/dcat#Dataset> <http://www.w3.org/2000/01/rdf-schema#label> "Dataset"@it .
<http://www.w3.org/ns/dcat#Dataset> <http://www.w3.org/2000/01/rdf-schema#label> "Datov\u00E1 sada"@cs .
<http://www.w3.org/ns/dcat#Dataset> <http://www.w3.org/2000/01/rdf-schema#label> "Jeu de donn\u00E9es"@fr .
<http://www.w3.org/ns/dcat#Dataset> <http://www.w3.org/2000/01/rdf-schema#label> "\u03A3\u03CD\u03BD\u03BF\u03BB\u03BF \u0394\u03B5\u03B4\u03BF\u03BC\u03AD\u03BD\u03C9\u03BD"@el .
<http://www.w3.org/ns/dcat#Dataset> <http://www.w3.org/2000/01/rdf-schema#label> "\u0642\u0627\u0626\u0645\u0629 \u0628\u064A\u0627\u0646\u0627\u062A"@ar .
<http://www.w3.org/ns/dcat#Dataset> <http://www.w3.org/2000/01/rdf-schema#label> "\u30C7\u30FC\u30BF\u30BB\u30C3\u30C8"@ja .
<http://www.w3.org/ns/dcat#Dataset> <http://www.w3.org/2000/01/rdf-schema#subClassOf> <http://www.w3.org/ns/dcat#Resource> .
<http://www.w3.org/ns/dcat#Dataset> <http://www.w3.org/2004/02/skos/core#changeNote> "2018-02 - odstran\u011Bno tvrzen\u00ED o podt\u0159\u00EDd\u011B dctype:Dataset, jeliko\u017E rozsah dcat:Dataset zahrnuje n\u011Bkolik dal\u0161\u00EDch typ\u016F ze slovn\u00EDku dctype."@cs .
<http://www.w3.org/ns/dcat#Dataset> <http://www.w3.org/2004/02/skos/core#changeNote> "2018-02 - se elimin\u00F3 el axioma de subclase con dctype:Dataset porque el alcance de dcat:Dataset incluye muchos otros tipos del vocabulario dctype."@es .
<http://www.w3.org/ns/dcat#Dataset> <http://www.w3.org/2004/02/skos/core#changeNote> "2018-02 - subclass of dctype:Dataset removed because scope of dcat:Dataset includes several other types from the dctype vocabulary."@en .
<http://www.w3.org/ns/dcat#Dataset> <http://www.w3.org/2004/02/skos/core#changeNote> "2018-02 - sottoclasse di dctype:Dataset rimosso perch\u00E9 l'ambito di dcat:Dataset include diversi altri tipi dal vocabolario dctype."@it .
<http://www.w3.org/ns/dcat#Dataset> <http://www.w3.org/2004/02/skos/core#definition> "1\u3064\u306E\u30A8\u30FC\u30B8\u30A7\u30F3\u30C8\u306B\u3088\u3063\u3066\u516C\u958B\u307E\u305F\u306F\u30AD\u30E5\u30EC\u30FC\u30C8\u3055\u308C\u30011\u3064\u4EE5\u4E0A\u306E\u5F62\u5F0F\u3067\u30A2\u30AF\u30BB\u30B9\u307E\u305F\u306F\u30C0\u30A6\u30F3\u30ED\u30FC\u30C9\u3067\u304D\u308B\u30C7\u30FC\u30BF\u306E\u96C6\u5408\u3002"@ja .
<http://www.w3.org/ns/dcat#Dataset> <http://www.w3.org/2004/02/skos/core#definition> "A collection of data, published or curated by a single source, and available for access or download in one or more represenations."@en .
<http://www.w3.org/ns/dcat#Dataset> <http://www.w3.org/2004/02/skos/core#definition> "Kolekce dat poskytovan\u00E1 \u010Di \u0159\u00EDzen\u00E1 jedn\u00EDm zdrojem, kter\u00E1 je k dispozici pro p\u0159\u00EDstup \u010Di sta\u017Een\u00ED v jednom \u010Di v\u00EDce form\u00E1tech."@cs .
<http://www.w3.org/ns/dcat#Dataset> <http://www.w3.org/2004/02/skos/core#definition> "Raccolta di dati, pubblicati o curati da un'unica fonte, disponibili per l'accesso o il download in uno o pi\u00F9 formati."@it .
<http://www.w3.org/ns/dcat#Dataset> <http://www.w3.org/2004/02/skos/core#definition> "Una colecci\u00F3n de datos, publicados o conservados por una \u00FAnica fuente, y disponibles para ser accedidos o descargados en uno o m\u00E1s formatos."@es .
<http://www.w3.org/ns/dcat#Dataset> <http://www.w3.org/2004/02/skos/core#definition> "Une collection de donn\u00E9es, publi\u00E9e ou \u00E9labor\u00E9e par une seule source, et disponible pour acc\u00E8s ou t\u00E9l\u00E9chargement dans un ou plusieurs formats."@fr .
<http://www.w3.org/ns/dcat#Dataset> <http://www.w3.org/2004/02/skos/core#definition> "\u039C\u03AF\u03B1 \u03C3\u03C5\u03BB\u03BB\u03BF\u03B3\u03AE \u03B1\u03C0\u03CC \u03B4\u03B5\u03B4\u03BF\u03BC\u03AD\u03BD\u03B1, \u03B4\u03B7\u03BC\u03BF\u03C3\u03B9\u03B5\u03C5\u03BC\u03AD\u03BD\u03B7 \u03AE \u03B5\u03C0\u03B9\u03BC\u03B5\u03BB\u03B7\u03BC\u03AD\u03BD\u03B7 \u03B1\u03C0\u03CC \u03BC\u03AF\u03B1 \u03BA\u03B1\u03B9 \u03BC\u03CC\u03BD\u03BF \u03C0\u03B7\u03B3\u03AE, \u03B4\u03B9\u03B1\u03B8\u03AD\u03C3\u03B9\u03BC\u03B7 \u03B4\u03B5 \u03C0\u03C1\u03BF\u03C2 \u03C0\u03C1\u03CC\u03C3\u03B2\u03B1\u03C3\u03B7 \u03AE \u03BC\u03B5\u03C4\u03B1\u03C6\u03CC\u03C1\u03C4\u03C9\u03C3\u03B7 \u03C3\u03B5 \u03BC\u03AF\u03B1 \u03AE \u03C0\u03B5\u03C1\u03B9\u03C3\u03C3\u03CC\u03C4\u03B5\u03C1\u03B5\u03C2 \u03BC\u03BF\u03C1\u03C6\u03AD\u03C2."@el .
<http://www.w3.org/ns/dcat#Dataset> <http://www.w3.org/2004/02/skos/core#definition> "\u0642\u0627\u0626\u0645\u0629 \u0628\u064A\u0627\u0646\u0627\u062A \u0645\u0646\u0634\u0648\u0631\u0629 \u0623\u0648 \u0645\u062C\u0645\u0648\u0639\u0629 \u0645\u0646 \u0642\u0628\u0644 \u0645\u0635\u062F\u0631 \u0645\u0627 \u0648 \u0645\u062A\u0627\u062D \u0627\u0644\u0648\u0635\u0648\u0644 \u0625\u0644\u064A\u0647\u0627 \u0623\u0648 \u062A\u062D\u0645\u064A\u0644\u0647\u0627"@ar .
<http://www.w3.org/ns/dcat#Dataset> <http://www.w3.org/2004/02/skos/core#scopeNote> "Cette classe repr\u00E9sente le jeu de donn\u00E9es publi\u00E9 par le fournisseur de donn\u00E9es. Dans les cas o\u00F9 une distinction est n\u00E9cessaire entre le jeu de don\u00E9nes et son entr\u00E9e dans le catalogue, la classe registre de donn\u00E9es peut \u00EAtre utilis\u00E9e pour ce dernier."@fr .
<http://www.w3.org/ns/dcat#Dataset> <http://www.w3.org/2004/02/skos/core#scopeNote> "Esta clase representa el conjunto de datos publicados. En los casos donde es necesario distinguir entre el conjunto de datos y su entrada en el cat\u00E1logo de datos, se debe utilizar la clase 'registro del cat\u00E1logo'."@es .
<http://www.w3.org/ns/dcat#Dataset> <http://www.w3.org/2004/02/skos/core#scopeNote> "Questa classe rappresenta il dataset come pubblicato dall\u2019editore. Nel caso in cui sia necessario operare  una distinzione fra i metadati originali del dataset e il record dei metadati ad esso associato nel catalogo (ad esempio, per distinguere la data di modifica del dataset da quella del dataset nel catalogo) si pu\u00F2 impiegare la classe catalog record."@it .
<http://www.w3.org/ns/dcat#Dataset> <http://www.w3.org/2004/02/skos/core#scopeNote> "Tato t\u0159\u00EDda reprezentuje datovou sadu tak, jak je publikov\u00E1na poskytovatelem dat. V p\u0159\u00EDpad\u011B pot\u0159eby rozli\u0161en\u00ED datov\u00E9 sady a jej\u00EDho katalogiza\u010Dn\u00EDho z\u00E1znamu (jeliko\u017E metadata jako datum modifikace se mohou li\u0161it) pro n\u011Bj m\u016F\u017Ee b\u00FDt pou\u017Eita t\u0159\u00EDda \"katalogiza\u010Dn\u00ED z\u00E1znam\"."@cs .
<http://www.w3.org/ns/dcat#Dataset> <http://www.w3.org/2004/02/skos/core#scopeNote> "This class describes the conceptual dataset. One or more representations might be available, with differing schematic layouts and formats or serializations."@en .
<http://www.w3.org/ns/dcat#Dataset> <http://www.w3.org/2004/02/skos/core#scopeNote> "Questa classe descrive il dataset dal punto di vista concettuale. Possono essere disponibili una o pi\u00F9 rappresentazioni, con diversi layout e formati schematici o serializzazioni."@it .
<http://www.w3.org/ns/dcat#Dataset> <http://www.w3.org/2004/02/skos/core#scopeNote> "This class represents the actual dataset as published by the dataset provider. In cases where a distinction between the actual dataset and its entry in the catalog is necessary (because metadata such as modification date and maintainer might differ), the catalog record class can be used for the latter."@en .
<http://www.w3.org/ns/dcat#Dataset> <http://www.w3.org/2004/02/skos/core#scopeNote> "\u0397 \u03BA\u03BB\u03AC\u03C3\u03B7 \u03B1\u03C5\u03C4\u03AE \u03B1\u03BD\u03B1\u03C0\u03B1\u03C1\u03B9\u03C3\u03C4\u03AC \u03C4\u03BF \u03C3\u03CD\u03BD\u03BF\u03BB\u03BF \u03B4\u03B5\u03B4\u03BF\u03BC\u03AD\u03BD\u03C9\u03BD \u03B1\u03C5\u03C4\u03CC \u03BA\u03B1\u03B8'\u03B5\u03B1\u03C5\u03C4\u03CC, \u03CC\u03C0\u03C9\u03C2 \u03AD\u03C7\u03B5\u03B9 \u03B4\u03B7\u03BC\u03BF\u03C3\u03B9\u03B5\u03C5\u03B8\u03B5\u03AF \u03B1\u03C0\u03CC \u03C4\u03BF\u03BD \u03B5\u03BA\u03B4\u03CC\u03C4\u03B7. \u03A3\u03B5 \u03C0\u03B5\u03C1\u03B9\u03C0\u03C4\u03CE\u03C3\u03B5\u03B9\u03C2 \u03CC\u03C0\u03BF\u03C5 \u03B5\u03AF\u03BD\u03B1\u03B9 \u03B1\u03C0\u03B1\u03C1\u03B1\u03AF\u03C4\u03B7\u03C4\u03BF\u03C2 \u03BF \u03B4\u03B9\u03B1\u03C7\u03C9\u03C1\u03B9\u03C3\u03BC\u03CC\u03C2 \u03BC\u03B5\u03C4\u03B1\u03BE\u03CD \u03C4\u03BF\u03C5 \u03C3\u03C5\u03BD\u03CC\u03BB\u03BF\u03C5 \u03B4\u03B5\u03B4\u03BF\u03BC\u03AD\u03BD\u03C9\u03BD \u03BA\u03B1\u03B9 \u03C4\u03B7\u03C2 \u03BA\u03B1\u03C4\u03B1\u03B3\u03C1\u03B1\u03C6\u03AE\u03C2 \u03B1\u03C5\u03C4\u03BF\u03CD \u03C3\u03C4\u03BF\u03BD \u03BA\u03B1\u03C4\u03AC\u03BB\u03BF\u03B3\u03BF (\u03B3\u03B9\u03B1\u03C4\u03AF \u03BC\u03B5\u03C4\u03B1\u03B4\u03B5\u03B4\u03BF\u03BC\u03AD\u03BD\u03B1 \u03CC\u03C0\u03C9\u03C2 \u03B7 \u03B7\u03BC\u03B5\u03C1\u03BF\u03BC\u03B7\u03BD\u03AF\u03B1 \u03B1\u03BB\u03BB\u03B1\u03B3\u03AE\u03C2 \u03BA\u03B1\u03B9 \u03BF \u03C3\u03C5\u03BD\u03C4\u03B7\u03C1\u03B7\u03C4\u03AE\u03C2 \u03BC\u03C0\u03BF\u03C1\u03B5\u03AF \u03BD\u03B1 \u03B4\u03B9\u03B1\u03C6\u03AD\u03C1\u03BF\u03C5\u03BD) \u03B7 \u03BA\u03BB\u03AC\u03C3\u03B7 \u03C4\u03B7\u03C2 \u03BA\u03B1\u03C4\u03B1\u03B3\u03C1\u03B1\u03C6\u03AE\u03C2 \u03BA\u03B1\u03C4\u03B1\u03BB\u03CC\u03B3\u03BF\u03C5 \u03BC\u03C0\u03BF\u03C1\u03B5\u03AF \u03BD\u03B1 \u03C7\u03C1\u03B7\u03C3\u03B9\u03BC\u03BF\u03C0\u03BF\u03B9\u03B7\u03B8\u03B5\u03AF \u03B3\u03B9\u03B1 \u03C4\u03BF \u03C4\u03B5\u03BB\u03B5\u03C5\u03C4\u03B1\u03AF\u03BF."@el .
<http://www.w3.org/ns/dcat#Dataset> <http://www.w3.org/2004/02/skos/core#scopeNote> "\u3053\u306E\u30AF\u30E9\u30B9\u306F\u3001\u30C7\u30FC\u30BF\u30BB\u30C3\u30C8\u306E\u516C\u958B\u8005\u304C\u516C\u958B\u3059\u308B\u5B9F\u969B\u306E\u30C7\u30FC\u30BF\u30BB\u30C3\u30C8\u3092\u8868\u308F\u3057\u307E\u3059\u3002\u30AB\u30BF\u30ED\u30B0\u5185\u306E\u5B9F\u969B\u306E\u30C7\u30FC\u30BF\u30BB\u30C3\u30C8\u3068\u305D\u306E\u30A8\u30F3\u30C8\u30EA\u30FC\u3068\u306E\u533A\u5225\u304C\u5FC5\u8981\u306A\u5834\u5408\uFF08\u4FEE\u6B63\u65E5\u3068\u7DAD\u6301\u8005\u306A\u3069\u306E\u30E1\u30BF\u30C7\u30FC\u30BF\u304C\u7570\u306A\u308B\u304B\u3082\u3057\u308C\u306A\u3044\u306E\u3067\uFF09\u306F\u3001\u5F8C\u8005\u306Bcatalog record\u3068\u3044\u3046\u30AF\u30E9\u30B9\u3092\u4F7F\u7528\u3067\u304D\u307E\u3059\u3002"@ja .
<http://www.w3.org/ns/dcat#Distribution> <http://www.w3.org/1999/02/22-rdf-syntax-ns#type> <http://www.w3.org/2000/01/rdf-schema#Class> .
<http://www.w3.org/ns/dcat#Distribution> <http://www.w3.org/1999/02/22-rdf-syntax-ns#type> <http://www.w3.org/2002/07/owl#Class> .
<http://www.w3.org/ns/dcat#Distribution> <http://www.w3.org/2000/01/rdf-schema#comment> "A specific representation of a dataset. A dataset might be available in multiple serializations that may differ in various ways, including natural language, media-type or format, schematic organization, temporal and spatial resolution, level of detail or profiles (which might specify any or all of the above)."@en .
<http://www.w3.org/ns/dcat#Distribution> <http://www.w3.org/2000/01/rdf-schema#comment> "Konkr\u00E9tn\u00ED reprezentace datov\u00E9 sady. Datov\u00E1 sada m\u016F\u017Ee b\u00FDt dostupn\u00E1 v r\u016Fzn\u00FDch serializac\u00EDch, kter\u00E9 se mohou navz\u00E1jem li\u0161it r\u016Fzn\u00FDmi zp\u016Fsoby, mimo jin\u00E9 p\u0159irozen\u00FDm jazykem, media-typem \u010Di form\u00E1tem, schematickou organizac\u00ED, \u010Dasov\u00FDm a prostorov\u00FDm rozli\u0161en\u00EDm, \u00FArovn\u00ED detailu \u010Di profily (kter\u00E9 mohou specifikovat n\u011Bkter\u00E9 \u010Di v\u0161echny tyto rozd\u00EDly)."@cs .
<http://www.w3.org/ns/dcat#Distribution> <http://www.w3.org/2000/01/rdf-schema#comment> "Rappresenta una forma disponibile e specifica del dataset. Ciascun dataset pu\u00F2 essere disponibile in forme differenti, che possono rappresentare formati diversi o diversi punti di accesso per un dataset. Esempi di distribuzioni sono un file CSV scaricabile, una API o un RSS feed."@it .
<http://www.w3.org/ns/dcat#Distribution> <http://www.w3.org/2000/01/rdf-schema#comment> "Repr\u00E9sente une forme sp\u00E9cifique d'un jeu de donn\u00E9es. Caque jeu de donn\u00E9es peut \u00EAtre disponible sous diff\u00E9rentes formes, celles-ci pouvant repr\u00E9senter diff\u00E9rents formats du jeu de donn\u00E9es ou diff\u00E9rents endpoint. Des exemples de distribution sont des fichirs CSV, des API ou des flux RSS."@fr .
<http://www.w3.org/ns/dcat#Distribution> <http://www.w3.org/2000/01/rdf-schema#comment> "Una representaci\u00F3n espec\u00EDfica de los datos. Cada conjunto de datos puede estar disponible en formas diferentes, las cu\u00E1les pueden variar en distintas formas, incluyendo el idioma, 'media-type' o formato, organizaci\u00F3n esquem\u00E1tica, resoluci\u00F3n temporal y espacial, nivel de detalle o perfiles (que pueden especificar cualquiera o todas las diferencias anteriores)."@es .
<http://www.w3.org/ns/dcat#Distribution> <http://www.w3.org/2000/01/rdf-schema#comment> "\u0391\u03BD\u03B1\u03C0\u03B1\u03C1\u03B9\u03C3\u03C4\u03AC \u03BC\u03AF\u03B1 \u03C3\u03C5\u03B3\u03BA\u03B5\u03BA\u03C1\u03B9\u03BC\u03AD\u03BD\u03B7 \u03B4\u03B9\u03B1\u03B8\u03AD\u03C3\u03B9\u03BC\u03B7 \u03BC\u03BF\u03C1\u03C6\u03AE \u03B5\u03BD\u03CC\u03C2 \u03C3\u03C5\u03BD\u03CC\u03BB\u03BF\u03C5 \u03B4\u03B5\u03B4\u03BF\u03BC\u03AD\u03BD\u03C9\u03BD. \u039A\u03AC\u03B8\u03B5 \u03C3\u03CD\u03BD\u03BF\u03BB\u03BF \u03B4\u03B5\u03B4\u03BF\u03BC\u03B5\u03BD\u03C9\u03BD \u03BC\u03C0\u03BF\u03C1\u03B5\u03AF \u03BD\u03B1 \u03B5\u03AF\u03BD\u03B1\u03B9 \u03B4\u03B9\u03B1\u03B8\u03AD\u03C3\u03B9\u03BC\u03BF \u03C3\u03B5 \u03B4\u03B9\u03B1\u03C6\u03BF\u03C1\u03B5\u03C4\u03B9\u03BA\u03AD\u03C2 \u03BC\u03BF\u03C1\u03C6\u03AD\u03C2, \u03BF\u03B9 \u03BC\u03BF\u03C1\u03C6\u03AD\u03C2 \u03B1\u03C5\u03C4\u03AD\u03C2 \u03BC\u03C0\u03BF\u03C1\u03B5\u03AF \u03BD\u03B1 \u03B1\u03BD\u03B1\u03C0\u03B1\u03C1\u03B9\u03C3\u03C4\u03BF\u03CD\u03BD \u03B4\u03B9\u03B1\u03C6\u03BF\u03C1\u03B5\u03C4\u03B9\u03BA\u03AD\u03C2 \u03BC\u03BF\u03C1\u03C6\u03AD\u03C2 \u03B1\u03C1\u03C7\u03B5\u03AF\u03C9\u03BD \u03AE \u03B4\u03B9\u03B1\u03C6\u03BF\u03C1\u03B5\u03C4\u03B9\u03BA\u03AC \u03C3\u03B7\u03BC\u03B5\u03AF\u03B1 \u03B4\u03B9\u03AC\u03B8\u03B5\u03C3\u03B7\u03C2. \u03A0\u03B1\u03C1\u03B1\u03B4\u03B5\u03AF\u03B3\u03BC\u03B1\u03C4\u03B1 \u03B4\u03B9\u03B1\u03BD\u03BF\u03BC\u03CE\u03BD \u03C3\u03C5\u03BC\u03C0\u03B5\u03C1\u03B9\u03BB\u03B1\u03BC\u03B2\u03AC\u03BD\u03BF\u03C5\u03BD \u03AD\u03BD\u03B1 \u03BC\u03B5\u03C4\u03B1\u03C6\u03BF\u03C1\u03C4\u03CE\u03C3\u03B9\u03BC\u03BF \u03B1\u03C1\u03C7\u03B5\u03AF\u03BF \u03BC\u03BF\u03C1\u03C6\u03AE\u03C2 CSV, \u03AD\u03BD\u03B1 API \u03AE \u03AD\u03BD\u03B1 RSS feed."@el .
<http://www.w3.org/ns/dcat#Distribution> <http://www.w3.org/2000/01/rdf-schema#comment> "\u0634\u0643\u0644 \u0645\u062D\u062F\u062F \u0644\u0642\u0627\u0626\u0645\u0629 \u0627\u0644\u0628\u064A\u0627\u0646\u0627\u062A \u064A\u0645\u0643\u0646 \u0627\u0644\u0648\u0635\u0648\u0644 \u0625\u0644\u064A\u0647. \u0642\u0627\u0626\u0645\u0629 \u0628\u064A\u0627\u0646\u0627\u062A \u0645\u0627 \u064A\u0645\u0643\u0646 \u0623\u0646 \u062A\u0643\u0648\u0646 \u0645\u062A\u0627\u062D\u0647 \u0628\u0627\u0634\u0643\u0627\u0644 \u0648 \u0623\u0646\u0648\u0627\u0639 \u0645\u062A\u0639\u062F\u062F\u0629.  \u0645\u0644\u0641 \u064A\u0645\u0643\u0646 \u062A\u062D\u0645\u064A\u0644\u0647 \u0623\u0648 \u0648\u0627\u062C\u0647\u0629 \u0628\u0631\u0645\u062C\u064A\u0629 \u064A\u0645\u0643\u0646 \u0645\u0646 \u062E\u0644\u0627\u0644\u0647\u0627 \u0627\u0644\u0648\u0635\u0648\u0644 \u0625\u0644\u0649 \u0627\u0644\u0628\u064A\u0627\u0646\u0627\u062A \u0647\u064A \u0623\u0645\u062B\u0644\u0629 \u0639\u0644\u0649 \u0630\u0644\u0643."@ar .
<http://www.w3.org/ns/dcat#Distribution> <http://www.w3.org/2000/01/rdf-schema#comment> "\u30C7\u30FC\u30BF\u30BB\u30C3\u30C8\u306E\u7279\u5B9A\u306E\u5229\u7528\u53EF\u80FD\u306A\u5F62\u5F0F\u3092\u8868\u308F\u3057\u307E\u3059\u3002\u5404\u30C7\u30FC\u30BF\u30BB\u30C3\u30C8\u306F\u3001\u7570\u306A\u308B\u5F62\u5F0F\u3067\u5229\u7528\u3067\u304D\u308B\u3053\u3068\u304C\u3042\u308A\u3001\u3053\u308C\u3089\u306E\u5F62\u5F0F\u306F\u3001\u30C7\u30FC\u30BF\u30BB\u30C3\u30C8\u306E\u7570\u306A\u308B\u5F62\u5F0F\u3084\u3001\u7570\u306A\u308B\u30A8\u30F3\u30C9\u30DD\u30A4\u30F3\u30C8\u3092\u8868\u308F\u3059\u53EF\u80FD\u6027\u304C\u3042\u308A\u307E\u3059\u3002\u914D\u4FE1\u306E\u4F8B\u306B\u306F\u3001\u30C0\u30A6\u30F3\u30ED\u30FC\u30C9\u53EF\u80FD\u306ACSV\u30D5\u30A1\u30A4\u30EB\u3001API\u3001RSS\u30D5\u30A3\u30FC\u30C9\u304C\u542B\u307E\u308C\u307E\u3059\u3002"@ja .
<http://www.w3.org/ns/dcat#Distribution> <http://www.w3.org/2000/01/rdf-schema#isDefinedBy> <http://www.w3.org/TR/vocab-dcat/> .
<http://www.w3.org/ns/dcat#Distribution> <http://www.w3.org/2000/01/rdf-schema#label> "Distribuce"@cs .
<http://www.w3.org/ns/dcat#Distribution> <http://www.w3.org/2000/01/rdf-schema#label> "Distribuci\u00F3n"@es .
<http://www.w3.org/ns/dcat#Distribution> <http://www.w3.org/2000/01/rdf-schema#label> "Distribution"@en .
<http://www.w3.org/ns/dcat#Distribution> <http://www.w3.org/2000/01/rdf-schema#label> "Distribution"@fr .
<http://www.w3.org/ns/dcat#Distribution> <http://www.w3.org/2000/01/rdf-schema#label> "Distribuzione"@it .
<http://www.w3.org/ns/dcat#Distribution> <http://www.w3.org/2000/01/rdf-schema#label> "\u0394\u03B9\u03B1\u03BD\u03BF\u03BC\u03AE"@el .
<http://www.w3.org/ns/dcat#Distribution> <http://www.w3.org/2000/01/rdf-schema#label> "\u0627\u0644\u062A\u0648\u0632\u064A\u0639"@ar .
<http://www.w3.org/ns/dcat#Distribution> <http://www.w3.org/2000/01/rdf-schema#label> "\u914D\u4FE1"@ja .
<http://www.w3.org/ns/dcat#Distribution> <http://www.w3.org/2004/02/skos/core#definition> "A specific representation of a dataset. A dataset might be available in multiple serializations that may differ in various ways, including natural language, media-type or format, schematic organization, temporal and spatial resolution, level of detail or profiles (which might specify any or all of the above)."@en .
<http://www.w3.org/ns/dcat#Distribution> <http://www.w3.org/2004/02/skos/core#definition> "Konkr\u00E9tn\u00ED reprezentace datov\u00E9 sady. Datov\u00E1 sada m\u016F\u017Ee b\u00FDt dostupn\u00E1 v r\u016Fzn\u00FDch serializac\u00EDch, kter\u00E9 se mohou navz\u00E1jem li\u0161it r\u016Fzn\u00FDmi zp\u016Fsoby, mimo jin\u00E9 p\u0159irozen\u00FDm jazykem, media-typem \u010Di form\u00E1tem, schematickou organizac\u00ED, \u010Dasov\u00FDm a prostorov\u00FDm rozli\u0161en\u00EDm, \u00FArovn\u00ED detailu \u010Di profily (kter\u00E9 mohou specifikovat n\u011Bkter\u00E9 \u010Di v\u0161echny tyto rozd\u00EDly)."@cs .
<http://www.w3.org/ns/dcat#Distribution> <http://www.w3.org/2004/02/skos/core#definition> "Rappresenta una forma disponibile e specifica del dataset. Ciascun dataset pu\u00F2 essere disponibile in forme differenti, che possono rappresentare formati diversi o diversi punti di accesso per un dataset. Esempi di distribuzioni sono un file CSV scaricabile, una API o un RSS feed."@it .
<http://www.w3.org/ns/dcat#Distribution> <http://www.w3.org/2004/02/skos/core#definition> "Repr\u00E9sente une forme sp\u00E9cifique d'un jeu de donn\u00E9es. Caque jeu de donn\u00E9es peut \u00EAtre disponible sous diff\u00E9rentes formes, celles-ci pouvant repr\u00E9senter diff\u00E9rents formats du jeu de donn\u00E9es ou diff\u00E9rents endpoint. Des exemples de distribution sont des fichirs CSV, des API ou des flux RSS."@fr .
<http://www.w3.org/ns/dcat#Distribution> <http://www.w3.org/2004/02/skos/core#definition> "Una representaci\u00F3n espec\u00EDfica de los datos. Cada conjunto de datos puede estar disponible en formas diferentes, las cu\u00E1les pueden variar en distintas formas, incluyendo el idioma, 'media-type' o formato, organizaci\u00F3n esquem\u00E1tica, resoluci\u00F3n temporal y espacial, nivel de detalle o perfiles (que pueden especificar cualquiera o todas las diferencias anteriores)."@es .
<http://www.w3.org/ns/dcat#Distribution> <http://www.w3.org/2004/02/skos/core#definition> "\u0391\u03BD\u03B1\u03C0\u03B1\u03C1\u03B9\u03C3\u03C4\u03AC \u03BC\u03AF\u03B1 \u03C3\u03C5\u03B3\u03BA\u03B5\u03BA\u03C1\u03B9\u03BC\u03AD\u03BD\u03B7 \u03B4\u03B9\u03B1\u03B8\u03AD\u03C3\u03B9\u03BC\u03B7 \u03BC\u03BF\u03C1\u03C6\u03AE \u03B5\u03BD\u03CC\u03C2 \u03C3\u03C5\u03BD\u03CC\u03BB\u03BF\u03C5 \u03B4\u03B5\u03B4\u03BF\u03BC\u03AD\u03BD\u03C9\u03BD. \u039A\u03AC\u03B8\u03B5 \u03C3\u03CD\u03BD\u03BF\u03BB\u03BF \u03B4\u03B5\u03B4\u03BF\u03BC\u03B5\u03BD\u03C9\u03BD \u03BC\u03C0\u03BF\u03C1\u03B5\u03AF \u03BD\u03B1 \u03B5\u03AF\u03BD\u03B1\u03B9 \u03B4\u03B9\u03B1\u03B8\u03AD\u03C3\u03B9\u03BC\u03BF \u03C3\u03B5 \u03B4\u03B9\u03B1\u03C6\u03BF\u03C1\u03B5\u03C4\u03B9\u03BA\u03AD\u03C2 \u03BC\u03BF\u03C1\u03C6\u03AD\u03C2, \u03BF\u03B9 \u03BC\u03BF\u03C1\u03C6\u03AD\u03C2 \u03B1\u03C5\u03C4\u03AD\u03C2 \u03BC\u03C0\u03BF\u03C1\u03B5\u03AF \u03BD\u03B1 \u03B1\u03BD\u03B1\u03C0\u03B1\u03C1\u03B9\u03C3\u03C4\u03BF\u03CD\u03BD \u03B4\u03B9\u03B1\u03C6\u03BF\u03C1\u03B5\u03C4\u03B9\u03BA\u03AD\u03C2 \u03BC\u03BF\u03C1\u03C6\u03AD\u03C2 \u03B1\u03C1\u03C7\u03B5\u03AF\u03C9\u03BD \u03AE \u03B4\u03B9\u03B1\u03C6\u03BF\u03C1\u03B5\u03C4\u03B9\u03BA\u03AC \u03C3\u03B7\u03BC\u03B5\u03AF\u03B1 \u03B4\u03B9\u03AC\u03B8\u03B5\u03C3\u03B7\u03C2. \u03A0\u03B1\u03C1\u03B1\u03B4\u03B5\u03AF\u03B3\u03BC\u03B1\u03C4\u03B1 \u03B4\u03B9\u03B1\u03BD\u03BF\u03BC\u03CE\u03BD \u03C3\u03C5\u03BC\u03C0\u03B5\u03C1\u03B9\u03BB\u03B1\u03BC\u03B2\u03AC\u03BD\u03BF\u03C5\u03BD \u03AD\u03BD\u03B1 \u03BC\u03B5\u03C4\u03B1\u03C6\u03BF\u03C1\u03C4\u03CE\u03C3\u03B9\u03BC\u03BF \u03B1\u03C1\u03C7\u03B5\u03AF\u03BF \u03BC\u03BF\u03C1\u03C6\u03AE\u03C2 CSV, \u03AD\u03BD\u03B1 API \u03AE \u03AD\u03BD\u03B1 RSS feed."@el .
<http://www.w3.org/ns/dcat#Distribution> <http://www.w3.org/2004/02/skos/core#definition> "\u0634\u0643\u0644 \u0645\u062D\u062F\u062F \u0644\u0642\u0627\u0626\u0645\u0629 \u0627\u0644\u0628\u064A\u0627\u0646\u0627\u062A \u064A\u0645\u0643\u0646 \u0627\u0644\u0648\u0635\u0648\u0644 \u0625\u0644\u064A\u0647. \u0642\u0627\u0626\u0645\u0629 \u0628\u064A\u0627\u0646\u0627\u062A \u0645\u0627 \u064A\u0645\u0643\u0646 \u0623\u0646 \u062A\u0643\u0648\u0646 \u0645\u062A\u0627\u062D\u0647 \u0628\u0627\u0634\u0643\u0627\u0644 \u0648 \u0623\u0646\u0648\u0627\u0639 \u0645\u062A\u0639\u062F\u062F\u0629.  \u0645\u0644\u0641 \u064A\u0645\u0643\u0646 \u062A\u062D\u0645\u064A\u0644\u0647 \u0623\u0648 \u0648\u0627\u062C\u0647\u0629 \u0628\u0631\u0645\u062C\u064A\u0629 \u064A\u0645\u0643\u0646 \u0645\u0646 \u062E\u0644\u0627\u0644\u0647\u0627 \u0627\u0644\u0648\u0635\u0648\u0644 \u0625\u0644\u0649 \u0627\u0644\u0628\u064A\u0627\u0646\u0627\u062A \u0647\u064A \u0623\u0645\u062B\u0644\u0629 \u0639\u0644\u0649 \u0630\u0644\u0643."@ar .
<http://www.w3.org/ns/dcat#Distribution> <http://www.w3.org/2004/02/skos/core#definition> "\u30C7\u30FC\u30BF\u30BB\u30C3\u30C8\u306E\u7279\u5B9A\u306E\u5229\u7528\u53EF\u80FD\u306A\u5F62\u5F0F\u3092\u8868\u308F\u3057\u307E\u3059\u3002\u5404\u30C7\u30FC\u30BF\u30BB\u30C3\u30C8\u306F\u3001\u7570\u306A\u308B\u5F62\u5F0F\u3067\u5229\u7528\u3067\u304D\u308B\u3053\u3068\u304C\u3042\u308A\u3001\u3053\u308C\u3089\u306E\u5F62\u5F0F\u306F\u3001\u30C7\u30FC\u30BF\u30BB\u30C3\u30C8\u306E\u7570\u306A\u308B\u5F62\u5F0F\u3084\u3001\u7570\u306A\u308B\u30A8\u30F3\u30C9\u30DD\u30A4\u30F3\u30C8\u3092\u8868\u308F\u3059\u53EF\u80FD\u6027\u304C\u3042\u308A\u307E\u3059\u3002\u914D\u4FE1\u306E\u4F8B\u306B\u306F\u3001\u30C0\u30A6\u30F3\u30ED\u30FC\u30C9\u53EF\u80FD\u306ACSV\u30D5\u30A1\u30A4\u30EB\u3001API\u3001RSS\u30D5\u30A3\u30FC\u30C9\u304C\u542B\u307E\u308C\u307E\u3059\u3002"@ja .
<http://www.w3.org/ns/dcat#Distribution> <http://www.w3.org/2004/02/skos/core#scopeNote> "Ceci repr\u00E9sente une disponibilit\u00E9 g\u00E9n\u00E9rale du jeu de donn\u00E9es, et implique qu'il n'existe pas d'information sur la m\u00E9thode d'acc\u00E8s r\u00E9elle des donn\u00E9es, par exple, si c'est un lien de t\u00E9l\u00E9chargement direct ou \u00E0 travers une page Web."@fr .
<http://www.w3.org/ns/dcat#Distribution> <http://www.w3.org/2004/02/skos/core#scopeNote> "Esta clase representa una disponibilidad general de un conjunto de datos, e implica que no existe informaci\u00F3n acerca del m\u00E9todo de acceso real a los datos, i.e., si es un enlace de descarga directa o a trav\u00E9s de una p\u00E1gina Web."@es .
<http://www.w3.org/ns/dcat#Distribution> <http://www.w3.org/2004/02/skos/core#scopeNote> "Questa classe rappresenta una disponibilit\u00E0 generale di un dataset e non implica alcuna informazione sul metodo di accesso effettivo ai dati, ad esempio se si tratta di un accesso a download diretto, API, o attraverso una pagina Web. L'utilizzo della propriet\u00E0 dcat:downloadURL indica distribuzioni direttamente scaricabili."@it .
<http://www.w3.org/ns/dcat#Distribution> <http://www.w3.org/2004/02/skos/core#scopeNote> "This represents a general availability of a dataset it implies no information about the actual access method of the data, i.e. whether by direct download, API, or through a Web page. The use of dcat:downloadURL property indicates directly downloadable distributions."@en .
<http://www.w3.org/ns/dcat#Distribution> <http://www.w3.org/2004/02/skos/core#scopeNote> "Toto popisuje obecnou dostupnost datov\u00E9 sady. Neimplikuje \u017E\u00E1dnou informaci o skute\u010Dn\u00E9 metod\u011B p\u0159\u00EDstupu k dat\u016Fm, tj. zda jsou p\u0159\u00EDmo ke sta\u017Een\u00ED, skrze API \u010Di p\u0159es webovou str\u00E1nku. Pou\u017Eit\u00ED vlastnosti dcat:downloadURL indikuje p\u0159\u00EDmo sta\u017Eiteln\u00E9 distribuce."@cs .
<http://www.w3.org/ns/dcat#Distribution> <http://www.w3.org/2004/02/skos/core#scopeNote> "\u0391\u03C5\u03C4\u03CC \u03B1\u03BD\u03B1\u03C0\u03B1\u03C1\u03B9\u03C3\u03C4\u03AC \u03BC\u03AF\u03B1 \u03B3\u03B5\u03BD\u03B9\u03BA\u03AE \u03B4\u03B9\u03B1\u03B8\u03B5\u03C3\u03B9\u03BC\u03CC\u03C4\u03B7\u03C4\u03B1 \u03B5\u03BD\u03CC\u03C2 \u03C3\u03C5\u03BD\u03CC\u03BB\u03BF\u03C5 \u03B4\u03B5\u03B4\u03BF\u03BC\u03AD\u03BD\u03C9\u03BD \u03BA\u03B1\u03B9 \u03B4\u03B5\u03BD \u03C5\u03C0\u03BF\u03BD\u03BF\u03B5\u03AF \u03C4\u03AF\u03C0\u03BF\u03C4\u03B1 \u03C0\u03B5\u03C1\u03AF \u03C4\u03BF\u03C5 \u03C0\u03C1\u03B1\u03B3\u03BC\u03B1\u03C4\u03B9\u03BA\u03BF\u03CD \u03C4\u03C1\u03CC\u03C0\u03BF\u03C5 \u03C0\u03C1\u03CC\u03C3\u03B2\u03B1\u03C3\u03B7\u03C2 \u03C3\u03C4\u03B1 \u03B4\u03B5\u03B4\u03BF\u03BC\u03AD\u03BD\u03B1, \u03B1\u03BD \u03B5\u03AF\u03BD\u03B1\u03B9 \u03AC\u03BC\u03B5\u03C3\u03B1 \u03BC\u03B5\u03C4\u03B1\u03C6\u03BF\u03C1\u03C4\u03CE\u03C3\u03B9\u03BC\u03B1, \u03BC\u03AD\u03C3\u03C9 API \u03AE \u03BC\u03AD\u03C3\u03C9 \u03BC\u03AF\u03B1\u03C2 \u03B9\u03C3\u03C4\u03BF\u03C3\u03B5\u03BB\u03AF\u03B4\u03B1\u03C2. \u0397 \u03C7\u03C1\u03AE\u03C3\u03B7 \u03C4\u03B7\u03C2 \u03B9\u03B4\u03B9\u03CC\u03C4\u03B7\u03C4\u03B1\u03C2 dcat:downloadURL \u03B4\u03B5\u03AF\u03C7\u03BD\u03B5\u03B9 \u03BC\u03CC\u03BD\u03BF \u03AC\u03BC\u03B5\u03C3\u03B1 \u03BC\u03B5\u03C4\u03B1\u03C6\u03BF\u03C1\u03C4\u03CE\u03C3\u03B9\u03BC\u03B5\u03C2 \u03B4\u03B9\u03B1\u03BD\u03BF\u03BC\u03AD\u03C2."@el .
<http://www.w3.org/ns/dcat#Distribution> <http://www.w3.org/2004/02/skos/core#scopeNote> "\u3053\u308C\u306F\u3001\u30C7\u30FC\u30BF\u30BB\u30C3\u30C8\u306E\u4E00\u822C\u7684\u306A\u5229\u7528\u53EF\u80FD\u6027\u3092\u8868\u308F\u3057\u3001\u30C7\u30FC\u30BF\u306E\u5B9F\u969B\u306E\u30A2\u30AF\u30BB\u30B9\u65B9\u5F0F\u306B\u95A2\u3059\u308B\u60C5\u5831\uFF08\u3064\u307E\u308A\u3001\u76F4\u63A5\u30C0\u30A6\u30F3\u30ED\u30FC\u30C9\u306A\u306E\u304B\u3001API\u306A\u306E\u304B\u3001\u30A6\u30A7\u30D6\u30DA\u30FC\u30B8\u3092\u4ECB\u3057\u305F\u3082\u306E\u306A\u306E\u304B\uFF09\u3092\u610F\u5473\u3057\u307E\u305B\u3093\u3002dcat:downloadURL\u30D7\u30ED\u30D1\u30C6\u30A3\u30FC\u306E\u4F7F\u7528\u306F\u3001\u76F4\u63A5\u30C0\u30A6\u30F3\u30ED\u30FC\u30C9\u53EF\u80FD\u306A\u914D\u4FE1\u3092\u610F\u5473\u3057\u307E\u3059\u3002"@ja .
_:genid29 <http://www.w3.org/1999/02/22-rdf-syntax-ns#type> <http://www.w3.org/2002/07/owl#Restriction> .
_:genid29 <http://www.w3.org/2002/07/owl#minCardinality> "1"^^<http://www.w3.org/2001/XMLSchema#nonNegativeInteger> .
_:genid29 <http://www.w3.org/2002/07/owl#onProperty> <http://purl.org/dc/terms/relation> .
<http://www.w3.org/ns/dcat#Relationship> <http://www.w3.org/1999/02/22-rdf-syntax-ns#type> <http://www.w3.org/2002/07/owl#Class> .
<http://www.w3.org/ns/dcat#Relationship> <http://www.w3.org/2000/01/rdf-schema#comment> "An association class for attaching additional information to a relationship between DCAT Resources."@en .
<http://www.w3.org/ns/dcat#Relationship> <http://www.w3.org/2000/01/rdf-schema#comment> "Asocia\u010Dn\u00ED t\u0159\u00EDda pro p\u0159ipojen\u00ED dodate\u010Dn\u00FDch informac\u00ED ke vztahu mezi zdroji DCAT."@cs .
<http://www.w3.org/ns/dcat#Relationship> <http://www.w3.org/2000/01/rdf-schema#comment> "Una clase de asociaci\u00F3n para adjuntar informaci\u00F3n adicional a una relaci\u00F3n entre recursos DCAT."@es .
<http://www.w3.org/ns/dcat#Relationship> <http://www.w3.org/2000/01/rdf-schema#comment> "Una classe di associazione per il collegamento di informazioni aggiuntive a una relazione tra le risorse DCAT."@it .
<http://www.w3.org/ns/dcat#Relationship> <http://www.w3.org/2000/01/rdf-schema#label> "Relaci\u00F3n"@es .
<http://www.w3.org/ns/dcat#Relationship> <http://www.w3.org/2000/01/rdf-schema#label> "Relationship"@en .
<http://www.w3.org/ns/dcat#Relationship> <http://www.w3.org/2000/01/rdf-schema#label> "Relazione"@it .
<http://www.w3.org/ns/dcat#Relationship> <http://www.w3.org/2000/01/rdf-schema#label> "Vztah"@cs .
<http://www.w3.org/ns/dcat#Relationship> <http://www.w3.org/2000/01/rdf-schema#subClassOf> _:genid29 .
<http://www.w3.org/ns/dcat#Relationship> <http://www.w3.org/2004/02/skos/core#changeNote> "New class added in DCAT 2.0."@en .
<http://www.w3.org/ns/dcat#Relationship> <http://www.w3.org/2004/02/skos/core#changeNote> "Nov\u00E1 t\u0159\u00EDda p\u0159idan\u00E1 ve verzi DCAT 2.0."@cs .
<http://www.w3.org/ns/dcat#Relationship> <http://www.w3.org/2004/02/skos/core#changeNote> "Nueva clase a\u00F1adida en DCAT 2.0."@es .
<http://www.w3.org/ns/dcat#Relationship> <http://www.w3.org/2004/02/skos/core#changeNote> "Nuova classe aggiunta in DCAT 2.0."@it .
<http://www.w3.org/ns/dcat#Relationship> <http://www.w3.org/2004/02/skos/core#definition> "An association class for attaching additional information to a relationship between DCAT Resources."@en .
<http://www.w3.org/ns/dcat#Relationship> <http://www.w3.org/2004/02/skos/core#definition> "Asocia\u010Dn\u00ED t\u0159\u00EDda pro p\u0159ipojen\u00ED dodate\u010Dn\u00FDch informac\u00ED ke vztahu mezi zdroji DCAT."@cs .
<http://www.w3.org/ns/dcat#Relationship> <http://www.w3.org/2004/02/skos/core#definition> "Una clase de asociaci\u00F3n para adjuntar informaci\u00F3n adicional a una relaci\u00F3n entre recursos DCAT."@es .
<http://www.w3.org/ns/dcat#Relationship> <http://www.w3.org/2004/02/skos/core#definition> "Una classe di associazione per il collegamento di informazioni aggiuntive a una relazione tra le risorse DCAT."@it .
<http://www.w3.org/ns/dcat#Relationship> <http://www.w3.org/2004/02/skos/core#scopeNote> "Pou\u017E\u00EDv\u00E1 se pro charakterizaci vztahu mezi datov\u00FDmi sadami a p\u0159\u00EDpadn\u011B i jin\u00FDmi zdroji, kde druh vztahu je sice zn\u00E1m, ale nen\u00ED p\u0159im\u011B\u0159en\u011B charakterizov\u00E1n standardn\u00EDmi vlastnostmi slovn\u00EDku Dublin Core (dct:hasPart, dct:isPartOf, dct:conformsTo, dct:isFormatOf, dct:hasFormat, dct:isVersionOf, dct:hasVersion, dct:replaces, dct:isReplacedBy, dct:references, dct:isReferencedBy, dct:requires, dct:isRequiredBy) \u010Di vlastnostmi slovn\u00EDku PROV-O (prov:wasDerivedFrom, prov:wasInfluencedBy, prov:wasQuotedFrom, prov:wasRevisionOf, prov:hadPrimarySource, prov:alternateOf, prov:specializationOf)."@cs .
<http://www.w3.org/ns/dcat#Relationship> <http://www.w3.org/2004/02/skos/core#scopeNote> "Se usa para caracterizar la relaci\u00F3n entre conjuntos de datos, y potencialmente otros recursos, donde la naturaleza de la relaci\u00F3n se conoce pero no est\u00E1 caracterizada adecuadamente con propiedades del est\u00E1ndar 'Dublin Core' (dct:hasPart, dct:isPartOf, dct:conformsTo, dct:isFormatOf, dct:hasFormat, dct:isVersionOf, dct:hasVersion, dct:replaces, dct:isReplacedBy, dct:references, dct:isReferencedBy, dct:requires, dct:isRequiredBy) or PROV-O properties (prov:wasDerivedFrom, prov:wasInfluencedBy, prov:wasQuotedFrom, prov:wasRevisionOf, prov:hadPrimarySource, prov:alternateOf, prov:specializationOf)."@es .
<http://www.w3.org/ns/dcat#Relationship> <http://www.w3.org/2004/02/skos/core#scopeNote> "Use to characterize a relationship between datasets, and potentially other resources, where the nature of the relationship is known but is not adequately characterized by the standard Dublin Core properties (dct:hasPart, dct:isPartOf, dct:conformsTo, dct:isFormatOf, dct:hasFormat, dct:isVersionOf, dct:hasVersion, dct:replaces, dct:isReplacedBy, dct:references, dct:isReferencedBy, dct:requires, dct:isRequiredBy) or PROV-O properties (prov:wasDerivedFrom, prov:wasInfluencedBy, prov:wasQuotedFrom, prov:wasRevisionOf, prov:hadPrimarySource, prov:alternateOf, prov:specializationOf)."@en .
<http://www.w3.org/ns/dcat#Relationship> <http://www.w3.org/2004/02/skos/core#scopeNote> "Viene utilizzato per caratterizzare la relazione tra insiemi di dati, e potenzialmente altri tipi di risorse, nei casi in cui la natura della relazione \u00E8 nota ma non adeguatamente caratterizzata dalle propriet\u00E0 dello standard 'Dublin Core' (dct:hasPart, dct:isPartOf, dct:conformsTo, dct:isFormatOf, dct:hasFormat, dct:isVersionOf, dct:hasVersion, dct:replaces, dct:isReplacedBy, dct:references, dct:isReferencedBy, dct:require, dct:isRequiredBy) o dalle propiet\u00E0 fornite da PROV-O  (prov:wasDerivedFrom, prov:wasInfluencedBy, prov:wasQuotedFrom, prov:wasRevisionOf, prov: hadPrimarySource, prov:alternateOf, prov:specializationOf)."@it .
<http://www.w3.org/ns/dcat#Resource> <http://www.w3.org/1999/02/22-rdf-syntax-ns#type> <http://www.w3.org/2002/07/owl#Class> .
<http://www.w3.org/ns/dcat#Resource> <http://www.w3.org/2000/01/rdf-schema#comment> "Recurso publicado o curado por un agente \u00FAnico."@es .
<http://www.w3.org/ns/dcat#Resource> <http://www.w3.org/2000/01/rdf-schema#comment> "Resource published or curated by a single agent."@en .
<http://www.w3.org/ns/dcat#Resource> <http://www.w3.org/2000/01/rdf-schema#comment> "Risorsa pubblicata o curata da un singolo agente."@it .
<http://www.w3.org/ns/dcat#Resource> <http://www.w3.org/2000/01/rdf-schema#comment> "Zdroj publikovan\u00FD \u010Di \u0159\u00EDzen\u00FD jedin\u00FDm \u010Dinitelem."@cs .
<http://www.w3.org/ns/dcat#Resource> <http://www.w3.org/2000/01/rdf-schema#label> "Catalogued resource"@en .
<http://www.w3.org/ns/dcat#Resource> <http://www.w3.org/2000/01/rdf-schema#label> "Katalogizovan\u00FD zdroj"@cs .
<http://www.w3.org/ns/dcat#Resource> <http://www.w3.org/2000/01/rdf-schema#label> "Recurso catalogado"@es .
<http://www.w3.org/ns/dcat#Resource> <http://www.w3.org/2000/01/rdf-schema#label> "Risorsa catalogata"@it .
<http://www.w3.org/ns/dcat#Resource> <http://www.w3.org/2004/02/skos/core#changeNote> "New class added in DCAT 2.0."@en .
<http://www.w3.org/ns/dcat#Resource> <http://www.w3.org/2004/02/skos/core#changeNote> "Nov\u00E1 t\u0159\u00EDda p\u0159idan\u00E1 ve verzi DCAT 2.0."@cs .
<http://www.w3.org/ns/dcat#Resource> <http://www.w3.org/2004/02/skos/core#changeNote> "Nueva clase agregada en DCAT 2.0."@es .
<http://www.w3.org/ns/dcat#Resource> <http://www.w3.org/2004/02/skos/core#changeNote> "Nuova classe aggiunta in DCAT 2.0."@it .
<http://www.w3.org/ns/dcat#Resource> <http://www.w3.org/2004/02/skos/core#definition> "Recurso publicado o curado por un agente \u00FAnico."@es .
<http://www.w3.org/ns/dcat#Resource> <http://www.w3.org/2004/02/skos/core#definition> "Resource published or curated by a single agent."@en .
<http://www.w3.org/ns/dcat#Resource> <http://www.w3.org/2004/02/skos/core#definition> "Risorsa pubblicata o curata da un singolo agente."@it .
<http://www.w3.org/ns/dcat#Resource> <http://www.w3.org/2004/02/skos/core#definition> "Zdroj publikovan\u00FD \u010Di \u0159\u00EDzen\u00FD jedin\u00FDm \u010Dinitelem."@cs .
<http://www.w3.org/ns/dcat#Resource> <http://www.w3.org/2004/02/skos/core#scopeNote> "La clase de todos los recursos catalogados, la superclase de dcat:Dataset, dcat:DataService, dcat:Catalog y cualquier otro miembro de un dcat:Catalog. Esta clase tiene propiedades comunes a todos los recursos catalogados, incluyendo conjuntos de datos y servicios de datos. Se recomienda fuertemente que se use una clase m\u00E1s espec\u00EDfica. Cuando se describe un recurso que no es un dcat:Dataset o dcat:DataService, se recomienda crear una sub-clase apropiada de dcat:Resource, o usar dcat:Resource con la propiedad dct:type to indicar el tipo espec\u00EDfico."@es .
<http://www.w3.org/ns/dcat#Resource> <http://www.w3.org/2004/02/skos/core#scopeNote> "La classe di tutte le risorse catalogate, la Superclasse di dcat:Dataset, dcat:DataService, dcat:Catalog e qualsiasi altro membro di dcat:Catalog. Questa classe porta propriet\u00E0 comuni a tutte le risorse catalogate, inclusi set di dati e servizi dati. Si raccomanda vivamente di utilizzare una sottoclasse pi\u00F9 specifica. Quando si descrive una risorsa che non \u00E8 un dcat:Dataset o dcat:DataService, si raccomanda di creare una sottoclasse di dcat:Resource appropriata, o utilizzare dcat:Resource con la propriet\u00E0 dct:type per indicare il tipo specifico."@it .
<http://www.w3.org/ns/dcat#Resource> <http://www.w3.org/2004/02/skos/core#scopeNote> "The class of all catalogued resources, the Superclass of dcat:Dataset, dcat:DataService, dcat:Catalog and any other member of a dcat:Catalog. This class carries properties common to all catalogued resources, including datasets and data services. It is strongly recommended to use a more specific sub-class. When describing a resource which is not a dcat:Dataset or dcat:DataService, it is recommended to create a suitable sub-class of dcat:Resource, or use dcat:Resource with the dct:type property to indicate the specific type."@en .
<http://www.w3.org/ns/dcat#Resource> <http://www.w3.org/2004/02/skos/core#scopeNote> "T\u0159\u00EDda v\u0161ech katalogizovan\u00FDch zdroj\u016F, nadt\u0159\u00EDda dcat:Dataset, dcat:DataService, dcat:Catalog a v\u0161ech ostatn\u00EDch \u010Dlen\u016F dcat:Catalog. Tato t\u0159\u00EDda nese vlastnosti spole\u010Dn\u00E9 v\u0161em katalogizovan\u00FDm zdroj\u016Fm v\u010Detn\u011B datov\u00FDch sad a datov\u00FDch slu\u017Eeb. Je siln\u011B doporu\u010Deno pou\u017E\u00EDvat specifi\u010Dt\u011Bj\u0161\u00ED podt\u0159\u00EDdy, pokud je to mo\u017En\u00E9. P\u0159i popisu zdroje, kter\u00FD nen\u00ED ani dcat:Dataset, ani dcat:DataService se doporu\u010Duje vytvo\u0159it odpov\u00EDdaj\u00EDc\u00ED podt\u0159\u00EDdu dcat:Resrouce a nebo pou\u017E\u00EDt dcat:Resource s vlastnost\u00ED dct:type pro ur\u010Den\u00ED konkr\u00E9tn\u00EDho typu."@cs .
<http://www.w3.org/ns/dcat#Resource> <http://www.w3.org/2004/02/skos/core#scopeNote> "dcat:Resource es un punto de extensi\u00F3n que permite la definici\u00F3n de cualquier tipo de cat\u00E1logo. Se pueden definir subclases adicionales en perfil de DCAT o una aplicaci\u00F3n para cat\u00E1logos de otro tipo de recursos."@es .
<http://www.w3.org/ns/dcat#Resource> <http://www.w3.org/2004/02/skos/core#scopeNote> "dcat:Resource is an extension point that enables the definition of any kind of catalog. Additional subclasses may be defined in a DCAT profile or application for catalogs of other kinds of resources."@en .
<http://www.w3.org/ns/dcat#Resource> <http://www.w3.org/2004/02/skos/core#scopeNote> "dcat:Resource je bod pro roz\u0161\u00ED\u0159en\u00ED umo\u017E\u0148uj\u00EDc\u00ED definici r\u016Fzn\u00FDch druh\u016F katalog\u016F. Dal\u0161\u00ED podt\u0159\u00EDdy lze definovat v profilech DCAT \u010Di aplikac\u00EDch pro katalogy zdroj\u016F jin\u00FDch druh\u016F."@cs .
<http://www.w3.org/ns/dcat#Resource> <http://www.w3.org/2004/02/skos/core#scopeNote> "dcat:Resource \u00E8 un punto di estensione che consente la definizione di qualsiasi tipo di catalogo. Sottoclassi aggiuntive possono essere definite in un profilo DCAT o in un'applicazione per cataloghi di altri tipi di risorse."@it .
<http://www.w3.org/ns/dcat#Role> <http://www.w3.org/1999/02/22-rdf-syntax-ns#type> <http://www.w3.org/2002/07/owl#Class> .
<http://www.w3.org/ns/dcat#Role> <http://www.w3.org/2000/01/rdf-schema#comment> "A role is the function of a resource or agent with respect to another resource, in the context of resource attribution or resource relationships."@en .
<http://www.w3.org/ns/dcat#Role> <http://www.w3.org/2000/01/rdf-schema#comment> "Role je funkce zdroje \u010Di agenta ve vztahu k jin\u00E9mu zdroji, v kontextu p\u0159i\u0159azen\u00ED zdroj\u016F \u010Di vztah\u016F mezi zdroji."@cs .
<http://www.w3.org/ns/dcat#Role> <http://www.w3.org/2000/01/rdf-schema#comment> "Un rol es la funci\u00F3n de un recurso o agente con respecto a otro recuros, en el contexto de atribuci\u00F3n del recurso o de las relaciones entre recursos."@es .
<http://www.w3.org/ns/dcat#Role> <http://www.w3.org/2000/01/rdf-schema#comment> "Un ruolo \u00E8 la funzione di una risorsa o di un agente rispetto ad un'altra risorsa, nel contesto dell'attribuzione delle risorse o delle relazioni tra risorse."@it .
<http://www.w3.org/ns/dcat#Role> <http://www.w3.org/2000/01/rdf-schema#label> "Rol"@es .
<http://www.w3.org/ns/dcat#Role> <http://www.w3.org/2000/01/rdf-schema#label> "Role"@cs .
<http://www.w3.org/ns/dcat#Role> <http://www.w3.org/2000/01/rdf-schema#label> "Role"@en .
<http://www.w3.org/ns/dcat#Role> <http://www.w3.org/2000/01/rdf-schema#label> "Ruolo"@it .
<http://www.w3.org/ns/dcat#Role> <http://www.w3.org/2000/01/rdf-schema#seeAlso> <http://www.w3.org/ns/dcat#hadRole> .
<http://www.w3.org/ns/dcat#Role> <http://www.w3.org/2000/01/rdf-schema#subClassOf> <http://www.w3.org/2004/02/skos/core#Concept> .
<http://www.w3.org/ns/dcat#Role> <http://www.w3.org/2004/02/skos/core#changeNote> "New class added in DCAT 2.0."@en .
<http://www.w3.org/ns/dcat#Role> <http://www.w3.org/2004/02/skos/core#changeNote> "Nov\u00E1 t\u0159\u00EDda p\u0159idan\u00E1 ve verzi DCAT 2.0."@cs .
<http://www.w3.org/ns/dcat#Role> <http://www.w3.org/2004/02/skos/core#changeNote> "Nueva clase agregada en DCAT 2.0."@es .
<http://www.w3.org/ns/dcat#Role> <http://www.w3.org/2004/02/skos/core#changeNote> "Nuova classe aggiunta in DCAT 2.0."@it .
<http://www.w3.org/ns/dcat#Role> <http://www.w3.org/2004/02/skos/core#definition> "A role is the function of a resource or agent with respect to another resource, in the context of resource attribution or resource relationships."@en .
<http://www.w3.org/ns/dcat#Role> <http://www.w3.org/2004/02/skos/core#definition> "Role je funkce zdroje \u010Di agenta ve vztahu k jin\u00E9mu zdroji, v kontextu p\u0159i\u0159azen\u00ED zdroj\u016F \u010Di vztah\u016F mezi zdroji."@cs .
<http://www.w3.org/ns/dcat#Role> <http://www.w3.org/2004/02/skos/core#definition> "Un rol es la funci\u00F3n de un recurso o agente con respecto a otro recuros, en el contexto de atribuci\u00F3n del recurso o de las relaciones entre recursos."@es .
<http://www.w3.org/ns/dcat#Role> <http://www.w3.org/2004/02/skos/core#definition> "Un ruolo \u00E8 la funzione di una risorsa o di un agente rispetto ad un'altra risorsa, nel contesto dell'attribuzione delle risorse o delle relazioni tra risorse."@it .
<http://www.w3.org/ns/dcat#Role> <http://www.w3.org/2004/02/skos/core#editorialNote> "Inclu\u00EDda en DCAT para complementar prov:Role (cuyo uso est\u00E1 limitado a roles en el contexto de una actividad, ya que es el rango es prov:hadRole)."@es .
<http://www.w3.org/ns/dcat#Role> <http://www.w3.org/2004/02/skos/core#editorialNote> "Introdotta in DCAT per completare prov:Role (il cui uso \u00E8 limitato ai ruoli nel contesto di un'attivit\u00E0, in conseguenza alla definizione del codominio di prov:hadRole)."@it .
<http://www.w3.org/ns/dcat#Role> <http://www.w3.org/2004/02/skos/core#editorialNote> "Introduced into DCAT to complement prov:Role (whose use is limited to roles in the context of an activity, as the range of prov:hadRole)."@en .
<http://www.w3.org/ns/dcat#Role> <http://www.w3.org/2004/02/skos/core#editorialNote> "P\u0159id\u00E1no do DCAT pro dopln\u011Bn\u00ED t\u0159\u00EDdy prov:Role (jej\u00ED\u017E u\u017Eit\u00ED je omezeno na role v kontextu aktivit, jako\u017Eto obor hodnot vlastnosti prov:hadRole)."@cs .
<http://www.w3.org/ns/dcat#Role> <http://www.w3.org/2004/02/skos/core#scopeNote> "Pou\u017Eito v kvalifikovan\u00E9m p\u0159i\u0159azen\u00ED pro specifikaci role Agenta ve vztahu k Entit\u011B. Je doporu\u010Deno mno\u017Einu hodnot spravovat jako \u0159\u00EDzen\u00FD slovn\u00EDk rol\u00ED agent\u016F, jako nap\u0159\u00EDklad http://registry.it.csiro.au/def/isotc211/CI_RoleCode."@cs .
<http://www.w3.org/ns/dcat#Role> <http://www.w3.org/2004/02/skos/core#scopeNote> "Pou\u017Eito v kvalifikovan\u00E9m vztahu pro specifikaci role Entity ve vztahu k jin\u00E9 Entit\u011B. Je doporu\u010Deno mno\u017Einu hodnot spravovat jako \u0159\u00EDzen\u00FD slovn\u00EDk rol\u00ED entit, jako nap\u0159\u00EDklad ISO 19115 DS_AssociationTypeCode http://registry.it.csiro.au/def/isotc211/DS_AssociationTypeCode, IANA Registry of Link Relations https://www.iana.org/assignments/link-relation, DataCite metadata schema, \u010Di MARC relators https://id.loc.gov/vocabulary/relators."@cs .
<http://www.w3.org/ns/dcat#Role> <http://www.w3.org/2004/02/skos/core#scopeNote> "Se usa en una atribuci\u00F3n cualificada para especificar el rol de un Agente con respecto a una Entidad. Se recomienda que los valores se administren como un vocabulario controlado de roles de agente, como por ejemplo http://registry.it.csiro.au/def/isotc211/CI_RoleCode."@es .
<http://www.w3.org/ns/dcat#Role> <http://www.w3.org/2004/02/skos/core#scopeNote> "Se usa en una relaci\u00F3n cualificada para especificar el rol de una Entidad con respecto a otra Entidad. Se recomienda que los valores se administren como los valores de un vocabulario controlado de roles de entidad como por ejemplo: ISO 19115 DS_AssociationTypeCode http://registry.it.csiro.au/def/isotc211/DS_AssociationTypeCode; IANA Registry of Link Relations https://www.iana.org/assignments/link-relation; el esquema de metadatos de DataCite; MARC relators https://id.loc.gov/vocabulary/relators."@es .
<http://www.w3.org/ns/dcat#Role> <http://www.w3.org/2004/02/skos/core#scopeNote> "Used in a qualified-attribution to specify the role of an Agent with respect to an Entity. It is recommended that the values be managed as a controlled vocabulary of agent roles, such as http://registry.it.csiro.au/def/isotc211/CI_RoleCode."@en .
<http://www.w3.org/ns/dcat#Role> <http://www.w3.org/2004/02/skos/core#scopeNote> "Used in a qualified-relation to specify the role of an Entity with respect to another Entity. It is recommended that the values be managed as a controlled vocabulary of entity roles such as: ISO 19115 DS_AssociationTypeCode http://registry.it.csiro.au/def/isotc211/DS_AssociationTypeCode; IANA Registry of Link Relations https://www.iana.org/assignments/link-relation;  DataCite metadata schema;  MARC relators https://id.loc.gov/vocabulary/relators."@en .
<http://www.w3.org/ns/dcat#Role> <http://www.w3.org/2004/02/skos/core#scopeNote> "Utilizzato in un'attribuzione qualificata per specificare il ruolo di un agente rispetto a un'entit\u00E0. Si consiglia di attribuire i valori considerando un vocabolario controllato dei ruoli dell'agente, ad esempio http://registry.it.csiro.au/def/isotc211/CI_RoleCode."@it .
<http://www.w3.org/ns/dcat#Role> <http://www.w3.org/2004/02/skos/core#scopeNote> "Utilizzato in una relazione qualificata per specificare il ruolo di un'entit\u00E0 rispetto a un'altra entit\u00E0. Si raccomanda che il valore sia preso da un vocabolario controllato di ruoli di entit\u00E0 come ISO 19115 DS_AssociationTypeCode http://registry.it.csiro.au/def/isotc211/DS_AssociationTypeCode, IANA Registry of Link Relations https://www.iana.org/assignments/link-relation, DataCite metadata schema, o MARC relators https://id.loc.gov/vocabulary/relators."@it .
<http://www.w3.org/ns/dcat#accessService> <http://www.w3.org/1999/02/22-rdf-syntax-ns#type> <http://www.w3.org/2002/07/owl#ObjectProperty> .
<http://www.w3.org/ns/dcat#accessService> <http://www.w3.org/2000/01/rdf-schema#comment> "A site or end-point that gives access to the distribution of the dataset."@en .
<http://www.w3.org/ns/dcat#accessService> <http://www.w3.org/2000/01/rdf-schema#comment> "Um\u00EDst\u011Bn\u00ED \u010Di p\u0159\u00EDstupov\u00FD bod zp\u0159\u00EDstup\u0148uj\u00EDc\u00ED distribuci datov\u00E9 sady."@cs .
<http://www.w3.org/ns/dcat#accessService> <http://www.w3.org/2000/01/rdf-schema#comment> "Un sitio o end-point que da acceso a la distribuci\u00F3n de un conjunto de datos."@es .
<http://www.w3.org/ns/dcat#accessService> <http://www.w3.org/2000/01/rdf-schema#comment> "Un sito o end-point che d\u00E0 accesso alla distribuzione del set di dati."@it .
<http://www.w3.org/ns/dcat#accessService> <http://www.w3.org/2000/01/rdf-schema#label> "data access service"@en .
<http://www.w3.org/ns/dcat#accessService> <http://www.w3.org/2000/01/rdf-schema#label> "servicio de acceso de datos"@es .
<http://www.w3.org/ns/dcat#accessService> <http://www.w3.org/2000/01/rdf-schema#label> "servizio di accesso ai dati"@it .
<http://www.w3.org/ns/dcat#accessService> <http://www.w3.org/2000/01/rdf-schema#label> "slu\u017Eba pro p\u0159\u00EDstup k dat\u016Fm"@cs .
<http://www.w3.org/ns/dcat#accessService> <http://www.w3.org/2000/01/rdf-schema#range> <http://www.w3.org/ns/dcat#DataService> .
<http://www.w3.org/ns/dcat#accessService> <http://www.w3.org/2004/02/skos/core#changeNote> "New property added in DCAT 2.0."@en .
<http://www.w3.org/ns/dcat#accessService> <http://www.w3.org/2004/02/skos/core#changeNote> "Nov\u00E1 vlastnost p\u0159idan\u00E1 ve verzi DCAT 2.0."@cs .
<http://www.w3.org/ns/dcat#accessService> <http://www.w3.org/2004/02/skos/core#changeNote> "Nueva propiedad agregada en DCAT 2.0."@es .
<http://www.w3.org/ns/dcat#accessService> <http://www.w3.org/2004/02/skos/core#changeNote> "Nuova propriet\u00E0 aggiunta in DCAT 2.0."@it .
<http://www.w3.org/ns/dcat#accessService> <http://www.w3.org/2004/02/skos/core#definition> "A site or end-point that gives access to the distribution of the dataset."@en .
<http://www.w3.org/ns/dcat#accessService> <http://www.w3.org/2004/02/skos/core#definition> "Um\u00EDst\u011Bn\u00ED \u010Di p\u0159\u00EDstupov\u00FD bod zp\u0159\u00EDstup\u0148uj\u00EDc\u00ED distribuci datov\u00E9 sady."@cs .
<http://www.w3.org/ns/dcat#accessService> <http://www.w3.org/2004/02/skos/core#definition> "Un sitio o end-point que da acceso a la distribuci\u00F3n de un conjunto de datos."@es .
<http://www.w3.org/ns/dcat#accessService> <http://www.w3.org/2004/02/skos/core#definition> "Un sito o end-point che d\u00E0 accesso alla distribuzione del set di dati."@it .
_:genid30 <http://www.w3.org/1999/02/22-rdf-syntax-ns#first> <http://www.w3.org/ns/dcat#endpointURL> .
_:genid30 <http://www.w3.org/1999/02/22-rdf-syntax-ns#rest> <http://www.w3.org/1999/02/22-rdf-syntax-ns#nil> .
_:genid31 <http://www.w3.org/1999/02/22-rdf-syntax-ns#first> <http://www.w3.org/ns/dcat#accessService> .
_:genid31 <http://www.w3.org/1999/02/22-rdf-syntax-ns#rest> _:genid30 .
<http://www.w3.org/ns/dcat#accessURL> <http://www.w3.org/1999/02/22-rdf-syntax-ns#type> <http://www.w3.org/1999/02/22-rdf-syntax-ns#Property> .
<http://www.w3.org/ns/dcat#accessURL> <http://www.w3.org/1999/02/22-rdf-syntax-ns#type> <http://www.w3.org/2002/07/owl#ObjectProperty> .
<http://www.w3.org/ns/dcat#accessURL> <http://www.w3.org/2000/01/rdf-schema#comment> "A URL of a resource that gives access to a distribution of the dataset. E.g. landing page, feed, SPARQL endpoint. Use for all cases except a simple download link, in which case downloadURL is preferred."@en .
<http://www.w3.org/ns/dcat#accessURL> <http://www.w3.org/2000/01/rdf-schema#comment> "Ceci peut \u00EAtre tout type d'URL qui donne acc\u00E8s \u00E0 une distribution du jeu de donn\u00E9es. Par exemple, un lien \u00E0 une page HTML contenant un lien au jeu de donn\u00E9es, un Flux RSS, un point d'acc\u00E8s SPARQL. Utilisez le lorsque votre catalogue ne contient pas d'information sur quoi il est ou quand ce n'est pas t\u00E9l\u00E9chargeable."@fr .
<http://www.w3.org/ns/dcat#accessURL> <http://www.w3.org/2000/01/rdf-schema#comment> "Puede ser cualquier tipo de URL que de acceso a una distribuci\u00F3n del conjunto de datos, e.g., p\u00E1gina de destino, descarga, URL feed, punto de acceso SPARQL. Esta propriedad se debe usar cuando su cat\u00E1logo de datos no tiene informaci\u00F3n sobre donde est\u00E1 o cuando no se puede descargar."@es .
<http://www.w3.org/ns/dcat#accessURL> <http://www.w3.org/2000/01/rdf-schema#comment> "URL zdroje, p\u0159es kter\u00E9 je p\u0159\u00EDstupn\u00E1 distribuce datov\u00E9 sady. P\u0159\u00EDkladem m\u016F\u017Ee b\u00FDt vstupn\u00ED str\u00E1nka, RSS kan\u00E1l \u010Di SPARQL endpoint. Pou\u017Eijte ve v\u0161ech p\u0159\u00EDpadech krom\u011B URL souboru ke sta\u017Een\u00ED, pro kter\u00E9 je lep\u0161\u00ED pou\u017E\u00EDt dcat:downloadURL."@cs .
<http://www.w3.org/ns/dcat#accessURL> <http://www.w3.org/2000/01/rdf-schema#comment> "Un URL di una risorsa che consente di accedere a una distribuzione del set di dati. Per esempio, pagina di destinazione, feed, endpoint SPARQL. Da utilizzare per tutti i casi, tranne  quando  si tratta di un semplice link per il download nel qual caso \u00E8 preferito downloadURL."@it .
<http://www.w3.org/ns/dcat#accessURL> <http://www.w3.org/2000/01/rdf-schema#comment> "\u039C\u03C0\u03BF\u03C1\u03B5\u03AF \u03BD\u03B1 \u03B5\u03AF\u03BD\u03B1\u03B9 \u03BF\u03C0\u03BF\u03B9\u03BF\u03C5\u03B4\u03AE\u03C0\u03BF\u03C4\u03B5 \u03B5\u03AF\u03B4\u03BF\u03C5\u03C2 URL \u03C0\u03BF\u03C5 \u03B4\u03AF\u03BD\u03B5\u03B9 \u03C0\u03C1\u03CC\u03C3\u03B2\u03B1\u03C3\u03B7 \u03C3\u03C4\u03B7 \u03B4\u03B9\u03B1\u03BD\u03BF\u03BC\u03AE \u03B5\u03BD\u03CC\u03C2 \u03C3\u03C5\u03BD\u03CC\u03BB\u03BF\u03C5 \u03B4\u03B5\u03B4\u03BF\u03BC\u03AD\u03BD\u03C9\u03BD. \u03A0.\u03C7. \u03B9\u03C3\u03C4\u03BF\u03C3\u03B5\u03BB\u03AF\u03B4\u03B1 \u03B1\u03C1\u03C7\u03B9\u03BA\u03AE\u03C2 \u03C0\u03C1\u03CC\u03C3\u03B2\u03B1\u03C3\u03B7\u03C2, \u03BC\u03B5\u03C4\u03B1\u03C6\u03CC\u03C1\u03C4\u03C9\u03C3\u03B7, feed URL, \u03C3\u03B7\u03BC\u03B5\u03AF\u03BF \u03B4\u03B9\u03AC\u03B8\u03B5\u03C3\u03B7\u03C2 SPARQL. \u039D\u03B1 \u03C7\u03C1\u03B7\u03C3\u03B9\u03BC\u03BF\u03C0\u03BF\u03B9\u03B5\u03AF\u03C4\u03B1\u03B9 \u03CC\u03C4\u03B1\u03BD \u03BF \u03BA\u03B1\u03C4\u03AC\u03BB\u03BF\u03B3\u03BF\u03C2 \u03B4\u03B5\u03BD \u03C0\u03B5\u03C1\u03B9\u03AD\u03C7\u03B5\u03B9 \u03C0\u03BB\u03B7\u03C1\u03BF\u03C6\u03BF\u03C1\u03AF\u03B5\u03C2 \u03B5\u03B1\u03BD \u03C0\u03C1\u03CC\u03BA\u03B5\u03B9\u03C4\u03B1\u03B9 \u03AE \u03CC\u03C7\u03B9 \u03B3\u03B9\u03B1 \u03BC\u03B5\u03C4\u03B1\u03C6\u03BF\u03C1\u03C4\u03CE\u03C3\u03B9\u03BC\u03BF \u03B1\u03C1\u03C7\u03B5\u03AF\u03BF."@el .
<http://www.w3.org/ns/dcat#accessURL> <http://www.w3.org/2000/01/rdf-schema#comment> "\u0623\u064A \u0631\u0627\u0628\u0637 \u064A\u062A\u064A\u062D \u0627\u0644\u0648\u0635\u0648\u0644 \u0625\u0644\u0649 \u0627\u0644\u0628\u064A\u0627\u0646\u0627\u062A. \u0625\u0630\u0627 \u0643\u0627\u0646 \u0627\u0644\u0631\u0627\u0628\u0637 \u0647\u0648 \u0631\u0628\u0637 \u0645\u0628\u0627\u0634\u0631 \u0644\u0645\u0644\u0641 \u064A\u0645\u0643\u0646 \u062A\u062D\u0645\u064A\u0644\u0647 \u0627\u0633\u062A\u062E\u062F\u0645 \u0627\u0644\u062E\u0627\u0635\u064A\u0629 downloadURL"@ar .
<http://www.w3.org/ns/dcat#accessURL> <http://www.w3.org/2000/01/rdf-schema#comment> "\u30C7\u30FC\u30BF\u30BB\u30C3\u30C8\u306E\u914D\u4FE1\u306B\u30A2\u30AF\u30BB\u30B9\u6A29\u3092\u4E0E\u3048\u308B\u30E9\u30F3\u30C7\u30A3\u30F3\u30B0\u30FB\u30DA\u30FC\u30B8\u3001\u30D5\u30A3\u30FC\u30C9\u3001SPARQL\u30A8\u30F3\u30C9\u30DD\u30A4\u30F3\u30C8\u3001\u305D\u306E\u4ED6\u306E\u7A2E\u985E\u306E\u8CC7\u6E90\u3002"@ja .
<http://www.w3.org/ns/dcat#accessURL> <http://www.w3.org/2000/01/rdf-schema#domain> <http://www.w3.org/ns/dcat#Distribution> .
<http://www.w3.org/ns/dcat#accessURL> <http://www.w3.org/2000/01/rdf-schema#isDefinedBy> <http://www.w3.org/TR/vocab-dcat/> .
<http://www.w3.org/ns/dcat#accessURL> <http://www.w3.org/2000/01/rdf-schema#label> "URL d'acc\u00E8s"@fr .
<http://www.w3.org/ns/dcat#accessURL> <http://www.w3.org/2000/01/rdf-schema#label> "URL de acceso"@es .
<http://www.w3.org/ns/dcat#accessURL> <http://www.w3.org/2000/01/rdf-schema#label> "URL \u03C0\u03C1\u03CC\u03C3\u03B2\u03B1\u03C3\u03B7\u03C2"@el .
<http://www.w3.org/ns/dcat#accessURL> <http://www.w3.org/2000/01/rdf-schema#label> "access address"@en .
<http://www.w3.org/ns/dcat#accessURL> <http://www.w3.org/2000/01/rdf-schema#label> "indirizzo di accesso"@it .
<http://www.w3.org/ns/dcat#accessURL> <http://www.w3.org/2000/01/rdf-schema#label> "p\u0159\u00EDstupov\u00E1 adresa"@cs .
<http://www.w3.org/ns/dcat#accessURL> <http://www.w3.org/2000/01/rdf-schema#label> "\u0631\u0627\u0628\u0637 \u0648\u0635\u0648\u0644"@ar .
<http://www.w3.org/ns/dcat#accessURL> <http://www.w3.org/2000/01/rdf-schema#label> "\u30A2\u30AF\u30BB\u30B9URL"@ja .
<http://www.w3.org/ns/dcat#accessURL> <http://www.w3.org/2000/01/rdf-schema#range> <http://www.w3.org/2000/01/rdf-schema#Resource> .
<http://www.w3.org/ns/dcat#accessURL> <http://www.w3.org/2002/07/owl#propertyChainAxiom> _:genid31 .
<http://www.w3.org/ns/dcat#accessURL> <http://www.w3.org/2004/02/skos/core#definition> "A URL of a resource that gives access to a distribution of the dataset. E.g. landing page, feed, SPARQL endpoint. Use for all cases except a simple download link, in which case downloadURL is preferred."@en .
<http://www.w3.org/ns/dcat#accessURL> <http://www.w3.org/2004/02/skos/core#definition> "Ceci peut \u00EAtre tout type d'URL qui donne acc\u00E8s \u00E0 une distribution du jeu de donn\u00E9es. Par exemple, un lien \u00E0 une page HTML contenant un lien au jeu de donn\u00E9es, un Flux RSS, un point d'acc\u00E8s SPARQL. Utilisez le lorsque votre catalogue ne contient pas d'information sur quoi il est ou quand ce n'est pas t\u00E9l\u00E9chargeable."@fr .
<http://www.w3.org/ns/dcat#accessURL> <http://www.w3.org/2004/02/skos/core#definition> "Puede ser cualquier tipo de URL que de acceso a una distribuci\u00F3n del conjunto de datos, e.g., p\u00E1gina de destino, descarga, URL feed, punto de acceso SPARQL. Esta propriedad se debe usar cuando su cat\u00E1logo de datos no tiene informaci\u00F3n sobre donde est\u00E1 o cuando no se puede descargar."@es .
<http://www.w3.org/ns/dcat#accessURL> <http://www.w3.org/2004/02/skos/core#definition> "URL zdroje, p\u0159es kter\u00E9 je p\u0159\u00EDstupn\u00E1 distribuce datov\u00E9 sady. P\u0159\u00EDkladem m\u016F\u017Ee b\u00FDt vstupn\u00ED str\u00E1nka, RSS kan\u00E1l \u010Di SPARQL endpoint. Pou\u017Eijte ve v\u0161ech p\u0159\u00EDpadech krom\u011B URL souboru ke sta\u017Een\u00ED, pro kter\u00E9 je lep\u0161\u00ED pou\u017E\u00EDt dcat:downloadURL."@cs .
<http://www.w3.org/ns/dcat#accessURL> <http://www.w3.org/2004/02/skos/core#definition> "Un URL di una risorsa che consente di accedere a una distribuzione del set di dati. Per esempio, pagina di destinazione, feed, endpoint SPARQL. Da utilizzare per tutti i casi, tranne  quando  si tratta di un semplice link per il download nel qual caso \u00E8 preferito downloadURL."@it .
<http://www.w3.org/ns/dcat#accessURL> <http://www.w3.org/2004/02/skos/core#definition> "\u039C\u03C0\u03BF\u03C1\u03B5\u03AF \u03BD\u03B1 \u03B5\u03AF\u03BD\u03B1\u03B9 \u03BF\u03C0\u03BF\u03B9\u03BF\u03C5\u03B4\u03AE\u03C0\u03BF\u03C4\u03B5 \u03B5\u03AF\u03B4\u03BF\u03C5\u03C2 URL \u03C0\u03BF\u03C5 \u03B4\u03AF\u03BD\u03B5\u03B9 \u03C0\u03C1\u03CC\u03C3\u03B2\u03B1\u03C3\u03B7 \u03C3\u03C4\u03B7 \u03B4\u03B9\u03B1\u03BD\u03BF\u03BC\u03AE \u03B5\u03BD\u03CC\u03C2 \u03C3\u03C5\u03BD\u03CC\u03BB\u03BF\u03C5 \u03B4\u03B5\u03B4\u03BF\u03BC\u03AD\u03BD\u03C9\u03BD. \u03A0.\u03C7. \u03B9\u03C3\u03C4\u03BF\u03C3\u03B5\u03BB\u03AF\u03B4\u03B1 \u03B1\u03C1\u03C7\u03B9\u03BA\u03AE\u03C2 \u03C0\u03C1\u03CC\u03C3\u03B2\u03B1\u03C3\u03B7\u03C2, \u03BC\u03B5\u03C4\u03B1\u03C6\u03CC\u03C1\u03C4\u03C9\u03C3\u03B7, feed URL, \u03C3\u03B7\u03BC\u03B5\u03AF\u03BF \u03B4\u03B9\u03AC\u03B8\u03B5\u03C3\u03B7\u03C2 SPARQL. \u039D\u03B1 \u03C7\u03C1\u03B7\u03C3\u03B9\u03BC\u03BF\u03C0\u03BF\u03B9\u03B5\u03AF\u03C4\u03B1\u03B9 \u03CC\u03C4\u03B1\u03BD \u03BF \u03BA\u03B1\u03C4\u03AC\u03BB\u03BF\u03B3\u03BF\u03C2 \u03B4\u03B5\u03BD \u03C0\u03B5\u03C1\u03B9\u03AD\u03C7\u03B5\u03B9 \u03C0\u03BB\u03B7\u03C1\u03BF\u03C6\u03BF\u03C1\u03AF\u03B5\u03C2 \u03B5\u03B1\u03BD \u03C0\u03C1\u03CC\u03BA\u03B5\u03B9\u03C4\u03B1\u03B9 \u03AE \u03CC\u03C7\u03B9 \u03B3\u03B9\u03B1 \u03BC\u03B5\u03C4\u03B1\u03C6\u03BF\u03C1\u03C4\u03CE\u03C3\u03B9\u03BC\u03BF \u03B1\u03C1\u03C7\u03B5\u03AF\u03BF."@el .
<http://www.w3.org/ns/dcat#accessURL> <http://www.w3.org/2004/02/skos/core#definition> "\u0623\u064A \u0631\u0627\u0628\u0637 \u064A\u062A\u064A\u062D \u0627\u0644\u0648\u0635\u0648\u0644 \u0625\u0644\u0649 \u0627\u0644\u0628\u064A\u0627\u0646\u0627\u062A. \u0625\u0630\u0627 \u0643\u0627\u0646 \u0627\u0644\u0631\u0627\u0628\u0637 \u0647\u0648 \u0631\u0628\u0637 \u0645\u0628\u0627\u0634\u0631 \u0644\u0645\u0644\u0641 \u064A\u0645\u0643\u0646 \u062A\u062D\u0645\u064A\u0644\u0647 \u0627\u0633\u062A\u062E\u062F\u0645 \u0627\u0644\u062E\u0627\u0635\u064A\u0629 downloadURL"@ar .
<http://www.w3.org/ns/dcat#accessURL> <http://www.w3.org/2004/02/skos/core#definition> "\u30C7\u30FC\u30BF\u30BB\u30C3\u30C8\u306E\u914D\u4FE1\u306B\u30A2\u30AF\u30BB\u30B9\u6A29\u3092\u4E0E\u3048\u308B\u30E9\u30F3\u30C7\u30A3\u30F3\u30B0\u30FB\u30DA\u30FC\u30B8\u3001\u30D5\u30A3\u30FC\u30C9\u3001SPARQL\u30A8\u30F3\u30C9\u30DD\u30A4\u30F3\u30C8\u3001\u305D\u306E\u4ED6\u306E\u7A2E\u985E\u306E\u8CC7\u6E90\u3002"@ja .
<http://www.w3.org/ns/dcat#accessURL> <http://www.w3.org/2004/02/skos/core#editorialNote> "Status: English Definition text modified by DCAT revision team, updated Italian and Czech translation provided, translations for other languages pending."@en .
<http://www.w3.org/ns/dcat#accessURL> <http://www.w3.org/2004/02/skos/core#editorialNote> "rdfs:label, rdfs:comment and skos:scopeNote have been modified. Non-english versions except for Italian must be updated."@en .
<http://www.w3.org/ns/dcat#accessURL> <http://www.w3.org/2004/02/skos/core#scopeNote> "El rango es una URL. Si la distribuci\u00F3n es accesible solamente trav\u00E9s de una p\u00E1gina de destino (es decir, si no se conoce una URL de descarga directa), entonces el enlance a la p\u00E1gina de destino debe ser duplicado como accessURL en la distribuci\u00F3n."@es .
<http://www.w3.org/ns/dcat#accessURL> <http://www.w3.org/2004/02/skos/core#scopeNote> "If the distribution(s) are accessible only through a landing page (i.e. direct download URLs are not known), then the landing page link should be duplicated as accessURL on a distribution."@en .
<http://www.w3.org/ns/dcat#accessURL> <http://www.w3.org/2004/02/skos/core#scopeNote> "La valeur est une URL. Si la distribution est accessible seulement au travers d'une page d'atterrissage (c-\u00E0-dire on n'ignore une URL de t\u00E9l\u00E9chargement direct), alors le lien \u00E0 la page d'atterrissage doit \u00EAtre dupliqu\u00E9 comee accessURL sur la distribution."@fr .
<http://www.w3.org/ns/dcat#accessURL> <http://www.w3.org/2004/02/skos/core#scopeNote> "Pokud jsou distribuce p\u0159\u00EDstupn\u00E9 pouze p\u0159es vstupn\u00ED str\u00E1nku (tj. URL pro p\u0159\u00EDm\u00E9 sta\u017Een\u00ED nejsou zn\u00E1ma), pak by URL p\u0159\u00EDstupov\u00E9 str\u00E1nky m\u011Blo b\u00FDt duplikov\u00E1no ve vlastnosti distribuce accessURL."@cs .
<http://www.w3.org/ns/dcat#accessURL> <http://www.w3.org/2004/02/skos/core#scopeNote> "Se le distribuzioni sono accessibili solo attraverso una pagina web (ad esempio, gli URL per il download diretto non sono noti), allora il link della pagina web deve essere duplicato come accessURL sulla distribuzione."@it .
<http://www.w3.org/ns/dcat#accessURL> <http://www.w3.org/2004/02/skos/core#scopeNote> "\u0397 \u03C4\u03B9\u03BC\u03AE \u03B5\u03AF\u03BD\u03B1\u03B9 \u03AD\u03BD\u03B1 URL. \u0391\u03BD \u03B7/\u03BF\u03B9 \u03B4\u03B9\u03B1\u03BD\u03BF\u03BC\u03AE/\u03AD\u03C2 \u03B5\u03AF\u03BD\u03B1\u03B9 \u03C0\u03C1\u03BF\u03C3\u03B2\u03AC\u03C3\u03B9\u03BC\u03B7/\u03B5\u03C2 \u03BC\u03CC\u03BD\u03BF \u03BC\u03AD\u03C3\u03C9 \u03BC\u03AF\u03B1\u03C2 \u03B9\u03C3\u03C4\u03BF\u03C3\u03B5\u03BB\u03AF\u03B4\u03B1\u03C2 \u03B1\u03C1\u03C7\u03B9\u03BA\u03AE\u03C2 \u03C0\u03C1\u03CC\u03C3\u03B2\u03B1\u03C3\u03B7\u03C2 (\u03B4\u03B7\u03BB\u03B1\u03B4\u03AE \u03B1\u03BD \u03B4\u03B5\u03BD \u03C5\u03C0\u03AC\u03C1\u03C7\u03BF\u03C5\u03BD \u03B3\u03BD\u03C9\u03C3\u03C4\u03AD\u03C2 \u03B4\u03B9\u03B5\u03C5\u03B8\u03CD\u03BD\u03C3\u03B5\u03B9\u03C2 \u03AC\u03BC\u03B5\u03C3\u03B7\u03C2 \u03BC\u03B5\u03C4\u03B1\u03C6\u03CC\u03C1\u03C4\u03C9\u03C3\u03B7\u03C2), \u03C4\u03CC\u03C4\u03B5 \u03BF \u03C3\u03CD\u03BD\u03B4\u03B5\u03C3\u03BC\u03BF\u03C2 \u03C4\u03B7\u03C2 \u03B9\u03C3\u03C4\u03BF\u03C3\u03B5\u03BB\u03AF\u03B4\u03B1\u03C2 \u03B1\u03C1\u03C7\u03B9\u03BA\u03AE\u03C2 \u03C0\u03C1\u03CC\u03C3\u03B2\u03B1\u03C3\u03B7\u03C2 \u03C0\u03C1\u03AD\u03C0\u03B5\u03B9 \u03BD\u03B1 \u03B1\u03BD\u03B1\u03C0\u03B1\u03C1\u03B1\u03C7\u03B8\u03B5\u03AF \u03C9\u03C2 accessURL \u03C3\u03B5 \u03BC\u03AF\u03B1 \u03B4\u03B9\u03B1\u03BD\u03BF\u03BC\u03AE."@el .
<http://www.w3.org/ns/dcat#accessURL> <http://www.w3.org/2004/02/skos/core#scopeNote> "\u78BA\u5B9F\u306B\u30C0\u30A6\u30F3\u30ED\u30FC\u30C9\u3067\u306A\u3044\u5834\u5408\u3084\u3001\u30C0\u30A6\u30F3\u30ED\u30FC\u30C9\u304B\u3069\u3046\u304B\u304C\u4E0D\u660E\u3067\u3042\u308B\u5834\u5408\u306F\u3001downloadURL\u3067\u306F\u306A\u304F\u3001accessURL\u3092\u7528\u3044\u3066\u304F\u3060\u3055\u3044\u3002\u30E9\u30F3\u30C7\u30A3\u30F3\u30B0\u30FB\u30DA\u30FC\u30B8\u3092\u901A\u3058\u3066\u3057\u304B\u914D\u4FE1\u306B\u30A2\u30AF\u30BB\u30B9\u3067\u304D\u306A\u3044\u5834\u5408\uFF08\u3064\u307E\u308A\u3001\u76F4\u63A5\u7684\u306A\u30C0\u30A6\u30F3\u30ED\u30FC\u30C9URL\u304C\u4E0D\u660E\uFF09\u306F\u3001\u914D\u4FE1\u306B\u304A\u3051\u308BaccessURL\u3068\u3057\u3066\u30E9\u30F3\u30C7\u30A3\u30F3\u30B0\u30FB\u30DA\u30FC\u30B8\u306E\u30EA\u30F3\u30AF\u3092\u30B3\u30D4\u30FC\u3059\u3079\u304D\u3067\u3059\uFF08SHOULD\uFF09\u3002"@ja .
<http://www.w3.org/ns/dcat#bbox> <http://www.w3.org/1999/02/22-rdf-syntax-ns#type> <http://www.w3.org/1999/02/22-rdf-syntax-ns#Property> .
<http://www.w3.org/ns/dcat#bbox> <http://www.w3.org/1999/02/22-rdf-syntax-ns#type> <http://www.w3.org/2002/07/owl#DatatypeProperty> .
<http://www.w3.org/ns/dcat#bbox> <http://www.w3.org/2000/01/rdf-schema#domain> <http://purl.org/dc/terms/Location> .
<http://www.w3.org/ns/dcat#bbox> <http://www.w3.org/2000/01/rdf-schema#label> "bounding box"@en .
<http://www.w3.org/ns/dcat#bbox> <http://www.w3.org/2000/01/rdf-schema#label> "quadro di delimitazione"@it .
<http://www.w3.org/ns/dcat#bbox> <http://www.w3.org/2000/01/rdf-schema#label> "cuadro delimitador"@es .
<http://www.w3.org/ns/dcat#bbox> <http://www.w3.org/2000/01/rdf-schema#label> "ohrani\u010Den\u00ED oblasti"@cs .
<http://www.w3.org/ns/dcat#bbox> <http://www.w3.org/2000/01/rdf-schema#range> <http://www.w3.org/2000/01/rdf-schema#Literal> .
<http://www.w3.org/ns/dcat#bbox> <http://www.w3.org/2004/02/skos/core#changeNote> "New property added in DCAT 2.0."@en .
<http://www.w3.org/ns/dcat#bbox> <http://www.w3.org/2004/02/skos/core#changeNote> "Nuova propriet\u00E0 aggiunta in DCAT 2.0."@it .
<http://www.w3.org/ns/dcat#bbox> <http://www.w3.org/2004/02/skos/core#changeNote> "Nov\u00E1 vlastnost p\u0159idan\u00E1 ve verzi DCAT 2.0."@cs .
<http://www.w3.org/ns/dcat#bbox> <http://www.w3.org/2004/02/skos/core#changeNote> "Propiedad nueva agregada en DCAT 2.0."@es .
<http://www.w3.org/ns/dcat#bbox> <http://www.w3.org/2004/02/skos/core#definition> "El cuadro delimitador geogr\u00E1fico para un recurso."@es .
<http://www.w3.org/ns/dcat#bbox> <http://www.w3.org/2004/02/skos/core#definition> "Ohrani\u010Den\u00ED geografick\u00E9 oblasti zdroje."@cs .
<http://www.w3.org/ns/dcat#bbox> <http://www.w3.org/2004/02/skos/core#definition> "The geographic bounding box of a resource."@en .
<http://www.w3.org/ns/dcat#bbox> <http://www.w3.org/2004/02/skos/core#definition> "Il riquadro di delimitazione geografica di una risorsa."@it .
<http://www.w3.org/ns/dcat#bbox> <http://www.w3.org/2004/02/skos/core#scopeNote> "El rango de esta propiedad es intencionalmente gen\u00E9rico con el prop\u00F3sito de permitir distintas codificaciones geom\u00E9tricas. Por ejemplo, la geometr\u00EDa puede ser codificada como WKT (geosparql:asWKT [GeoSPARQL]) o [GML] (geosparql:asGML [GeoSPARQL])."@es .
<http://www.w3.org/ns/dcat#bbox> <http://www.w3.org/2004/02/skos/core#scopeNote> "Obor hodnot t\u00E9to vlastnosti je \u00FAmysln\u011B obecn\u00FD, aby umo\u017Enil r\u016Fzn\u00E9 k\u00F3dov\u00E1n\u00ED geometri\u00ED. Geometrie by kup\u0159\u00EDkladu mohla b\u00FDt k\u00F3dov\u00E1na jako WKT (geosparql:asWKT [GeoSPARQL]) \u010Di [GML] (geosparql:asGML [GeoSPARQL])."@cs .
<http://www.w3.org/ns/dcat#bbox> <http://www.w3.org/2004/02/skos/core#scopeNote> "The range of this property is intentionally generic, with the purpose of allowing different geometry encodings. E.g., the geometry could be encoded with as WKT (geosparql:asWKT [GeoSPARQL]) or [GML] (geosparql:asGML [GeoSPARQL])."@en .
<http://www.w3.org/ns/dcat#bbox> <http://www.w3.org/2004/02/skos/core#scopeNote> "Il range di questa propriet\u00E0 \u00E8 volutamente generica, con lo scopo di consentire diverse codifiche geometriche. Ad esempio, la geometria potrebbe essere codificata con WKT (geosparql:asWKT [GeoSPARQL]) o [GML] (geosparql:asGML [GeoSPARQL])."@it .
<http://www.w3.org/ns/dcat#byteSize> <http://www.w3.org/1999/02/22-rdf-syntax-ns#type> <http://www.w3.org/1999/02/22-rdf-syntax-ns#Property> .
<http://www.w3.org/ns/dcat#byteSize> <http://www.w3.org/1999/02/22-rdf-syntax-ns#type> <http://www.w3.org/2002/07/owl#DatatypeProperty> .
<http://www.w3.org/ns/dcat#byteSize> <http://www.w3.org/2000/01/rdf-schema#comment> "El tama\u00F1o de una distribuci\u00F3n en bytes."@es .
<http://www.w3.org/ns/dcat#byteSize> <http://www.w3.org/2000/01/rdf-schema#comment> "La dimensione di una distribuzione in byte."@it .
<http://www.w3.org/ns/dcat#byteSize> <http://www.w3.org/2000/01/rdf-schema#comment> "La taille de la distribution en octects"@fr .
<http://www.w3.org/ns/dcat#byteSize> <http://www.w3.org/2000/01/rdf-schema#comment> "The size of a distribution in bytes."@en .
<http://www.w3.org/ns/dcat#byteSize> <http://www.w3.org/2000/01/rdf-schema#comment> "Velikost distribuce v bajtech."@cs .
<http://www.w3.org/ns/dcat#byteSize> <http://www.w3.org/2000/01/rdf-schema#comment> "\u03A4\u03BF \u03BC\u03AD\u03B3\u03B5\u03B8\u03BF\u03C2 \u03BC\u03B9\u03B1\u03C2 \u03B4\u03B9\u03B1\u03BD\u03BF\u03BC\u03AE\u03C2 \u03C3\u03B5 bytes."@el .
<http://www.w3.org/ns/dcat#byteSize> <http://www.w3.org/2000/01/rdf-schema#comment> "\u0627\u0644\u062D\u062C\u0645 \u0628\u0627\u0644\u0628\u0627\u064A\u062A\u0627\u062A "@ar .
<http://www.w3.org/ns/dcat#byteSize> <http://www.w3.org/2000/01/rdf-schema#comment> "\u30D0\u30A4\u30C8\u306B\u3088\u308B\u914D\u4FE1\u306E\u30B5\u30A4\u30BA\u3002"@ja .
<http://www.w3.org/ns/dcat#byteSize> <http://www.w3.org/2000/01/rdf-schema#domain> <http://www.w3.org/ns/dcat#Distribution> .
<http://www.w3.org/ns/dcat#byteSize> <http://www.w3.org/2000/01/rdf-schema#isDefinedBy> <http://www.w3.org/TR/vocab-dcat/> .
<http://www.w3.org/ns/dcat#byteSize> <http://www.w3.org/2000/01/rdf-schema#label> "byte size"@en .
<http://www.w3.org/ns/dcat#byteSize> <http://www.w3.org/2000/01/rdf-schema#label> "dimensione in byte"@it .
<http://www.w3.org/ns/dcat#byteSize> <http://www.w3.org/2000/01/rdf-schema#label> "taille en octects"@fr .
<http://www.w3.org/ns/dcat#byteSize> <http://www.w3.org/2000/01/rdf-schema#label> "tama\u00F1o en bytes"@es .
<http://www.w3.org/ns/dcat#byteSize> <http://www.w3.org/2000/01/rdf-schema#label> "velikost v bajtech"@cs .
<http://www.w3.org/ns/dcat#byteSize> <http://www.w3.org/2000/01/rdf-schema#label> "\u03BC\u03AD\u03B3\u03B5\u03B8\u03BF\u03C2 \u03C3\u03B5 bytes"@el .
<http://www.w3.org/ns/dcat#byteSize> <http://www.w3.org/2000/01/rdf-schema#label> "\u0627\u0644\u062D\u062C\u0645 \u0628\u0627\u0644\u0628\u0627\u064A\u062A"@ar .
<http://www.w3.org/ns/dcat#byteSize> <http://www.w3.org/2000/01/rdf-schema#label> "\u30D0\u30A4\u30C8\u30FB\u30B5\u30A4\u30BA"@ja .
<http://www.w3.org/ns/dcat#byteSize> <http://www.w3.org/2000/01/rdf-schema#range> <http://www.w3.org/2000/01/rdf-schema#Literal> .
<http://www.w3.org/ns/dcat#byteSize> <http://www.w3.org/2004/02/skos/core#definition> "El tama\u00F1o de una distribuci\u00F3n en bytes."@es .
<http://www.w3.org/ns/dcat#byteSize> <http://www.w3.org/2004/02/skos/core#definition> "La dimensione di una distribuzione in byte."@it .
<http://www.w3.org/ns/dcat#byteSize> <http://www.w3.org/2004/02/skos/core#definition> "La taille de la distribution en octects."@fr .
<http://www.w3.org/ns/dcat#byteSize> <http://www.w3.org/2004/02/skos/core#definition> "The size of a distribution in bytes."@en .
<http://www.w3.org/ns/dcat#byteSize> <http://www.w3.org/2004/02/skos/core#definition> "Velikost distribuce v bajtech."@cs .
<http://www.w3.org/ns/dcat#byteSize> <http://www.w3.org/2004/02/skos/core#definition> "\u03A4\u03BF \u03BC\u03AD\u03B3\u03B5\u03B8\u03BF\u03C2 \u03BC\u03B9\u03B1\u03C2 \u03B4\u03B9\u03B1\u03BD\u03BF\u03BC\u03AE\u03C2 \u03C3\u03B5 bytes."@el .
<http://www.w3.org/ns/dcat#byteSize> <http://www.w3.org/2004/02/skos/core#definition> "\u0627\u0644\u062D\u062C\u0645 \u0628\u0627\u0644\u0628\u0627\u064A\u062A\u0627\u062A "@ar .
<http://www.w3.org/ns/dcat#byteSize> <http://www.w3.org/2004/02/skos/core#definition> "\u30D0\u30A4\u30C8\u306B\u3088\u308B\u914D\u4FE1\u306E\u30B5\u30A4\u30BA\u3002"@ja .
<http://www.w3.org/ns/dcat#byteSize> <http://www.w3.org/2004/02/skos/core#scopeNote> "El tama\u00F1o en bytes puede ser aproximado cuando se desconoce el tama\u00F1o exacto. El valor literal de dcat:byteSize debe tener tipo 'xsd:decimal'."@es .
<http://www.w3.org/ns/dcat#byteSize> <http://www.w3.org/2004/02/skos/core#scopeNote> "La dimensione in byte pu\u00F2 essere approssimata quando non si conosce la dimensione precisa. Il valore di dcat:byteSize dovrebbe essere espresso come un xsd:decimal."@it .
<http://www.w3.org/ns/dcat#byteSize> <http://www.w3.org/2004/02/skos/core#scopeNote> "La taille en octects peut \u00EAtre approximative lorsque l'on ignore la taille r\u00E9elle. La valeur litt\u00E9rale de dcat:byteSize doit \u00EAtre de type xsd:decimal."@fr .
<http://www.w3.org/ns/dcat#byteSize> <http://www.w3.org/2004/02/skos/core#scopeNote> "The size in bytes can be approximated when the precise size is not known. The literal value of dcat:byteSize should by typed as xsd:decimal."@en .
<http://www.w3.org/ns/dcat#byteSize> <http://www.w3.org/2004/02/skos/core#scopeNote> "Velikost v bajtech m\u016F\u017Ee b\u00FDt p\u0159ibli\u017En\u00E1, pokud jej\u00ED p\u0159esn\u00E1 hodnota nen\u00ED zn\u00E1ma. Liter\u00E1l s hodnotou dcat:byteSize by m\u011Bl m\u00EDt datov\u00FD typ xsd:decimal."@cs .
<http://www.w3.org/ns/dcat#byteSize> <http://www.w3.org/2004/02/skos/core#scopeNote> "\u03A4\u03BF \u03BC\u03AD\u03B3\u03B5\u03B8\u03BF\u03C2 \u03C3\u03B5 bytes \u03BC\u03C0\u03BF\u03C1\u03B5\u03AF \u03BD\u03B1 \u03C0\u03C1\u03BF\u03C3\u03B5\u03B3\u03B3\u03B9\u03C3\u03C4\u03B5\u03AF \u03CC\u03C4\u03B1\u03BD \u03B7 \u03B1\u03BA\u03C1\u03B9\u03B2\u03AE\u03C2 \u03C4\u03B9\u03BC\u03AE \u03B4\u03B5\u03BD \u03B5\u03AF\u03BD\u03B1\u03B9 \u03B3\u03BD\u03C9\u03C3\u03C4\u03AE. \u0397 \u03C4\u03B9\u03BC\u03AE \u03C4\u03B7\u03C2 dcat:byteSize \u03B8\u03B1 \u03C0\u03C1\u03AD\u03C0\u03B5\u03B9 \u03BD\u03B1 \u03B4\u03AF\u03BD\u03B5\u03C4\u03B1\u03B9 \u03BC\u03B5 \u03C4\u03CD\u03C0\u03BF \u03B4\u03B5\u03B4\u03BF\u03BC\u03AD\u03BD\u03C9\u03BD xsd:decimal."@el .
<http://www.w3.org/ns/dcat#byteSize> <http://www.w3.org/2004/02/skos/core#scopeNote> "\u0627\u0644\u062D\u062C\u0645 \u064A\u0645\u0643\u0646 \u0623\u0646 \u064A\u0643\u0648\u0646 \u062A\u0642\u0631\u064A\u0628\u064A \u0625\u0630\u0627 \u0643\u0627\u0646 \u0627\u0644\u062D\u062C\u0645 \u0627\u0644\u062F\u0642\u064A\u0642 \u063A\u064A\u0631 \u0645\u0639\u0631\u0648\u0641"@ar .
<http://www.w3.org/ns/dcat#byteSize> <http://www.w3.org/2004/02/skos/core#scopeNote> "\u6B63\u78BA\u306A\u30B5\u30A4\u30BA\u304C\u4E0D\u660E\u3067\u3042\u308B\u5834\u5408\u3001\u30B5\u30A4\u30BA\u306F\u3001\u30D0\u30A4\u30C8\u306B\u3088\u308B\u8FD1\u4F3C\u5024\u3092\u793A\u3059\u3053\u3068\u304C\u3067\u304D\u307E\u3059\u3002"@ja .
<http://www.w3.org/ns/dcat#catalog> <http://www.w3.org/1999/02/22-rdf-syntax-ns#type> <http://www.w3.org/2002/07/owl#ObjectProperty> .
<http://www.w3.org/ns/dcat#catalog> <http://www.w3.org/2000/01/rdf-schema#comment> "A catalog whose contents are of interest in the context of this catalog."@en .
<http://www.w3.org/ns/dcat#catalog> <http://www.w3.org/2000/01/rdf-schema#comment> "Katalog, jeho\u017E obsah je v kontextu tohoto katalogu zaj\u00EDmav\u00FD."@cs .
<http://www.w3.org/ns/dcat#catalog> <http://www.w3.org/2000/01/rdf-schema#comment> "Un catalogo i cui contenuti sono di interesse nel contesto di questo catalogo."@it .
<http://www.w3.org/ns/dcat#catalog> <http://www.w3.org/2000/01/rdf-schema#comment> "Un cat\u00E1logo cuyo contenido es de inter\u00E9s en el contexto del cat\u00E1logo que est\u00E1 siendo descripto."@es .
<http://www.w3.org/ns/dcat#catalog> <http://www.w3.org/2000/01/rdf-schema#domain> <http://www.w3.org/ns/dcat#Catalog> .
<http://www.w3.org/ns/dcat#catalog> <http://www.w3.org/2000/01/rdf-schema#label> "catalog"@en .
<http://www.w3.org/ns/dcat#catalog> <http://www.w3.org/2000/01/rdf-schema#label> "catalogo"@it .
<http://www.w3.org/ns/dcat#catalog> <http://www.w3.org/2000/01/rdf-schema#label> "cat\u00E1logo"@es .
<http://www.w3.org/ns/dcat#catalog> <http://www.w3.org/2000/01/rdf-schema#label> "katalog"@cs .
<http://www.w3.org/ns/dcat#catalog> <http://www.w3.org/2000/01/rdf-schema#range> <http://www.w3.org/ns/dcat#Catalog> .
<http://www.w3.org/ns/dcat#catalog> <http://www.w3.org/2000/01/rdf-schema#subPropertyOf> <http://purl.org/dc/terms/hasPart> .
<http://www.w3.org/ns/dcat#catalog> <http://www.w3.org/2000/01/rdf-schema#subPropertyOf> <http://www.w3.org/2000/01/rdf-schema#member> .
<http://www.w3.org/ns/dcat#catalog> <http://www.w3.org/2004/02/skos/core#changeNote> "New property added in DCAT 2.0."@en .
<http://www.w3.org/ns/dcat#catalog> <http://www.w3.org/2004/02/skos/core#changeNote> "Nov\u00E1 vlastnost p\u0159idan\u00E1 ve verzi DCAT 2.0."@cs .
<http://www.w3.org/ns/dcat#catalog> <http://www.w3.org/2004/02/skos/core#changeNote> "Nueva propiedad agregada en DCAT 2.0."@es .
<http://www.w3.org/ns/dcat#catalog> <http://www.w3.org/2004/02/skos/core#changeNote> "Nuova propriet\u00E0 aggiunta in DCAT 2.0."@it .
<http://www.w3.org/ns/dcat#catalog> <http://www.w3.org/2004/02/skos/core#definition> "A catalog whose contents are of interest in the context of this catalog."@en .
<http://www.w3.org/ns/dcat#catalog> <http://www.w3.org/2004/02/skos/core#definition> "Katalog, jeho\u017E obsah je v kontextu tohoto katalogu zaj\u00EDmav\u00FD."@cs .
<http://www.w3.org/ns/dcat#catalog> <http://www.w3.org/2004/02/skos/core#definition> "Un catalogo i cui contenuti sono di interesse nel contesto di questo catalogo."@it .
<http://www.w3.org/ns/dcat#catalog> <http://www.w3.org/2004/02/skos/core#definition> "Un cat\u00E1logo cuyo contenido es de inter\u00E9s en el contexto del cat\u00E1logo que est\u00E1 siendo descripto."@es .
<http://www.w3.org/ns/dcat#centroid> <http://www.w3.org/1999/02/22-rdf-syntax-ns#type> <http://www.w3.org/1999/02/22-rdf-syntax-ns#Property> .
<http://www.w3.org/ns/dcat#centroid> <http://www.w3.org/1999/02/22-rdf-syntax-ns#type> <http://www.w3.org/2002/07/owl#DatatypeProperty> .
<http://www.w3.org/ns/dcat#centroid> <http://www.w3.org/2000/01/rdf-schema#domain> <http://purl.org/dc/terms/Location> .
<http://www.w3.org/ns/dcat#centroid> <http://www.w3.org/2000/01/rdf-schema#label> "centroid"@cs .
<http://www.w3.org/ns/dcat#centroid> <http://www.w3.org/2000/01/rdf-schema#label> "centroid"@en .
<http://www.w3.org/ns/dcat#centroid> <http://www.w3.org/2000/01/rdf-schema#label> "centroide"@it .
<http://www.w3.org/ns/dcat#centroid> <http://www.w3.org/2000/01/rdf-schema#label> "centroide"@es .
<http://www.w3.org/ns/dcat#centroid> <http://www.w3.org/2000/01/rdf-schema#range> <http://www.w3.org/2000/01/rdf-schema#Literal> .
<http://www.w3.org/ns/dcat#centroid> <http://www.w3.org/2004/02/skos/core#changeNote> "New property added in DCAT 2.0."@en .
<http://www.w3.org/ns/dcat#centroid> <http://www.w3.org/2004/02/skos/core#changeNote> "Nuova propriet\u00E0 aggiunta in DCAT 2.0."@it .
<http://www.w3.org/ns/dcat#centroid> <http://www.w3.org/2004/02/skos/core#changeNote> "Nov\u00E1 vlastnost p\u0159idan\u00E1 ve verzi DCAT 2.0."@cs .
<http://www.w3.org/ns/dcat#centroid> <http://www.w3.org/2004/02/skos/core#changeNote> "Nueva propiedad agregada en DCAT 2.0."@es .
<http://www.w3.org/ns/dcat#centroid> <http://www.w3.org/2004/02/skos/core#definition> "El centro geogr\u00E1fico (centroide) de un recurso."@es .
<http://www.w3.org/ns/dcat#centroid> <http://www.w3.org/2004/02/skos/core#definition> "Geografick\u00FD st\u0159ed (centroid) zdroje."@cs .
<http://www.w3.org/ns/dcat#centroid> <http://www.w3.org/2004/02/skos/core#definition> "The geographic center (centroid) of a resource."@en .
<http://www.w3.org/ns/dcat#centroid> <http://www.w3.org/2004/02/skos/core#definition> "Il centro geografico (centroide) di una risorsa."@it .
<http://www.w3.org/ns/dcat#centroid> <http://www.w3.org/2004/02/skos/core#scopeNote> "El rango de esta propiedad es intencionalmente gen\u00E9rico con el objetivo de permitir distintas codificaciones geom\u00E9tricas. Por ejemplo, la geometr\u00EDa puede codificarse como WKT (geosparql:asWKT [GeoSPARQL]) o [GML] (geosparql:asGML [GeoSPARQL])."@es .
<http://www.w3.org/ns/dcat#centroid> <http://www.w3.org/2004/02/skos/core#scopeNote> "Obor hodnot t\u00E9to vlastnosti je \u00FAmysln\u011B obecn\u00FD, aby umo\u017Enil r\u016Fzn\u00E9 k\u00F3dov\u00E1n\u00ED geometri\u00ED. Geometrie by kup\u0159\u00EDkladu mohla b\u00FDt k\u00F3dov\u00E1na jako WKT (geosparql:asWKT [GeoSPARQL]) \u010Di [GML] (geosparql:asGML [GeoSPARQL])."@cs .
<http://www.w3.org/ns/dcat#centroid> <http://www.w3.org/2004/02/skos/core#scopeNote> "The range of this property is intentionally generic, with the purpose of allowing different geometry encodings. E.g., the geometry could be encoded with as WKT (geosparql:asWKT [GeoSPARQL]) or [GML] (geosparql:asGML [GeoSPARQL])."@en .
<http://www.w3.org/ns/dcat#centroid> <http://www.w3.org/2004/02/skos/core#scopeNote> "Il range di questa propriet\u00E0 \u00E8 volutamente generica, con lo scopo di consentire diverse codifiche geometriche. Ad esempio, la geometria potrebbe essere codificata con WKT (geosparql:asWKT [GeoSPARQL]) o [GML] (geosparql:asGML [GeoSPARQL])."@it .
<http://www.w3.org/ns/dcat#compressFormat> <http://www.w3.org/1999/02/22-rdf-syntax-ns#type> <http://www.w3.org/1999/02/22-rdf-syntax-ns#Property> .
<http://www.w3.org/ns/dcat#compressFormat> <http://www.w3.org/1999/02/22-rdf-syntax-ns#type> <http://www.w3.org/2002/07/owl#ObjectProperty> .
<http://www.w3.org/ns/dcat#compressFormat> <http://www.w3.org/2000/01/rdf-schema#comment> "El formato de la distribuci\u00F3n en el que los datos est\u00E1n en forma comprimida, e.g. para reducir el tama\u00F1o del archivo a bajar."@es .
<http://www.w3.org/ns/dcat#compressFormat> <http://www.w3.org/2000/01/rdf-schema#comment> "Form\u00E1t komprese souboru, ve kter\u00E9m jsou data poskytov\u00E1na v komprimovan\u00E9 podob\u011B, nap\u0159. ke sn\u00ED\u017Een\u00ED velikosti souboru ke sta\u017Een\u00ED."@cs .
<http://www.w3.org/ns/dcat#compressFormat> <http://www.w3.org/2000/01/rdf-schema#comment> "Il formato di compressione della distribuzione nel quale i dati sono in forma compressa, ad es. per ridurre le dimensioni del file da scaricare."@it .
<http://www.w3.org/ns/dcat#compressFormat> <http://www.w3.org/2000/01/rdf-schema#comment> "The compression format of the distribution in which the data is contained in a compressed form, e.g. to reduce the size of the downloadable file."@en .
<http://www.w3.org/ns/dcat#compressFormat> <http://www.w3.org/2000/01/rdf-schema#domain> <http://www.w3.org/ns/dcat#Distribution> .
<http://www.w3.org/ns/dcat#compressFormat> <http://www.w3.org/2000/01/rdf-schema#isDefinedBy> <https://www.w3.org/TR/vocab-dcat-2/> .
<http://www.w3.org/ns/dcat#compressFormat> <http://www.w3.org/2000/01/rdf-schema#label> "compression format"@en .
<http://www.w3.org/ns/dcat#compressFormat> <http://www.w3.org/2000/01/rdf-schema#label> "formato de compresi\u00F3n"@es .
<http://www.w3.org/ns/dcat#compressFormat> <http://www.w3.org/2000/01/rdf-schema#label> "formato di compressione"@it .
<http://www.w3.org/ns/dcat#compressFormat> <http://www.w3.org/2000/01/rdf-schema#label> "form\u00E1t komprese"@cs .
<http://www.w3.org/ns/dcat#compressFormat> <http://www.w3.org/2000/01/rdf-schema#range> <http://purl.org/dc/terms/MediaType> .
<http://www.w3.org/ns/dcat#compressFormat> <http://www.w3.org/2000/01/rdf-schema#subPropertyOf> <http://purl.org/dc/terms/format> .
<http://www.w3.org/ns/dcat#compressFormat> <http://www.w3.org/2004/02/skos/core#changeNote> "New property added in DCAT 2.0."@en .
<http://www.w3.org/ns/dcat#compressFormat> <http://www.w3.org/2004/02/skos/core#changeNote> "Nov\u00E1 vlastnost p\u0159idan\u00E1 ve verzi DCAT 2.0."@cs .
<http://www.w3.org/ns/dcat#compressFormat> <http://www.w3.org/2004/02/skos/core#changeNote> "Nueva propiedad agregada en DCAT 2.0."@es .
<http://www.w3.org/ns/dcat#compressFormat> <http://www.w3.org/2004/02/skos/core#changeNote> "Nuova propriet\u00E0 aggiunta in DCAT 2.0."@it .
<http://www.w3.org/ns/dcat#compressFormat> <http://www.w3.org/2004/02/skos/core#definition> "El formato de la distribuci\u00F3n en el que los datos est\u00E1n en forma comprimida, e.g. para reducir el tama\u00F1o del archivo a bajar."@es .
<http://www.w3.org/ns/dcat#compressFormat> <http://www.w3.org/2004/02/skos/core#definition> "Form\u00E1t komprese souboru, ve kter\u00E9m jsou data poskytov\u00E1na v komprimovan\u00E9 podob\u011B, nap\u0159. ke sn\u00ED\u017Een\u00ED velikosti souboru ke sta\u017Een\u00ED."@cs .
<http://www.w3.org/ns/dcat#compressFormat> <http://www.w3.org/2004/02/skos/core#definition> "Il formato di compressione della distribuzione nel quale i dati sono in forma compressa, ad es. per ridurre le dimensioni del file da scaricare."@it .
<http://www.w3.org/ns/dcat#compressFormat> <http://www.w3.org/2004/02/skos/core#definition> "The compression format of the distribution in which the data is contained in a compressed form, e.g. to reduce the size of the downloadable file."@en .
<http://www.w3.org/ns/dcat#compressFormat> <http://www.w3.org/2004/02/skos/core#scopeNote> "Esta propiedad se debe usar cuando los archivos de la distribuci\u00F3n est\u00E1n comprimidos, por ejemplo en un archivo ZIP. El formato DEBER\u00CDA expresarse usando un 'media type', tales como los definidos en el registro IANA de 'media types' https://www.iana.org/assignments/media-types/, si est\u00E1 disponibles."@es .
<http://www.w3.org/ns/dcat#compressFormat> <http://www.w3.org/2004/02/skos/core#scopeNote> "Questa propriet\u00E0 deve essere utilizzata quando i file nella distribuzione sono compressi, ad es. in un file ZIP. Il formato DOVREBBE essere espresso usando un tipo di media come definito dal registro dei tipi di media IANA https://www.iana.org/assignments/media-types/, se disponibile."@it .
<http://www.w3.org/ns/dcat#compressFormat> <http://www.w3.org/2004/02/skos/core#scopeNote> "Tato vlastnost se pou\u017Eije, kdy\u017E jsou soubory v distribuci komprimov\u00E1ny, nap\u0159. v ZIP souboru. Form\u00E1t BY M\u011AL b\u00FDt vyj\u00E1d\u0159en pomoc\u00ED typu m\u00E9dia definovan\u00E9ho v registru IANA https://www.iana.org/assignments/media-types/, pokud existuje."@cs .
<http://www.w3.org/ns/dcat#compressFormat> <http://www.w3.org/2004/02/skos/core#scopeNote> "This property is to be used when the files in the distribution are compressed, e.g. in a ZIP file. The format SHOULD be expressed using a media type as defined by IANA media types registry https://www.iana.org/assignments/media-types/, if available."@en .
<http://www.w3.org/ns/dcat#contactPoint> <http://www.w3.org/1999/02/22-rdf-syntax-ns#type> <http://www.w3.org/1999/02/22-rdf-syntax-ns#Property> .
<http://www.w3.org/ns/dcat#contactPoint> <http://www.w3.org/1999/02/22-rdf-syntax-ns#type> <http://www.w3.org/2002/07/owl#ObjectProperty> .
<http://www.w3.org/ns/dcat#contactPoint> <http://www.w3.org/2000/01/rdf-schema#comment> "Informaci\u00F3n relevante de contacto para el recurso catalogado. Se recomienda el uso de vCard."@es .
<http://www.w3.org/ns/dcat#contactPoint> <http://www.w3.org/2000/01/rdf-schema#comment> "Informazioni di contatto rilevanti per la risorsa catalogata. Si raccomanda l'uso di vCard."@it .
<http://www.w3.org/ns/dcat#contactPoint> <http://www.w3.org/2000/01/rdf-schema#comment> "Relevant contact information for the catalogued resource. Use of vCard is recommended."@en .
<http://www.w3.org/ns/dcat#contactPoint> <http://www.w3.org/2000/01/rdf-schema#comment> "Relevantn\u00ED kontaktn\u00ED informace pro katalogizovan\u00FD zdroj. Doporu\u010Duje se pou\u017E\u00EDt slovn\u00EDk VCard."@cs .
<http://www.w3.org/ns/dcat#contactPoint> <http://www.w3.org/2000/01/rdf-schema#comment> "Relie un jeu de donn\u00E9es \u00E0 une information de contact utile en utilisant VCard."@fr .
<http://www.w3.org/ns/dcat#contactPoint> <http://www.w3.org/2000/01/rdf-schema#comment> "\u03A3\u03C5\u03BD\u03B4\u03AD\u03B5\u03B9 \u03AD\u03BD\u03B1 \u03C3\u03CD\u03BD\u03BF\u03BB\u03BF \u03B4\u03B5\u03B4\u03BF\u03BC\u03AD\u03BD\u03C9\u03BD \u03BC\u03B5 \u03AD\u03BD\u03B1 \u03C3\u03C7\u03B5\u03C4\u03B9\u03BA\u03CC \u03C3\u03B7\u03BC\u03B5\u03AF\u03BF \u03B5\u03C0\u03B9\u03BA\u03BF\u03B9\u03BD\u03C9\u03BD\u03AF\u03B1\u03C2, \u03BC\u03AD\u03C3\u03C9 VCard."@el .
<http://www.w3.org/ns/dcat#contactPoint> <http://www.w3.org/2000/01/rdf-schema#comment> "\u062A\u0631\u0628\u0637 \u0642\u0627\u0626\u0645\u0629 \u0627\u0644\u0628\u064A\u0627\u0646\u0627\u062A \u0628\u0639\u0646\u0648\u0627\u0646 \u0627\u062A\u0635\u0627\u0644 \u0645\u0648\u0635\u0641  \u0628\u0627\u0633\u062A\u062E\u062F\u0627\u0645 VCard"@ar .
<http://www.w3.org/ns/dcat#contactPoint> <http://www.w3.org/2000/01/rdf-schema#comment> "\u30C7\u30FC\u30BF\u30BB\u30C3\u30C8\u3092\u3001VCard\u3092\u7528\u3044\u3066\u63D0\u4F9B\u3055\u308C\u3066\u3044\u308B\u9069\u5207\u306A\u9023\u7D61\u5148\u60C5\u5831\u306B\u30EA\u30F3\u30AF\u3057\u307E\u3059\u3002"@ja .
<http://www.w3.org/ns/dcat#contactPoint> <http://www.w3.org/2000/01/rdf-schema#isDefinedBy> <http://www.w3.org/TR/vocab-dcat/> .
<http://www.w3.org/ns/dcat#contactPoint> <http://www.w3.org/2000/01/rdf-schema#label> "Punto de contacto"@es .
<http://www.w3.org/ns/dcat#contactPoint> <http://www.w3.org/2000/01/rdf-schema#label> "contact point"@en .
<http://www.w3.org/ns/dcat#contactPoint> <http://www.w3.org/2000/01/rdf-schema#label> "kontaktn\u00ED bod"@cs .
<http://www.w3.org/ns/dcat#contactPoint> <http://www.w3.org/2000/01/rdf-schema#label> "point de contact"@fr .
<http://www.w3.org/ns/dcat#contactPoint> <http://www.w3.org/2000/01/rdf-schema#label> "punto di contatto"@it .
<http://www.w3.org/ns/dcat#contactPoint> <http://www.w3.org/2000/01/rdf-schema#label> "\u03C3\u03B7\u03BC\u03B5\u03AF\u03BF \u03B5\u03C0\u03B9\u03BA\u03BF\u03B9\u03BD\u03C9\u03BD\u03AF\u03B1\u03C2"@el .
<http://www.w3.org/ns/dcat#contactPoint> <http://www.w3.org/2000/01/rdf-schema#label> "\u0639\u0646\u0648\u0627\u0646 \u0627\u062A\u0635\u0627\u0644"@ar .
<http://www.w3.org/ns/dcat#contactPoint> <http://www.w3.org/2000/01/rdf-schema#label> "\u7A93\u53E3"@ja .
<http://www.w3.org/ns/dcat#contactPoint> <http://www.w3.org/2000/01/rdf-schema#range> <http://www.w3.org/2006/vcard/ns#Kind> .
<http://www.w3.org/ns/dcat#contactPoint> <http://www.w3.org/2004/02/skos/core#definition> "Informaci\u00F3n relevante de contacto para el recurso catalogado. Se recomienda el uso de vCard."@es .
<http://www.w3.org/ns/dcat#contactPoint> <http://www.w3.org/2004/02/skos/core#definition> "Informazioni di contatto rilevanti per la risorsa catalogata. Si raccomanda l'uso di vCard."@it .
<http://www.w3.org/ns/dcat#contactPoint> <http://www.w3.org/2004/02/skos/core#definition> "Relevant contact information for the catalogued resource. Use of vCard is recommended."@en .
<http://www.w3.org/ns/dcat#contactPoint> <http://www.w3.org/2004/02/skos/core#definition> "Relevantn\u00ED kontaktn\u00ED informace pro katalogizovan\u00FD zdroj. Doporu\u010Duje se pou\u017E\u00EDt slovn\u00EDk VCard."@cs .
<http://www.w3.org/ns/dcat#contactPoint> <http://www.w3.org/2004/02/skos/core#definition> "Relie un jeu de donn\u00E9es \u00E0 une information de contact utile en utilisant VCard."@fr .
<http://www.w3.org/ns/dcat#contactPoint> <http://www.w3.org/2004/02/skos/core#definition> "\u03A3\u03C5\u03BD\u03B4\u03AD\u03B5\u03B9 \u03AD\u03BD\u03B1 \u03C3\u03CD\u03BD\u03BF\u03BB\u03BF \u03B4\u03B5\u03B4\u03BF\u03BC\u03AD\u03BD\u03C9\u03BD \u03BC\u03B5 \u03AD\u03BD\u03B1 \u03C3\u03C7\u03B5\u03C4\u03B9\u03BA\u03CC \u03C3\u03B7\u03BC\u03B5\u03AF\u03BF \u03B5\u03C0\u03B9\u03BA\u03BF\u03B9\u03BD\u03C9\u03BD\u03AF\u03B1\u03C2, \u03BC\u03AD\u03C3\u03C9 VCard."@el .
<http://www.w3.org/ns/dcat#contactPoint> <http://www.w3.org/2004/02/skos/core#definition> "\u062A\u0631\u0628\u0637 \u0642\u0627\u0626\u0645\u0629 \u0627\u0644\u0628\u064A\u0627\u0646\u0627\u062A \u0628\u0639\u0646\u0648\u0627\u0646 \u0627\u062A\u0635\u0627\u0644 \u0645\u0648\u0635\u0641  \u0628\u0627\u0633\u062A\u062E\u062F\u0627\u0645 VCard"@ar .
<http://www.w3.org/ns/dcat#contactPoint> <http://www.w3.org/2004/02/skos/core#definition> "\u30C7\u30FC\u30BF\u30BB\u30C3\u30C8\u3092\u3001VCard\u3092\u7528\u3044\u3066\u63D0\u4F9B\u3055\u308C\u3066\u3044\u308B\u9069\u5207\u306A\u9023\u7D61\u5148\u60C5\u5831\u306B\u30EA\u30F3\u30AF\u3057\u307E\u3059\u3002"@ja .
<http://www.w3.org/ns/dcat#contactPoint> <http://www.w3.org/2004/02/skos/core#editorialNote> "Status: English Definition text modified by DCAT revision team, Italian, Spanish and Czech translations provided, other translations pending."@en .
<http://www.w3.org/ns/dcat#dataset> <http://www.w3.org/1999/02/22-rdf-syntax-ns#type> <http://www.w3.org/1999/02/22-rdf-syntax-ns#Property> .
<http://www.w3.org/ns/dcat#dataset> <http://www.w3.org/1999/02/22-rdf-syntax-ns#type> <http://www.w3.org/2002/07/owl#ObjectProperty> .
<http://www.w3.org/ns/dcat#dataset> <http://www.w3.org/2000/01/rdf-schema#comment> "A collection of data that is listed in the catalog."@en .
<http://www.w3.org/ns/dcat#dataset> <http://www.w3.org/2000/01/rdf-schema#comment> "Kolekce dat, kter\u00E1 je katalogizov\u00E1na v katalogu."@cs .
<http://www.w3.org/ns/dcat#dataset> <http://www.w3.org/2000/01/rdf-schema#comment> "Relie un catalogue \u00E0 un jeu de donn\u00E9es faisant partie de ce catalogue."@fr .
<http://www.w3.org/ns/dcat#dataset> <http://www.w3.org/2000/01/rdf-schema#comment> "Un conjunto de datos que se lista en el cat\u00E1logo."@es .
<http://www.w3.org/ns/dcat#dataset> <http://www.w3.org/2000/01/rdf-schema#comment> "Una raccolta di dati che \u00E8 elencata nel catalogo."@it .
<http://www.w3.org/ns/dcat#dataset> <http://www.w3.org/2000/01/rdf-schema#comment> "\u03A3\u03C5\u03BD\u03B4\u03AD\u03B5\u03B9 \u03AD\u03BD\u03B1\u03BD \u03BA\u03B1\u03C4\u03AC\u03BB\u03BF\u03B3\u03BF \u03BC\u03B5 \u03AD\u03BD\u03B1 \u03C3\u03CD\u03BD\u03BF\u03BB\u03BF \u03B4\u03B5\u03B4\u03BF\u03BC\u03AD\u03BD\u03C9\u03BD \u03C4\u03BF \u03BF\u03C0\u03BF\u03AF\u03BF \u03B1\u03BD\u03AE\u03BA\u03B5\u03B9 \u03C3\u03C4\u03BF\u03BD \u03B5\u03BD \u03BB\u03CC\u03B3\u03C9 \u03BA\u03B1\u03C4\u03AC\u03BB\u03BF\u03B3\u03BF."@el .
<http://www.w3.org/ns/dcat#dataset> <http://www.w3.org/2000/01/rdf-schema#comment> "\u062A\u0631\u0628\u0637 \u0627\u0644\u0641\u0647\u0631\u0633 \u0628\u0642\u0627\u0626\u0645\u0629 \u0628\u064A\u0627\u0646\u0627\u062A \u0636\u0645\u0646\u0647"@ar .
<http://www.w3.org/ns/dcat#dataset> <http://www.w3.org/2000/01/rdf-schema#comment> "\u30AB\u30BF\u30ED\u30B0\u306E\u4E00\u90E8\u3067\u3042\u308B\u30C7\u30FC\u30BF\u30BB\u30C3\u30C8\u3002"@ja .
<http://www.w3.org/ns/dcat#dataset> <http://www.w3.org/2000/01/rdf-schema#domain> <http://www.w3.org/ns/dcat#Catalog> .
<http://www.w3.org/ns/dcat#dataset> <http://www.w3.org/2000/01/rdf-schema#isDefinedBy> <http://www.w3.org/TR/vocab-dcat/> .
<http://www.w3.org/ns/dcat#dataset> <http://www.w3.org/2000/01/rdf-schema#label> "conjunto de datos"@es .
<http://www.w3.org/ns/dcat#dataset> <http://www.w3.org/2000/01/rdf-schema#label> "dataset"@en .
<http://www.w3.org/ns/dcat#dataset> <http://www.w3.org/2000/01/rdf-schema#label> "dataset"@it .
<http://www.w3.org/ns/dcat#dataset> <http://www.w3.org/2000/01/rdf-schema#label> "datov\u00E1 sada"@cs .
<http://www.w3.org/ns/dcat#dataset> <http://www.w3.org/2000/01/rdf-schema#label> "jeu de donn\u00E9es"@fr .
<http://www.w3.org/ns/dcat#dataset> <http://www.w3.org/2000/01/rdf-schema#label> "\u03C3\u03CD\u03BD\u03BF\u03BB\u03BF \u03B4\u03B5\u03B4\u03BF\u03BC\u03AD\u03BD\u03C9\u03BD"@el .
<http://www.w3.org/ns/dcat#dataset> <http://www.w3.org/2000/01/rdf-schema#label> "\u0642\u0627\u0626\u0645\u0629 \u0628\u064A\u0627\u0646\u0627\u062A"@ar .
<http://www.w3.org/ns/dcat#dataset> <http://www.w3.org/2000/01/rdf-schema#label> "\u30C7\u30FC\u30BF\u30BB\u30C3\u30C8"@ja .
<http://www.w3.org/ns/dcat#dataset> <http://www.w3.org/2000/01/rdf-schema#range> <http://www.w3.org/ns/dcat#Dataset> .
<http://www.w3.org/ns/dcat#dataset> <http://www.w3.org/2000/01/rdf-schema#subPropertyOf> <http://purl.org/dc/terms/hasPart> .
<http://www.w3.org/ns/dcat#dataset> <http://www.w3.org/2000/01/rdf-schema#subPropertyOf> <http://www.w3.org/2000/01/rdf-schema#member> .
<http://www.w3.org/ns/dcat#dataset> <http://www.w3.org/2004/02/skos/core#definition> "A collection of data that is listed in the catalog."@en .
<http://www.w3.org/ns/dcat#dataset> <http://www.w3.org/2004/02/skos/core#definition> "Kolekce dat, kter\u00E1 je katalogizov\u00E1na v katalogu."@cs .
<http://www.w3.org/ns/dcat#dataset> <http://www.w3.org/2004/02/skos/core#definition> "Relie un catalogue \u00E0 un jeu de donn\u00E9es faisant partie de ce catalogue."@fr .
<http://www.w3.org/ns/dcat#dataset> <http://www.w3.org/2004/02/skos/core#definition> "Un conjunto de datos que se lista en el cat\u00E1logo."@es .
<http://www.w3.org/ns/dcat#dataset> <http://www.w3.org/2004/02/skos/core#definition> "Una raccolta di dati che \u00E8 elencata nel catalogo."@it .
<http://www.w3.org/ns/dcat#dataset> <http://www.w3.org/2004/02/skos/core#definition> "\u03A3\u03C5\u03BD\u03B4\u03AD\u03B5\u03B9 \u03AD\u03BD\u03B1\u03BD \u03BA\u03B1\u03C4\u03AC\u03BB\u03BF\u03B3\u03BF \u03BC\u03B5 \u03AD\u03BD\u03B1 \u03C3\u03CD\u03BD\u03BF\u03BB\u03BF \u03B4\u03B5\u03B4\u03BF\u03BC\u03AD\u03BD\u03C9\u03BD \u03C4\u03BF \u03BF\u03C0\u03BF\u03AF\u03BF \u03B1\u03BD\u03AE\u03BA\u03B5\u03B9 \u03C3\u03C4\u03BF\u03BD \u03B5\u03BD \u03BB\u03CC\u03B3\u03C9 \u03BA\u03B1\u03C4\u03AC\u03BB\u03BF\u03B3\u03BF."@el .
<http://www.w3.org/ns/dcat#dataset> <http://www.w3.org/2004/02/skos/core#definition> "\u062A\u0631\u0628\u0637 \u0627\u0644\u0641\u0647\u0631\u0633 \u0628\u0642\u0627\u0626\u0645\u0629 \u0628\u064A\u0627\u0646\u0627\u062A \u0636\u0645\u0646\u0647"@ar .
<http://www.w3.org/ns/dcat#dataset> <http://www.w3.org/2004/02/skos/core#definition> "\u30AB\u30BF\u30ED\u30B0\u306E\u4E00\u90E8\u3067\u3042\u308B\u30C7\u30FC\u30BF\u30BB\u30C3\u30C8\u3002"@ja .
<http://www.w3.org/ns/dcat#dataset> <http://www.w3.org/2004/02/skos/core#editorialNote> "Status: English Definition text modified by DCAT revision team, Italian, Spanish and Czech translation provided, other translations pending."@en .
<http://www.w3.org/ns/dcat#distribution> <http://www.w3.org/1999/02/22-rdf-syntax-ns#type> <http://www.w3.org/1999/02/22-rdf-syntax-ns#Property> .
<http://www.w3.org/ns/dcat#distribution> <http://www.w3.org/1999/02/22-rdf-syntax-ns#type> <http://www.w3.org/2002/07/owl#ObjectProperty> .
<http://www.w3.org/ns/dcat#distribution> <http://www.w3.org/2000/01/rdf-schema#comment> "An available distribution of the dataset."@en .
<http://www.w3.org/ns/dcat#distribution> <http://www.w3.org/2000/01/rdf-schema#comment> "Connecte un jeu de donn\u00E9es \u00E0 des distributions disponibles."@fr .
<http://www.w3.org/ns/dcat#distribution> <http://www.w3.org/2000/01/rdf-schema#comment> "Dostupn\u00E1 distribuce datov\u00E9 sady."@cs .
<http://www.w3.org/ns/dcat#distribution> <http://www.w3.org/2000/01/rdf-schema#comment> "Una distribuci\u00F3n disponible del conjunto de datos."@es .
<http://www.w3.org/ns/dcat#distribution> <http://www.w3.org/2000/01/rdf-schema#comment> "Una distribuzione disponibile per il set di dati."@it .
<http://www.w3.org/ns/dcat#distribution> <http://www.w3.org/2000/01/rdf-schema#comment> "\u03A3\u03C5\u03BD\u03B4\u03AD\u03B5\u03B9 \u03AD\u03BD\u03B1 \u03C3\u03CD\u03BD\u03BF\u03BB\u03BF \u03B4\u03B5\u03B4\u03BF\u03BC\u03AD\u03BD\u03C9\u03BD \u03BC\u03B5 \u03BC\u03AF\u03B1 \u03B1\u03C0\u03CC \u03C4\u03B9\u03C2 \u03B4\u03B9\u03B1\u03B8\u03AD\u03C3\u03B9\u03BC\u03B5\u03C2 \u03B4\u03B9\u03B1\u03BD\u03BF\u03BC\u03AD\u03C2 \u03C4\u03BF\u03C5."@el .
<http://www.w3.org/ns/dcat#distribution> <http://www.w3.org/2000/01/rdf-schema#comment> "\u062A\u0631\u0628\u0637 \u0642\u0627\u0626\u0645\u0629 \u0627\u0644\u0628\u064A\u0627\u0646\u0627\u062A \u0628\u0637\u0631\u064A\u0642\u0629 \u0623\u0648 \u0628\u0634\u0643\u0644 \u064A\u0633\u0645\u062D  \u0627\u0644\u0648\u0635\u0648\u0644 \u0627\u0644\u0649 \u0627\u0644\u0628\u064A\u0627\u0646\u0627\u062A"@ar .
<http://www.w3.org/ns/dcat#distribution> <http://www.w3.org/2000/01/rdf-schema#comment> "\u30C7\u30FC\u30BF\u30BB\u30C3\u30C8\u3092\u3001\u305D\u306E\u5229\u7528\u53EF\u80FD\u306A\u914D\u4FE1\u306B\u63A5\u7D9A\u3057\u307E\u3059\u3002"@ja .
<http://www.w3.org/ns/dcat#distribution> <http://www.w3.org/2000/01/rdf-schema#domain> <http://www.w3.org/ns/dcat#Dataset> .
<http://www.w3.org/ns/dcat#distribution> <http://www.w3.org/2000/01/rdf-schema#isDefinedBy> <http://www.w3.org/TR/vocab-dcat/> .
<http://www.w3.org/ns/dcat#distribution> <http://www.w3.org/2000/01/rdf-schema#label> "distribuce"@cs .
<http://www.w3.org/ns/dcat#distribution> <http://www.w3.org/2000/01/rdf-schema#label> "distribuci\u00F3n"@es .
<http://www.w3.org/ns/dcat#distribution> <http://www.w3.org/2000/01/rdf-schema#label> "distribution"@en .
<http://www.w3.org/ns/dcat#distribution> <http://www.w3.org/2000/01/rdf-schema#label> "distribution"@fr .
<http://www.w3.org/ns/dcat#distribution> <http://www.w3.org/2000/01/rdf-schema#label> "distribuzione"@it .
<http://www.w3.org/ns/dcat#distribution> <http://www.w3.org/2000/01/rdf-schema#label> "\u03B4\u03B9\u03B1\u03BD\u03BF\u03BC\u03AE"@el .
<http://www.w3.org/ns/dcat#distribution> <http://www.w3.org/2000/01/rdf-schema#label> "\u062A\u0648\u0632\u064A\u0639"@ar .
<http://www.w3.org/ns/dcat#distribution> <http://www.w3.org/2000/01/rdf-schema#label> "\u30C7\u30FC\u30BF\u30BB\u30C3\u30C8\u914D\u4FE1"@ja .
<http://www.w3.org/ns/dcat#distribution> <http://www.w3.org/2000/01/rdf-schema#range> <http://www.w3.org/ns/dcat#Distribution> .
<http://www.w3.org/ns/dcat#distribution> <http://www.w3.org/2000/01/rdf-schema#subPropertyOf> <http://purl.org/dc/terms/relation> .
<http://www.w3.org/ns/dcat#distribution> <http://www.w3.org/2004/02/skos/core#definition> "An available distribution of the dataset."@en .
<http://www.w3.org/ns/dcat#distribution> <http://www.w3.org/2004/02/skos/core#definition> "Connecte un jeu de donn\u00E9es \u00E0 des distributions disponibles."@fr .
<http://www.w3.org/ns/dcat#distribution> <http://www.w3.org/2004/02/skos/core#definition> "Dostupn\u00E1 distribuce datov\u00E9 sady."@cs .
<http://www.w3.org/ns/dcat#distribution> <http://www.w3.org/2004/02/skos/core#definition> "Una distribuci\u00F3n disponible del conjunto de datos."@es .
<http://www.w3.org/ns/dcat#distribution> <http://www.w3.org/2004/02/skos/core#definition> "Una distribuzione disponibile per il set di dati."@it .
<http://www.w3.org/ns/dcat#distribution> <http://www.w3.org/2004/02/skos/core#definition> "\u03A3\u03C5\u03BD\u03B4\u03AD\u03B5\u03B9 \u03AD\u03BD\u03B1 \u03C3\u03CD\u03BD\u03BF\u03BB\u03BF \u03B4\u03B5\u03B4\u03BF\u03BC\u03AD\u03BD\u03C9\u03BD \u03BC\u03B5 \u03BC\u03AF\u03B1 \u03B1\u03C0\u03CC \u03C4\u03B9\u03C2 \u03B4\u03B9\u03B1\u03B8\u03AD\u03C3\u03B9\u03BC\u03B5\u03C2 \u03B4\u03B9\u03B1\u03BD\u03BF\u03BC\u03AD\u03C2 \u03C4\u03BF\u03C5."@el .
<http://www.w3.org/ns/dcat#distribution> <http://www.w3.org/2004/02/skos/core#definition> "\u062A\u0631\u0628\u0637 \u0642\u0627\u0626\u0645\u0629 \u0627\u0644\u0628\u064A\u0627\u0646\u0627\u062A \u0628\u0637\u0631\u064A\u0642\u0629 \u0623\u0648 \u0628\u0634\u0643\u0644 \u064A\u0633\u0645\u062D  \u0627\u0644\u0648\u0635\u0648\u0644 \u0627\u0644\u0649 \u0627\u0644\u0628\u064A\u0627\u0646\u0627\u062A"@ar .
<http://www.w3.org/ns/dcat#distribution> <http://www.w3.org/2004/02/skos/core#definition> "\u30C7\u30FC\u30BF\u30BB\u30C3\u30C8\u3092\u3001\u305D\u306E\u5229\u7528\u53EF\u80FD\u306A\u914D\u4FE1\u306B\u63A5\u7D9A\u3057\u307E\u3059\u3002"@ja .
<http://www.w3.org/ns/dcat#distribution> <http://www.w3.org/2004/02/skos/core#editorialNote> "Status: English Definition text modified by DCAT revision team, translations pending (except for Italian, Spanish and Czech)."@en .
<http://www.w3.org/ns/dcat#downloadURL> <http://www.w3.org/1999/02/22-rdf-syntax-ns#type> <http://www.w3.org/1999/02/22-rdf-syntax-ns#Property> .
<http://www.w3.org/ns/dcat#downloadURL> <http://www.w3.org/1999/02/22-rdf-syntax-ns#type> <http://www.w3.org/2002/07/owl#ObjectProperty> .
<http://www.w3.org/ns/dcat#downloadURL> <http://www.w3.org/2000/01/rdf-schema#comment> "Ceci est un lien direct \u00E0 un fichier t\u00E9l\u00E9chargeable en un format donn\u00E9e. Exple fichier CSV ou RDF. Le format est d\u00E9crit par les propri\u00E9t\u00E9s de distribution dct:format et/ou dcat:mediaType."@fr .
<http://www.w3.org/ns/dcat#downloadURL> <http://www.w3.org/2000/01/rdf-schema#comment> "La URL de un archivo descargable en el formato dato. Por ejemplo, archivo CSV o archivo RDF. El formato se describe con las propiedades de la distribuci\u00F3n dct:format y/o dcat:mediaType."@es .
<http://www.w3.org/ns/dcat#downloadURL> <http://www.w3.org/2000/01/rdf-schema#comment> "Questo \u00E8 un link diretto al file scaricabile in un dato formato. E.g. un file CSV o un file RDF. Il formato \u00E8 descritto dal dct:format e/o dal dcat:mediaType della distribuzione."@it .
<http://www.w3.org/ns/dcat#downloadURL> <http://www.w3.org/2000/01/rdf-schema#comment> "The URL of the downloadable file in a given format. E.g. CSV file or RDF file. The format is indicated by the distribution's dct:format and/or dcat:mediaType."@en .
<http://www.w3.org/ns/dcat#downloadURL> <http://www.w3.org/2000/01/rdf-schema#comment> "URL souboru ke sta\u017Een\u00ED v dan\u00E9m form\u00E1tu, nap\u0159\u00EDklad CSV nebo RDF soubor. Form\u00E1t je pops\u00E1n vlastnost\u00ED distribuce dct:format a/nebo dcat:mediaType."@cs .
<http://www.w3.org/ns/dcat#downloadURL> <http://www.w3.org/2000/01/rdf-schema#comment> "dcat:downloadURL\u306Fdcat:accessURL\u306E\u7279\u5B9A\u306E\u5F62\u5F0F\u3067\u3059\u3002\u3057\u304B\u3057\u3001DCAT\u30D7\u30ED\u30D5\u30A1\u30A4\u30EB\u304C\u975E\u30C0\u30A6\u30F3\u30ED\u30FC\u30C9\u30FB\u30ED\u30B1\u30FC\u30B7\u30E7\u30F3\u306B\u5BFE\u3057\u3066\u306E\u307FaccessURL\u3092\u7528\u3044\u308B\u5834\u5408\u306B\u306F\u3001\u3088\u308A\u5F37\u3044\u5206\u96E2\u3092\u8AB2\u3059\u3053\u3068\u3092\u671B\u3080\u53EF\u80FD\u6027\u304C\u3042\u308B\u305F\u3081\u3001\u3053\u306E\u542B\u610F\u3092\u5F37\u5316\u3057\u306A\u3044\u3088\u3046\u306B\u3001DCAT\u306F\u3001dcat:downloadURL\u3092dcat:accessURL\u306E\u30B5\u30D6\u30D7\u30ED\u30D1\u30C6\u30A3\u30FC\u3067\u3042\u308B\u3068\u5B9A\u7FA9\u3057\u307E\u305B\u3093\u3002"@ja .
<http://www.w3.org/ns/dcat#downloadURL> <http://www.w3.org/2000/01/rdf-schema#comment> "\u0395\u03AF\u03BD\u03B1\u03B9 \u03AD\u03BD\u03B1\u03C2 \u03C3\u03CD\u03BD\u03B4\u03B5\u03C3\u03BC\u03BF\u03C2 \u03AC\u03BC\u03B5\u03C3\u03B7\u03C2 \u03BC\u03B5\u03C4\u03B1\u03C6\u03CC\u03C1\u03C4\u03C9\u03C3\u03B7\u03C2 \u03B5\u03BD\u03CC\u03C2 \u03B1\u03C1\u03C7\u03B5\u03AF\u03BF\u03C5 \u03C3\u03B5 \u03BC\u03B9\u03B1 \u03B4\u03B5\u03B4\u03BF\u03BC\u03AD\u03BD\u03B7 \u03BC\u03BF\u03C1\u03C6\u03AE. \u03A0.\u03C7. \u03AD\u03BD\u03B1 \u03B1\u03C1\u03C7\u03B5\u03AF\u03BF CSV \u03AE RDF. \u0397 \u03BC\u03BF\u03C1\u03C6\u03B7 \u03B1\u03C1\u03C7\u03B5\u03AF\u03BF\u03C5 \u03C0\u03B5\u03C1\u03B9\u03B3\u03C1\u03AC\u03C6\u03B5\u03C4\u03B1\u03B9 \u03B1\u03C0\u03CC \u03C4\u03B9\u03C2 \u03B9\u03B4\u03B9\u03CC\u03C4\u03B7\u03C4\u03B5\u03C2 dct:format \u03AE/\u03BA\u03B1\u03B9 dcat:mediaType \u03C4\u03B7\u03C2 \u03B4\u03B9\u03B1\u03BD\u03BF\u03BC\u03AE\u03C2."@el .
<http://www.w3.org/ns/dcat#downloadURL> <http://www.w3.org/2000/01/rdf-schema#comment> "\u0631\u0627\u0628\u0637 \u0645\u0628\u0627\u0634\u0631 \u0644\u0645\u0644\u0641 \u064A\u0645\u0643\u0646 \u062A\u062D\u0645\u064A\u0644\u0647. \u0646\u0648\u0639 \u0627\u0644\u0645\u0644\u0641 \u064A\u062A\u0645 \u062A\u0648\u0635\u064A\u0641\u0647 \u0628\u0627\u0633\u062A\u062E\u062F\u0627\u0645 \u0627\u0644\u062E\u0627\u0635\u064A\u0629 dct:format dcat:mediaType "@ar .
<http://www.w3.org/ns/dcat#downloadURL> <http://www.w3.org/2000/01/rdf-schema#domain> <http://www.w3.org/ns/dcat#Distribution> .
<http://www.w3.org/ns/dcat#downloadURL> <http://www.w3.org/2000/01/rdf-schema#isDefinedBy> <http://www.w3.org/TR/vocab-dcat/> .
<http://www.w3.org/ns/dcat#downloadURL> <http://www.w3.org/2000/01/rdf-schema#label> "URL de descarga"@es .
<http://www.w3.org/ns/dcat#downloadURL> <http://www.w3.org/2000/01/rdf-schema#label> "URL de t\u00E9l\u00E9chargement"@fr .
<http://www.w3.org/ns/dcat#downloadURL> <http://www.w3.org/2000/01/rdf-schema#label> "URL di scarico"@it .
<http://www.w3.org/ns/dcat#downloadURL> <http://www.w3.org/2000/01/rdf-schema#label> "URL souboru ke sta\u017Een\u00ED"@cs .
<http://www.w3.org/ns/dcat#downloadURL> <http://www.w3.org/2000/01/rdf-schema#label> "URL \u03BC\u03B5\u03C4\u03B1\u03C6\u03CC\u03C1\u03C4\u03C9\u03C3\u03B7\u03C2"@el .
<http://www.w3.org/ns/dcat#downloadURL> <http://www.w3.org/2000/01/rdf-schema#label> "download URL"@en .
<http://www.w3.org/ns/dcat#downloadURL> <http://www.w3.org/2000/01/rdf-schema#label> "\u0631\u0627\u0628\u0637 \u062A\u062D\u0645\u064A\u0644"@ar .
<http://www.w3.org/ns/dcat#downloadURL> <http://www.w3.org/2000/01/rdf-schema#label> "\u30C0\u30A6\u30F3\u30ED\u30FC\u30C9URL"@ja .
<http://www.w3.org/ns/dcat#downloadURL> <http://www.w3.org/2000/01/rdf-schema#range> <http://www.w3.org/2000/01/rdf-schema#Resource> .
<http://www.w3.org/ns/dcat#downloadURL> <http://www.w3.org/2004/02/skos/core#definition> "Ceci est un lien direct \u00E0 un fichier t\u00E9l\u00E9chargeable en un format donn\u00E9e. Exple fichier CSV ou RDF. Le format est d\u00E9crit par les propri\u00E9t\u00E9s de distribution dct:format et/ou dcat:mediaType."@fr .
<http://www.w3.org/ns/dcat#downloadURL> <http://www.w3.org/2004/02/skos/core#definition> "La URL de un archivo descargable en el formato dato. Por ejemplo, archivo CSV o archivo RDF. El formato se describe con las propiedades de la distribuci\u00F3n dct:format y/o dcat:mediaType."@es .
<http://www.w3.org/ns/dcat#downloadURL> <http://www.w3.org/2004/02/skos/core#definition> "Questo \u00E8 un link diretto al file scaricabile in un dato formato. E.g. un file CSV o un file RDF. Il formato \u00E8 descritto dal dct:format e/o dal dcat:mediaType della distribuzione."@it .
<http://www.w3.org/ns/dcat#downloadURL> <http://www.w3.org/2004/02/skos/core#definition> "The URL of the downloadable file in a given format. E.g. CSV file or RDF file. The format is indicated by the distribution's dct:format and/or dcat:mediaType."@en .
<http://www.w3.org/ns/dcat#downloadURL> <http://www.w3.org/2004/02/skos/core#definition> "URL souboru ke sta\u017Een\u00ED v dan\u00E9m form\u00E1tu, nap\u0159\u00EDklad CSV nebo RDF soubor. Form\u00E1t je pops\u00E1n vlastnost\u00ED distribuce dct:format a/nebo dcat:mediaType."@cs .
<http://www.w3.org/ns/dcat#downloadURL> <http://www.w3.org/2004/02/skos/core#definition> "dcat:downloadURL\u306Fdcat:accessURL\u306E\u7279\u5B9A\u306E\u5F62\u5F0F\u3067\u3059\u3002\u3057\u304B\u3057\u3001DCAT\u30D7\u30ED\u30D5\u30A1\u30A4\u30EB\u304C\u975E\u30C0\u30A6\u30F3\u30ED\u30FC\u30C9\u30FB\u30ED\u30B1\u30FC\u30B7\u30E7\u30F3\u306B\u5BFE\u3057\u3066\u306E\u307FaccessURL\u3092\u7528\u3044\u308B\u5834\u5408\u306B\u306F\u3001\u3088\u308A\u5F37\u3044\u5206\u96E2\u3092\u8AB2\u3059\u3053\u3068\u3092\u671B\u3080\u53EF\u80FD\u6027\u304C\u3042\u308B\u305F\u3081\u3001\u3053\u306E\u542B\u610F\u3092\u5F37\u5316\u3057\u306A\u3044\u3088\u3046\u306B\u3001DCAT\u306F\u3001dcat:downloadURL\u3092dcat:accessURL\u306E\u30B5\u30D6\u30D7\u30ED\u30D1\u30C6\u30A3\u30FC\u3067\u3042\u308B\u3068\u5B9A\u7FA9\u3057\u307E\u305B\u3093\u3002"@ja .
<http://www.w3.org/ns/dcat#downloadURL> <http://www.w3.org/2004/02/skos/core#definition> "\u0395\u03AF\u03BD\u03B1\u03B9 \u03AD\u03BD\u03B1\u03C2 \u03C3\u03CD\u03BD\u03B4\u03B5\u03C3\u03BC\u03BF\u03C2 \u03AC\u03BC\u03B5\u03C3\u03B7\u03C2 \u03BC\u03B5\u03C4\u03B1\u03C6\u03CC\u03C1\u03C4\u03C9\u03C3\u03B7\u03C2 \u03B5\u03BD\u03CC\u03C2 \u03B1\u03C1\u03C7\u03B5\u03AF\u03BF\u03C5 \u03C3\u03B5 \u03BC\u03B9\u03B1 \u03B4\u03B5\u03B4\u03BF\u03BC\u03AD\u03BD\u03B7 \u03BC\u03BF\u03C1\u03C6\u03AE. \u03A0.\u03C7. \u03AD\u03BD\u03B1 \u03B1\u03C1\u03C7\u03B5\u03AF\u03BF CSV \u03AE RDF. \u0397 \u03BC\u03BF\u03C1\u03C6\u03B7 \u03B1\u03C1\u03C7\u03B5\u03AF\u03BF\u03C5 \u03C0\u03B5\u03C1\u03B9\u03B3\u03C1\u03AC\u03C6\u03B5\u03C4\u03B1\u03B9 \u03B1\u03C0\u03CC \u03C4\u03B9\u03C2 \u03B9\u03B4\u03B9\u03CC\u03C4\u03B7\u03C4\u03B5\u03C2 dct:format \u03AE/\u03BA\u03B1\u03B9 dcat:mediaType \u03C4\u03B7\u03C2 \u03B4\u03B9\u03B1\u03BD\u03BF\u03BC\u03AE\u03C2."@el .
<http://www.w3.org/ns/dcat#downloadURL> <http://www.w3.org/2004/02/skos/core#definition> "\u0631\u0627\u0628\u0637 \u0645\u0628\u0627\u0634\u0631 \u0644\u0645\u0644\u0641 \u064A\u0645\u0643\u0646 \u062A\u062D\u0645\u064A\u0644\u0647. \u0646\u0648\u0639 \u0627\u0644\u0645\u0644\u0641 \u064A\u062A\u0645 \u062A\u0648\u0635\u064A\u0641\u0647 \u0628\u0627\u0633\u062A\u062E\u062F\u0627\u0645 \u0627\u0644\u062E\u0627\u0635\u064A\u0629 dct:format dcat:mediaType "@ar .
<http://www.w3.org/ns/dcat#downloadURL> <http://www.w3.org/2004/02/skos/core#editorialNote> "Status: English  Definition text modified by DCAT revision team, Italian, Spanish and Czech translation updated, other translations pending."@en .
<http://www.w3.org/ns/dcat#downloadURL> <http://www.w3.org/2004/02/skos/core#editorialNote> "rdfs:label, rdfs:comment and/or skos:scopeNote have been modified. Non-english versions must be updated."@en .
<http://www.w3.org/ns/dcat#downloadURL> <http://www.w3.org/2004/02/skos/core#scopeNote> "El valor es una URL."@es .
<http://www.w3.org/ns/dcat#downloadURL> <http://www.w3.org/2004/02/skos/core#scopeNote> "La valeur est une URL."@fr .
<http://www.w3.org/ns/dcat#downloadURL> <http://www.w3.org/2004/02/skos/core#scopeNote> "dcat:downloadURL BY M\u011ALA b\u00FDt pou\u017Eita pro adresu, ze kter\u00E9 je distribuce p\u0159\u00EDmo p\u0159\u00EDstupn\u00E1, typicky skrze po\u017Eadavek HTTP Get."@cs .
<http://www.w3.org/ns/dcat#downloadURL> <http://www.w3.org/2004/02/skos/core#scopeNote> "dcat:downloadURL DOVREBBE essere utilizzato per l'indirizzo a cui questa distribuzione \u00E8 disponibile direttamente, in genere attraverso una richiesta Get HTTP."@it .
<http://www.w3.org/ns/dcat#downloadURL> <http://www.w3.org/2004/02/skos/core#scopeNote> "dcat:downloadURL SHOULD be used for the address at which this distribution is available directly, typically through a HTTP Get request."@en .
<http://www.w3.org/ns/dcat#downloadURL> <http://www.w3.org/2004/02/skos/core#scopeNote> "\u0397 \u03C4\u03B9\u03BC\u03AE \u03B5\u03AF\u03BD\u03B1\u03B9 \u03AD\u03BD\u03B1 URL."@el .
<http://www.w3.org/ns/dcat#endDate> <http://www.w3.org/1999/02/22-rdf-syntax-ns#type> <http://www.w3.org/1999/02/22-rdf-syntax-ns#Property> .
<http://www.w3.org/ns/dcat#endDate> <http://www.w3.org/1999/02/22-rdf-syntax-ns#type> <http://www.w3.org/2002/07/owl#DatatypeProperty> .
<http://www.w3.org/ns/dcat#endDate> <http://www.w3.org/2000/01/rdf-schema#domain> <http://purl.org/dc/terms/PeriodOfTime> .
<http://www.w3.org/ns/dcat#endDate> <http://www.w3.org/2000/01/rdf-schema#label> "datum konce"@cs .
<http://www.w3.org/ns/dcat#endDate> <http://www.w3.org/2000/01/rdf-schema#label> "end date"@en .
<http://www.w3.org/ns/dcat#endDate> <http://www.w3.org/2000/01/rdf-schema#label> "data di fine"@it .
<http://www.w3.org/ns/dcat#endDate> <http://www.w3.org/2000/01/rdf-schema#label> "fecha final"@es .
<http://www.w3.org/ns/dcat#endDate> <http://www.w3.org/2000/01/rdf-schema#range> <http://www.w3.org/2000/01/rdf-schema#Literal> .
<http://www.w3.org/ns/dcat#endDate> <http://www.w3.org/2004/02/skos/core#changeNote> "New property added in DCAT 2.0."@en .
<http://www.w3.org/ns/dcat#endDate> <http://www.w3.org/2004/02/skos/core#changeNote> "Nuova propriet\u00E0 aggiunta in DCAT 2.0."@it .
<http://www.w3.org/ns/dcat#endDate> <http://www.w3.org/2004/02/skos/core#changeNote> "Nov\u00E1 vlastnost p\u0159idan\u00E1 ve verzi DCAT 2.0."@cs .
<http://www.w3.org/ns/dcat#endDate> <http://www.w3.org/2004/02/skos/core#changeNote> "Nueva propiedad agregada en DCAT 2.0."@es .
<http://www.w3.org/ns/dcat#endDate> <http://www.w3.org/2004/02/skos/core#definition> "El fin del per\u00EDodo."@es .
<http://www.w3.org/ns/dcat#endDate> <http://www.w3.org/2004/02/skos/core#definition> "Konec doby trv\u00E1n\u00ED."@cs .
<http://www.w3.org/ns/dcat#endDate> <http://www.w3.org/2004/02/skos/core#definition> "The end of the period."@en .
<http://www.w3.org/ns/dcat#endDate> <http://www.w3.org/2004/02/skos/core#definition> "La fine del periodo."@it .
<http://www.w3.org/ns/dcat#endDate> <http://www.w3.org/2004/02/skos/core#scopeNote> "El rango de esta propiedad es intencionalmente gen\u00E9rico con el prop\u00F3sito de permitir distintos niveles de precisi\u00F3n temporal para especificar el fin del per\u00EDodo. Por ejemplo, puede expresarse como una fecha (xsd:date), una fecha y un tiempo (xsd:dateTime), o un a\u00F1o (xsd:gYear)."@es .
<http://www.w3.org/ns/dcat#endDate> <http://www.w3.org/2004/02/skos/core#scopeNote> "Obor hodnot t\u00E9to vlastnosti je \u00FAmysln\u011B obecn\u00FD, aby umo\u017Enil r\u016Fzn\u00E9 \u00FArovn\u011B \u010Dasov\u00E9ho rozli\u0161en\u00ED pro specifikaci konce doby trv\u00E1n\u00ED. Ten m\u016F\u017Ee b\u00FDt kup\u0159\u00EDkladu vyj\u00E1d\u0159en datumem (xsd:date), datumem a \u010Dasem (xsd:dateTime) \u010Di rokem (xsd:gYear)."@cs .
<http://www.w3.org/ns/dcat#endDate> <http://www.w3.org/2004/02/skos/core#scopeNote> "The range of this property is intentionally generic, with the purpose of allowing different level of temporal precision for specifying the end of a period. E.g., it can be expressed with a date (xsd:date), a date and time (xsd:dateTime), or a year (xsd:gYear)."@en .
<http://www.w3.org/ns/dcat#endDate> <http://www.w3.org/2004/02/skos/core#scopeNote> "La range di questa propriet\u00E0 \u00E8 volutamente generico, con lo scopo di consentire diversi livelli di precisione temporale per specificare la fine di un periodo. Ad esempio, pu\u00F2 essere espresso con una data (xsd:date), una data e un'ora (xsd:dateTime), o un anno (xsd:gYear)."@it .
<http://www.w3.org/ns/dcat#endpointDescription> <http://www.w3.org/1999/02/22-rdf-syntax-ns#type> <http://www.w3.org/2002/07/owl#ObjectProperty> .
<http://www.w3.org/ns/dcat#endpointDescription> <http://www.w3.org/2000/01/rdf-schema#comment> "A description of the service end-point, including its operations, parameters etc."@en .
<http://www.w3.org/ns/dcat#endpointDescription> <http://www.w3.org/2000/01/rdf-schema#comment> "Popis p\u0159\u00EDstupov\u00E9ho bodu slu\u017Eby v\u010Detn\u011B operac\u00ED, parametr\u016F apod."@cs .
<http://www.w3.org/ns/dcat#endpointDescription> <http://www.w3.org/2000/01/rdf-schema#comment> "Una descripci\u00F3n del end-point del servicio, incluyendo sus operaciones, par\u00E1metros, etc."@es .
<http://www.w3.org/ns/dcat#endpointDescription> <http://www.w3.org/2000/01/rdf-schema#comment> "Una descrizione dell'endpoint del servizio, incluse le sue operazioni, parametri, ecc."@it .
<http://www.w3.org/ns/dcat#endpointDescription> <http://www.w3.org/2000/01/rdf-schema#domain> <http://www.w3.org/ns/dcat#DataService> .
<http://www.w3.org/ns/dcat#endpointDescription> <http://www.w3.org/2000/01/rdf-schema#label> "descripci\u00F3n del end-point del servicio"@es .
<http://www.w3.org/ns/dcat#endpointDescription> <http://www.w3.org/2000/01/rdf-schema#label> "description of service end-point"@en .
<http://www.w3.org/ns/dcat#endpointDescription> <http://www.w3.org/2000/01/rdf-schema#label> "descrizione dell'endpoint del servizio"@it .
<http://www.w3.org/ns/dcat#endpointDescription> <http://www.w3.org/2000/01/rdf-schema#label> "popis p\u0159\u00EDstupov\u00E9ho bodu slu\u017Eby"@cs .
<http://www.w3.org/ns/dcat#endpointDescription> <http://www.w3.org/2004/02/skos/core#changeNote> "New property in DCAT 2.0."@en .
<http://www.w3.org/ns/dcat#endpointDescription> <http://www.w3.org/2004/02/skos/core#changeNote> "Nov\u00E1 vlastnost p\u0159idan\u00E1 ve verzi DCAT 2.0."@cs .
<http://www.w3.org/ns/dcat#endpointDescription> <http://www.w3.org/2004/02/skos/core#changeNote> "Nueva propiedad agregada en DCAT 2.0."@en .
<http://www.w3.org/ns/dcat#endpointDescription> <http://www.w3.org/2004/02/skos/core#changeNote> "Nuova propriet\u00E0 in DCAT 2.0."@it .
<http://www.w3.org/ns/dcat#endpointDescription> <http://www.w3.org/2004/02/skos/core#definition> "A description of the service end-point, including its operations, parameters etc."@en .
<http://www.w3.org/ns/dcat#endpointDescription> <http://www.w3.org/2004/02/skos/core#definition> "Popis p\u0159\u00EDstupov\u00E9ho bodu slu\u017Eby v\u010Detn\u011B operac\u00ED, parametr\u016F apod."@cs .
<http://www.w3.org/ns/dcat#endpointDescription> <http://www.w3.org/2004/02/skos/core#definition> "Una descripci\u00F3n del end-point del servicio, incluyendo sus operaciones, par\u00E1metros, etc.."@es .
<http://www.w3.org/ns/dcat#endpointDescription> <http://www.w3.org/2004/02/skos/core#definition> "Una descrizione dell'endpoint del servizio, incluse le sue operazioni, parametri, ecc."@it .
<http://www.w3.org/ns/dcat#endpointDescription> <http://www.w3.org/2004/02/skos/core#scopeNote> "An endpoint description may be expressed in a machine-readable form, such as an OpenAPI (Swagger) description, an OGC GetCapabilities response, a SPARQL Service Description, an OpenSearch or WSDL document, a Hydra API description, else in text or some other informal mode if a formal representation is not possible."@en .
<http://www.w3.org/ns/dcat#endpointDescription> <http://www.w3.org/2004/02/skos/core#scopeNote> "La descripci\u00F3n del endpoint brinda detalles espec\u00EDficos de la instancia del endpoint, mientras que dct:conformsTo se usa para indicar el est\u00E1ndar general o especificaci\u00F3n que implementa el endpoint."@es .
<http://www.w3.org/ns/dcat#endpointDescription> <http://www.w3.org/2004/02/skos/core#scopeNote> "La descrizione dell'endpoint fornisce dettagli specifici dell'istanza dell'endpoint reale, mentre dct:conformsTo viene utilizzato per indicare lo standard o le specifiche implementate dall'endpoint."@it .
<http://www.w3.org/ns/dcat#endpointDescription> <http://www.w3.org/2004/02/skos/core#scopeNote> "Popis p\u0159\u00EDstupov\u00E9ho bodu d\u00E1v\u00E1 specifick\u00E9 detaily jeho konkr\u00E9tn\u00ED instance, zat\u00EDmco dct:conformsTo indikuje obecn\u00FD standard \u010Di specifikaci kterou p\u0159\u00EDstupov\u00FD bod implementuje."@cs .
<http://www.w3.org/ns/dcat#endpointDescription> <http://www.w3.org/2004/02/skos/core#scopeNote> "Popis p\u0159\u00EDstupov\u00E9ho bodu m\u016F\u017Ee b\u00FDt vyj\u00E1d\u0159en ve strojov\u011B \u010Diteln\u00E9 form\u011B, nap\u0159\u00EDklad jako popis OpenAPI (Swagger), odpov\u011B\u010F slu\u017Eby OGC getCapabilities, pomoc\u00ED slovn\u00EDku SPARQL Service Description, jako OpenSearch \u010Di WSDL document, jako popis API dle slovn\u00EDku Hydra, a nebo textov\u011B nebo jin\u00FDm neform\u00E1ln\u00EDm zp\u016Fsobem, pokud nen\u00ED mo\u017Eno pou\u017E\u00EDt form\u00E1ln\u00ED reprezentaci."@cs .
<http://www.w3.org/ns/dcat#endpointDescription> <http://www.w3.org/2004/02/skos/core#scopeNote> "The endpoint decription gives specific details of the actual endpoint instance, while dct:conformsTo is used to indicate the general standard or specification that the endpoint implements."@en .
<http://www.w3.org/ns/dcat#endpointDescription> <http://www.w3.org/2004/02/skos/core#scopeNote> "Una descripci\u00F3n del endpoint del servicio puede expresarse en un formato que la m\u00E1quina puede interpretar, tal como una descripci\u00F3n basada en OpenAPI (Swagger), una respuesta OGC GetCapabilities, una descripci\u00F3n de un servicio SPARQL, un documento OpenSearch o WSDL, una descripci\u00F3n con la Hydra API, o en texto u otro modo informal si la representaci\u00F3n formal no es posible."@es .
<http://www.w3.org/ns/dcat#endpointDescription> <http://www.w3.org/2004/02/skos/core#scopeNote> "Una descrizione dell'endpoint pu\u00F2 essere espressa in un formato leggibile dalla macchina, come una descrizione OpenAPI (Swagger), una risposta GetCapabilities OGC, una descrizione del servizio SPARQL, un documento OpenSearch o WSDL, una descrizione API Hydra, o con del testo o qualche altra modalit\u00E0 informale se una rappresentazione formale non \u00E8 possibile."@it .
<http://www.w3.org/ns/dcat#endpointURL> <http://www.w3.org/1999/02/22-rdf-syntax-ns#type> <http://www.w3.org/2002/07/owl#ObjectProperty> .
<http://www.w3.org/ns/dcat#endpointURL> <http://www.w3.org/2000/01/rdf-schema#comment> "Ko\u0159enov\u00E9 um\u00EDst\u011Bn\u00ED nebo hlavn\u00ED p\u0159\u00EDstupov\u00FD bod slu\u017Eby (IRI p\u0159\u00EDstupn\u00E9 p\u0159es Web)."@cs .
<http://www.w3.org/ns/dcat#endpointURL> <http://www.w3.org/2000/01/rdf-schema#comment> "La locazione principale o l'endpoint primario del servizio (un IRI risolvibile via web)."@it .
<http://www.w3.org/ns/dcat#endpointURL> <http://www.w3.org/2000/01/rdf-schema#comment> "La posici\u00F3n ra\u00EDz o end-point principal del servicio (una IRI web)."@es .
<http://www.w3.org/ns/dcat#endpointURL> <http://www.w3.org/2000/01/rdf-schema#comment> "The root location or primary endpoint of the service (a web-resolvable IRI)."@en .
<http://www.w3.org/ns/dcat#endpointURL> <http://www.w3.org/2000/01/rdf-schema#domain> <http://www.w3.org/ns/dcat#DataService> .
<http://www.w3.org/ns/dcat#endpointURL> <http://www.w3.org/2000/01/rdf-schema#label> "end-point del servicio"@es .
<http://www.w3.org/ns/dcat#endpointURL> <http://www.w3.org/2000/01/rdf-schema#label> "end-point del servizio"@it .
<http://www.w3.org/ns/dcat#endpointURL> <http://www.w3.org/2000/01/rdf-schema#label> "p\u0159\u00EDstupov\u00FD bod slu\u017Eby"@cs .
<http://www.w3.org/ns/dcat#endpointURL> <http://www.w3.org/2000/01/rdf-schema#label> "service end-point"@en .
<http://www.w3.org/ns/dcat#endpointURL> <http://www.w3.org/2000/01/rdf-schema#range> <http://www.w3.org/2000/01/rdf-schema#Resource> .
<http://www.w3.org/ns/dcat#endpointURL> <http://www.w3.org/2004/02/skos/core#changeNote> "New property in DCAT 2.0."@en .
<http://www.w3.org/ns/dcat#endpointURL> <http://www.w3.org/2004/02/skos/core#changeNote> "Nov\u00E1 vlastnost p\u0159idan\u00E1 ve verzi DCAT 2.0."@cs .
<http://www.w3.org/ns/dcat#endpointURL> <http://www.w3.org/2004/02/skos/core#changeNote> "Nueva propiedad agregada en DCAT 2.0."@es .
<http://www.w3.org/ns/dcat#endpointURL> <http://www.w3.org/2004/02/skos/core#changeNote> "Nuova propriet\u00E0 in DCAT 2.0."@it .
<http://www.w3.org/ns/dcat#endpointURL> <http://www.w3.org/2004/02/skos/core#definition> "Ko\u0159enov\u00E9 um\u00EDst\u011Bn\u00ED nebo hlavn\u00ED p\u0159\u00EDstupov\u00FD bod slu\u017Eby (IRI p\u0159\u00EDstupn\u00E9 p\u0159es Web)."@cs .
<http://www.w3.org/ns/dcat#endpointURL> <http://www.w3.org/2004/02/skos/core#definition> "La locazione principale o l'endpoint primario del servizio (un IRI risolvibile via web)."@it .
<http://www.w3.org/ns/dcat#endpointURL> <http://www.w3.org/2004/02/skos/core#definition> "La posici\u00F3n ra\u00EDz o end-point principal del servicio (una IRI web)."@es .
<http://www.w3.org/ns/dcat#endpointURL> <http://www.w3.org/2004/02/skos/core#definition> "The root location or primary endpoint of the service (a web-resolvable IRI)."@en .
_:genid32 <http://www.w3.org/1999/02/22-rdf-syntax-ns#first> <http://www.w3.org/ns/dcat#Relationship> .
_:genid32 <http://www.w3.org/1999/02/22-rdf-syntax-ns#rest> <http://www.w3.org/1999/02/22-rdf-syntax-ns#nil> .
_:genid33 <http://www.w3.org/1999/02/22-rdf-syntax-ns#first> <http://www.w3.org/ns/prov#Attribution> .
_:genid33 <http://www.w3.org/1999/02/22-rdf-syntax-ns#rest> _:genid32 .
_:genid34 <http://www.w3.org/1999/02/22-rdf-syntax-ns#type> <http://www.w3.org/2002/07/owl#Class> .
_:genid34 <http://www.w3.org/2002/07/owl#unionOf> _:genid33 .
<http://www.w3.org/ns/dcat#hadRole> <http://www.w3.org/1999/02/22-rdf-syntax-ns#type> <http://www.w3.org/2002/07/owl#ObjectProperty> .
<http://www.w3.org/ns/dcat#hadRole> <http://www.w3.org/2000/01/rdf-schema#comment> "Funkce entity \u010Di agenta ve vztahu k jin\u00E9 entit\u011B \u010Di zdroji."@cs .
<http://www.w3.org/ns/dcat#hadRole> <http://www.w3.org/2000/01/rdf-schema#comment> "La funci\u00F3n de una entidad o agente con respecto a otra entidad o recurso."@es .
<http://www.w3.org/ns/dcat#hadRole> <http://www.w3.org/2000/01/rdf-schema#comment> "La funzione di un'entit\u00E0 o un agente rispetto ad un'altra entit\u00E0 o risorsa."@it .
<http://www.w3.org/ns/dcat#hadRole> <http://www.w3.org/2000/01/rdf-schema#comment> "The function of an entity or agent with respect to another entity or resource."@en .
<http://www.w3.org/ns/dcat#hadRole> <http://www.w3.org/2000/01/rdf-schema#domain> _:genid34 .
<http://www.w3.org/ns/dcat#hadRole> <http://www.w3.org/2000/01/rdf-schema#label> "haRuolo"@it .
<http://www.w3.org/ns/dcat#hadRole> <http://www.w3.org/2000/01/rdf-schema#label> "hadRole"@en .
<http://www.w3.org/ns/dcat#hadRole> <http://www.w3.org/2000/01/rdf-schema#label> "sehran\u00E1 role"@cs .
<http://www.w3.org/ns/dcat#hadRole> <http://www.w3.org/2000/01/rdf-schema#label> "tiene rol"@it .
<http://www.w3.org/ns/dcat#hadRole> <http://www.w3.org/2000/01/rdf-schema#range> <http://www.w3.org/ns/dcat#Role> .
<http://www.w3.org/ns/dcat#hadRole> <http://www.w3.org/2004/02/skos/core#changeNote> "New property added in DCAT 2.0."@en .
<http://www.w3.org/ns/dcat#hadRole> <http://www.w3.org/2004/02/skos/core#changeNote> "Nov\u00E1 vlastnost p\u0159idan\u00E1 ve verzi DCAT 2.0."@cs .
<http://www.w3.org/ns/dcat#hadRole> <http://www.w3.org/2004/02/skos/core#changeNote> "Nueva propiedad agregada en DCAT 2.0."@es .
<http://www.w3.org/ns/dcat#hadRole> <http://www.w3.org/2004/02/skos/core#changeNote> "Nuova propriet\u00E0 aggiunta in DCAT 2.0."@it .
<http://www.w3.org/ns/dcat#hadRole> <http://www.w3.org/2004/02/skos/core#definition> "Funkce entity \u010Di agenta ve vztahu k jin\u00E9 entit\u011B \u010Di zdroji."@cs .
<http://www.w3.org/ns/dcat#hadRole> <http://www.w3.org/2004/02/skos/core#definition> "La funci\u00F3n de una entidad o agente con respecto a otra entidad o recurso."@es .
<http://www.w3.org/ns/dcat#hadRole> <http://www.w3.org/2004/02/skos/core#definition> "La funzione di un'entit\u00E0 o un agente rispetto ad un'altra entit\u00E0 o risorsa."@it .
<http://www.w3.org/ns/dcat#hadRole> <http://www.w3.org/2004/02/skos/core#definition> "The function of an entity or agent with respect to another entity or resource."@en .
<http://www.w3.org/ns/dcat#hadRole> <http://www.w3.org/2004/02/skos/core#editorialNote> "Agregada en DCAT para complementar prov:hadRole (cuyo uso est\u00E1 limitado a roles en el contexto de una actividad, con dominio prov:Association."@es .
<http://www.w3.org/ns/dcat#hadRole> <http://www.w3.org/2004/02/skos/core#editorialNote> "Introdotta in DCAT per completare prov:hadRole (il cui uso \u00E8 limitato ai ruoli nel contesto di un'attivit\u00E0, con il dominio di prov:Association."@it .
<http://www.w3.org/ns/dcat#hadRole> <http://www.w3.org/2004/02/skos/core#editorialNote> "Introduced into DCAT to complement prov:hadRole (whose use is limited to roles in the context of an activity, with the domain of prov:Association."@en .
<http://www.w3.org/ns/dcat#hadRole> <http://www.w3.org/2004/02/skos/core#editorialNote> "P\u0159id\u00E1no do DCAT pro dopln\u011Bn\u00ED vlastnosti prov:hadRole (jej\u00ED\u017E u\u017Eit\u00ED je omezeno na role v kontextu aktivity, s defini\u010Dn\u00EDm oborem prov:Association)."@cs .
<http://www.w3.org/ns/dcat#hadRole> <http://www.w3.org/2004/02/skos/core#scopeNote> "May be used in a qualified-attribution to specify the role of an Agent with respect to an Entity. It is recommended that the value be taken from a controlled vocabulary of agent roles, such as http://registry.it.csiro.au/def/isotc211/CI_RoleCode."@en .
<http://www.w3.org/ns/dcat#hadRole> <http://www.w3.org/2004/02/skos/core#scopeNote> "May be used in a qualified-relation to specify the role of an Entity with respect to another Entity.  It is recommended that the value be taken from a controlled vocabulary of entity roles such as: ISO 19115 DS_AssociationTypeCode http://registry.it.csiro.au/def/isotc211/DS_AssociationTypeCode; IANA Registry of Link Relations https://www.iana.org/assignments/link-relation; DataCite metadata schema; MARC relators https://id.loc.gov/vocabulary/relators."@en .
<http://www.w3.org/ns/dcat#hadRole> <http://www.w3.org/2004/02/skos/core#scopeNote> "M\u016F\u017Ee b\u00FDt pou\u017Eito v kvalifikovan\u00E9m p\u0159i\u0159azen\u00ED pro specifikaci role Agenta ve vztahu k Entit\u011B. Je doporu\u010Deno hodnotu vybrat z \u0159\u00EDzen\u00E9ho slovn\u00EDku rol\u00ED agent\u016F, jako nap\u0159\u00EDklad http://registry.it.csiro.au/def/isotc211/CI_RoleCode."@cs .
<http://www.w3.org/ns/dcat#hadRole> <http://www.w3.org/2004/02/skos/core#scopeNote> "M\u016F\u017Ee b\u00FDt pou\u017Eito v kvalifikovan\u00E9m vztahu pro specifikaci role Entity ve vztahu k jin\u00E9 Entit\u011B. Je doporu\u010Deno pou\u017E\u00EDt hodnotu z \u0159\u00EDzen\u00E9ho slovn\u00EDku rol\u00ED entit, jako nap\u0159\u00EDklad ISO 19115 DS_AssociationTypeCode http://registry.it.csiro.au/def/isotc211/DS_AssociationTypeCode, IANA Registry of Link Relations https://www.iana.org/assignments/link-relation, DataCite metadata schema, MARC relators https://id.loc.gov/vocabulary/relators."@cs .
<http://www.w3.org/ns/dcat#hadRole> <http://www.w3.org/2004/02/skos/core#scopeNote> "Puede usarse en una atribuci\u00F3n cualificada para especificar el rol de un Agente con respecto a una Entidad. Se recomienda que el valor sea de un vocabulario controlado de roles de agentes, como por ejemplo http://registry.it.csiro.au/def/isotc211/CI_RoleCode."@es .
<http://www.w3.org/ns/dcat#hadRole> <http://www.w3.org/2004/02/skos/core#scopeNote> "Puede usarse en una atribuci\u00F3n cualificada para especificar el rol de una Entidad con respecto a otra Entidad. Se recomienda que su valor se tome de un vocabulario controlado de roles de entidades como por ejemplo: ISO 19115 DS_AssociationTypeCode http://registry.it.csiro.au/def/isotc211/DS_AssociationTypeCode; IANA Registry of Link Relations https://www.iana.org/assignments/link-relation; esquema de metadatos de DataCite; MARC relators https://id.loc.gov/vocabulary/relators."@es .
<http://www.w3.org/ns/dcat#hadRole> <http://www.w3.org/2004/02/skos/core#scopeNote> "Pu\u00F2 essere utilizzata in una relazione qualificata per specificare il ruolo di un'entit\u00E0 rispetto a un'altra entit\u00E0. Si raccomanda che il valore sia preso da un vocabolario controllato di ruoli di entit\u00E0 come ISO 19115 DS_AssociationTypeCode http://registry.it.csiro.au/def/isotc211/DS_AssociationTypeCode, IANA Registry of Link Relations https://www.iana.org/assignments/link-relation, DataCite metadata schema, o MARC relators https://id.loc.gov/vocabulary/relators."@it .
<http://www.w3.org/ns/dcat#hadRole> <http://www.w3.org/2004/02/skos/core#scopeNote> "Pu\u00F2 essere utilizzato in un'attribuzione qualificata per specificare il ruolo di un agente rispetto a un'entit\u00E0. Si raccomanda che il valore sia preso da un vocabolario controllato di ruoli di agente, come ad esempio http://registry.it.csiro.au/def/isotc211/CI_RoleCode."@it .
<http://www.w3.org/ns/dcat#keyword> <http://www.w3.org/1999/02/22-rdf-syntax-ns#type> <http://www.w3.org/1999/02/22-rdf-syntax-ns#Property> .
<http://www.w3.org/ns/dcat#keyword> <http://www.w3.org/1999/02/22-rdf-syntax-ns#type> <http://www.w3.org/2002/07/owl#DatatypeProperty> .
<http://www.w3.org/ns/dcat#keyword> <http://www.w3.org/2000/01/rdf-schema#comment> "A keyword or tag describing a resource."@en .
<http://www.w3.org/ns/dcat#keyword> <http://www.w3.org/2000/01/rdf-schema#comment> "Kl\u00ED\u010Dov\u00E9 slovo nebo zna\u010Dka popisuj\u00EDc\u00ED zdroj."@cs .
<http://www.w3.org/ns/dcat#keyword> <http://www.w3.org/2000/01/rdf-schema#comment> "Un mot-cl\u00E9 ou \u00E9tiquette d\u00E9crivant une ressource."@fr .
<http://www.w3.org/ns/dcat#keyword> <http://www.w3.org/2000/01/rdf-schema#comment> "Una palabra clave o etiqueta que describe un recurso."@es .
<http://www.w3.org/ns/dcat#keyword> <http://www.w3.org/2000/01/rdf-schema#comment> "Una parola chiave o un'etichetta per descrivere la risorsa."@it .
<http://www.w3.org/ns/dcat#keyword> <http://www.w3.org/2000/01/rdf-schema#comment> "\u039C\u03AF\u03B1 \u03BB\u03AD\u03BE\u03B7-\u03BA\u03BB\u03B5\u03B9\u03B4\u03AF \u03AE \u03BC\u03AF\u03B1 \u03B5\u03C4\u03B9\u03BA\u03AD\u03C4\u03B1 \u03C0\u03BF\u03C5 \u03C0\u03B5\u03C1\u03B9\u03B3\u03C1\u03AC\u03C6\u03B5\u03B9 \u03C4\u03BF \u03C3\u03CD\u03BD\u03BF\u03BB\u03BF \u03B4\u03B5\u03B4\u03BF\u03BC\u03AD\u03BD\u03C9\u03BD."@el .
<http://www.w3.org/ns/dcat#keyword> <http://www.w3.org/2000/01/rdf-schema#comment> "\u0643\u0644\u0645\u0629  \u0645\u0641\u062A\u0627\u062D\u064A\u0647 \u062A\u0648\u0635\u0641 \u0642\u0627\u0626\u0645\u0629 \u0627\u0644\u0628\u064A\u0627\u0646\u0627\u062A"@ar .
<http://www.w3.org/ns/dcat#keyword> <http://www.w3.org/2000/01/rdf-schema#comment> "\u30C7\u30FC\u30BF\u30BB\u30C3\u30C8\u3092\u8A18\u8FF0\u3057\u3066\u3044\u308B\u30AD\u30FC\u30EF\u30FC\u30C9\u307E\u305F\u306F\u30BF\u30B0\u3002"@ja .
<http://www.w3.org/ns/dcat#keyword> <http://www.w3.org/2000/01/rdf-schema#isDefinedBy> <http://www.w3.org/TR/vocab-dcat/> .
<http://www.w3.org/ns/dcat#keyword> <http://www.w3.org/2000/01/rdf-schema#label> "keyword"@en .
<http://www.w3.org/ns/dcat#keyword> <http://www.w3.org/2000/01/rdf-schema#label> "kl\u00ED\u010Dov\u00E9 slovo"@cs .
<http://www.w3.org/ns/dcat#keyword> <http://www.w3.org/2000/01/rdf-schema#label> "mot-cl\u00E9s "@fr .
<http://www.w3.org/ns/dcat#keyword> <http://www.w3.org/2000/01/rdf-schema#label> "palabra clave"@es .
<http://www.w3.org/ns/dcat#keyword> <http://www.w3.org/2000/01/rdf-schema#label> "parola chiave"@it .
<http://www.w3.org/ns/dcat#keyword> <http://www.w3.org/2000/01/rdf-schema#label> "\u03BB\u03AD\u03BE\u03B7-\u03BA\u03BB\u03B5\u03B9\u03B4\u03AF"@el .
<http://www.w3.org/ns/dcat#keyword> <http://www.w3.org/2000/01/rdf-schema#label> "\u0643\u0644\u0645\u0629  \u0645\u0641\u062A\u0627\u062D\u064A\u0629 "@ar .
<http://www.w3.org/ns/dcat#keyword> <http://www.w3.org/2000/01/rdf-schema#label> "\u30AD\u30FC\u30EF\u30FC\u30C9/\u30BF\u30B0"@ja .
<http://www.w3.org/ns/dcat#keyword> <http://www.w3.org/2000/01/rdf-schema#range> <http://www.w3.org/2000/01/rdf-schema#Literal> .
<http://www.w3.org/ns/dcat#keyword> <http://www.w3.org/2000/01/rdf-schema#subPropertyOf> <http://purl.org/dc/terms/subject> .
<http://www.w3.org/ns/dcat#keyword> <http://www.w3.org/2004/02/skos/core#definition> "A keyword or tag describing a resource."@en .
<http://www.w3.org/ns/dcat#keyword> <http://www.w3.org/2004/02/skos/core#definition> "Kl\u00ED\u010Dov\u00E9 slovo nebo zna\u010Dka popisuj\u00EDc\u00ED zdroj."@cs .
<http://www.w3.org/ns/dcat#keyword> <http://www.w3.org/2004/02/skos/core#definition> "Un mot-cl\u00E9 ou \u00E9tiquette d\u00E9crivant une ressource."@fr .
<http://www.w3.org/ns/dcat#keyword> <http://www.w3.org/2004/02/skos/core#definition> "Una palabra clave o etiqueta que describe un recurso."@es .
<http://www.w3.org/ns/dcat#keyword> <http://www.w3.org/2004/02/skos/core#definition> "Una parola chiave o un'etichetta per descrivere la risorsa."@it .
<http://www.w3.org/ns/dcat#keyword> <http://www.w3.org/2004/02/skos/core#definition> "\u039C\u03AF\u03B1 \u03BB\u03AD\u03BE\u03B7-\u03BA\u03BB\u03B5\u03B9\u03B4\u03AF \u03AE \u03BC\u03AF\u03B1 \u03B5\u03C4\u03B9\u03BA\u03AD\u03C4\u03B1 \u03C0\u03BF\u03C5 \u03C0\u03B5\u03C1\u03B9\u03B3\u03C1\u03AC\u03C6\u03B5\u03B9 \u03C4\u03BF \u03C3\u03CD\u03BD\u03BF\u03BB\u03BF \u03B4\u03B5\u03B4\u03BF\u03BC\u03AD\u03BD\u03C9\u03BD."@el .
<http://www.w3.org/ns/dcat#keyword> <http://www.w3.org/2004/02/skos/core#definition> "\u0643\u0644\u0645\u0629  \u0645\u0641\u062A\u0627\u062D\u064A\u0647 \u062A\u0648\u0635\u0641 \u0642\u0627\u0626\u0645\u0629 \u0627\u0644\u0628\u064A\u0627\u0646\u0627\u062A"@ar .
<http://www.w3.org/ns/dcat#keyword> <http://www.w3.org/2004/02/skos/core#definition> "\u30C7\u30FC\u30BF\u30BB\u30C3\u30C8\u3092\u8A18\u8FF0\u3057\u3066\u3044\u308B\u30AD\u30FC\u30EF\u30FC\u30C9\u307E\u305F\u306F\u30BF\u30B0\u3002"@ja .
<http://www.w3.org/ns/dcat#landingPage> <http://www.w3.org/1999/02/22-rdf-syntax-ns#type> <http://www.w3.org/1999/02/22-rdf-syntax-ns#Property> .
<http://www.w3.org/ns/dcat#landingPage> <http://www.w3.org/1999/02/22-rdf-syntax-ns#type> <http://www.w3.org/2002/07/owl#ObjectProperty> .
<http://www.w3.org/ns/dcat#landingPage> <http://www.w3.org/2000/01/rdf-schema#comment> "A Web page that can be navigated to in a Web browser to gain access to the catalog, a dataset, its distributions and/or additional information."@en .
<http://www.w3.org/ns/dcat#landingPage> <http://www.w3.org/2000/01/rdf-schema#comment> "Una pagina web che pu\u00F2 essere navigata per ottenere l'accesso al catalogo, ad un dataset, alle distribuzioni del dataset e/o ad informazioni addizionali."@it .
<http://www.w3.org/ns/dcat#landingPage> <http://www.w3.org/2000/01/rdf-schema#comment> "Una p\u00E1gina web que puede ser visitada en un explorador Web para tener acceso el cat\u00E1logo, un conjunto de datos, sus distribuciones y/o informaci\u00F3n adicional."@es .
<http://www.w3.org/ns/dcat#landingPage> <http://www.w3.org/2000/01/rdf-schema#comment> "Une page Web accessible par un navigateur Web donnant acc\u00E8s au catalogue, un jeu de donn\u00E9es, ses distributions et/ou des informations additionnelles."@fr .
<http://www.w3.org/ns/dcat#landingPage> <http://www.w3.org/2000/01/rdf-schema#comment> "Webov\u00E1 str\u00E1nka, na kterou lze pro z\u00EDsk\u00E1n\u00ED p\u0159\u00EDstupu ke katalogu, datov\u00E9 sad\u011B, jej\u00EDm distribuc\u00EDm a/nebo dal\u0161\u00EDm informac\u00EDm p\u0159istoupit webov\u00FDm prohl\u00ED\u017Ee\u010Dem."@cs .
<http://www.w3.org/ns/dcat#landingPage> <http://www.w3.org/2000/01/rdf-schema#comment> "\u039C\u03AF\u03B1 \u03B9\u03C3\u03C4\u03BF\u03C3\u03B5\u03BB\u03AF\u03B4\u03B1 \u03C0\u03BB\u03BF\u03B7\u03B3\u03AF\u03C3\u03B9\u03BC\u03B7 \u03BC\u03AD\u03C3\u03C9 \u03B5\u03BD\u03CC\u03C2 \u03C6\u03C5\u03BB\u03BB\u03BF\u03BC\u03B5\u03C4\u03C1\u03B7\u03C4\u03AE (Web browser) \u03C0\u03BF\u03C5 \u03B4\u03AF\u03BD\u03B5\u03B9 \u03C0\u03C1\u03CC\u03C3\u03B2\u03B1\u03C3\u03B7 \u03C3\u03C4\u03BF \u03C3\u03CD\u03BD\u03BF\u03BB\u03BF \u03B4\u03B5\u03B4\u03BF\u03BC\u03AD\u03BD\u03C9\u03BD, \u03C4\u03B9\u03C2 \u03B4\u03B9\u03B1\u03BD\u03BF\u03BC\u03AD\u03C2 \u03B1\u03C5\u03C4\u03BF\u03CD \u03AE/\u03BA\u03B1\u03B9 \u03B5\u03C0\u03B9\u03C0\u03C1\u03CC\u03C3\u03B8\u03B5\u03C4\u03B5\u03C2 \u03C0\u03BB\u03B7\u03C1\u03BF\u03C6\u03BF\u03C1\u03AF\u03B5\u03C2."@el .
<http://www.w3.org/ns/dcat#landingPage> <http://www.w3.org/2000/01/rdf-schema#comment> "\u0635\u0641\u062D\u0629 \u0648\u0628 \u064A\u0645\u0643\u0646 \u0645\u0646 \u062E\u0644\u0627\u0644\u0647\u0627 \u0627\u0644\u0648\u0635\u0648\u0644 \u0627\u0644\u0649 \u0642\u0627\u0626\u0645\u0629 \u0627\u0644\u0628\u064A\u0627\u0646\u0627\u062A \u0623\u0648 \u0625\u0644\u0649 \u0645\u0639\u0644\u0648\u0645\u0627\u062A \u0625\u0636\u0627\u0641\u064A\u0629 \u0645\u062A\u0639\u0644\u0642\u0629 \u0628\u0647\u0627 "@ar .
<http://www.w3.org/ns/dcat#landingPage> <http://www.w3.org/2000/01/rdf-schema#comment> "\u30C7\u30FC\u30BF\u30BB\u30C3\u30C8\u3001\u305D\u306E\u914D\u4FE1\u304A\u3088\u3073\uFF08\u307E\u305F\u306F\uFF09\u8FFD\u52A0\u60C5\u5831\u306B\u30A2\u30AF\u30BB\u30B9\u3059\u308B\u305F\u3081\u306B\u30A6\u30A8\u30D6\u30FB\u30D6\u30E9\u30A6\u30B6\u3067\u30CA\u30D3\u30B2\u30FC\u30C8\u3067\u304D\u308B\u30A6\u30A7\u30D6\u30DA\u30FC\u30B8\u3002"@ja .
<http://www.w3.org/ns/dcat#landingPage> <http://www.w3.org/2000/01/rdf-schema#isDefinedBy> <http://www.w3.org/TR/vocab-dcat/> .
<http://www.w3.org/ns/dcat#landingPage> <http://www.w3.org/2000/01/rdf-schema#label> "landing page"@en .
<http://www.w3.org/ns/dcat#landingPage> <http://www.w3.org/2000/01/rdf-schema#label> "page d'atterrissage"@fr .
<http://www.w3.org/ns/dcat#landingPage> <http://www.w3.org/2000/01/rdf-schema#label> "pagina di destinazione"@it .
<http://www.w3.org/ns/dcat#landingPage> <http://www.w3.org/2000/01/rdf-schema#label> "p\u00E1gina de destino"@es .
<http://www.w3.org/ns/dcat#landingPage> <http://www.w3.org/2000/01/rdf-schema#label> "vstupn\u00ED str\u00E1nka"@cs .
<http://www.w3.org/ns/dcat#landingPage> <http://www.w3.org/2000/01/rdf-schema#label> "\u03B9\u03C3\u03C4\u03BF\u03C3\u03B5\u03BB\u03AF\u03B4\u03B1 \u03B1\u03C1\u03C7\u03B9\u03BA\u03AE\u03C2 \u03C0\u03C1\u03CC\u03C3\u03B2\u03B1\u03C3\u03B7\u03C2"@el .
<http://www.w3.org/ns/dcat#landingPage> <http://www.w3.org/2000/01/rdf-schema#label> "\u0635\u0641\u062D\u0629 \u0648\u0635\u0648\u0644"@ar .
<http://www.w3.org/ns/dcat#landingPage> <http://www.w3.org/2000/01/rdf-schema#label> "\u30E9\u30F3\u30C7\u30A3\u30F3\u30B0\u30FB\u30DA\u30FC\u30B8"@ja .
<http://www.w3.org/ns/dcat#landingPage> <http://www.w3.org/2000/01/rdf-schema#range> <http://xmlns.com/foaf/0.1/Document> .
<http://www.w3.org/ns/dcat#landingPage> <http://www.w3.org/2000/01/rdf-schema#subPropertyOf> <http://xmlns.com/foaf/0.1/page> .
<http://www.w3.org/ns/dcat#landingPage> <http://www.w3.org/2004/02/skos/core#definition> "A Web page that can be navigated to in a Web browser to gain access to the catalog, a dataset, its distributions and/or additional information."@en .
<http://www.w3.org/ns/dcat#landingPage> <http://www.w3.org/2004/02/skos/core#definition> "Una pagina web che pu\u00F2 essere navigata per ottenere l'accesso al catalogo, ad un dataset, alle distribuzioni del dataset e/o ad informazioni addizionali."@it .
<http://www.w3.org/ns/dcat#landingPage> <http://www.w3.org/2004/02/skos/core#definition> "Una p\u00E1gina web que puede ser visitada en un explorador Web para tener acceso el cat\u00E1logo, un conjunto de datos, sus distribuciones y/o informaci\u00F3n adicional."@es .
<http://www.w3.org/ns/dcat#landingPage> <http://www.w3.org/2004/02/skos/core#definition> "Une page Web accessible par un navigateur Web donnant acc\u00E8s au catalogue, un jeu de donn\u00E9es, ses distributions et/ou des informations additionnelles."@fr .
<http://www.w3.org/ns/dcat#landingPage> <http://www.w3.org/2004/02/skos/core#definition> "Webov\u00E1 str\u00E1nka, na kterou lze pro z\u00EDsk\u00E1n\u00ED p\u0159\u00EDstupu ke katalogu, datov\u00E9 sad\u011B, jej\u00EDm distribuc\u00EDm a/nebo dal\u0161\u00EDm informac\u00EDm p\u0159istoupit webov\u00FDm prohl\u00ED\u017Ee\u010Dem."@cs .
<http://www.w3.org/ns/dcat#landingPage> <http://www.w3.org/2004/02/skos/core#definition> "\u039C\u03AF\u03B1 \u03B9\u03C3\u03C4\u03BF\u03C3\u03B5\u03BB\u03AF\u03B4\u03B1 \u03C0\u03BB\u03BF\u03B7\u03B3\u03AF\u03C3\u03B9\u03BC\u03B7 \u03BC\u03AD\u03C3\u03C9 \u03B5\u03BD\u03CC\u03C2 \u03C6\u03C5\u03BB\u03BB\u03BF\u03BC\u03B5\u03C4\u03C1\u03B7\u03C4\u03AE (Web browser) \u03C0\u03BF\u03C5 \u03B4\u03AF\u03BD\u03B5\u03B9 \u03C0\u03C1\u03CC\u03C3\u03B2\u03B1\u03C3\u03B7 \u03C3\u03C4\u03BF \u03C3\u03CD\u03BD\u03BF\u03BB\u03BF \u03B4\u03B5\u03B4\u03BF\u03BC\u03AD\u03BD\u03C9\u03BD, \u03C4\u03B9\u03C2 \u03B4\u03B9\u03B1\u03BD\u03BF\u03BC\u03AD\u03C2 \u03B1\u03C5\u03C4\u03BF\u03CD \u03AE/\u03BA\u03B1\u03B9 \u03B5\u03C0\u03B9\u03C0\u03C1\u03CC\u03C3\u03B8\u03B5\u03C4\u03B5\u03C2 \u03C0\u03BB\u03B7\u03C1\u03BF\u03C6\u03BF\u03C1\u03AF\u03B5\u03C2."@el .
<http://www.w3.org/ns/dcat#landingPage> <http://www.w3.org/2004/02/skos/core#definition> "\u0635\u0641\u062D\u0629 \u0648\u0628 \u064A\u0645\u0643\u0646 \u0645\u0646 \u062E\u0644\u0627\u0644\u0647\u0627 \u0627\u0644\u0648\u0635\u0648\u0644 \u0627\u0644\u0649 \u0642\u0627\u0626\u0645\u0629 \u0627\u0644\u0628\u064A\u0627\u0646\u0627\u062A \u0623\u0648 \u0625\u0644\u0649 \u0645\u0639\u0644\u0648\u0645\u0627\u062A \u0625\u0636\u0627\u0641\u064A\u0629 \u0645\u062A\u0639\u0644\u0642\u0629 \u0628\u0647\u0627 "@ar .
<http://www.w3.org/ns/dcat#landingPage> <http://www.w3.org/2004/02/skos/core#definition> "\u30C7\u30FC\u30BF\u30BB\u30C3\u30C8\u3001\u305D\u306E\u914D\u4FE1\u304A\u3088\u3073\uFF08\u307E\u305F\u306F\uFF09\u8FFD\u52A0\u60C5\u5831\u306B\u30A2\u30AF\u30BB\u30B9\u3059\u308B\u305F\u3081\u306B\u30A6\u30A8\u30D6\u30FB\u30D6\u30E9\u30A6\u30B6\u3067\u30CA\u30D3\u30B2\u30FC\u30C8\u3067\u304D\u308B\u30A6\u30A7\u30D6\u30DA\u30FC\u30B8\u3002"@ja .
<http://www.w3.org/ns/dcat#landingPage> <http://www.w3.org/2004/02/skos/core#scopeNote> "If the distribution(s) are accessible only through a landing page (i.e. direct download URLs are not known), then the landing page link should be duplicated as accessURL on a distribution."@en .
<http://www.w3.org/ns/dcat#landingPage> <http://www.w3.org/2004/02/skos/core#scopeNote> "Pokud je distribuce dostupn\u00E1 pouze p\u0159es vstupn\u00ED str\u00E1nku, t.j. p\u0159\u00EDm\u00FD URL odkaz ke sta\u017Een\u00ED nen\u00ED zn\u00E1m, URL p\u0159\u00EDstupov\u00E9 str\u00E1nky by m\u011Blo b\u00FDt duplikov\u00E1no ve vlastnosti distribuce accessURL."@cs .
<http://www.w3.org/ns/dcat#landingPage> <http://www.w3.org/2004/02/skos/core#scopeNote> "Se la distribuzione \u00E8 accessibile solo attraverso una pagina di destinazione (cio\u00E8, un URL di download diretto non \u00E8 noto), il link alla pagina di destinazione deve essere duplicato come accessURL sulla distribuzione."@it .
<http://www.w3.org/ns/dcat#landingPage> <http://www.w3.org/2004/02/skos/core#scopeNote> "Si la distribuci\u00F3n es accesible solamente trav\u00E9s de una p\u00E1gina de aterrizaje (i.e., no se conoce una URL de descarga directa), entonces el enlance a la p\u00E1gina de aterrizaje debe ser duplicado como accessURL sobre la distribuci\u00F3n."@es .
<http://www.w3.org/ns/dcat#landingPage> <http://www.w3.org/2004/02/skos/core#scopeNote> "Si la distribution est seulement accessible \u00E0 travers une page d'atterrissage (exple. pas de connaissance d'URLS de t\u00E9l\u00E9chargement direct ), alors le lien de la page d'atterrissage doit \u00EAtre dupliqu\u00E9 comme accessURL sur la distribution."@fr .
<http://www.w3.org/ns/dcat#landingPage> <http://www.w3.org/2004/02/skos/core#scopeNote> "\u0391\u03BD \u03B7/\u03BF\u03B9 \u03B4\u03B9\u03B1\u03BD\u03BF\u03BC\u03AE/\u03AD\u03C2 \u03B5\u03AF\u03BD\u03B1\u03B9 \u03C0\u03C1\u03BF\u03C3\u03B2\u03AC\u03C3\u03B9\u03BC\u03B7/\u03B5\u03C2 \u03BC\u03CC\u03BD\u03BF \u03BC\u03AD\u03C3\u03C9 \u03BC\u03AF\u03B1\u03C2 \u03B9\u03C3\u03C4\u03BF\u03C3\u03B5\u03BB\u03AF\u03B4\u03B1\u03C2 \u03B1\u03C1\u03C7\u03B9\u03BA\u03AE\u03C2 \u03C0\u03C1\u03CC\u03C3\u03B2\u03B1\u03C3\u03B7\u03C2 (\u03B4\u03B7\u03BB\u03B1\u03B4\u03AE \u03B1\u03BD \u03B4\u03B5\u03BD \u03C5\u03C0\u03AC\u03C1\u03C7\u03BF\u03C5\u03BD \u03B3\u03BD\u03C9\u03C3\u03C4\u03AD\u03C2 \u03B4\u03B9\u03B5\u03C5\u03B8\u03CD\u03BD\u03C3\u03B5\u03B9\u03C2 \u03AC\u03BC\u03B5\u03C3\u03B7\u03C2 \u03BC\u03B5\u03C4\u03B1\u03C6\u03CC\u03C1\u03C4\u03C9\u03C3\u03B7\u03C2), \u03C4\u03CC\u03C4\u03B5 \u03BF \u03C3\u03CD\u03BD\u03B4\u03B5\u03C3\u03BC\u03BF\u03C2 \u03C4\u03B7\u03C2 \u03B9\u03C3\u03C4\u03BF\u03C3\u03B5\u03BB\u03AF\u03B4\u03B1\u03C2 \u03B1\u03C1\u03C7\u03B9\u03BA\u03AE\u03C2 \u03C0\u03C1\u03CC\u03C3\u03B2\u03B1\u03C3\u03B7\u03C2 \u03C0\u03C1\u03AD\u03C0\u03B5\u03B9 \u03BD\u03B1 \u03B1\u03BD\u03B1\u03C0\u03B1\u03C1\u03B1\u03C7\u03B8\u03B5\u03AF \u03C9\u03C2 accessURL \u03C3\u03B5 \u03BC\u03AF\u03B1 \u03B4\u03B9\u03B1\u03BD\u03BF\u03BC\u03AE."@el .
<http://www.w3.org/ns/dcat#landingPage> <http://www.w3.org/2004/02/skos/core#scopeNote> "\u30E9\u30F3\u30C7\u30A3\u30F3\u30B0\u30FB\u30DA\u30FC\u30B8\u3092\u901A\u3058\u3066\u3057\u304B\u914D\u4FE1\u306B\u30A2\u30AF\u30BB\u30B9\u3067\u304D\u306A\u3044\u5834\u5408\uFF08\u3064\u307E\u308A\u3001\u76F4\u63A5\u7684\u306A\u30C0\u30A6\u30F3\u30ED\u30FC\u30C9URL\u304C\u4E0D\u660E\uFF09\u306B\u306F\u3001\u914D\u4FE1\u306B\u304A\u3051\u308BaccessURL\u3068\u3057\u3066\u30E9\u30F3\u30C7\u30A3\u30F3\u30B0\u30FB\u30DA\u30FC\u30B8\u306E\u30EA\u30F3\u30AF\u3092\u30B3\u30D4\u30FC\u3059\u3079\u304D\u3067\u3059\uFF08SHOULD\uFF09\u3002"@ja .
<http://www.w3.org/ns/dcat#mediaType> <http://www.w3.org/1999/02/22-rdf-syntax-ns#type> <http://www.w3.org/1999/02/22-rdf-syntax-ns#Property> .
<http://www.w3.org/ns/dcat#mediaType> <http://www.w3.org/1999/02/22-rdf-syntax-ns#type> <http://www.w3.org/2002/07/owl#ObjectProperty> .
<http://www.w3.org/ns/dcat#mediaType> <http://www.w3.org/2000/01/rdf-schema#comment> "Cette propri\u00E9t\u00E9 doit \u00EAtre utilis\u00E9e quand c'est d\u00E9finit le type de m\u00E9dia de la distribution en IANA, sinon dct:format DOIT \u00EAtre utilis\u00E9 avec diff\u00E9rentes valeurs."@fr .
<http://www.w3.org/ns/dcat#mediaType> <http://www.w3.org/2000/01/rdf-schema#comment> "Esta propiedad debe ser usada cuando est\u00E1 definido el tipo de media de la distribuci\u00F3n en IANA, de otra manera dct:format puede ser utilizado con diferentes valores"@es .
<http://www.w3.org/ns/dcat#mediaType> <http://www.w3.org/2000/01/rdf-schema#comment> "Il tipo di media della distribuzione come definito da IANA"@it .
<http://www.w3.org/ns/dcat#mediaType> <http://www.w3.org/2000/01/rdf-schema#comment> "The media type of the distribution as defined by IANA"@en .
<http://www.w3.org/ns/dcat#mediaType> <http://www.w3.org/2000/01/rdf-schema#comment> "Typ m\u00E9dia distribuce definovan\u00FD v IANA."@cs .
<http://www.w3.org/ns/dcat#mediaType> <http://www.w3.org/2000/01/rdf-schema#comment> "\u0397 \u03B9\u03B4\u03B9\u03CC\u03C4\u03B7\u03C4\u03B1 \u03B1\u03C5\u03C4\u03AE \u0398\u0391 \u03A0\u03A1\u0395\u03A0\u0395\u0399 \u03BD\u03B1 \u03C7\u03C1\u03B7\u03C3\u03B9\u03BC\u03BF\u03C0\u03BF\u03B9\u03B5\u03AF\u03C4\u03B1\u03B9 \u03CC\u03C4\u03B1\u03BD \u03BF \u03C4\u03CD\u03C0\u03BF\u03C2 \u03BC\u03AD\u03C3\u03BF\u03C5 \u03BC\u03AF\u03B1\u03C2 \u03B4\u03B9\u03B1\u03BD\u03BF\u03BC\u03AE\u03C2 \u03B5\u03AF\u03BD\u03B1\u03B9 \u03BF\u03C1\u03B9\u03C3\u03BC\u03AD\u03BD\u03BF\u03C2 \u03C3\u03C4\u03BF IANA, \u03B1\u03BB\u03BB\u03B9\u03CE\u03C2 \u03B7 \u03B9\u03B4\u03B9\u03CC\u03C4\u03B7\u03C4\u03B1 dct:format \u0394\u03A5\u039D\u0391\u03A4\u0391\u0399 \u03BD\u03B1 \u03C7\u03C1\u03B7\u03C3\u03B9\u03BC\u03BF\u03C0\u03BF\u03B9\u03B7\u03B8\u03B5\u03AF \u03BC\u03B5 \u03B4\u03B9\u03B1\u03C6\u03BF\u03C1\u03B5\u03C4\u03B9\u03BA\u03AD\u03C2 \u03C4\u03B9\u03BC\u03AD\u03C2."@el .
<http://www.w3.org/ns/dcat#mediaType> <http://www.w3.org/2000/01/rdf-schema#comment> "\u064A\u062C\u0628 \u0627\u0633\u062A\u062E\u062F\u0627\u0645 \u0647\u0630\u0647 \u0627\u0644\u062E\u0627\u0635\u064A\u0629 \u0625\u0630\u0627 \u0643\u0627\u0646 \u0646\u0648\u0639 \u0627\u0644\u0645\u0644\u0641 \u0645\u0639\u0631\u0641 \u0636\u0645\u0646 IANA"@ar .
<http://www.w3.org/ns/dcat#mediaType> <http://www.w3.org/2000/01/rdf-schema#comment> "\u3053\u306E\u30D7\u30ED\u30D1\u30C6\u30A3\u30FC\u306F\u3001\u914D\u4FE1\u306E\u30E1\u30C7\u30A3\u30A2\u30FB\u30BF\u30A4\u30D7\u304CIANA\u3067\u5B9A\u7FA9\u3055\u308C\u3066\u3044\u308B\u3068\u304D\u306B\u4F7F\u7528\u3059\u3079\u304D\u3067\uFF08SHOULD\uFF09\u3001\u305D\u3046\u3067\u306A\u3044\u5834\u5408\u306B\u306F\u3001dct:format\u3092\u69D8\u3005\u306A\u5024\u3068\u5171\u306B\u4F7F\u7528\u3067\u304D\u307E\u3059\uFF08MAY\uFF09\u3002"@ja .
<http://www.w3.org/ns/dcat#mediaType> <http://www.w3.org/2000/01/rdf-schema#domain> <http://www.w3.org/ns/dcat#Distribution> .
<http://www.w3.org/ns/dcat#mediaType> <http://www.w3.org/2000/01/rdf-schema#isDefinedBy> <http://www.w3.org/TR/vocab-dcat/> .
<http://www.w3.org/ns/dcat#mediaType> <http://www.w3.org/2000/01/rdf-schema#label> "media type"@en .
<http://www.w3.org/ns/dcat#mediaType> <http://www.w3.org/2000/01/rdf-schema#label> "tipo de media"@es .
<http://www.w3.org/ns/dcat#mediaType> <http://www.w3.org/2000/01/rdf-schema#label> "tipo di media"@it .
<http://www.w3.org/ns/dcat#mediaType> <http://www.w3.org/2000/01/rdf-schema#label> "typ m\u00E9dia"@cs .
<http://www.w3.org/ns/dcat#mediaType> <http://www.w3.org/2000/01/rdf-schema#label> "type de m\u00E9dia"@fr .
<http://www.w3.org/ns/dcat#mediaType> <http://www.w3.org/2000/01/rdf-schema#label> "\u03C4\u03CD\u03C0\u03BF\u03C2 \u03BC\u03AD\u03C3\u03BF\u03C5"@el .
<http://www.w3.org/ns/dcat#mediaType> <http://www.w3.org/2000/01/rdf-schema#label> "\u0646\u0648\u0639 \u0627\u0644\u0645\u064A\u062F\u064A\u0627"@ar .
<http://www.w3.org/ns/dcat#mediaType> <http://www.w3.org/2000/01/rdf-schema#label> "\u30E1\u30C7\u30A3\u30A2\u30FB\u30BF\u30A4\u30D7"@ja .
<http://www.w3.org/ns/dcat#mediaType> <http://www.w3.org/2000/01/rdf-schema#range> <http://purl.org/dc/terms/MediaType> .
<http://www.w3.org/ns/dcat#mediaType> <http://www.w3.org/2000/01/rdf-schema#subPropertyOf> <http://purl.org/dc/terms/format> .
<http://www.w3.org/ns/dcat#mediaType> <http://www.w3.org/2004/02/skos/core#changeNote> "Obor hodnot dcat:mediaType byl z\u00FA\u017Een v t\u00E9to revizi DCAT."@cs .
<http://www.w3.org/ns/dcat#mediaType> <http://www.w3.org/2004/02/skos/core#changeNote> "The range of dcat:mediaType has been tightened as part of the revision of DCAT."@en .
<http://www.w3.org/ns/dcat#mediaType> <http://www.w3.org/2004/02/skos/core#changeNote> "Il range di dcat:mediaType \u00E8 stato ristretto  come parte della revisione di DCAT."@it .
<http://www.w3.org/ns/dcat#mediaType> <http://www.w3.org/2004/02/skos/core#definition> "Cette propri\u00E9t\u00E9 doit \u00EAtre utilis\u00E9e quand c'est d\u00E9finit le type de m\u00E9dia de la distribution en IANA, sinon dct:format DOIT \u00EAtre utilis\u00E9 avec diff\u00E9rentes valeurs."@fr .
<http://www.w3.org/ns/dcat#mediaType> <http://www.w3.org/2004/02/skos/core#definition> "Esta propiedad debe ser usada cuando est\u00E1 definido el tipo de media de la distribuci\u00F3n en IANA, de otra manera dct:format puede ser utilizado con diferentes valores."@es .
<http://www.w3.org/ns/dcat#mediaType> <http://www.w3.org/2004/02/skos/core#definition> "Il tipo di media della distribuzione come definito da IANA."@it .
<http://www.w3.org/ns/dcat#mediaType> <http://www.w3.org/2004/02/skos/core#definition> "The media type of the distribution as defined by IANA."@en .
<http://www.w3.org/ns/dcat#mediaType> <http://www.w3.org/2004/02/skos/core#definition> "Typ m\u00E9dia distribuce definovan\u00FD v IANA."@cs .
<http://www.w3.org/ns/dcat#mediaType> <http://www.w3.org/2004/02/skos/core#definition> "\u0397 \u03B9\u03B4\u03B9\u03CC\u03C4\u03B7\u03C4\u03B1 \u03B1\u03C5\u03C4\u03AE \u0398\u0391 \u03A0\u03A1\u0395\u03A0\u0395\u0399 \u03BD\u03B1 \u03C7\u03C1\u03B7\u03C3\u03B9\u03BC\u03BF\u03C0\u03BF\u03B9\u03B5\u03AF\u03C4\u03B1\u03B9 \u03CC\u03C4\u03B1\u03BD \u03BF \u03C4\u03CD\u03C0\u03BF\u03C2 \u03BC\u03AD\u03C3\u03BF\u03C5 \u03BC\u03AF\u03B1\u03C2 \u03B4\u03B9\u03B1\u03BD\u03BF\u03BC\u03AE\u03C2 \u03B5\u03AF\u03BD\u03B1\u03B9 \u03BF\u03C1\u03B9\u03C3\u03BC\u03AD\u03BD\u03BF\u03C2 \u03C3\u03C4\u03BF IANA, \u03B1\u03BB\u03BB\u03B9\u03CE\u03C2 \u03B7 \u03B9\u03B4\u03B9\u03CC\u03C4\u03B7\u03C4\u03B1 dct:format \u0394\u03A5\u039D\u0391\u03A4\u0391\u0399 \u03BD\u03B1 \u03C7\u03C1\u03B7\u03C3\u03B9\u03BC\u03BF\u03C0\u03BF\u03B9\u03B7\u03B8\u03B5\u03AF \u03BC\u03B5 \u03B4\u03B9\u03B1\u03C6\u03BF\u03C1\u03B5\u03C4\u03B9\u03BA\u03AD\u03C2 \u03C4\u03B9\u03BC\u03AD\u03C2."@el .
<http://www.w3.org/ns/dcat#mediaType> <http://www.w3.org/2004/02/skos/core#definition> "\u064A\u062C\u0628 \u0627\u0633\u062A\u062E\u062F\u0627\u0645 \u0647\u0630\u0647 \u0627\u0644\u062E\u0627\u0635\u064A\u0629 \u0625\u0630\u0627 \u0643\u0627\u0646 \u0646\u0648\u0639 \u0627\u0644\u0645\u0644\u0641 \u0645\u0639\u0631\u0641 \u0636\u0645\u0646 IANA"@ar .
<http://www.w3.org/ns/dcat#mediaType> <http://www.w3.org/2004/02/skos/core#definition> "\u3053\u306E\u30D7\u30ED\u30D1\u30C6\u30A3\u30FC\u306F\u3001\u914D\u4FE1\u306E\u30E1\u30C7\u30A3\u30A2\u30FB\u30BF\u30A4\u30D7\u304CIANA\u3067\u5B9A\u7FA9\u3055\u308C\u3066\u3044\u308B\u3068\u304D\u306B\u4F7F\u7528\u3059\u3079\u304D\u3067\uFF08SHOULD\uFF09\u3001\u305D\u3046\u3067\u306A\u3044\u5834\u5408\u306B\u306F\u3001dct:format\u3092\u69D8\u3005\u306A\u5024\u3068\u5171\u306B\u4F7F\u7528\u3067\u304D\u307E\u3059\uFF08MAY\uFF09\u3002"@ja .
<http://www.w3.org/ns/dcat#mediaType> <http://www.w3.org/2004/02/skos/core#editorialNote> "Status: English Definition text modified by DCAT revision team, Italian and Czech translation provided, other translations pending. Note some inconsistency on def vs. usage."@en .
<http://www.w3.org/ns/dcat#mediaType> <http://www.w3.org/2004/02/skos/core#scopeNote> "Esta propiedad DEBER\u00CDA usarse cuando el 'media type' de la distribuci\u00F3n est\u00E1 definido en el registro IANA de 'media types' https://www.iana.org/assignments/media-types/, de lo contrario, dct:format PUEDE usarse con distintos valores."@es .
<http://www.w3.org/ns/dcat#mediaType> <http://www.w3.org/2004/02/skos/core#scopeNote> "Questa propriet\u00E0 DEVE essere usata quando il tipo di media della distribuzione \u00E8 definito nel registro dei tipi di media IANA https://www.iana.org/assignments/media-types/, altrimenti dct:format PUO 'essere usato con differenti valori."@it .
<http://www.w3.org/ns/dcat#mediaType> <http://www.w3.org/2004/02/skos/core#scopeNote> "Tato vlastnost BY M\u011ALA b\u00FDt pou\u017Eita, je-li typ m\u00E9dia distribuce definov\u00E1n v registru IANA https://www.iana.org/assignments/media-types/. V ostatn\u00EDch p\u0159\u00EDpadech M\u016E\u017DE b\u00FDt pou\u017Eita vlastnost dct:format s jin\u00FDmi hodnotami."@cs .
<http://www.w3.org/ns/dcat#mediaType> <http://www.w3.org/2004/02/skos/core#scopeNote> "This property SHOULD be used when the media type of the distribution is defined in the IANA media types registry https://www.iana.org/assignments/media-types/, otherwise dct:format MAY be used with different values."@en .
<http://www.w3.org/ns/dcat#packageFormat> <http://www.w3.org/1999/02/22-rdf-syntax-ns#type> <http://www.w3.org/1999/02/22-rdf-syntax-ns#Property> .
<http://www.w3.org/ns/dcat#packageFormat> <http://www.w3.org/1999/02/22-rdf-syntax-ns#type> <http://www.w3.org/2002/07/owl#ObjectProperty> .
<http://www.w3.org/ns/dcat#packageFormat> <http://www.w3.org/2000/01/rdf-schema#comment> "Bal\u00ED\u010Dkov\u00FD form\u00E1t souboru, ve kter\u00E9m je jeden \u010Di v\u00EDce soubor\u016F seskupeno dohromady, nap\u0159. aby bylo mo\u017En\u00E9 st\u00E1hnout sadu souvisej\u00EDc\u00EDch soubor\u016F nar\u00E1z."@cs .
<http://www.w3.org/ns/dcat#packageFormat> <http://www.w3.org/2000/01/rdf-schema#comment> "El formato del archivo en que se agrupan uno o m\u00E1s archivos de datos, e.g. para permitir que un conjunto de archivos relacionados se bajen juntos."@es .
<http://www.w3.org/ns/dcat#packageFormat> <http://www.w3.org/2000/01/rdf-schema#comment> "Il formato di impacchettamento della distribuzione in cui uno o pi\u00F9 file di dati sono raggruppati insieme, ad es. per abilitare un insieme di file correlati da scaricare insieme."@it .
<http://www.w3.org/ns/dcat#packageFormat> <http://www.w3.org/2000/01/rdf-schema#comment> "The package format of the distribution in which one or more data files are grouped together, e.g. to enable a set of related files to be downloaded together."@en .
<http://www.w3.org/ns/dcat#packageFormat> <http://www.w3.org/2000/01/rdf-schema#domain> <http://www.w3.org/ns/dcat#Distribution> .
<http://www.w3.org/ns/dcat#packageFormat> <http://www.w3.org/2000/01/rdf-schema#isDefinedBy> <https://www.w3.org/TR/vocab-dcat-2/> .
<http://www.w3.org/ns/dcat#packageFormat> <http://www.w3.org/2000/01/rdf-schema#label> "formato de empaquetado"@es .
<http://www.w3.org/ns/dcat#packageFormat> <http://www.w3.org/2000/01/rdf-schema#label> "formato di impacchettamento"@it .
<http://www.w3.org/ns/dcat#packageFormat> <http://www.w3.org/2000/01/rdf-schema#label> "form\u00E1t bal\u00ED\u010Dku"@cs .
<http://www.w3.org/ns/dcat#packageFormat> <http://www.w3.org/2000/01/rdf-schema#label> "packaging format"@en .
<http://www.w3.org/ns/dcat#packageFormat> <http://www.w3.org/2000/01/rdf-schema#range> <http://purl.org/dc/terms/MediaType> .
<http://www.w3.org/ns/dcat#packageFormat> <http://www.w3.org/2000/01/rdf-schema#subPropertyOf> <http://purl.org/dc/terms/format> .
<http://www.w3.org/ns/dcat#packageFormat> <http://www.w3.org/2004/02/skos/core#changeNote> "New property added in DCAT 2.0."@en .
<http://www.w3.org/ns/dcat#packageFormat> <http://www.w3.org/2004/02/skos/core#changeNote> "Nov\u00E1 vlastnost p\u0159idan\u00E1 ve verzi DCAT 2.0."@cs .
<http://www.w3.org/ns/dcat#packageFormat> <http://www.w3.org/2004/02/skos/core#changeNote> "Nueva propiedad agregada en DCAT 2.0."@es .
<http://www.w3.org/ns/dcat#packageFormat> <http://www.w3.org/2004/02/skos/core#changeNote> "Nuova propriet\u00E0 aggiunta in DCAT 2.0."@it .
<http://www.w3.org/ns/dcat#packageFormat> <http://www.w3.org/2004/02/skos/core#definition> "Bal\u00ED\u010Dkov\u00FD form\u00E1t souboru, ve kter\u00E9m je jeden \u010Di v\u00EDce soubor\u016F seskupeno dohromady, nap\u0159. aby bylo mo\u017En\u00E9 st\u00E1hnout sadu souvisej\u00EDc\u00EDch soubor\u016F nar\u00E1z."@cs .
<http://www.w3.org/ns/dcat#packageFormat> <http://www.w3.org/2004/02/skos/core#definition> "El formato del archivo en que se agrupan uno o m\u00E1s archivos de datos, e.g. para permitir que un conjunto de archivos relacionados se bajen juntos."@es .
<http://www.w3.org/ns/dcat#packageFormat> <http://www.w3.org/2004/02/skos/core#definition> "Il formato di impacchettamento della distribuzione in cui uno o pi\u00F9 file di dati sono raggruppati insieme, ad es. per abilitare un insieme di file correlati da scaricare insieme."@it .
<http://www.w3.org/ns/dcat#packageFormat> <http://www.w3.org/2004/02/skos/core#definition> "The package format of the distribution in which one or more data files are grouped together, e.g. to enable a set of related files to be downloaded together."@en .
<http://www.w3.org/ns/dcat#packageFormat> <http://www.w3.org/2004/02/skos/core#scopeNote> "Esta propiedad se debe usar cuando los archivos de la distribuci\u00F3n est\u00E1n empaquetados, por ejemplo en un archivo TAR, Frictionless Data Package o Bagit. El formato DEBER\u00CDA expresarse usando un 'media type', tales como los definidos en el registro IANA de 'media types' https://www.iana.org/assignments/media-types/, si est\u00E1 disponibles."@es .
<http://www.w3.org/ns/dcat#packageFormat> <http://www.w3.org/2004/02/skos/core#scopeNote> "Questa propriet\u00E0 deve essere utilizzata quando i file nella distribuzione sono impacchettati, ad esempio in un file TAR, Frictionless Data Package o Bagit. Il formato DOVREBBE essere espresso utilizzando un tipo di supporto come definito dal registro dei tipi di media IANA https://www.iana.org/assignments/media-types/, se disponibili."@it .
<http://www.w3.org/ns/dcat#packageFormat> <http://www.w3.org/2004/02/skos/core#scopeNote> "Tato vlastnost se pou\u017Eije, kdy\u017E jsou soubory v distribuci zabaleny, nap\u0159. v souboru TAR, v bal\u00ED\u010Dku Frictionless Data Package nebo v souboru Bagit. Form\u00E1t BY M\u011AL b\u00FDt vyj\u00E1d\u0159en pomoc\u00ED typu m\u00E9dia definovan\u00E9ho v registru IANA https://www.iana.org/assignments/media-types/, pokud existuje."@cs .
<http://www.w3.org/ns/dcat#packageFormat> <http://www.w3.org/2004/02/skos/core#scopeNote> "This property to be used when the files in the distribution are packaged, e.g. in a TAR file, a Frictionless Data Package or a Bagit file. The format SHOULD be expressed using a media type as defined by IANA media types registry https://www.iana.org/assignments/media-types/, if available."@en .
<http://www.w3.org/ns/dcat#qualifiedRelation> <http://www.w3.org/1999/02/22-rdf-syntax-ns#type> <http://www.w3.org/2002/07/owl#ObjectProperty> .
<http://www.w3.org/ns/dcat#qualifiedRelation> <http://www.w3.org/2000/01/rdf-schema#comment> "Enlace a una descripci\u00F3n de la relaci\u00F3n con otro recurso."@es .
<http://www.w3.org/ns/dcat#qualifiedRelation> <http://www.w3.org/2000/01/rdf-schema#comment> "Link a una descrizione di una relazione con un'altra risorsa."@it .
<http://www.w3.org/ns/dcat#qualifiedRelation> <http://www.w3.org/2000/01/rdf-schema#comment> "Link to a description of a relationship with another resource."@en .
<http://www.w3.org/ns/dcat#qualifiedRelation> <http://www.w3.org/2000/01/rdf-schema#comment> "Odkaz na popis vztahu s jin\u00FDm zdrojem."@cs .
<http://www.w3.org/ns/dcat#qualifiedRelation> <http://www.w3.org/2000/01/rdf-schema#domain> <http://www.w3.org/ns/dcat#Resource> .
<http://www.w3.org/ns/dcat#qualifiedRelation> <http://www.w3.org/2000/01/rdf-schema#label> "kvalifikovan\u00FD vztah"@cs .
<http://www.w3.org/ns/dcat#qualifiedRelation> <http://www.w3.org/2000/01/rdf-schema#label> "qualified relation"@en .
<http://www.w3.org/ns/dcat#qualifiedRelation> <http://www.w3.org/2000/01/rdf-schema#label> "relaci\u00F3n calificada"@es .
<http://www.w3.org/ns/dcat#qualifiedRelation> <http://www.w3.org/2000/01/rdf-schema#label> "relazione qualificata"@it .
<http://www.w3.org/ns/dcat#qualifiedRelation> <http://www.w3.org/2000/01/rdf-schema#range> <http://www.w3.org/ns/dcat#Relationship> .
<http://www.w3.org/ns/dcat#qualifiedRelation> <http://www.w3.org/2004/02/skos/core#changeNote> "New property added in DCAT 2.0."@en .
<http://www.w3.org/ns/dcat#qualifiedRelation> <http://www.w3.org/2004/02/skos/core#changeNote> "Nov\u00E1 vlastnost p\u0159idan\u00E1 ve verzi DCAT 2.0."@cs .
<http://www.w3.org/ns/dcat#qualifiedRelation> <http://www.w3.org/2004/02/skos/core#changeNote> "Nuova propriet\u00E0 aggiunta in DCAT 2.0."@it .
<http://www.w3.org/ns/dcat#qualifiedRelation> <http://www.w3.org/2004/02/skos/core#changeNote> "Propiedad nueva a\u00F1adida en DCAT 2.0."@es .
<http://www.w3.org/ns/dcat#qualifiedRelation> <http://www.w3.org/2004/02/skos/core#definition> "Enlace a una descripci\u00F3n de la relaci\u00F3n con otro recurso."@es .
<http://www.w3.org/ns/dcat#qualifiedRelation> <http://www.w3.org/2004/02/skos/core#definition> "Link a una descrizione di una relazione con un'altra risorsa."@it .
<http://www.w3.org/ns/dcat#qualifiedRelation> <http://www.w3.org/2004/02/skos/core#definition> "Link to a description of a relationship with another resource."@en .
<http://www.w3.org/ns/dcat#qualifiedRelation> <http://www.w3.org/2004/02/skos/core#definition> "Odkaz na popis vztahu s jin\u00FDm zdrojem."@cs .
<http://www.w3.org/ns/dcat#qualifiedRelation> <http://www.w3.org/2004/02/skos/core#editorialNote> "Introdotta in DCAT per integrare le altre relazioni qualificate di PROV."@it .
<http://www.w3.org/ns/dcat#qualifiedRelation> <http://www.w3.org/2004/02/skos/core#editorialNote> "Introduced into DCAT to complement the other PROV qualified relations. "@en .
<http://www.w3.org/ns/dcat#qualifiedRelation> <http://www.w3.org/2004/02/skos/core#editorialNote> "P\u0159id\u00E1no do DCAT k dopln\u011Bn\u00ED jin\u00FDch kvalifikovan\u00FDch vztah\u016F ze slovn\u00EDku PROV."@cs .
<http://www.w3.org/ns/dcat#qualifiedRelation> <http://www.w3.org/2004/02/skos/core#editorialNote> "Se incluy\u00F3 en DCAT para complementar las relaciones calificadas disponibles en PROV."@es .
<http://www.w3.org/ns/dcat#qualifiedRelation> <http://www.w3.org/2004/02/skos/core#scopeNote> "Pou\u017Eito pro odkazov\u00E1n\u00ED na jin\u00FD zdroj, kde druh vztahu je zn\u00E1m, ale neodpov\u00EDd\u00E1 standardn\u00EDm vlastnostem ze slovn\u00EDku Dublin Core (dct:hasPart, dct:isPartOf, dct:conformsTo, dct:isFormatOf, dct:hasFormat, dct:isVersionOf, dct:hasVersion, dct:replaces, dct:isReplacedBy, dct:references, dct:isReferencedBy, dct:requires, dct:isRequiredBy) \u010Di slovn\u00EDku PROV-O (prov:wasDerivedFrom, prov:wasInfluencedBy, prov:wasQuotedFrom, prov:wasRevisionOf, prov:hadPrimarySource, prov:alternateOf, prov:specializationOf)."@cs .
<http://www.w3.org/ns/dcat#qualifiedRelation> <http://www.w3.org/2004/02/skos/core#scopeNote> "Se usa para asociar con otro recurso para el cu\u00E1l la naturaleza de la relaci\u00F3n es conocida pero no es ninguna de las propiedades que provee el est\u00E1ndar Dublin Core (dct:hasPart, dct:isPartOf, dct:conformsTo, dct:isFormatOf, dct:hasFormat, dct:isVersionOf, dct:hasVersion, dct:replaces, dct:isReplacedBy, dct:references, dct:isReferencedBy, dct:requires, dct:isRequiredBy) or PROV-O properties (prov:wasDerivedFrom, prov:wasInfluencedBy, prov:wasQuotedFrom, prov:wasRevisionOf, prov:hadPrimarySource, prov:alternateOf, prov:specializationOf)."@es .
<http://www.w3.org/ns/dcat#qualifiedRelation> <http://www.w3.org/2004/02/skos/core#scopeNote> "Used to link to another resource where the nature of the relationship is known but does not match one of the standard Dublin Core properties (dct:hasPart, dct:isPartOf, dct:conformsTo, dct:isFormatOf, dct:hasFormat, dct:isVersionOf, dct:hasVersion, dct:replaces, dct:isReplacedBy, dct:references, dct:isReferencedBy, dct:requires, dct:isRequiredBy) or PROV-O properties (prov:wasDerivedFrom, prov:wasInfluencedBy, prov:wasQuotedFrom, prov:wasRevisionOf, prov:hadPrimarySource, prov:alternateOf, prov:specializationOf)."@en .
<http://www.w3.org/ns/dcat#qualifiedRelation> <http://www.w3.org/2004/02/skos/core#scopeNote> "Viene utilizzato per associarsi a un'altra risorsa nei casi per i quali la natura della relazione \u00E8 nota ma non \u00E8 alcuna delle propriet\u00E0 fornite dallo standard Dublin Core (dct:hasPart, dct:isPartOf, dct:conformsTo, dct:isFormatOf, dct:hasFormat , dct:isVersionOf, dct:hasVersion, dct:replaces, dct:isReplacedBy, dct:references, dct:isReferencedBy, dct:require, dct:isRequiredBy) o dalle propriet\u00E0 fornite da PROV-O (prov:wasDerivedFrom, prov:wasInfluencedBy, prov:wasQuotedFrom , prov:wasRevisionOf, prov:hadPrimarySource, prov:alternateOf, prov:specializationOf)."@it .
<http://www.w3.org/ns/dcat#record> <http://www.w3.org/1999/02/22-rdf-syntax-ns#type> <http://www.w3.org/1999/02/22-rdf-syntax-ns#Property> .
<http://www.w3.org/ns/dcat#record> <http://www.w3.org/1999/02/22-rdf-syntax-ns#type> <http://www.w3.org/2002/07/owl#ObjectProperty> .
<http://www.w3.org/ns/dcat#record> <http://www.w3.org/2000/01/rdf-schema#comment> "A record describing the registration of a single dataset or data service that is part of the catalog."@en .
<http://www.w3.org/ns/dcat#record> <http://www.w3.org/2000/01/rdf-schema#comment> "Describe la registraci\u00F3n de un conjunto de datos o un servicio de datos en el cat\u00E1logo."@es .
<http://www.w3.org/ns/dcat#record> <http://www.w3.org/2000/01/rdf-schema#comment> "Propojuje katalog a jeho z\u00E1znamy."@cs .
<http://www.w3.org/ns/dcat#record> <http://www.w3.org/2000/01/rdf-schema#comment> "Relie un catalogue \u00E0 ses registres."@fr .
<http://www.w3.org/ns/dcat#record> <http://www.w3.org/2000/01/rdf-schema#comment> "Un record che descrive la registrazione di un singolo set di dati o di un servizio dati che fa parte del catalogo."@it .
<http://www.w3.org/ns/dcat#record> <http://www.w3.org/2000/01/rdf-schema#comment> "Z\u00E1znam popisuj\u00EDc\u00ED registraci jedn\u00E9 datov\u00E9 sady \u010Di datov\u00E9 slu\u017Eby jako\u017Eto sou\u010D\u00E1sti katalogu."@cs .
<http://www.w3.org/ns/dcat#record> <http://www.w3.org/2000/01/rdf-schema#comment> "\u03A3\u03C5\u03BD\u03B4\u03AD\u03B5\u03B9 \u03AD\u03BD\u03B1\u03BD \u03BA\u03B1\u03C4\u03AC\u03BB\u03BF\u03B3\u03BF \u03BC\u03B5 \u03C4\u03B9\u03C2 \u03BA\u03B1\u03C4\u03B1\u03B3\u03C1\u03B1\u03C6\u03AD\u03C2 \u03C4\u03BF\u03C5."@el .
<http://www.w3.org/ns/dcat#record> <http://www.w3.org/2000/01/rdf-schema#comment> "\u062A\u0631\u0628\u0637 \u0627\u0644\u0641\u0647\u0631\u0633 \u0628\u0633\u062C\u0644 \u0636\u0645\u0646\u0647"@ar .
<http://www.w3.org/ns/dcat#record> <http://www.w3.org/2000/01/rdf-schema#comment> "\u30AB\u30BF\u30ED\u30B0\u306E\u4E00\u90E8\u3067\u3042\u308B\u30AB\u30BF\u30ED\u30B0\u30FB\u30EC\u30B3\u30FC\u30C9\u3002"@ja .
<http://www.w3.org/ns/dcat#record> <http://www.w3.org/2000/01/rdf-schema#domain> <http://www.w3.org/ns/dcat#Catalog> .
<http://www.w3.org/ns/dcat#record> <http://www.w3.org/2000/01/rdf-schema#isDefinedBy> <http://www.w3.org/TR/vocab-dcat/> .
<http://www.w3.org/ns/dcat#record> <http://www.w3.org/2000/01/rdf-schema#label> "record"@en .
<http://www.w3.org/ns/dcat#record> <http://www.w3.org/2000/01/rdf-schema#label> "record"@it .
<http://www.w3.org/ns/dcat#record> <http://www.w3.org/2000/01/rdf-schema#label> "registre"@fr .
<http://www.w3.org/ns/dcat#record> <http://www.w3.org/2000/01/rdf-schema#label> "registro"@es .
<http://www.w3.org/ns/dcat#record> <http://www.w3.org/2000/01/rdf-schema#label> "z\u00E1znam"@cs .
<http://www.w3.org/ns/dcat#record> <http://www.w3.org/2000/01/rdf-schema#label> "\u03BA\u03B1\u03C4\u03B1\u03B3\u03C1\u03B1\u03C6\u03AE"@el .
<http://www.w3.org/ns/dcat#record> <http://www.w3.org/2000/01/rdf-schema#label> "\u0633\u062C\u0644"@ar .
<http://www.w3.org/ns/dcat#record> <http://www.w3.org/2000/01/rdf-schema#label> "\u30AB\u30BF\u30ED\u30B0\u30FB\u30EC\u30B3\u30FC\u30C9"@ja .
<http://www.w3.org/ns/dcat#record> <http://www.w3.org/2000/01/rdf-schema#range> <http://www.w3.org/ns/dcat#CatalogRecord> .
<http://www.w3.org/ns/dcat#record> <http://www.w3.org/2004/02/skos/core#definition> "A record describing the registration of a single dataset or data service that is part of the catalog."@en .
<http://www.w3.org/ns/dcat#record> <http://www.w3.org/2004/02/skos/core#definition> "Describe la registraci\u00F3n de un conjunto de datos o un servicio de datos en el cat\u00E1logo."@es .
<http://www.w3.org/ns/dcat#record> <http://www.w3.org/2004/02/skos/core#definition> "Propojuje katalog a jeho z\u00E1znamy."@cs .
<http://www.w3.org/ns/dcat#record> <http://www.w3.org/2004/02/skos/core#definition> "Relie un catalogue \u00E0 ses registres."@fr .
<http://www.w3.org/ns/dcat#record> <http://www.w3.org/2004/02/skos/core#definition> "Un record che descrive la registrazione di un singolo set di dati o di un servizio dati che fa parte del catalogo."@it .
<http://www.w3.org/ns/dcat#record> <http://www.w3.org/2004/02/skos/core#definition> "Z\u00E1znam popisuj\u00EDc\u00ED registraci jedn\u00E9 datov\u00E9 sady \u010Di datov\u00E9 slu\u017Eby jako\u017Eto sou\u010D\u00E1sti katalogu."@cs .
<http://www.w3.org/ns/dcat#record> <http://www.w3.org/2004/02/skos/core#definition> "\u03A3\u03C5\u03BD\u03B4\u03AD\u03B5\u03B9 \u03AD\u03BD\u03B1\u03BD \u03BA\u03B1\u03C4\u03AC\u03BB\u03BF\u03B3\u03BF \u03BC\u03B5 \u03C4\u03B9\u03C2 \u03BA\u03B1\u03C4\u03B1\u03B3\u03C1\u03B1\u03C6\u03AD\u03C2 \u03C4\u03BF\u03C5."@el .
<http://www.w3.org/ns/dcat#record> <http://www.w3.org/2004/02/skos/core#definition> "\u062A\u0631\u0628\u0637 \u0627\u0644\u0641\u0647\u0631\u0633 \u0628\u0633\u062C\u0644 \u0636\u0645\u0646\u0647"@ar .
<http://www.w3.org/ns/dcat#record> <http://www.w3.org/2004/02/skos/core#definition> "\u30AB\u30BF\u30ED\u30B0\u306E\u4E00\u90E8\u3067\u3042\u308B\u30AB\u30BF\u30ED\u30B0\u30FB\u30EC\u30B3\u30FC\u30C9\u3002"@ja .
<http://www.w3.org/ns/dcat#record> <http://www.w3.org/2004/02/skos/core#editorialNote> "Status: English, Italian, Spanish and Czech Definitions modified by DCAT revision team, other translations pending."@en .
<http://www.w3.org/ns/dcat#servesDataset> <http://www.w3.org/1999/02/22-rdf-syntax-ns#type> <http://www.w3.org/2002/07/owl#ObjectProperty> .
<http://www.w3.org/ns/dcat#servesDataset> <http://www.w3.org/2000/01/rdf-schema#comment> "A collection of data that this DataService can distribute."@en .
<http://www.w3.org/ns/dcat#servesDataset> <http://www.w3.org/2000/01/rdf-schema#comment> "Kolekce dat, kterou je tato Datov\u00E1 slu\u017Eba schopna poskytnout."@cs .
<http://www.w3.org/ns/dcat#servesDataset> <http://www.w3.org/2000/01/rdf-schema#comment> "Una colecci\u00F3n de datos que este Servicio de Datos puede distribuir."@es .
<http://www.w3.org/ns/dcat#servesDataset> <http://www.w3.org/2000/01/rdf-schema#comment> "Una raccolta di dati che questo DataService pu\u00F2 distribuire."@it .
<http://www.w3.org/ns/dcat#servesDataset> <http://www.w3.org/2000/01/rdf-schema#domain> <http://www.w3.org/ns/dcat#DataService> .
<http://www.w3.org/ns/dcat#servesDataset> <http://www.w3.org/2000/01/rdf-schema#label> "poskytuje datovou sadu"@cs .
<http://www.w3.org/ns/dcat#servesDataset> <http://www.w3.org/2000/01/rdf-schema#label> "provee conjunto de datos"@es .
<http://www.w3.org/ns/dcat#servesDataset> <http://www.w3.org/2000/01/rdf-schema#label> "serve set di dati"@it .
<http://www.w3.org/ns/dcat#servesDataset> <http://www.w3.org/2000/01/rdf-schema#label> "serves dataset"@en .
<http://www.w3.org/ns/dcat#servesDataset> <http://www.w3.org/2000/01/rdf-schema#range> <http://www.w3.org/ns/dcat#Dataset> .
<http://www.w3.org/ns/dcat#servesDataset> <http://www.w3.org/2004/02/skos/core#changeNote> "New property in DCAT 2.0."@en .
<http://www.w3.org/ns/dcat#servesDataset> <http://www.w3.org/2004/02/skos/core#changeNote> "Nov\u00E1 vlastnost p\u0159idan\u00E1 ve verzi DCAT 2.0."@cs .
<http://www.w3.org/ns/dcat#servesDataset> <http://www.w3.org/2004/02/skos/core#changeNote> "Nueva propiedad agregada en DCAT 2.0."@es .
<http://www.w3.org/ns/dcat#servesDataset> <http://www.w3.org/2004/02/skos/core#changeNote> "Nuova propriet\u00E0 in DCAT 2.0."@it .
<http://www.w3.org/ns/dcat#servesDataset> <http://www.w3.org/2004/02/skos/core#definition> "A collection of data that this DataService can distribute."@en .
<http://www.w3.org/ns/dcat#servesDataset> <http://www.w3.org/2004/02/skos/core#definition> "Kolekce dat, kterou je tato Datov\u00E1 slu\u017Eba schopna poskytnout."@cs .
<http://www.w3.org/ns/dcat#servesDataset> <http://www.w3.org/2004/02/skos/core#definition> "Una colecci\u00F3n de datos que este Servicio de Datos puede distribuir."@es .
<http://www.w3.org/ns/dcat#servesDataset> <http://www.w3.org/2004/02/skos/core#definition> "Una raccolta di dati che questo DataService pu\u00F2 distribuire."@it .
<http://www.w3.org/ns/dcat#service> <http://www.w3.org/1999/02/22-rdf-syntax-ns#type> <http://www.w3.org/2002/07/owl#ObjectProperty> .
<http://www.w3.org/ns/dcat#service> <http://www.w3.org/2000/01/rdf-schema#comment> "A site or endpoint that is listed in the catalog."@en .
<http://www.w3.org/ns/dcat#service> <http://www.w3.org/2000/01/rdf-schema#comment> "Um\u00EDst\u011Bn\u00ED \u010Di p\u0159\u00EDstupov\u00FD bod registrovan\u00FD v katalogu."@cs .
<http://www.w3.org/ns/dcat#service> <http://www.w3.org/2000/01/rdf-schema#comment> "Un sitio o 'endpoint' que est\u00E1 listado en el cat\u00E1logo."@es .
<http://www.w3.org/ns/dcat#service> <http://www.w3.org/2000/01/rdf-schema#comment> "Un sito o endpoint elencato nel catalogo."@it .
<http://www.w3.org/ns/dcat#service> <http://www.w3.org/2000/01/rdf-schema#domain> <http://www.w3.org/ns/dcat#Catalog> .
<http://www.w3.org/ns/dcat#service> <http://www.w3.org/2000/01/rdf-schema#label> "service"@en .
<http://www.w3.org/ns/dcat#service> <http://www.w3.org/2000/01/rdf-schema#label> "servicio"@es .
<http://www.w3.org/ns/dcat#service> <http://www.w3.org/2000/01/rdf-schema#label> "servizio"@it .
<http://www.w3.org/ns/dcat#service> <http://www.w3.org/2000/01/rdf-schema#label> "slu\u017Eba"@cs .
<http://www.w3.org/ns/dcat#service> <http://www.w3.org/2000/01/rdf-schema#range> <http://www.w3.org/ns/dcat#DataService> .
<http://www.w3.org/ns/dcat#service> <http://www.w3.org/2000/01/rdf-schema#subPropertyOf> <http://purl.org/dc/terms/hasPart> .
<http://www.w3.org/ns/dcat#service> <http://www.w3.org/2000/01/rdf-schema#subPropertyOf> <http://www.w3.org/2000/01/rdf-schema#member> .
<http://www.w3.org/ns/dcat#service> <http://www.w3.org/2004/02/skos/core#changeNote> "New property added in DCAT 2.0."@en .
<http://www.w3.org/ns/dcat#service> <http://www.w3.org/2004/02/skos/core#changeNote> "Nov\u00E1 vlastnost p\u0159idan\u00E1 ve verzi DCAT 2.0."@cs .
<http://www.w3.org/ns/dcat#service> <http://www.w3.org/2004/02/skos/core#changeNote> "Nueva propiedad a\u00F1adida en DCAT 2.0."@es .
<http://www.w3.org/ns/dcat#service> <http://www.w3.org/2004/02/skos/core#changeNote> "Nuova propriet\u00E0 aggiunta in DCAT 2.0."@it .
<http://www.w3.org/ns/dcat#service> <http://www.w3.org/2004/02/skos/core#definition> "A site or endpoint that is listed in the catalog."@en .
<http://www.w3.org/ns/dcat#service> <http://www.w3.org/2004/02/skos/core#definition> "Um\u00EDst\u011Bn\u00ED \u010Di p\u0159\u00EDstupov\u00FD bod registrovan\u00FD v katalogu."@cs .
<http://www.w3.org/ns/dcat#service> <http://www.w3.org/2004/02/skos/core#definition> "Un sitio o 'endpoint' que est\u00E1 listado en el cat\u00E1logo."@es .
<http://www.w3.org/ns/dcat#service> <http://www.w3.org/2004/02/skos/core#definition> "Un sito o endpoint elencato nel catalogo."@it .
<http://www.w3.org/ns/dcat#spatialResolutionInMeters> <http://www.w3.org/1999/02/22-rdf-syntax-ns#type> <http://www.w3.org/2002/07/owl#DatatypeProperty> .
<http://www.w3.org/ns/dcat#spatialResolutionInMeters> <http://www.w3.org/2000/01/rdf-schema#comment> "minimum spatial separation resolvable in a dataset, measured in meters."@en-US .
<http://www.w3.org/ns/dcat#spatialResolutionInMeters> <http://www.w3.org/2000/01/rdf-schema#comment> "minimum spatial separation resolvable in a dataset, measured in metres."@en-GB .
<http://www.w3.org/ns/dcat#spatialResolutionInMeters> <http://www.w3.org/2000/01/rdf-schema#comment> "minim\u00E1ln\u00ED prostorov\u00FD rozestup rozeznateln\u00FD v datov\u00E9 sad\u011B, m\u011B\u0159eno v metrech."@cs .
<http://www.w3.org/ns/dcat#spatialResolutionInMeters> <http://www.w3.org/2000/01/rdf-schema#comment> "m\u00EDnima separac\u00EDon espacial disponible en un conjunto de datos, medida en metros."@es .
<http://www.w3.org/ns/dcat#spatialResolutionInMeters> <http://www.w3.org/2000/01/rdf-schema#comment> "separazione spaziale minima risolvibile in un set di dati, misurata in metri."@it .
<http://www.w3.org/ns/dcat#spatialResolutionInMeters> <http://www.w3.org/2000/01/rdf-schema#label> "prostorov\u00E9 rozli\u0161en\u00ED (metry)"@cs .
<http://www.w3.org/ns/dcat#spatialResolutionInMeters> <http://www.w3.org/2000/01/rdf-schema#label> "resoluci\u00F3n espacial (metros)"@es .
<http://www.w3.org/ns/dcat#spatialResolutionInMeters> <http://www.w3.org/2000/01/rdf-schema#label> "risoluzione spaziale (metros)"@it .
<http://www.w3.org/ns/dcat#spatialResolutionInMeters> <http://www.w3.org/2000/01/rdf-schema#label> "spatial resolution (meters)"@en-US .
<http://www.w3.org/ns/dcat#spatialResolutionInMeters> <http://www.w3.org/2000/01/rdf-schema#label> "spatial resolution (metres)"@en-GB .
<http://www.w3.org/ns/dcat#spatialResolutionInMeters> <http://www.w3.org/2000/01/rdf-schema#range> <http://www.w3.org/2001/XMLSchema#decimal> .
<http://www.w3.org/ns/dcat#spatialResolutionInMeters> <http://www.w3.org/2004/02/skos/core#changeNote> "New property added in DCAT 2.0."@en .
<http://www.w3.org/ns/dcat#spatialResolutionInMeters> <http://www.w3.org/2004/02/skos/core#changeNote> "Nov\u00E1 vlastnost p\u0159idan\u00E1 ve verzi DCAT 2.0."@cs .
<http://www.w3.org/ns/dcat#spatialResolutionInMeters> <http://www.w3.org/2004/02/skos/core#changeNote> "Nueva propiedad a\u00F1adida en DCAT 2.0."@es .
<http://www.w3.org/ns/dcat#spatialResolutionInMeters> <http://www.w3.org/2004/02/skos/core#changeNote> "Nuova propriet\u00E0 aggiunta in DCAT 2.0."@it .
<http://www.w3.org/ns/dcat#spatialResolutionInMeters> <http://www.w3.org/2004/02/skos/core#definition> "minimum spatial separation resolvable in a dataset, measured in meters."@en-US .
<http://www.w3.org/ns/dcat#spatialResolutionInMeters> <http://www.w3.org/2004/02/skos/core#definition> "minimum spatial separation resolvable in a dataset, measured in metres."@en-GB .
<http://www.w3.org/ns/dcat#spatialResolutionInMeters> <http://www.w3.org/2004/02/skos/core#definition> "minim\u00E1ln\u00ED prostorov\u00FD rozestup rozeznateln\u00FD v datov\u00E9 sad\u011B, m\u011B\u0159eno v metrech."@cs .
<http://www.w3.org/ns/dcat#spatialResolutionInMeters> <http://www.w3.org/2004/02/skos/core#definition> "m\u00EDnima separac\u00EDon espacial disponible en un conjunto de datos, medida en metros."@es .
<http://www.w3.org/ns/dcat#spatialResolutionInMeters> <http://www.w3.org/2004/02/skos/core#definition> "separazione spaziale minima risolvibile in un set di dati, misurata in metri."@it .
<http://www.w3.org/ns/dcat#spatialResolutionInMeters> <http://www.w3.org/2004/02/skos/core#editorialNote> "Might appear in the description of a Dataset or a Distribution, so no domain is specified."@en .
<http://www.w3.org/ns/dcat#spatialResolutionInMeters> <http://www.w3.org/2004/02/skos/core#editorialNote> "M\u016F\u017Ee se vyskytnout v popisu Datov\u00E9 sady nebo Distribuce, tak\u017Ee nebyl specifikov\u00E1n defini\u010Dn\u00ED obor."@cs .
<http://www.w3.org/ns/dcat#spatialResolutionInMeters> <http://www.w3.org/2004/02/skos/core#scopeNote> "Alternative spatial resolutions might be provided as different dataset distributions."@en .
<http://www.w3.org/ns/dcat#spatialResolutionInMeters> <http://www.w3.org/2004/02/skos/core#scopeNote> "Distintas distribuciones de un conjunto de datos pueden tener resoluciones espaciales diferentes."@es .
<http://www.w3.org/ns/dcat#spatialResolutionInMeters> <http://www.w3.org/2004/02/skos/core#scopeNote> "If the dataset is an image or grid this should correspond to the spacing of items. For other kinds of spatial dataset, this property will usually indicate the smallest distance between items in the dataset."@en .
<http://www.w3.org/ns/dcat#spatialResolutionInMeters> <http://www.w3.org/2004/02/skos/core#scopeNote> "Pokud je datov\u00E1 sada obraz \u010Di m\u0159\u00ED\u017Eka, m\u011Bla by tato vlastnost odpov\u00EDdat rozestupu polo\u017Eek. Pro ostatn\u00ED druhy prostorov\u00FDch datov\u00FDch sad bude tato vlastnost obvykle indikovat nejmen\u0161\u00ED vzd\u00E1lenost mezi polo\u017Ekami t\u00E9to datov\u00E9 sady."@cs .
<http://www.w3.org/ns/dcat#spatialResolutionInMeters> <http://www.w3.org/2004/02/skos/core#scopeNote> "Risoluzioni spaziali alternative possono essere fornite come diverse distribuzioni di set di dati."@it .
<http://www.w3.org/ns/dcat#spatialResolutionInMeters> <http://www.w3.org/2004/02/skos/core#scopeNote> "R\u016Fzn\u00E1 prostorov\u00E1 rozli\u0161en\u00ED mohou b\u00FDt poskytov\u00E1na jako r\u016Fzn\u00E9 distribuce datov\u00E9 sady."@cs .
<http://www.w3.org/ns/dcat#spatialResolutionInMeters> <http://www.w3.org/2004/02/skos/core#scopeNote> "Se il set di dati \u00E8 un'immagine o una griglia, questo dovrebbe corrispondere alla spaziatura degli elementi. Per altri tipi di set di dati spaziali, questa propriet\u00E0 di solito indica la distanza minima tra gli elementi nel set di dati."@it .
<http://www.w3.org/ns/dcat#spatialResolutionInMeters> <http://www.w3.org/2004/02/skos/core#scopeNote> "Si el conjunto de datos es una im\u00E1gen o grilla, esta propiedad corresponde al espaciado de los elementos. Para otro tipo de conjunto de datos espaciales, esta propieda usualmente indica la menor distancia entre los elementos de dichos datos."@es .
<http://www.w3.org/ns/dcat#startDate> <http://www.w3.org/1999/02/22-rdf-syntax-ns#type> <http://www.w3.org/1999/02/22-rdf-syntax-ns#Property> .
<http://www.w3.org/ns/dcat#startDate> <http://www.w3.org/1999/02/22-rdf-syntax-ns#type> <http://www.w3.org/2002/07/owl#DatatypeProperty> .
<http://www.w3.org/ns/dcat#startDate> <http://www.w3.org/2000/01/rdf-schema#domain> <http://purl.org/dc/terms/PeriodOfTime> .
<http://www.w3.org/ns/dcat#startDate> <http://www.w3.org/2000/01/rdf-schema#label> "datum za\u010D\u00E1tku"@cs .
<http://www.w3.org/ns/dcat#startDate> <http://www.w3.org/2000/01/rdf-schema#label> "start date"@en .
<http://www.w3.org/ns/dcat#startDate> <http://www.w3.org/2000/01/rdf-schema#label> "data di inizio"@it .
<http://www.w3.org/ns/dcat#startDate> <http://www.w3.org/2000/01/rdf-schema#range> <http://www.w3.org/2000/01/rdf-schema#Literal> .
<http://www.w3.org/ns/dcat#startDate> <http://www.w3.org/2004/02/skos/core#changeNote> "New property added in DCAT 2.0."@en .
<http://www.w3.org/ns/dcat#startDate> <http://www.w3.org/2004/02/skos/core#changeNote> "Nuova propriet\u00E0 aggiunta in DCAT 2.0."@it .
<http://www.w3.org/ns/dcat#startDate> <http://www.w3.org/2004/02/skos/core#changeNote> "Nov\u00E1 vlastnost p\u0159idan\u00E1 ve verzi DCAT 2.0."@cs .
<http://www.w3.org/ns/dcat#startDate> <http://www.w3.org/2004/02/skos/core#changeNote> "Nueva propiedad agregada en DCAT 2.0."@es .
<http://www.w3.org/ns/dcat#startDate> <http://www.w3.org/2004/02/skos/core#definition> "El comienzo del per\u00EDodo"@es .
<http://www.w3.org/ns/dcat#startDate> <http://www.w3.org/2004/02/skos/core#definition> "The start of the period"@en .
<http://www.w3.org/ns/dcat#startDate> <http://www.w3.org/2004/02/skos/core#definition> "L'inizio del periodo"@it .
<http://www.w3.org/ns/dcat#startDate> <http://www.w3.org/2004/02/skos/core#definition> "Za\u010D\u00E1tek doby trv\u00E1n\u00ED"@cs .
<http://www.w3.org/ns/dcat#startDate> <http://www.w3.org/2004/02/skos/core#scopeNote> "El rango de esta propiedad es intencionalmente gen\u00E9rico con el prop\u00F3sito de permitir distintos niveles de precisi\u00F3n temporal para especificar el comienzo de un per\u00EDodo. Por ejemplo, puede expresarse como una fecha (xsd:date), una fecha y un tiempo (xsd:dateTime), o un a\u00F1o (xsd:gYear)."@es .
<http://www.w3.org/ns/dcat#startDate> <http://www.w3.org/2004/02/skos/core#scopeNote> "Obor hodnot t\u00E9to vlastnosti je \u00FAmysln\u011B obecn\u00FD, aby umo\u017Enil r\u016Fzn\u00E9 \u00FArovn\u011B \u010Dasov\u00E9ho rozli\u0161en\u00ED pro specifikaci za\u010D\u00E1tku doby trv\u00E1n\u00ED. Ten m\u016F\u017Ee b\u00FDt kup\u0159\u00EDkladu vyj\u00E1d\u0159en datumem (xsd:date), datumem a \u010Dasem (xsd:dateTime) \u010Di rokem (xsd:gYear)."@cs .
<http://www.w3.org/ns/dcat#startDate> <http://www.w3.org/2004/02/skos/core#scopeNote> "The range of this property is intentionally generic, with the purpose of allowing different level of temporal precision for specifying the start of a period. E.g., it can be expressed with a date (xsd:date), a date and time (xsd:dateTime), or a year (xsd:gYear)."@en .
<http://www.w3.org/ns/dcat#startDate> <http://www.w3.org/2004/02/skos/core#scopeNote> "Il range di questa propriet\u00E0 \u00E8 volutamente generico, con lo scopo di consentire diversi livelli di precisione temporale per specificare l'inizio di un periodo. Ad esempio, pu\u00F2 essere espresso con una data (xsd:date), una data e un'ora (xsd:dateTime), o un anno (xsd:gYear)."@it .
<http://www.w3.org/ns/dcat#temporalResolution> <http://www.w3.org/1999/02/22-rdf-syntax-ns#type> <http://www.w3.org/2002/07/owl#DatatypeProperty> .
<http://www.w3.org/ns/dcat#temporalResolution> <http://www.w3.org/2000/01/rdf-schema#comment> "minimum time period resolvable in a dataset."@en .
<http://www.w3.org/ns/dcat#temporalResolution> <http://www.w3.org/2000/01/rdf-schema#comment> "minim\u00E1ln\u00ED doba trv\u00E1n\u00ED rozli\u0161iteln\u00E1 v datov\u00E9 sad\u011B."@cs .
<http://www.w3.org/ns/dcat#temporalResolution> <http://www.w3.org/2000/01/rdf-schema#comment> "periodo di tempo minimo risolvibile in un set di dati."@it .
<http://www.w3.org/ns/dcat#temporalResolution> <http://www.w3.org/2000/01/rdf-schema#comment> "per\u00EDodo de tiempo m\u00EDnimo en el conjunto de datos."@es .
<http://www.w3.org/ns/dcat#temporalResolution> <http://www.w3.org/2000/01/rdf-schema#label> "resoluci\u00F3n temporal"@es .
<http://www.w3.org/ns/dcat#temporalResolution> <http://www.w3.org/2000/01/rdf-schema#label> "risoluzione temporale"@it .
<http://www.w3.org/ns/dcat#temporalResolution> <http://www.w3.org/2000/01/rdf-schema#label> "temporal resolution"@en .
<http://www.w3.org/ns/dcat#temporalResolution> <http://www.w3.org/2000/01/rdf-schema#label> "\u010Dasov\u00E9 rozli\u0161en\u00ED"@cs .
<http://www.w3.org/ns/dcat#temporalResolution> <http://www.w3.org/2000/01/rdf-schema#range> <http://www.w3.org/2001/XMLSchema#duration> .
<http://www.w3.org/ns/dcat#temporalResolution> <http://www.w3.org/2004/02/skos/core#changeNote> "New property added in DCAT 2.0."@en .
<http://www.w3.org/ns/dcat#temporalResolution> <http://www.w3.org/2004/02/skos/core#changeNote> "Nov\u00E1 vlastnost p\u0159idan\u00E1 ve verzi DCAT 2.0."@cs .
<http://www.w3.org/ns/dcat#temporalResolution> <http://www.w3.org/2004/02/skos/core#changeNote> "Nueva propiedad a\u00F1adida en DCAT 2.0."@es .
<http://www.w3.org/ns/dcat#temporalResolution> <http://www.w3.org/2004/02/skos/core#changeNote> "Nuova propriet\u00E0 aggiunta in DCAT 2.0."@it .
<http://www.w3.org/ns/dcat#temporalResolution> <http://www.w3.org/2004/02/skos/core#definition> "minimum time period resolvable in a dataset."@en .
<http://www.w3.org/ns/dcat#temporalResolution> <http://www.w3.org/2004/02/skos/core#definition> "minim\u00E1ln\u00ED doba trv\u00E1n\u00ED rozli\u0161iteln\u00E1 v datov\u00E9 sad\u011B."@cs .
<http://www.w3.org/ns/dcat#temporalResolution> <http://www.w3.org/2004/02/skos/core#definition> "periodo di tempo minimo risolvibile in un set di dati."@it .
<http://www.w3.org/ns/dcat#temporalResolution> <http://www.w3.org/2004/02/skos/core#definition> "per\u00EDodo de tiempo m\u00EDnimo en el conjunto de datos."@es .
<http://www.w3.org/ns/dcat#temporalResolution> <http://www.w3.org/2004/02/skos/core#editorialNote> "Might appear in the description of a Dataset or a Distribution, so no domain is specified."@en .
<http://www.w3.org/ns/dcat#temporalResolution> <http://www.w3.org/2004/02/skos/core#editorialNote> "M\u016F\u017Ee se vyskytnout v popisu Datov\u00E9 sady nebo Distribuce, tak\u017Ee nebyl specifikov\u00E1n defini\u010Dn\u00ED obor."@cs .
<http://www.w3.org/ns/dcat#temporalResolution> <http://www.w3.org/2004/02/skos/core#scopeNote> "Alternative temporal resolutions might be provided as different dataset distributions."@en .
<http://www.w3.org/ns/dcat#temporalResolution> <http://www.w3.org/2004/02/skos/core#scopeNote> "Distintas distribuciones del conjunto de datos pueden tener resoluciones temporales diferentes."@es .
<http://www.w3.org/ns/dcat#temporalResolution> <http://www.w3.org/2004/02/skos/core#scopeNote> "If the dataset is a time-series this should correspond to the spacing of items in the series. For other kinds of dataset, this property will usually indicate the smallest time difference between items in the dataset."@en .
<http://www.w3.org/ns/dcat#temporalResolution> <http://www.w3.org/2004/02/skos/core#scopeNote> "Pokud je datov\u00E1 sada \u010Dasovou \u0159adou, m\u011Bla by tato vlastnost odpov\u00EDdat rozestupu polo\u017Eek v \u0159ad\u011B. Pro ostatn\u00ED druhy datov\u00FDch sad bude tato vlastnost obvykle indikovat nejmen\u0161\u00ED \u010Dasovou vzd\u00E1lenost mezi polo\u017Ekami t\u00E9to datov\u00E9 sady."@cs .
<http://www.w3.org/ns/dcat#temporalResolution> <http://www.w3.org/2004/02/skos/core#scopeNote> "Risoluzioni temporali alternative potrebbero essere fornite come diverse distribuzioni di set di dati."@it .
<http://www.w3.org/ns/dcat#temporalResolution> <http://www.w3.org/2004/02/skos/core#scopeNote> "R\u016Fzn\u00E1 \u010Dasov\u00E1 rozli\u0161en\u00ED mohou b\u00FDt poskytov\u00E1na jako r\u016Fzn\u00E9 distribuce datov\u00E9 sady."@cs .
<http://www.w3.org/ns/dcat#temporalResolution> <http://www.w3.org/2004/02/skos/core#scopeNote> "Se il set di dati \u00E8 una serie temporale, questo dovrebbe corrispondere alla spaziatura degli elementi della serie. Per altri tipi di set di dati, questa propriet\u00E0 di solito indica la pi\u00F9 piccola differenza di tempo tra gli elementi nel set di dati."@it .
<http://www.w3.org/ns/dcat#temporalResolution> <http://www.w3.org/2004/02/skos/core#scopeNote> "Si el conjunto de datos es una serie temporal, debe corresponder al espaciado de los elementos de la serie. Para otro tipo de conjuntos de datos, esta propiedad indicar\u00E1 usualmente la menor diferencia de tiempo entre elementos en el dataset."@es .
<http://www.w3.org/ns/dcat#theme> <http://www.w3.org/1999/02/22-rdf-syntax-ns#type> <http://www.w3.org/1999/02/22-rdf-syntax-ns#Property> .
<http://www.w3.org/ns/dcat#theme> <http://www.w3.org/1999/02/22-rdf-syntax-ns#type> <http://www.w3.org/2002/07/owl#ObjectProperty> .
<http://www.w3.org/ns/dcat#theme> <http://www.w3.org/2000/01/rdf-schema#comment> "A main category of the resource. A resource can have multiple themes."@en .
<http://www.w3.org/ns/dcat#theme> <http://www.w3.org/2000/01/rdf-schema#comment> "Hlavn\u00ED t\u00E9ma zdroje. Zdroj m\u016F\u017Ee m\u00EDt v\u00EDce t\u00E9mat."@cs .
<http://www.w3.org/ns/dcat#theme> <http://www.w3.org/2000/01/rdf-schema#comment> "La categoria principale della risorsa. Una risorsa pu\u00F2 avere pi\u00F9 temi."@it .
<http://www.w3.org/ns/dcat#theme> <http://www.w3.org/2000/01/rdf-schema#comment> "La categor\u00EDa principal del recurso. Un recurso puede tener varios temas."@es .
<http://www.w3.org/ns/dcat#theme> <http://www.w3.org/2000/01/rdf-schema#comment> "La cat\u00E9gorie principale de la ressource. Une ressource peut avoir plusieurs th\u00E8mes."@fr .
<http://www.w3.org/ns/dcat#theme> <http://www.w3.org/2000/01/rdf-schema#comment> "\u0397 \u03BA\u03CD\u03C1\u03B9\u03B1 \u03BA\u03B1\u03C4\u03B7\u03B3\u03BF\u03C1\u03AF\u03B1 \u03C4\u03BF\u03C5 \u03C3\u03C5\u03BD\u03CC\u03BB\u03BF\u03C5 \u03B4\u03B5\u03B4\u03BF\u03BC\u03AD\u03BD\u03C9\u03BD. \u0388\u03BD\u03B1 \u03C3\u03CD\u03BD\u03BF\u03BB\u03BF \u03B4\u03B5\u03B4\u03BF\u03BC\u03AD\u03BD\u03C9\u03BD \u03B4\u03CD\u03BD\u03B1\u03C4\u03B1\u03B9 \u03BD\u03B1 \u03AD\u03C7\u03B5\u03B9 \u03C0\u03BF\u03BB\u03BB\u03B1\u03C0\u03BB\u03AC \u03B8\u03AD\u03BC\u03B1\u03C4\u03B1."@el .
<http://www.w3.org/ns/dcat#theme> <http://www.w3.org/2000/01/rdf-schema#comment> "\u0627\u0644\u062A\u0635\u0646\u064A\u0641 \u0627\u0644\u0631\u0626\u064A\u0633\u064A \u0644\u0642\u0627\u0626\u0645\u0629 \u0627\u0644\u0628\u064A\u0627\u0646\u0627\u062A. \u0642\u0627\u0626\u0645\u0629 \u0627\u0644\u0628\u064A\u0627\u0646\u0627\u062A \u064A\u0645\u0643\u0646 \u0623\u0646 \u062A\u0645\u0644\u0643 \u0623\u0643\u062B\u0631 \u0645\u0646 \u062A\u0635\u0646\u064A\u0641 \u0631\u0626\u064A\u0633\u064A \u0648\u0627\u062D\u062F."@ar .
<http://www.w3.org/ns/dcat#theme> <http://www.w3.org/2000/01/rdf-schema#comment> "\u30C7\u30FC\u30BF\u30BB\u30C3\u30C8\u306E\u4E3B\u8981\u30AB\u30C6\u30B4\u30EA\u30FC\u3002\u30C7\u30FC\u30BF\u30BB\u30C3\u30C8\u306F\u8907\u6570\u306E\u30C6\u30FC\u30DE\u3092\u6301\u3064\u3053\u3068\u304C\u3067\u304D\u307E\u3059\u3002"@ja .
<http://www.w3.org/ns/dcat#theme> <http://www.w3.org/2000/01/rdf-schema#isDefinedBy> <http://www.w3.org/TR/vocab-dcat/> .
<http://www.w3.org/ns/dcat#theme> <http://www.w3.org/2000/01/rdf-schema#label> "tema"@es .
<http://www.w3.org/ns/dcat#theme> <http://www.w3.org/2000/01/rdf-schema#label> "tema"@it .
<http://www.w3.org/ns/dcat#theme> <http://www.w3.org/2000/01/rdf-schema#label> "theme"@en .
<http://www.w3.org/ns/dcat#theme> <http://www.w3.org/2000/01/rdf-schema#label> "th\u00E8me"@fr .
<http://www.w3.org/ns/dcat#theme> <http://www.w3.org/2000/01/rdf-schema#label> "t\u00E9ma"@cs .
<http://www.w3.org/ns/dcat#theme> <http://www.w3.org/2000/01/rdf-schema#label> "\u0398\u03AD\u03BC\u03B1"@el .
<http://www.w3.org/ns/dcat#theme> <http://www.w3.org/2000/01/rdf-schema#label> "\u0627\u0644\u062A\u0635\u0646\u064A\u0641"@ar .
<http://www.w3.org/ns/dcat#theme> <http://www.w3.org/2000/01/rdf-schema#label> "\u30C6\u30FC\u30DE/\u30AB\u30C6\u30B4\u30EA\u30FC"@ja .
<http://www.w3.org/ns/dcat#theme> <http://www.w3.org/2000/01/rdf-schema#range> <http://www.w3.org/2004/02/skos/core#Concept> .
<http://www.w3.org/ns/dcat#theme> <http://www.w3.org/2000/01/rdf-schema#subPropertyOf> <http://purl.org/dc/terms/subject> .
<http://www.w3.org/ns/dcat#theme> <http://www.w3.org/2004/02/skos/core#definition> "A main category of the resource. A resource can have multiple themes."@en .
<http://www.w3.org/ns/dcat#theme> <http://www.w3.org/2004/02/skos/core#definition> "Hlavn\u00ED t\u00E9ma zdroje. Zdroj m\u016F\u017Ee m\u00EDt v\u00EDce t\u00E9mat."@cs .
<http://www.w3.org/ns/dcat#theme> <http://www.w3.org/2004/02/skos/core#definition> "La categoria principale della risorsa. Una risorsa pu\u00F2 avere pi\u00F9 temi."@it .
<http://www.w3.org/ns/dcat#theme> <http://www.w3.org/2004/02/skos/core#definition> "La categor\u00EDa principal del recurso. Un recurso puede tener varios temas."@es .
<http://www.w3.org/ns/dcat#theme> <http://www.w3.org/2004/02/skos/core#definition> "La cat\u00E9gorie principale de la ressource. Une ressource peut avoir plusieurs th\u00E8mes."@fr .
<http://www.w3.org/ns/dcat#theme> <http://www.w3.org/2004/02/skos/core#definition> "\u0397 \u03BA\u03CD\u03C1\u03B9\u03B1 \u03BA\u03B1\u03C4\u03B7\u03B3\u03BF\u03C1\u03AF\u03B1 \u03C4\u03BF\u03C5 \u03C3\u03C5\u03BD\u03CC\u03BB\u03BF\u03C5 \u03B4\u03B5\u03B4\u03BF\u03BC\u03AD\u03BD\u03C9\u03BD. \u0388\u03BD\u03B1 \u03C3\u03CD\u03BD\u03BF\u03BB\u03BF \u03B4\u03B5\u03B4\u03BF\u03BC\u03AD\u03BD\u03C9\u03BD \u03B4\u03CD\u03BD\u03B1\u03C4\u03B1\u03B9 \u03BD\u03B1 \u03AD\u03C7\u03B5\u03B9 \u03C0\u03BF\u03BB\u03BB\u03B1\u03C0\u03BB\u03AC \u03B8\u03AD\u03BC\u03B1\u03C4\u03B1."@el .
<http://www.w3.org/ns/dcat#theme> <http://www.w3.org/2004/02/skos/core#definition> "\u0627\u0644\u062A\u0635\u0646\u064A\u0641 \u0627\u0644\u0631\u0626\u064A\u0633\u064A \u0644\u0642\u0627\u0626\u0645\u0629 \u0627\u0644\u0628\u064A\u0627\u0646\u0627\u062A. \u0642\u0627\u0626\u0645\u0629 \u0627\u0644\u0628\u064A\u0627\u0646\u0627\u062A \u064A\u0645\u0643\u0646 \u0623\u0646 \u062A\u0645\u0644\u0643 \u0623\u0643\u062B\u0631 \u0645\u0646 \u062A\u0635\u0646\u064A\u0641 \u0631\u0626\u064A\u0633\u064A \u0648\u0627\u062D\u062F."@ar .
<http://www.w3.org/ns/dcat#theme> <http://www.w3.org/2004/02/skos/core#definition> "\u30C7\u30FC\u30BF\u30BB\u30C3\u30C8\u306E\u4E3B\u8981\u30AB\u30C6\u30B4\u30EA\u30FC\u3002\u30C7\u30FC\u30BF\u30BB\u30C3\u30C8\u306F\u8907\u6570\u306E\u30C6\u30FC\u30DE\u3092\u6301\u3064\u3053\u3068\u304C\u3067\u304D\u307E\u3059\u3002"@ja .
<http://www.w3.org/ns/dcat#theme> <http://www.w3.org/2004/02/skos/core#editorialNote> "Status: English Definition text modified by DCAT revision team, all except for Italian and Czech translations are pending."@en .
<http://www.w3.org/ns/dcat#theme> <http://www.w3.org/2004/02/skos/core#scopeNote> "El conjunto de skos:Concepts utilizados para categorizar los recursos est\u00E1n organizados en un skos:ConceptScheme que describe todas las categor\u00EDas y sus relaciones en el cat\u00E1logo."@es .
<http://www.w3.org/ns/dcat#theme> <http://www.w3.org/2004/02/skos/core#scopeNote> "Il set di concetti skos usati per categorizzare le risorse sono organizzati in skos:ConceptScheme che descrive tutte le categorie e le loro relazioni nel catalogo."@it .
<http://www.w3.org/ns/dcat#theme> <http://www.w3.org/2004/02/skos/core#scopeNote> "Sada instanc\u00ED t\u0159\u00EDdy skos:Concept pou\u017Eit\u00E1 pro kategorizaci zdroj\u016F je organizov\u00E1na do sch\u00E9matu koncept\u016F skos:ConceptScheme, kter\u00E9 popisuje v\u0161echny kategorie v katalogu a jejich vztahy."@cs .
<http://www.w3.org/ns/dcat#theme> <http://www.w3.org/2004/02/skos/core#scopeNote> "The set of skos:Concepts used to categorize the resources are organized in a skos:ConceptScheme describing all the categories and their relations in the catalog."@en .
<http://www.w3.org/ns/dcat#theme> <http://www.w3.org/2004/02/skos/core#scopeNote> "Un ensemble de skos:Concepts utilis\u00E9s pour cat\u00E9goriser les ressources sont organis\u00E9s en un skos:ConceptScheme d\u00E9crivant toutes les cat\u00E9gories et ses relations dans le catalogue."@fr .
<http://www.w3.org/ns/dcat#theme> <http://www.w3.org/2004/02/skos/core#scopeNote> "\u03A4\u03BF \u03C3\u03B5\u03C4 \u03C4\u03C9\u03BD skos:Concepts \u03C0\u03BF\u03C5 \u03C7\u03C1\u03B7\u03C3\u03B9\u03BC\u03BF\u03C0\u03BF\u03B9\u03B5\u03AF\u03C4\u03B1\u03B9 \u03B3\u03B9\u03B1 \u03BD\u03B1 \u03BA\u03B1\u03C4\u03B7\u03B3\u03BF\u03C1\u03B9\u03BF\u03C0\u03BF\u03B9\u03AE\u03C3\u03B5\u03B9 \u03C4\u03B1 \u03C3\u03CD\u03BD\u03BF\u03BB\u03B1 \u03B4\u03B5\u03B4\u03BF\u03BC\u03AD\u03BD\u03C9\u03BD \u03B5\u03AF\u03BD\u03B1\u03B9 \u03BF\u03C1\u03B3\u03B1\u03BD\u03C9\u03BC\u03AD\u03BD\u03BF \u03B5\u03BD\u03C4\u03CC\u03C2 \u03B5\u03BD\u03CC\u03C2 skos:ConceptScheme \u03C0\u03BF\u03C5 \u03C0\u03B5\u03C1\u03B9\u03B3\u03C1\u03AC\u03C6\u03B5\u03B9 \u03CC\u03BB\u03B5\u03C2 \u03C4\u03B9\u03C2 \u03BA\u03B1\u03C4\u03B7\u03B3\u03BF\u03C1\u03AF\u03B5\u03C2 \u03BA\u03B1\u03B9 \u03C4\u03B9\u03C2 \u03C3\u03C7\u03AD\u03C3\u03B5\u03B9\u03C2 \u03B1\u03C5\u03C4\u03CE\u03BD \u03C3\u03C4\u03BF\u03BD \u03BA\u03B1\u03C4\u03AC\u03BB\u03BF\u03B3\u03BF."@el .
<http://www.w3.org/ns/dcat#theme> <http://www.w3.org/2004/02/skos/core#scopeNote> "\u30C7\u30FC\u30BF\u30BB\u30C3\u30C8\u3092\u5206\u985E\u3059\u308B\u305F\u3081\u306B\u7528\u3044\u3089\u308C\u308Bskos:Concept\u306E\u96C6\u5408\u306F\u3001\u30AB\u30BF\u30ED\u30B0\u306E\u3059\u3079\u3066\u306E\u30AB\u30C6\u30B4\u30EA\u30FC\u3068\u305D\u308C\u3089\u306E\u95A2\u4FC2\u3092\u8A18\u8FF0\u3057\u3066\u3044\u308Bskos:ConceptScheme\u3067\u7D44\u7E54\u5316\u3055\u308C\u307E\u3059\u3002"@ja .
<http://www.w3.org/ns/dcat#themeTaxonomy> <http://www.w3.org/1999/02/22-rdf-syntax-ns#type> <http://www.w3.org/1999/02/22-rdf-syntax-ns#Property> .
<http://www.w3.org/ns/dcat#themeTaxonomy> <http://www.w3.org/1999/02/22-rdf-syntax-ns#type> <http://www.w3.org/2002/07/owl#ObjectProperty> .
<http://www.w3.org/ns/dcat#themeTaxonomy> <http://schema.org/rangeIncludes> <http://www.w3.org/2002/07/owl#Ontology> .
<http://www.w3.org/ns/dcat#themeTaxonomy> <http://schema.org/rangeIncludes> <http://www.w3.org/2004/02/skos/core#Collection> .
<http://www.w3.org/ns/dcat#themeTaxonomy> <http://schema.org/rangeIncludes> <http://www.w3.org/2004/02/skos/core#ConceptScheme> .
<http://www.w3.org/ns/dcat#themeTaxonomy> <http://www.w3.org/2000/01/rdf-schema#comment> "El sistema de organizaci\u00F3n del conocimiento utilizado para clasificar conjuntos de datos de cat\u00E1logos."@es .
<http://www.w3.org/ns/dcat#themeTaxonomy> <http://www.w3.org/2000/01/rdf-schema#comment> "Il sistema di organizzazione della conoscenza (KOS) usato per classificare i dataset del catalogo."@it .
<http://www.w3.org/ns/dcat#themeTaxonomy> <http://www.w3.org/2000/01/rdf-schema#comment> "Le systh\u00E8me d'ogranisation de connaissances utilis\u00E9 pour classifier les jeux de donn\u00E9es du catalogue."@fr .
<http://www.w3.org/ns/dcat#themeTaxonomy> <http://www.w3.org/2000/01/rdf-schema#comment> "Syst\u00E9m organizace znalost\u00ED (KOS) pou\u017Eit\u00FD pro klasifikaci datov\u00FDch sad v katalogu."@cs .
<http://www.w3.org/ns/dcat#themeTaxonomy> <http://www.w3.org/2000/01/rdf-schema#comment> "The knowledge organization system (KOS) used to classify catalog's datasets."@en .
<http://www.w3.org/ns/dcat#themeTaxonomy> <http://www.w3.org/2000/01/rdf-schema#comment> "\u03A4\u03BF \u03C3\u03CD\u03C3\u03C4\u03B7\u03BC\u03B1 \u03BF\u03C1\u03B3\u03AC\u03BD\u03C9\u03C3\u03B7\u03C2 \u03B3\u03BD\u03CE\u03C3\u03B7\u03C2 \u03C0\u03BF\u03C5 \u03C7\u03C1\u03B7\u03C3\u03B9\u03BC\u03BF\u03C0\u03BF\u03B9\u03B5\u03AF\u03C4\u03B1\u03B9 \u03B3\u03B9\u03B1 \u03C4\u03B7\u03BD \u03BA\u03B1\u03C4\u03B7\u03B3\u03BF\u03C1\u03B9\u03BF\u03C0\u03BF\u03AF\u03B7\u03C3\u03B7 \u03C4\u03C9\u03BD \u03C3\u03C5\u03BD\u03CC\u03BB\u03C9\u03BD \u03B4\u03B5\u03B4\u03BF\u03BC\u03AD\u03BD\u03C9\u03BD \u03C4\u03BF\u03C5 \u03BA\u03B1\u03C4\u03B1\u03BB\u03CC\u03B3\u03BF\u03C5."@el .
<http://www.w3.org/ns/dcat#themeTaxonomy> <http://www.w3.org/2000/01/rdf-schema#comment> "\u0644\u0627\u0626\u062D\u0629 \u0627\u0644\u062A\u0635\u0646\u064A\u0641\u0627\u062A \u0627\u0644\u0645\u0633\u062A\u062E\u062F\u0645\u0647 \u0644\u062A\u0635\u0646\u064A\u0641 \u0642\u0648\u0627\u0626\u0645 \u0627\u0644\u0628\u064A\u0627\u0646\u0627\u062A \u0636\u0645\u0646 \u0627\u0644\u0641\u0647\u0631\u0633"@ar .
<http://www.w3.org/ns/dcat#themeTaxonomy> <http://www.w3.org/2000/01/rdf-schema#comment> "\u30AB\u30BF\u30ED\u30B0\u306E\u30C7\u30FC\u30BF\u30BB\u30C3\u30C8\u3092\u5206\u985E\u3059\u308B\u305F\u3081\u306B\u7528\u3044\u3089\u308C\u308B\u77E5\u8B58\u7D44\u7E54\u5316\u4F53\u7CFB\uFF08KOS\uFF1Bknowledge organization system\uFF09\u3002"@ja .
<http://www.w3.org/ns/dcat#themeTaxonomy> <http://www.w3.org/2000/01/rdf-schema#domain> <http://www.w3.org/ns/dcat#Catalog> .
<http://www.w3.org/ns/dcat#themeTaxonomy> <http://www.w3.org/2000/01/rdf-schema#isDefinedBy> <http://www.w3.org/TR/vocab-dcat/> .
<http://www.w3.org/ns/dcat#themeTaxonomy> <http://www.w3.org/2000/01/rdf-schema#label> "tassonomia dei temi"@it .
<http://www.w3.org/ns/dcat#themeTaxonomy> <http://www.w3.org/2000/01/rdf-schema#label> "taxonomie de th\u00E8mes"@fr .
<http://www.w3.org/ns/dcat#themeTaxonomy> <http://www.w3.org/2000/01/rdf-schema#label> "taxonomie t\u00E9mat"@cs .
<http://www.w3.org/ns/dcat#themeTaxonomy> <http://www.w3.org/2000/01/rdf-schema#label> "taxonom\u00EDa de temas"@es .
<http://www.w3.org/ns/dcat#themeTaxonomy> <http://www.w3.org/2000/01/rdf-schema#label> "theme taxonomy"@en .
<http://www.w3.org/ns/dcat#themeTaxonomy> <http://www.w3.org/2000/01/rdf-schema#label> "\u03A4\u03B1\u03BE\u03B9\u03BD\u03BF\u03BC\u03AF\u03B1 \u03B8\u03B5\u03BC\u03B1\u03C4\u03B9\u03BA\u03CE\u03BD \u03BA\u03B1\u03C4\u03B7\u03B3\u03BF\u03C1\u03B9\u03CE\u03BD."@el .
<http://www.w3.org/ns/dcat#themeTaxonomy> <http://www.w3.org/2000/01/rdf-schema#label> "\u0642\u0627\u0626\u0645\u0629 \u0627\u0644\u062A\u0635\u0646\u064A\u0641\u0627\u062A"@ar .
<http://www.w3.org/ns/dcat#themeTaxonomy> <http://www.w3.org/2000/01/rdf-schema#label> "\u30C6\u30FC\u30DE"@ja .
<http://www.w3.org/ns/dcat#themeTaxonomy> <http://www.w3.org/2000/01/rdf-schema#range> <http://www.w3.org/2000/01/rdf-schema#Resource> .
<http://www.w3.org/ns/dcat#themeTaxonomy> <http://www.w3.org/2004/02/skos/core#definition> "El sistema de organizaci\u00F3n del conocimiento utilizado para clasificar conjuntos de datos de cat\u00E1logos."@es .
<http://www.w3.org/ns/dcat#themeTaxonomy> <http://www.w3.org/2004/02/skos/core#definition> "Il sistema di organizzazione della conoscenza (KOS) usato per classificare i dataset del catalogo."@it .
<http://www.w3.org/ns/dcat#themeTaxonomy> <http://www.w3.org/2004/02/skos/core#definition> "Le systh\u00E8me d'ogranisation de connaissances utilis\u00E9 pour classifier les jeux de donn\u00E9es du catalogue."@fr .
<http://www.w3.org/ns/dcat#themeTaxonomy> <http://www.w3.org/2004/02/skos/core#definition> "Syst\u00E9m organizace znalost\u00ED (KOS) pou\u017Eit\u00FD pro klasifikaci datov\u00FDch sad v katalogu."@cs .
<http://www.w3.org/ns/dcat#themeTaxonomy> <http://www.w3.org/2004/02/skos/core#definition> "The knowledge organization system (KOS) used to classify catalog's datasets."@en .
<http://www.w3.org/ns/dcat#themeTaxonomy> <http://www.w3.org/2004/02/skos/core#definition> "\u03A4\u03BF \u03C3\u03CD\u03C3\u03C4\u03B7\u03BC\u03B1 \u03BF\u03C1\u03B3\u03AC\u03BD\u03C9\u03C3\u03B7\u03C2 \u03B3\u03BD\u03CE\u03C3\u03B7\u03C2 \u03C0\u03BF\u03C5 \u03C7\u03C1\u03B7\u03C3\u03B9\u03BC\u03BF\u03C0\u03BF\u03B9\u03B5\u03AF\u03C4\u03B1\u03B9 \u03B3\u03B9\u03B1 \u03C4\u03B7\u03BD \u03BA\u03B1\u03C4\u03B7\u03B3\u03BF\u03C1\u03B9\u03BF\u03C0\u03BF\u03AF\u03B7\u03C3\u03B7 \u03C4\u03C9\u03BD \u03C3\u03C5\u03BD\u03CC\u03BB\u03C9\u03BD \u03B4\u03B5\u03B4\u03BF\u03BC\u03AD\u03BD\u03C9\u03BD \u03C4\u03BF\u03C5 \u03BA\u03B1\u03C4\u03B1\u03BB\u03CC\u03B3\u03BF\u03C5."@el .
<http://www.w3.org/ns/dcat#themeTaxonomy> <http://www.w3.org/2004/02/skos/core#definition> "\u0644\u0627\u0626\u062D\u0629 \u0627\u0644\u062A\u0635\u0646\u064A\u0641\u0627\u062A \u0627\u0644\u0645\u0633\u062A\u062E\u062F\u0645\u0647 \u0644\u062A\u0635\u0646\u064A\u0641 \u0642\u0648\u0627\u0626\u0645 \u0627\u0644\u0628\u064A\u0627\u0646\u0627\u062A \u0636\u0645\u0646 \u0627\u0644\u0641\u0647\u0631\u0633"@ar .
<http://www.w3.org/ns/dcat#themeTaxonomy> <http://www.w3.org/2004/02/skos/core#definition> "\u30AB\u30BF\u30ED\u30B0\u306E\u30C7\u30FC\u30BF\u30BB\u30C3\u30C8\u3092\u5206\u985E\u3059\u308B\u305F\u3081\u306B\u7528\u3044\u3089\u308C\u308B\u77E5\u8B58\u7D44\u7E54\u5316\u4F53\u7CFB\uFF08KOS\uFF1Bknowledge organization system\uFF09\u3002"@ja .
<http://www.w3.org/ns/dcat#themeTaxonomy> <http://www.w3.org/2004/02/skos/core#scopeNote> "It is recommended that the taxonomy is organized in a skos:ConceptScheme, skos:Collection, owl:Ontology or similar, which allows each member to be denoted by an IRI and published as linked-data."@en .
<http://www.w3.org/ns/dcat#themeTaxonomy> <http://www.w3.org/2004/02/skos/core#scopeNote> "Si raccomanda che la tassonomia sia organizzata in uno skos:ConceptScheme, skos:Collection, owl:Ontology o simili, che permette ad ogni membro di essere indicato da un IRI e pubblicato come linked-data."@it .
<http://www.w3.org/ns/dcat#themeTaxonomy> <http://www.w3.org/2004/02/skos/core#scopeNote> "Je doporu\u010Deno, aby byla taxonomie vyj\u00E1d\u0159ena jako skos:ConceptScheme, skos:Collection, owl:Ontology nebo podobn\u00E9, aby mohla b\u00FDt ka\u017Ed\u00E1 polo\u017Eka identifikov\u00E1na pomoc\u00ED IRI a publikov\u00E1na jako propojen\u00E1 data."@cs .
<http://www.w3.org/ns/dcat#themeTaxonomy> <http://www.w3.org/2004/02/skos/core#scopeNote> "Se recomienda que la taxonom\u00EDa se organice como un skos:ConceptScheme, skos:Collection, owl:Ontology o similar, los cu\u00E1les permiten que cada miembro se denote con una IRI y se publique como datos enlazados."@es .
<http://xmlns.com/foaf/0.1/homepage> <http://www.w3.org/1999/02/22-rdf-syntax-ns#type> <http://www.w3.org/2002/07/owl#ObjectProperty> .
<http://xmlns.com/foaf/0.1/homepage> <http://www.w3.org/2000/01/rdf-schema#comment> "This axiom needed so that Protege loads DCAT2 without errors." .
<http://xmlns.com/foaf/0.1/primaryTopic> <http://www.w3.org/1999/02/22-rdf-syntax-ns#type> <http://www.w3.org/2002/07/owl#ObjectProperty> .
<http://xmlns.com/foaf/0.1/primaryTopic> <http://www.w3.org/2000/01/rdf-schema#comment> "This axiom needed so that Protege loads DCAT2 without errors." .
