@prefix owl: <http://www.w3.org/2002/07/owl#> .
@prefix xsd: <http://www.w3.org/2001/XMLSchema#> .
@prefix rdfs: <http://www.w3.org/2000/01/rdf-schema#> .
@prefix rdf: <http://www.w3.org/1999/02/22-rdf-syntax-ns#> .
@prefix dc: <http://purl.org/dc/terms/> .

<http://www.w3.org/ns/hydra/core> a owl:Ontology ;
  <http://creativecommons.org/ns#attributionName> "Hydra W3C Community Group" ;
  <http://creativecommons.org/ns#attributionURL> <http://www.hydra-cg.com/> ;
  <http://creativecommons.org/ns#license> <http://creativecommons.org/licenses/by/4.0/> ;
  dc:description "The Hydra Core Vocabulary is a lightweight vocabulary to create hypermedia-driven Web APIs. By specifying a number of concepts commonly used in Web APIs it enables the creation of generic API clients." ;
  dc:publisher "Hydra W3C Community Group" ;
  dc:rights "Copyright Â© 2012-2014 the Contributors to the Hydra Core Vocabulary Specification" ;
  <http://purl.org/vocab/vann/preferredNamespacePrefix> "hydra" ;
  rdfs:comment "A lightweight vocabulary for hypermedia-driven Web APIs" ;
  rdfs:label "The Hydra Core Vocabulary" ;
  rdfs:seeAlso <https://www.hydra-cg.com/spec/latest/core/> .

<http://www.w3.org/ns/hydra/core#ApiDocumentation> a <http://www.w3.org/ns/hydra/core#Class> ;
  rdfs:comment "The Hydra API documentation class" ;
  rdfs:isDefinedBy <http://www.w3.org/ns/hydra/core> ;
  rdfs:label "ApiDocumentation" ;
  rdfs:subClassOf <http://www.w3.org/ns/hydra/core#Resource> ;
  <http://www.w3.org/2003/06/sw-vocab-status/ns#term_status> "testing" .

<http://www.w3.org/ns/hydra/core#BaseUriSource> a <http://www.w3.org/ns/hydra/core#Class> ;
  rdfs:comment "Provides a base abstract for base Uri source for Iri template resolution." ;
  rdfs:isDefinedBy <http://www.w3.org/ns/hydra/core> ;
  rdfs:label "Base Uri source" ;
  rdfs:subClassOf <http://www.w3.org/ns/hydra/core#Resource> ;
  <http://www.w3.org/2003/06/sw-vocab-status/ns#term_status> "testing" .

<http://www.w3.org/ns/hydra/core#BasicRepresentation> a <http://www.w3.org/ns/hydra/core#VariableRepresentation> ;
  rdfs:comment "A representation that serializes just the lexical form of a variable value, but omits language and type information." ;
  rdfs:isDefinedBy <http://www.w3.org/ns/hydra/core> ;
  rdfs:label "BasicRepresentation" ;
  <http://www.w3.org/2003/06/sw-vocab-status/ns#term_status> "testing" .

<http://www.w3.org/ns/hydra/core#Class> a rdfs:Class ;
  a <http://www.w3.org/ns/hydra/core#Resource> ;
  rdfs:comment "The class of Hydra classes." ;
  rdfs:isDefinedBy <http://www.w3.org/ns/hydra/core> ;
  rdfs:label "Hydra Class" ;
  rdfs:subClassOf rdfs:Class ;
  <http://www.w3.org/2003/06/sw-vocab-status/ns#term_status> "testing" .

<http://www.w3.org/ns/hydra/core#Collection> a <http://www.w3.org/ns/hydra/core#Class> ;
  rdfs:comment "A collection holding references to a number of related resources." ;
  rdfs:isDefinedBy <http://www.w3.org/ns/hydra/core> ;
  rdfs:label "Collection" ;
  rdfs:subClassOf <http://www.w3.org/ns/hydra/core#Resource> ;
  <http://www.w3.org/2003/06/sw-vocab-status/ns#term_status> "testing" .

<http://www.w3.org/ns/hydra/core#Error> a <http://www.w3.org/ns/hydra/core#Class> ;
  rdfs:comment "A runtime error, used to report information beyond the returned status code." ;
  rdfs:isDefinedBy <http://www.w3.org/ns/hydra/core> ;
  rdfs:label "Error" ;
  rdfs:subClassOf <http://www.w3.org/ns/hydra/core#Status> ;
  <http://www.w3.org/2003/06/sw-vocab-status/ns#term_status> "testing" .

<http://www.w3.org/ns/hydra/core#ExplicitRepresentation> a <http://www.w3.org/ns/hydra/core#VariableRepresentation> ;
  rdfs:comment "A representation that serializes a variable value including its language and type information and thus differentiating between IRIs and literals." ;
  rdfs:isDefinedBy <http://www.w3.org/ns/hydra/core> ;
  rdfs:label "ExplicitRepresentation" ;
  <http://www.w3.org/2003/06/sw-vocab-status/ns#term_status> "testing" .

<http://www.w3.org/ns/hydra/core#HeaderSpecification> a rdfs:Class ;
  rdfs:comment "Specifies a possible either expected or returned header values" ;
  rdfs:isDefinedBy <http://www.w3.org/ns/hydra/core> ;
  rdfs:label "Header specification" ;
  rdfs:subClassOf <http://www.w3.org/ns/hydra/core#Resource> ;
  <http://www.w3.org/2003/06/sw-vocab-status/ns#term_status> "testing" .

<http://www.w3.org/ns/hydra/core#IriTemplate> a <http://www.w3.org/ns/hydra/core#Class> ;
  rdfs:comment "The class of IRI templates." ;
  rdfs:isDefinedBy <http://www.w3.org/ns/hydra/core> ;
  rdfs:label "IRI Template" ;
  <http://www.w3.org/2003/06/sw-vocab-status/ns#term_status> "testing" .

<http://www.w3.org/ns/hydra/core#IriTemplateMapping> a <http://www.w3.org/ns/hydra/core#Class> ;
  rdfs:comment "A mapping from an IRI template variable to a property." ;
  rdfs:isDefinedBy <http://www.w3.org/ns/hydra/core> ;
  rdfs:label "IriTemplateMapping" ;
  <http://www.w3.org/2003/06/sw-vocab-status/ns#term_status> "testing" .

<http://www.w3.org/ns/hydra/core#Link> a <http://www.w3.org/ns/hydra/core#Class> ;
  rdfs:comment "The class of properties representing links." ;
  rdfs:isDefinedBy <http://www.w3.org/ns/hydra/core> ;
  rdfs:label "Link" ;
  rdfs:subClassOf rdf:Property ;
  rdfs:subClassOf <http://www.w3.org/ns/hydra/core#Resource> ;
  <http://www.w3.org/2003/06/sw-vocab-status/ns#term_status> "testing" .

<http://www.w3.org/ns/hydra/core#LinkContext> a <http://www.w3.org/ns/hydra/core#BaseUriSource> ;
  rdfs:comment "States that the link's context IRI, as defined in RFC 5988, should be used as the base Uri" ;
  rdfs:isDefinedBy <http://www.w3.org/ns/hydra/core> ;
  rdfs:label "Link context" ;
  <http://www.w3.org/2003/06/sw-vocab-status/ns#term_status> "testing" .

<http://www.w3.org/ns/hydra/core#Operation> a <http://www.w3.org/ns/hydra/core#Class> ;
  rdfs:comment "An operation." ;
  rdfs:isDefinedBy <http://www.w3.org/ns/hydra/core> ;
  rdfs:label "Operation" ;
  <http://www.w3.org/2003/06/sw-vocab-status/ns#term_status> "testing" .

<http://www.w3.org/ns/hydra/core#PartialCollectionView> a <http://www.w3.org/ns/hydra/core#Class> ;
  rdfs:comment "A PartialCollectionView describes a partial view of a Collection. Multiple PartialCollectionViews can be connected with the the next/previous properties to allow a client to retrieve all members of the collection." ;
  rdfs:isDefinedBy <http://www.w3.org/ns/hydra/core> ;
  rdfs:label "PartialCollectionView" ;
  rdfs:subClassOf <http://www.w3.org/ns/hydra/core#Resource> ;
  <http://www.w3.org/2003/06/sw-vocab-status/ns#term_status> "testing" .

<http://www.w3.org/ns/hydra/core#Resource> a <http://www.w3.org/ns/hydra/core#Class> ;
  rdfs:comment "The class of dereferenceable resources by means a client can attempt to dereference; however, the received responses should still be verified." ;
  rdfs:isDefinedBy <http://www.w3.org/ns/hydra/core> ;
  rdfs:label "Hydra Resource" ;
  <http://www.w3.org/2003/06/sw-vocab-status/ns#term_status> "testing" .

<http://www.w3.org/ns/hydra/core#Rfc3986> a <http://www.w3.org/ns/hydra/core#BaseUriSource> ;
  rdfs:comment "States that the base Uri should be established using RFC 3986 reference resolution algorithm specified in section 5." ;
  rdfs:isDefinedBy <http://www.w3.org/ns/hydra/core> ;
  rdfs:label "RFC 3986 based" ;
  <http://www.w3.org/2003/06/sw-vocab-status/ns#term_status> "testing" .

<http://www.w3.org/ns/hydra/core#Rfc6570Template> a rdfs:Datatype ;
  rdfs:comment "An IRI template as defined by RFC6570." ;
  rdfs:isDefinedBy <http://www.w3.org/ns/hydra/core> ;
  rdfs:label "RFC6570 IRI template" ;
  rdfs:range xsd:string ;
  rdfs:seeAlso <http://tools.ietf.org/html/rfc6570> ;
  <http://www.w3.org/2003/06/sw-vocab-status/ns#term_status> "testing" .

<http://www.w3.org/ns/hydra/core#Status> a <http://www.w3.org/ns/hydra/core#Class> ;
  rdfs:comment "Additional information about a status code that might be returned." ;
  rdfs:isDefinedBy <http://www.w3.org/ns/hydra/core> ;
  rdfs:label "Status code description" ;
  <http://www.w3.org/2003/06/sw-vocab-status/ns#term_status> "testing" .

<http://www.w3.org/ns/hydra/core#SupportedProperty> a <http://www.w3.org/ns/hydra/core#Class> ;
  rdfs:comment "A property known to be supported by a Hydra class." ;
  rdfs:isDefinedBy <http://www.w3.org/ns/hydra/core> ;
  rdfs:label "Supported Property" ;
  <http://www.w3.org/2003/06/sw-vocab-status/ns#term_status> "testing" .

<http://www.w3.org/ns/hydra/core#TemplatedLink> a <http://www.w3.org/ns/hydra/core#Class> ;
  rdfs:comment "A templated link." ;
  rdfs:isDefinedBy <http://www.w3.org/ns/hydra/core> ;
  rdfs:label "Templated Link" ;
  rdfs:subClassOf rdf:Property ;
  rdfs:subClassOf <http://www.w3.org/ns/hydra/core#Resource> ;
  <http://www.w3.org/2003/06/sw-vocab-status/ns#term_status> "testing" .

<http://www.w3.org/ns/hydra/core#VariableRepresentation> a <http://www.w3.org/ns/hydra/core#Class> ;
  rdfs:comment "A representation specifies how to serialize variable values into strings." ;
  rdfs:isDefinedBy <http://www.w3.org/ns/hydra/core> ;
  rdfs:label "VariableRepresentation" ;
  <http://www.w3.org/2003/06/sw-vocab-status/ns#term_status> "testing" .

<http://www.w3.org/ns/hydra/core#apiDocumentation> a <http://www.w3.org/ns/hydra/core#Link> ;
  rdfs:comment "A link to the API documentation" ;
  rdfs:domain <http://www.w3.org/ns/hydra/core#Resource> ;
  rdfs:isDefinedBy <http://www.w3.org/ns/hydra/core> ;
  rdfs:label "apiDocumentation" ;
  rdfs:range <http://www.w3.org/ns/hydra/core#ApiDocumentation> ;
  <http://www.w3.org/2003/06/sw-vocab-status/ns#term_status> "testing" .

<http://www.w3.org/ns/hydra/core#closedSet> a rdf:Property ;
  rdfs:comment "Determines whether the provided set of header values is closed or not." ;
  rdfs:domain <http://www.w3.org/ns/hydra/core#HeaderSpecification> ;
  rdfs:isDefinedBy <http://www.w3.org/ns/hydra/core> ;
  rdfs:label "closed set" ;
  rdfs:range xsd:boolean ;
  <http://www.w3.org/2003/06/sw-vocab-status/ns#term_status> "testing" .

<http://www.w3.org/ns/hydra/core#collection> a <http://www.w3.org/ns/hydra/core#Link> ;
  rdfs:comment "Collections somehow related to this resource." ;
  rdfs:isDefinedBy <http://www.w3.org/ns/hydra/core> ;
  rdfs:label "collection" ;
  rdfs:range <http://www.w3.org/ns/hydra/core#Collection> ;
  <http://www.w3.org/2003/06/sw-vocab-status/ns#term_status> "testing" .

<http://www.w3.org/ns/hydra/core#description> a rdf:Property ;
  <http://schema.org/domainIncludes> <http://www.w3.org/ns/hydra/core#ApiDocumentation> ;
  <http://schema.org/domainIncludes> <http://www.w3.org/ns/hydra/core#Class> ;
  <http://schema.org/domainIncludes> <http://www.w3.org/ns/hydra/core#Link> ;
  <http://schema.org/domainIncludes> <http://www.w3.org/ns/hydra/core#Operation> ;
  <http://schema.org/domainIncludes> <http://www.w3.org/ns/hydra/core#Status> ;
  <http://schema.org/domainIncludes> <http://www.w3.org/ns/hydra/core#SupportedProperty> ;
  <http://schema.org/domainIncludes> <http://www.w3.org/ns/hydra/core#TemplatedLink> ;
  rdfs:comment "A description." ;
  rdfs:isDefinedBy <http://www.w3.org/ns/hydra/core> ;
  rdfs:label "description" ;
  rdfs:range xsd:string ;
  rdfs:subPropertyOf rdfs:comment ;
  <http://www.w3.org/2003/06/sw-vocab-status/ns#term_status> "testing" .

<http://www.w3.org/ns/hydra/core#entrypoint> a <http://www.w3.org/ns/hydra/core#Link> ;
  rdfs:comment "A link to main entry point of the Web API" ;
  rdfs:domain <http://www.w3.org/ns/hydra/core#ApiDocumentation> ;
  rdfs:isDefinedBy <http://www.w3.org/ns/hydra/core> ;
  rdfs:label "entrypoint" ;
  rdfs:range <http://www.w3.org/ns/hydra/core#Resource> ;
  <http://www.w3.org/2003/06/sw-vocab-status/ns#term_status> "testing" .

<http://www.w3.org/ns/hydra/core#expects> a <http://www.w3.org/ns/hydra/core#Link> ;
  <http://schema.org/rangeIncludes> rdfs:Class ;
  <http://schema.org/rangeIncludes> rdfs:Resource ;
  <http://schema.org/rangeIncludes> <http://www.w3.org/ns/hydra/core#Class> ;
  <http://schema.org/rangeIncludes> <http://www.w3.org/ns/hydra/core#Resource> ;
  rdfs:comment "The information expected by the Web API." ;
  rdfs:domain <http://www.w3.org/ns/hydra/core#Operation> ;
  rdfs:isDefinedBy <http://www.w3.org/ns/hydra/core> ;
  rdfs:label "expects" ;
  <http://www.w3.org/2003/06/sw-vocab-status/ns#term_status> "testing" .

<http://www.w3.org/ns/hydra/core#expectsHeader> a rdf:Property ;
  <http://schema.org/rangeIncludes> xsd:string ;
  <http://schema.org/rangeIncludes> <http://www.w3.org/ns/hydra/core#HeaderSpecification> ;
  rdfs:comment "Specification of the header expected by the operation." ;
  rdfs:domain <http://www.w3.org/ns/hydra/core#Operation> ;
  rdfs:isDefinedBy <http://www.w3.org/ns/hydra/core> ;
  rdfs:label "expects header" ;
  <http://www.w3.org/2003/06/sw-vocab-status/ns#term_status> "testing" .

<http://www.w3.org/ns/hydra/core#extension> a rdf:Property ;
  rdfs:comment "Hint on what kind of extensions are in use." ;
  rdfs:domain <http://www.w3.org/ns/hydra/core#ApiDocumentation> ;
  rdfs:isDefinedBy <http://www.w3.org/ns/hydra/core> ;
  rdfs:label "extension" ;
  <http://www.w3.org/2003/06/sw-vocab-status/ns#term_status> "testing" .

<http://www.w3.org/ns/hydra/core#first> a <http://www.w3.org/ns/hydra/core#Link> ;
  rdfs:comment "The first resource of an interlinked set of resources." ;
  rdfs:domain <http://www.w3.org/ns/hydra/core#Resource> ;
  rdfs:isDefinedBy <http://www.w3.org/ns/hydra/core> ;
  rdfs:label "first" ;
  rdfs:range <http://www.w3.org/ns/hydra/core#Resource> ;
  <http://www.w3.org/2003/06/sw-vocab-status/ns#term_status> "testing" .

<http://www.w3.org/ns/hydra/core#freetextQuery> a rdf:Property ;
  rdfs:comment "A property representing a freetext query." ;
  rdfs:domain <http://www.w3.org/ns/hydra/core#Resource> ;
  rdfs:isDefinedBy <http://www.w3.org/ns/hydra/core> ;
  rdfs:label "freetext query" ;
  rdfs:range xsd:string ;
  <http://www.w3.org/2003/06/sw-vocab-status/ns#term_status> "testing" .

<http://www.w3.org/ns/hydra/core#headerName> a rdf:Property ;
  rdfs:comment "Name of the header." ;
  rdfs:domain <http://www.w3.org/ns/hydra/core#HeaderSpecification> ;
  rdfs:isDefinedBy <http://www.w3.org/ns/hydra/core> ;
  rdfs:label "header name" ;
  rdfs:range xsd:string ;
  <http://www.w3.org/2003/06/sw-vocab-status/ns#term_status> "testing" .

<http://www.w3.org/ns/hydra/core#last> a <http://www.w3.org/ns/hydra/core#Link> ;
  rdfs:comment "The last resource of an interlinked set of resources." ;
  rdfs:domain <http://www.w3.org/ns/hydra/core#Resource> ;
  rdfs:isDefinedBy <http://www.w3.org/ns/hydra/core> ;
  rdfs:label "last" ;
  rdfs:range <http://www.w3.org/ns/hydra/core#Resource> ;
  <http://www.w3.org/2003/06/sw-vocab-status/ns#term_status> "testing" .

<http://www.w3.org/ns/hydra/core#limit> a rdf:Property ;
  rdfs:comment "Instructs to limit set only to N elements." ;
  rdfs:isDefinedBy <http://www.w3.org/ns/hydra/core> ;
  rdfs:label "take" ;
  rdfs:range xsd:nonNegativeInteger ;
  <http://www.w3.org/2003/06/sw-vocab-status/ns#term_status> "testing" .

<http://www.w3.org/ns/hydra/core#manages> rdfs:comment "This predicate is left for compatibility purposes and hydra:memberAssertion should be used instead." ;
  rdfs:isDefinedBy <http://www.w3.org/ns/hydra/core> ;
  rdfs:label "manages" ;
  rdfs:subPropertyOf <http://www.w3.org/ns/hydra/core#memberAssertion> ;
  <http://www.w3.org/2003/06/sw-vocab-status/ns#term_status> "archaic" .

<http://www.w3.org/ns/hydra/core#mapping> a rdf:Property ;
  rdfs:comment "A variable-to-property mapping of the IRI template." ;
  rdfs:domain <http://www.w3.org/ns/hydra/core#IriTemplate> ;
  rdfs:isDefinedBy <http://www.w3.org/ns/hydra/core> ;
  rdfs:label "mapping" ;
  rdfs:range <http://www.w3.org/ns/hydra/core#IriTemplateMapping> ;
  <http://www.w3.org/2003/06/sw-vocab-status/ns#term_status> "testing" .

<http://www.w3.org/ns/hydra/core#member> a <http://www.w3.org/ns/hydra/core#Link> ;
  rdfs:comment "A member of the collection" ;
  rdfs:domain <http://www.w3.org/ns/hydra/core#Collection> ;
  rdfs:isDefinedBy <http://www.w3.org/ns/hydra/core> ;
  rdfs:label "member" ;
  <http://www.w3.org/2003/06/sw-vocab-status/ns#term_status> "testing" .

<http://www.w3.org/ns/hydra/core#memberAssertion> rdfs:comment "Semantics of each member provided by the collection." ;
  rdfs:domain <http://www.w3.org/ns/hydra/core#Collection> ;
  rdfs:isDefinedBy <http://www.w3.org/ns/hydra/core> ;
  rdfs:label "member assertion" ;
  <http://www.w3.org/2003/06/sw-vocab-status/ns#term_status> "testing" .

<http://www.w3.org/ns/hydra/core#method> a rdf:Property ;
  rdfs:comment "The HTTP method." ;
  rdfs:domain <http://www.w3.org/ns/hydra/core#Operation> ;
  rdfs:isDefinedBy <http://www.w3.org/ns/hydra/core> ;
  rdfs:label "method" ;
  rdfs:range xsd:string ;
  <http://www.w3.org/2003/06/sw-vocab-status/ns#term_status> "testing" .

<http://www.w3.org/ns/hydra/core#next> a <http://www.w3.org/ns/hydra/core#Link> ;
  rdfs:comment "The resource following the current instance in an interlinked set of resources." ;
  rdfs:domain <http://www.w3.org/ns/hydra/core#Resource> ;
  rdfs:isDefinedBy <http://www.w3.org/ns/hydra/core> ;
  rdfs:label "next" ;
  rdfs:range <http://www.w3.org/ns/hydra/core#Resource> ;
  <http://www.w3.org/2003/06/sw-vocab-status/ns#term_status> "testing" .

<http://www.w3.org/ns/hydra/core#object> rdfs:comment "The object." ;
  rdfs:isDefinedBy <http://www.w3.org/ns/hydra/core> ;
  rdfs:label "object" ;
  <http://www.w3.org/2003/06/sw-vocab-status/ns#term_status> "testing" .

<http://www.w3.org/ns/hydra/core#offset> a rdf:Property ;
  rdfs:comment "Instructs to skip N elements of the set." ;
  rdfs:isDefinedBy <http://www.w3.org/ns/hydra/core> ;
  rdfs:label "skip" ;
  rdfs:range xsd:nonNegativeInteger ;
  <http://www.w3.org/2003/06/sw-vocab-status/ns#term_status> "testing" .

<http://www.w3.org/ns/hydra/core#operation> a <http://www.w3.org/ns/hydra/core#Link> ;
  rdfs:comment "An operation supported by the Hydra resource" ;
  rdfs:domain <http://www.w3.org/ns/hydra/core#Resource> ;
  rdfs:isDefinedBy <http://www.w3.org/ns/hydra/core> ;
  rdfs:label "operation" ;
  rdfs:range <http://www.w3.org/ns/hydra/core#Operation> ;
  <http://www.w3.org/2003/06/sw-vocab-status/ns#term_status> "testing" .

<http://www.w3.org/ns/hydra/core#pageIndex> a rdf:Property ;
  rdfs:comment "Instructs to provide a specific page of the collection at a given index." ;
  rdfs:isDefinedBy <http://www.w3.org/ns/hydra/core> ;
  rdfs:label "page index" ;
  rdfs:range xsd:nonNegativeInteger ;
  rdfs:subPropertyOf <http://www.w3.org/ns/hydra/core#pageReference> ;
  <http://www.w3.org/2003/06/sw-vocab-status/ns#term_status> "testing" .

<http://www.w3.org/ns/hydra/core#pageReference> a rdf:Property ;
  rdfs:comment "Instructs to provide a specific page reference of the collection." ;
  rdfs:isDefinedBy <http://www.w3.org/ns/hydra/core> ;
  rdfs:label "page reference" ;
  <http://www.w3.org/2003/06/sw-vocab-status/ns#term_status> "testing" .

<http://www.w3.org/ns/hydra/core#possibleStatus> a <http://www.w3.org/ns/hydra/core#Link> ;
  <http://schema.org/domainIncludes> <http://www.w3.org/ns/hydra/core#ApiDocumentation> ;
  <http://schema.org/domainIncludes> <http://www.w3.org/ns/hydra/core#Operation> ;
  rdfs:comment "A status that might be returned by the Web API (other statuses should be expected and properly handled as well)" ;
  rdfs:isDefinedBy <http://www.w3.org/ns/hydra/core> ;
  rdfs:label "possible status" ;
  rdfs:range <http://www.w3.org/ns/hydra/core#Status> ;
  <http://www.w3.org/2003/06/sw-vocab-status/ns#term_status> "testing" .

<http://www.w3.org/ns/hydra/core#possibleValue> a rdf:Property ;
  rdfs:comment "Possible value of the header." ;
  rdfs:domain <http://www.w3.org/ns/hydra/core#HeaderSpecification> ;
  rdfs:isDefinedBy <http://www.w3.org/ns/hydra/core> ;
  rdfs:label "possible header value" ;
  rdfs:range xsd:string ;
  <http://www.w3.org/2003/06/sw-vocab-status/ns#term_status> "testing" .

<http://www.w3.org/ns/hydra/core#previous> a <http://www.w3.org/ns/hydra/core#Link> ;
  rdfs:comment "The resource preceding the current instance in an interlinked set of resources." ;
  rdfs:domain <http://www.w3.org/ns/hydra/core#Resource> ;
  rdfs:isDefinedBy <http://www.w3.org/ns/hydra/core> ;
  rdfs:label "previous" ;
  rdfs:range <http://www.w3.org/ns/hydra/core#Resource> ;
  <http://www.w3.org/2003/06/sw-vocab-status/ns#term_status> "testing" .

<http://www.w3.org/ns/hydra/core#property> a rdf:Property ;
  <http://schema.org/domainIncludes> <http://www.w3.org/ns/hydra/core#IriTemplateMapping> ;
  <http://schema.org/domainIncludes> <http://www.w3.org/ns/hydra/core#SupportedProperty> ;
  rdfs:comment "A property" ;
  rdfs:isDefinedBy <http://www.w3.org/ns/hydra/core> ;
  rdfs:label "property" ;
  rdfs:range rdf:Property ;
  <http://www.w3.org/2003/06/sw-vocab-status/ns#term_status> "testing" .

<http://www.w3.org/ns/hydra/core#readable> a rdf:Property ;
  rdfs:comment "True if the client can retrieve the property's value, false otherwise." ;
  rdfs:domain <http://www.w3.org/ns/hydra/core#SupportedProperty> ;
  rdfs:isDefinedBy <http://www.w3.org/ns/hydra/core> ;
  rdfs:label "readable" ;
  rdfs:range xsd:boolean ;
  <http://www.w3.org/2003/06/sw-vocab-status/ns#term_status> "testing" .

<http://www.w3.org/ns/hydra/core#required> a rdf:Property ;
  <http://schema.org/domainIncludes> <http://www.w3.org/ns/hydra/core#IriTemplateMapping> ;
  <http://schema.org/domainIncludes> <http://www.w3.org/ns/hydra/core#SupportedProperty> ;
  rdfs:comment "True if the property is required, false otherwise." ;
  rdfs:isDefinedBy <http://www.w3.org/ns/hydra/core> ;
  rdfs:label "required" ;
  rdfs:range xsd:boolean ;
  <http://www.w3.org/2003/06/sw-vocab-status/ns#term_status> "testing" .

<http://www.w3.org/ns/hydra/core#resolveRelativeUsing> a rdf:Property ;
  rdfs:domain <http://www.w3.org/ns/hydra/core#IriTemplate> ;
  rdfs:isDefinedBy <http://www.w3.org/ns/hydra/core> ;
  rdfs:label "relative Uri resolution" ;
  rdfs:range <http://www.w3.org/ns/hydra/core#BaseUriSource> ;
  <http://www.w3.org/2003/06/sw-vocab-status/ns#term_status> "testing" .

<http://www.w3.org/ns/hydra/core#returns> a <http://www.w3.org/ns/hydra/core#Link> ;
  <http://schema.org/rangeIncludes> rdfs:Class ;
  <http://schema.org/rangeIncludes> rdfs:Resource ;
  <http://schema.org/rangeIncludes> <http://www.w3.org/ns/hydra/core#Class> ;
  <http://schema.org/rangeIncludes> <http://www.w3.org/ns/hydra/core#Resource> ;
  rdfs:comment "The information returned by the Web API on success" ;
  rdfs:domain <http://www.w3.org/ns/hydra/core#Operation> ;
  rdfs:isDefinedBy <http://www.w3.org/ns/hydra/core> ;
  rdfs:label "returns" ;
  <http://www.w3.org/2003/06/sw-vocab-status/ns#term_status> "testing" .

<http://www.w3.org/ns/hydra/core#returnsHeader> a rdf:Property ;
  <http://schema.org/rangeIncludes> xsd:string ;
  <http://schema.org/rangeIncludes> <http://www.w3.org/ns/hydra/core#HeaderSpecification> ;
  rdfs:comment "Name of the header returned by the operation." ;
  rdfs:domain <http://www.w3.org/ns/hydra/core#Operation> ;
  rdfs:isDefinedBy <http://www.w3.org/ns/hydra/core> ;
  rdfs:label "returns header" ;
  <http://www.w3.org/2003/06/sw-vocab-status/ns#term_status> "testing" .

<http://www.w3.org/ns/hydra/core#search> a <http://www.w3.org/ns/hydra/core#TemplatedLink> ;
  rdfs:comment "A IRI template that can be used to query a collection." ;
  rdfs:domain <http://www.w3.org/ns/hydra/core#Resource> ;
  rdfs:isDefinedBy <http://www.w3.org/ns/hydra/core> ;
  rdfs:label "search" ;
  rdfs:range <http://www.w3.org/ns/hydra/core#IriTemplate> ;
  <http://www.w3.org/2003/06/sw-vocab-status/ns#term_status> "testing" .

<http://www.w3.org/ns/hydra/core#statusCode> a rdf:Property ;
  rdfs:comment "The HTTP status code. Please note it may happen this value will be different to actual status code received." ;
  rdfs:domain <http://www.w3.org/ns/hydra/core#Status> ;
  rdfs:isDefinedBy <http://www.w3.org/ns/hydra/core> ;
  rdfs:label "status code" ;
  rdfs:range xsd:integer ;
  <http://www.w3.org/2003/06/sw-vocab-status/ns#term_status> "testing" .

<http://www.w3.org/ns/hydra/core#subject> rdfs:comment "The subject." ;
  rdfs:isDefinedBy <http://www.w3.org/ns/hydra/core> ;
  rdfs:label "subject" ;
  <http://www.w3.org/2003/06/sw-vocab-status/ns#term_status> "testing" .

<http://www.w3.org/ns/hydra/core#supportedClass> a <http://www.w3.org/ns/hydra/core#Link> ;
  rdfs:comment "A class known to be supported by the Web API" ;
  rdfs:domain <http://www.w3.org/ns/hydra/core#ApiDocumentation> ;
  rdfs:isDefinedBy <http://www.w3.org/ns/hydra/core> ;
  rdfs:label "supported classes" ;
  rdfs:range rdfs:Class ;
  <http://www.w3.org/2003/06/sw-vocab-status/ns#term_status> "testing" .

<http://www.w3.org/ns/hydra/core#supportedOperation> a <http://www.w3.org/ns/hydra/core#Link> ;
  <http://schema.org/domainIncludes> rdfs:Class ;
  <http://schema.org/domainIncludes> <http://www.w3.org/ns/hydra/core#Class> ;
  <http://schema.org/domainIncludes> <http://www.w3.org/ns/hydra/core#Link> ;
  <http://schema.org/domainIncludes> <http://www.w3.org/ns/hydra/core#SupportedProperty> ;
  <http://schema.org/domainIncludes> <http://www.w3.org/ns/hydra/core#TemplatedLink> ;
  rdfs:comment "An operation supported by instances of the specific Hydra class, or the target of the Hydra link, or IRI template." ;
  rdfs:isDefinedBy <http://www.w3.org/ns/hydra/core> ;
  rdfs:label "supported operation" ;
  rdfs:range <http://www.w3.org/ns/hydra/core#Operation> ;
  <http://www.w3.org/2003/06/sw-vocab-status/ns#term_status> "testing" .

<http://www.w3.org/ns/hydra/core#supportedProperty> a <http://www.w3.org/ns/hydra/core#Link> ;
  rdfs:comment "The properties known to be supported by a Hydra class" ;
  rdfs:domain rdfs:Class ;
  rdfs:isDefinedBy <http://www.w3.org/ns/hydra/core> ;
  rdfs:label "supported properties" ;
  rdfs:range <http://www.w3.org/ns/hydra/core#SupportedProperty> ;
  <http://www.w3.org/2003/06/sw-vocab-status/ns#term_status> "testing" .

<http://www.w3.org/ns/hydra/core#template> a rdf:Property ;
  rdfs:comment "A templated string with placeholders. The literal's datatype indicates the template syntax; if not specified, hydra:Rfc6570Template is assumed." ;
  rdfs:domain <http://www.w3.org/ns/hydra/core#IriTemplate> ;
  rdfs:isDefinedBy <http://www.w3.org/ns/hydra/core> ;
  rdfs:label "template" ;
  rdfs:range <http://www.w3.org/ns/hydra/core#Rfc6570Template> ;
  rdfs:seeAlso <http://www.w3.org/ns/hydra/core#Rfc6570Template> ;
  <http://www.w3.org/2003/06/sw-vocab-status/ns#term_status> "testing" .

<http://www.w3.org/ns/hydra/core#title> a rdf:Property ;
  <http://schema.org/domainIncludes> <http://www.w3.org/ns/hydra/core#ApiDocumentation> ;
  <http://schema.org/domainIncludes> <http://www.w3.org/ns/hydra/core#Class> ;
  <http://schema.org/domainIncludes> <http://www.w3.org/ns/hydra/core#Link> ;
  <http://schema.org/domainIncludes> <http://www.w3.org/ns/hydra/core#Operation> ;
  <http://schema.org/domainIncludes> <http://www.w3.org/ns/hydra/core#Status> ;
  <http://schema.org/domainIncludes> <http://www.w3.org/ns/hydra/core#SupportedProperty> ;
  <http://schema.org/domainIncludes> <http://www.w3.org/ns/hydra/core#TemplatedLink> ;
  rdfs:comment "A title, often used along with a description." ;
  rdfs:isDefinedBy <http://www.w3.org/ns/hydra/core> ;
  rdfs:label "title" ;
  rdfs:range xsd:string ;
  rdfs:subPropertyOf rdfs:label ;
  <http://www.w3.org/2003/06/sw-vocab-status/ns#term_status> "testing" .

<http://www.w3.org/ns/hydra/core#totalItems> a rdf:Property ;
  rdfs:comment "The total number of items referenced by a collection." ;
  rdfs:domain <http://www.w3.org/ns/hydra/core#Collection> ;
  rdfs:isDefinedBy <http://www.w3.org/ns/hydra/core> ;
  rdfs:label "total items" ;
  rdfs:range xsd:integer ;
  <http://www.w3.org/2003/06/sw-vocab-status/ns#term_status> "testing" .

<http://www.w3.org/ns/hydra/core#variable> a rdf:Property ;
  rdfs:comment "An IRI template variable" ;
  rdfs:domain <http://www.w3.org/ns/hydra/core#IriTemplateMapping> ;
  rdfs:isDefinedBy <http://www.w3.org/ns/hydra/core> ;
  rdfs:label "variable" ;
  rdfs:range xsd:string ;
  <http://www.w3.org/2003/06/sw-vocab-status/ns#term_status> "testing" .

<http://www.w3.org/ns/hydra/core#variableRepresentation> a rdf:Property ;
  rdfs:comment "The representation format to use when expanding the IRI template." ;
  rdfs:domain <http://www.w3.org/ns/hydra/core#IriTemplateMapping> ;
  rdfs:isDefinedBy <http://www.w3.org/ns/hydra/core> ;
  rdfs:label "variable representation" ;
  rdfs:range <http://www.w3.org/ns/hydra/core#VariableRepresentation> ;
  <http://www.w3.org/2003/06/sw-vocab-status/ns#term_status> "testing" .

<http://www.w3.org/ns/hydra/core#view> a <http://www.w3.org/ns/hydra/core#Link> ;
  rdfs:comment "A specific view of a resource." ;
  rdfs:isDefinedBy <http://www.w3.org/ns/hydra/core> ;
  rdfs:label "view" ;
  <http://www.w3.org/2003/06/sw-vocab-status/ns#term_status> "testing" .

<http://www.w3.org/ns/hydra/core#writable> a rdf:Property ;
  rdfs:comment "True if the client can change the property's value, false otherwise." ;
  rdfs:domain <http://www.w3.org/ns/hydra/core#SupportedProperty> ;
  rdfs:isDefinedBy <http://www.w3.org/ns/hydra/core> ;
  rdfs:label "writable" ;
  rdfs:range xsd:boolean ;
  <http://www.w3.org/2003/06/sw-vocab-status/ns#term_status> "testing" .

<http://www.w3.org/ns/hydra/core#writeable> rdfs:comment "This property is left for compatibility purposes and hydra:writable should be used instead." ;
  rdfs:isDefinedBy <http://www.w3.org/ns/hydra/core> ;
  rdfs:label "writable" ;
  rdfs:subPropertyOf <http://www.w3.org/ns/hydra/core#writable> ;
  <http://www.w3.org/2003/06/sw-vocab-status/ns#term_status> "archaic" .

