@prefix rdf: <http://www.w3.org/1999/02/22-rdf-syntax-ns#> .
@prefix rdfs: <http://www.w3.org/2000/01/rdf-schema#> .
@prefix owl: <http://www.w3.org/2002/07/owl#> .
@prefix xsd: <http://www.w3.org/2001/XMLSchema#> .
@prefix dcterms: <http://purl.org/dc/terms/> .
@prefix foaf: <http://xmlns.com/foaf/0.1/> .
@prefix skos: <http://www.w3.org/2004/02/skos/core#>

<http://www.exemple.com/sin#> a owl:Ontology ;
    rdfs:label "Structured Information Need Ontology"@en ;
    skos:altLabel "SIN-O" ;
    rdfs:comment "This document is an ontology to describe an information need as a structured set of questions that require answers."@en ;
    owl:versionInfo "Second attempt" ;
    dcterms:creator <https://orcid.org/0000-0001-6907-0136> ;
    dcterms:created "2022-25-08"^^xsd:date ;
    dcterms:modified "2022-01-12"^^xsd:date ;
    dcterms:contributor [foaf:name "Sylvie Cazalens"] , [foaf:name "Philippe Lamarre"] ;
    rdfs:seeAlso "https://dekalog.univ-nantes.fr/" .


#################################
#            Classes            #
#################################

# Information Need
:InformationNeed rdf:type rdfs:Class ;
    rdfs:label "Information Need"@en ;
    rdfs:comment "Defines a set of questions that must be answered as well as a structuration of these questions through the use of tags."@en .

# Question
:Question rdf:type rdfs:Class ;
    rdfs:label "Question"@en ;
    rdfs:comment "A sentence in natural language used to find out information."@en .

# Query
:Query rdf:type rdfs:Class ;
    rdfs:label "Query"@en ;
    rdfs:comment "A query expressed in a query language, for instance a SPARQL query."@en .

# Labeling
:Labeling rdf:type rdfs:Class ;
    rdfs:label "Labeling"@en ;
    rdfs:comment "A labeling is an associating between a question and a tag. The question is also given a weight which correspond to its relative importance regarding the tag."@en .

# Tag
:Tag rdf:type rdfs:Class ;
    rdfs:label "Tag"@en ;
    rdfs:comment "Word or sentence used to classify questions."@en .


#################################
#           Properties          #
#################################

# belongs To
:belongsTo rdf:type rdf:Property ;
    rdfs:label "belongs to"@en ;
    rdfs:comment "The tag belongs to an Information Need."@en ;
    rdfs:domain :Tag ;
    rdfs:range :InformationNeed .

# structures
:structures rdf:type rdf:Property ;
    rdfs:label "structures"@en ;
    rdfs:comment "Associate a Labeling to an Information Need in order to structure its questions."@en ;
    rdfs:domain :Labeling ;
    rdfs:range :InformationNeed .

# required By
:requiredBy rdf:type rdf:Property ;
    rdfs:label "required by"@en ;
    rdfs:comment "Associate a question with an Information Need that requires answers to it."@en ;
    rdfs:domain :Question ;
    rdfs:range :InformationNeed .

# tag With
:tagWith rdf:type rdf:Property ;
    rdfs:label "tag with"@en ;
    rdfs:comment "The tag used in the labeling."@en ;
    rdfs:domain :Labeling ;
    rdfs:range :Tag .

# question Tagged
:questionTagged rdf:type rdf:Property ;
    rdfs:label "question tagged"@en ;
    rdfs:comment "The question tagged with the labeling."@en ;
    rdfs:domain :Labeling ;
    rdfs:range :Question .

# is Child Of
:isChildOf rdf:type rdf:Property ;
    rdfs:label "is child of"@en ;
    rdfs:comment "Relation between a tag and another tag in order to provide a hierarchical structure to the tags. Means that the first tag is the child node of the second tag in the hierarchy."@en ;
    rdfs:domain :Tag ;
    rdfs:range :Tag .

# weight
:weight rdf:type rdf:Property ;
    rdfs:label "weight"@en ;
    rdfs:comment "Number representing the relative importance of the element compared to the similar elements. Should be use for a tagging to give the relative importance of the question compared to the questions with the same tag ; and for a tag to give its relative importance compared to its siblings."@en .

###########################
:isFollowedBy rdf:type rdf:Property ;
    rdfs:label "is followed by"@en ;
    rdfs:comment "A query is followed by another query if the the second complement the first one."@en ;
    rdfs:domain :Query ;
    rdfs:range :Query .


#################################
#            Entities           #
#################################

# root
:root rdf:type :Tag ;
    rdfs:label "root of trees"@en ;
    rdfs:comment "The root of all trees of tags."@en ;
    :weight "1"^^xsd:decimal .
    # :isChildOf :root .
