@prefix adms: <http://www.w3.org/ns/adms#> .
@prefix cc: <http://creativecommons.org/ns#> .
@prefix dataid: <http://dataid.dbpedia.org/ns/core#> .
@prefix dcat: <http://www.w3.org/ns/dcat#> .
@prefix dce: <http://purl.org/dc/elements/1.1/> .
@prefix dcmitype: <http://purl.org/dc/dcmitype/> .
@prefix dcterms: <http://purl.org/dc/terms/> .
@prefix doap: <http://usefulinc.com/ns/doap#> .
@prefix dbpo: <http://dbpedia.org/ontology/> .
@prefix dqv: <http://www.w3.org/ns/dqv#> .
@prefix earl: <http://www.w3.org/ns/earl#> .
@prefix fabio: <http://purl.org/spar/fabio/> .
@prefix foaf: <http://xmlns.com/foaf/0.1/> .
@prefix hydra: <http://www.w3.org/ns/hydra/core#> .
@prefix kgi: <http://ns.inria.fr/kg/index#> .
@prefix mf: <http://www.w3.org/2001/sw/DataAccess/tests/test-manifest#> .
@prefix mod: <https://w3id.org/mod#> .
@prefix nie: <http://www.semanticdesktop.org/ontologies/2007/01/19/nie#> .
@prefix owl: <http://www.w3.org/2002/07/owl#> .
@prefix pav: <http://purl.org/pav/> .
@prefix prov: <http://www.w3.org/ns/prov#> .
@prefix rdf: <http://www.w3.org/1999/02/22-rdf-syntax-ns#> .
@prefix rdfs: <http://www.w3.org/2000/01/rdf-schema#> .
@prefix sd: <http://www.w3.org/ns/sparql-service-description#> .
@prefix schema: <http://schema.org/> .
@prefix skos: <http://www.w3.org/2004/02/skos/core#> .
@prefix sparqles: <https://sparqles.ai.wu.ac.at/#> .
@prefix sto: <https://w3id.org/i40/sto#> .
@prefix vann: <http://purl.org/vocab/vann/> .
@prefix voaf: <http://purl.org/vocommons/voaf#>.
@prefix void: <http://rdfs.org/ns/void#> .
@prefix xhv: <http://www.w3.org/1999/xhtml/vocab#> .
@prefix xsd: <http://www.w3.org/2001/XMLSchema#> .

kgi: rdf:type owl:Ontology, voaf:Vocabulary ;
    rdfs:label "IndeGx vocabulary"@en ;
    dcterms:creator "Pierre Maillot", <https://orcid.org/0000-0002-9814-439X> ;
    dcterms:publisher "INRIA, Team WIMMICS", <https://www.inria.fr/fr/wimmics> ;
    dcterms:title  "IndeGx vocabulary"@en ;
    dcterms:description "Vocabulary extending the manifest and EARL vocabularies for the declaration of the IndeGx framework and the content of an index generated by the IndeGx framework"@en ;
    dcterms:date "2021-10" ;
    pav:lastUpdateOn "2023-06-20" ;
    dcterms:format "RDF" ;
    dcterms:identifier kgi: ;
    voaf:extends void: , mf: , earl: ;
    voaf:generalizes mf: , earl: ;
    # owl:imports earl: , mf: , dcat: , void: , sd: 
    .

# Index structuration vocabulary

kgi:IndeGxDataset rdf:type dcat:Dataset, schema:Dataset, void:Dataset, prov:Entity, sd:Dataset ;
    rdfs:label "IndeGx dataset root" ;
    rdfs:isDefinedBy kgi: ;
    rdfs:comment "Root of a dataset generated by IndeGx rules. Default resource used to represent the catalog at the root of the index."@en .

kgi:original rdf:type owl:ObjectProperty ;
    rdfs:label "original"@en ;
    rdfs:comment "Original description graph. Used to link the description of the indexation to the named graph containing the original data directly extracted from an endpoint by IndeGx"@en ;
    rdfs:isDefinedBy kgi: ;
    rdfs:domain prov:Activity ;
    rdfs:range sd:NamedGraph .

kgi:originalResource rdf:type owl:ObjectProperty ;
    rdfs:label "original resource"@en ;
    rdfs:comment "Original description resource. Resource describing a dataset of the endpoint directly extracted from the endpoint."@en ;
    rdfs:isDefinedBy kgi: ;
    rdfs:domain prov:Activity ;
    rdfs:range prov:Entity .

kgi:curated rdf:type owl:ObjectProperty ;
    rdfs:label "curated"@en ;
    rdfs:comment "Generated description graph. Used to link the description of the indexation to the named graph contaning the curated data generated by IndeGx."@en ;
    rdfs:isDefinedBy kgi: ;
    rdfs:domain prov:Activity ;
    rdfs:range sd:NamedGraph .

kgi:curatedResource rdf:type owl:ObjectProperty ;
    rdfs:label "curated resource"@en ;
    rdfs:comment "Generated description resource. Resource generated from the application of generation assets by IndeGx but not directly extracted from an endpoint."@en ;
    rdfs:isDefinedBy kgi: ;
    rdfs:domain prov:Activity ;
    rdfs:range prov:Entity .

kgi:summary rdf:type owl:ObjectProperty ;
    rdfs:label "summary"@en ;
    rdf:comment "Link between the indexation activity of an endpoint and the graph containing the summary of its content."@en ;
    rdfs:domain void:Dataset ;
    rdfs:range sd:NamedGraph .

kgi:trace rdf:type owl:ObjectProperty ;
    rdfs:label "trace"@en ;
    rdfs:comment "Trace report of the metadata generation. EARL report resulting in the execution of a query during the generation of the metadata."@en ;
    rdfs:isDefinedBy kgi: ;
    rdfs:domain prov:Entity ;
    rdfs:range earl:Assertion .

# Generation assets structuration vocabulary

kgi:endpoint rdf:type owl:ObjectProperty ;
    rdfs:label "endpoint"@en ;
    rdfs:comment "Indicates the endpoint to send a test or action."@en ;
    rdfs:domain [ owl:unionOf ( kgi:TestQuery kgi:Action ) ] ;
    rdfs:isDefinedBy kgi: .

kgi:TestQuery rdf:type rdfs:Class ;
    rdfs:label "Query test"@en ;
    rdfs:comment "Test based on a SPARQL query execution. Test the result of the execution of rdf:type query in the manner of rdf:type SHACL shape but allows declaration of constraints on the HTTP response and the result."@en ;
    rdfs:isDefinedBy kgi: ;
    rdfs:subClassOf earl:TestCase .

kgi:onSuccess rdf:type owl:ObjectProperty ;
    rdfs:label "on success"@en ;
    rdfs:comment "List of actions triggered by the success of the test present at the URI of the entry."@en ;
    rdfs:isDefinedBy kgi: ;
    rdfs:domain mf:ManifestEntry ;
    rdfs:range rdf:List .

kgi:onFailure rdf:type owl:ObjectProperty ;
    rdfs:label "on failure"@en ;
    rdfs:comment "List of actions triggered by the failure of the test present at the URI of the entry."@en ;
    rdfs:isDefinedBy kgi: ;
    rdfs:domain mf:ManifestEntry ;
    rdfs:range rdf:List .

kgi:DummyTest rdf:type rdfs:Class ;
    rdfs:label "Placeholder test"@en ;
    rdfs:isDefinedBy kgi: ;
    rdfs:comment "Placeholder class for the test of a rule only affecting the index data. Some tests and actions are 'meta' rules that do not need interaction with remote endpoints. This class is for a test that always succeed for these rules."@en ;
    rdfs:subClassOf earl:TestCase .

kgi:GenerationAsset rdf:type rdfs:Class ;
    rdfs:label "Generation asset."@en ;
    rdfs:isDefinedBy kgi: ;
    rdfs:comment "A generation asset is a test or an action that can be applied by IndeGx to a dataset to generate its description."@en .

kgi:requiredAssets rdf:type owl:ObjectProperty ;
    rdfs:label "required assets"@en ;
    rdfs:comment "Generation assets that must be applied for this generation asset to be applied."@en ;
    rdfs:isDefinedBy kgi: ;
    rdfs:domain kgi:GenerationAsset ;
    rdfs:range rdf:List .

kgi:Action rdf:type owl:Class ;
    rdfs:subClassOf kgi:GenerationAsset ;
    rdfs:label "Action"@en ;
    rdfs:comment "Action object. Must be linked with the property kgi:action to a SPARQL query"@en .

# Modifying existing vocabularies

earl:TestCase rdfs:subClassOf kgi:GenerationAsset .

mf:ManifestEntry rdfs:subClassOf kgi:GenerationAsset .

mf:Manifest rdfs:subClassOf kgi:GenerationAsset .

mf:action rdfs:domain kgi:Action .

# properties to set up the parameters of the indexation

kgi:timeout rdf:type owl:DatatypeProperty ;
    rdfs:label "timeout"@en ;
    rdfs:isDefinedBy kgi: ;
    rdfs:comment "Specify a timeout for a test or action. Queries sent during test and actions may need a specific timeout, generally longer than normal. This property specify the timeout for a test or an action."@en ;
    rdfs:domain kgi:Action ;
    rdfs:range xsd:duration .

kgi:recommendedPagination rdf:type owl:DatatypeProperty ;
    rdfs:label "recommended pagination"@en ;
    rdfs:comment "Recommended size for pagination during retrieval of the results of an action. This indicates the size of the page to use in the actions queries."@en ;
    rdfs:isDefinedBy kgi: ;
    rdfs:domain kgi:Action ;
    rdfs:range xsd:integer .

# Trace of indexation

kgi:sentQuery rdf:type owl:DatatypeProperty ;
    rdfs:comment "Query sent to the server. String representation of the SPARQL query sent to the server after transformation to adapt it to the endpoint, if necessary."@en ;
    rdfs:label "query sent"@en ;
    rdfs:domain earl:TestResult ;
    rdfs:range xsd:string .

# Pseudo-partitions and linksets

kgi:linkset rdf:type owl:ObjectProperty ;
    rdfs:label "linkset"@en ;
    rdfs:comment "Link a dataset description to the linkset that were retrieved during its indexation"@en ;
    rdfs:isDefinedBy kgi: ;
    rdfs:domain void:Dataset ;
    rdfs:range void:Linkset .

kgi:resourceHostname rdf:type owl:ObjectProperty ;
    rdfs:label "resource hostname"@en ;
    rdfs:comment "Hostname of the resources of the dataset. Linked to URIs representing the hostnames of the resources of the dataset."@en ;
    rdfs:isDefinedBy kgi: ;
    rdfs:domain void:Dataset .

kgi:hostnamePartition rdf:type owl:ObjectProperty ;
    rdfs:label "hostname partition"@en ;
    rdfs:comment "Partition of the dataset according to the hostname used the URIs of instances. This property is to be used on the same model as void:classPartition and void:propertyPartition."@en ;
    rdfs:subPropertyOf void:subset ;
    rdfs:isDefinedBy kgi: ;
    rdfs:domain void:Dataset .

kgi:vocabularyPartition rdf:type owl:ObjectProperty ;
    rdfs:label "vocabulary partition"@en ;
    rdfs:comment "Partition of the dataset according to the vocabulary used in triples. This property is to be used on the same model as void:classPartition and void:propertyPartition."@en ;
    rdfs:subPropertyOf void:subset ;
    rdfs:isDefinedBy kgi: ;
    rdfs:domain void:Dataset .

# Other dataset description properties

kgi:availableLiteralDatatypes rdf:type owl:ObjectProperty ;
    rdfs:label "available literal datatypes"@en ;
    rdfs:comment "Used to describe the datatype of the literals in the dataset."@en ;
    rdfs:isDefinedBy kgi: ;
    rdfs:domain void:Dataset ;
    rdfs:range xsd:string .

kgi:resourceHostname rdf:type owl:ObjectProperty ;
    rdfs:label "resource hostname"@en ;
    rdfs:comment "Used to describe the hostname of the resources of the dataset."@en ;
    rdfs:domain void:Dataset ;
    rdfs:isDefinedBy kgi: .

kgi:summary rdf:type owl:ObjectProperty ;
    rdfs:label "summary"@en ;
    rdfs:comment "Link between a dataset and a summary of its content."@en ;
    rdfs:domain void:Dataset ;
    rdfs:range sd:NamedGraph .

kgi:graph rdf:type owl:ObjectProperty ;
    rdfs:label "graph"@en ;
    rdfs:comment "Link between a dataset and a graph containing its content."@en ;
    rdfs:domain void:Dataset ;
    rdfs:range sd:NamedGraph .

kgi:endpointURLextension rdf:type owl:DatatypeProperty ;
    rdfs:label "Domain extension of the endpoint's URL"
    rdfs:domain dcat:DataService , sd:Service ;
    rdfs:range xsd:string .

# Description of the common elements between datasets

kgi:CommonalityDescription rdf:type rdfs:Class ;
    rdfs:label "Commonality description"@en;
    rdfs:comment "Description of the common elements between datasets. This is designed to give the elements that are common between the descriptions of groups of datasets"@en;
    rdfs:isDefinedBy kgi: .

kgi:dataset rdf:type owl:ObjectProperty ;
    rdfs:label "dataset"@en ;
    rdf:comment "Indicates the datasets whose commonalities are described by an instance of CommonalityDescription."@en ;
    rdfs:domain kgi:CommonalityDescription ;
    rdfs:range void:Dataset ;
    rdfs:isDefinedBy kgi: .

kgi:VocabularyCommonalityDescription rdf:subClassOf kgi:CommonalityDescription ;
    rdfs:label "Common vocabularies"@en ;
    rdfs:comment "Description of the common vocabularies used in different datasets. This shoud be used with kgi:vocabulary and kgi:dataset to list the vocabularies common to a group of datasets"@en ;
    rdfs:isDefinedBy kgi: .

kgi:ClassCommonalityDescription rdf:subClassOf kgi:CommonalityDescription ;
    rdfs:label "Common classes"@en ;
    rdfs:comment "Description of the common classes used in different datasets. This shoud be used with kgi:class and kgi:dataset to list the classes common to a group of datasets"@en ;
    rdfs:isDefinedBy kgi: .

kgi:PropertyCommonalityDescription rdf:subClassOf kgi:CommonalityDescription ;
    rdfs:label "Common properties"@en ;
    rdfs:comment "Description of the common properties used in different datasets. This shoud be used with kgi:property and kgi:dataset to list the properties common to a group of datasets"@en ;
    rdfs:isDefinedBy kgi: .

kgi:DatatypeCommonalityDescription rdf:subClassOf kgi:CommonalityDescription ;
    rdfs:label "Common datatypes"@en ;
    rdfs:comment "Description of the common datatypes used in different datasets. This shoud be used with kgi:datatype and kgi:dataset to list the datatypes common to a group of datasets"@en ;
    rdfs:isDefinedBy kgi: .

kgi:ResourceHostnameCommonalityDescription rdf:subClassOf kgi:CommonalityDescription ;
    rdfs:label "common resource hostnames"@en ;
    rdfs:comment "Description of the common resources hostnames used in different datasets. This shoud be used with kgi:hostname and kgi:dataset to list the resources hostnames common to a group of datasets"@en ;
    rdfs:isDefinedBy kgi: .

kgi:commonVocabularyDescription rdf:type owl:ObjectProperty ;
    rdfs:label "common vocabularies"@en ;
    rdfs:comment "Links a dataset to its vocabulary commonalities descriptions."@en ;
    rdfs:domain void:Dataset ;
    rdfs:range kgi:VocabularyCommonalityDescription ;
    rdfs:isDefinedBy kgi: .

kgi:vocabulary rdf:type owl:ObjectProperty ;
    rdfs:label "vocabulary"@en ;
    rdfs:comment "Indicates the vocabularies that are common to a group of datasets in an instance of CommonalityDescription."@en ;
    rdfs:domain kgi:VocabularyCommonalityDescription ;
    rdfs:isDefinedBy kgi: .

kgi:commonClassDescription rdf:type owl:ObjectProperty ;
    rdfs:label "common classes"@en ;
    rdfs:comment "Links a dataset to its class commonalities descriptions."@en ;
    rdfs:domain void:Dataset ;
    rdfs:range kgi:ClassCommonalityDescription ;
    rdfs:isDefinedBy kgi: .

kgi:class rdf:type owl:ObjectProperty ;
    rdfs:label "class"@en ;
    rdfs:comment "Indicates the classes that are common to a group of datasets in an instance of CommonalityDescription."@en ;
    rdfs:domain kgi:ClassCommonalityDescription ;
    rdfs:isDefinedBy kgi: .

kgi:commonPropertyDescription rdf:type owl:ObjectProperty ;
    rdfs:label "common properties"@en ;
    rdfs:comment "Links a dataset to its property commonalities descriptions."@en ;
    rdfs:domain void:Dataset ;
    rdfs:range kgi:PropertyCommonalityDescription ;
    rdfs:isDefinedBy kgi: .

kgi:property rdf:type owl:ObjectProperty ;
    rdfs:label "property"@en ;
    rdfs:comment "Indicates the properties that are common to a group of datasets in an instance of CommonalityDescription."@en ;
    rdfs:domain kgi:PropertyCommonalityDescription ;
    rdfs:isDefinedBy kgi: .

kgi:commonDatatypeDescription rdf:type owl:ObjectProperty ;
    rdfs:label "common datatypes"@en ;
    rdfs:comment "Links a dataset to its datatype commonalities descriptions."@en ;
    rdfs:domain void:Dataset ;
    rdfs:range kgi:DatatypeCommonalityDescription ;
    rdfs:isDefinedBy kgi: .

kgi:datatype rdf:type owl:ObjectProperty ;
    rdfs:label "datatype"@en ;
    rdfs:comment "Indicates the datatypes that are common to a group of datasets in an instance of CommonalityDescription."@en ;
    rdfs:domain kgi:DatatypeCommonalityDescription ;
    rdfs:isDefinedBy kgi: .

kgi:commonHostnameDescription rdf:type owl:ObjectProperty ;
    rdfs:label "common resource hostnames"@en ;
    rdfs:comment "Links a dataset to its hostname commonalities descriptions."@en ;
    rdfs:domain void:Dataset ;
    rdfs:range kgi:ResourceHostnameCommonalityDescription ;
    rdfs:isDefinedBy kgi: .

kgi:hostname rdf:type owl:ObjectProperty ;
    rdfs:label "resource hostname"@en ;
    rdfs:comment "Indicates the resource hostnames that are common to a group of datasets in an instance of CommonalityDescription."@en ;
    rdfs:comment "To not be confused with kgi:resourceHostname, which lists the resource hostnames appearing in a dataset."@en ;
    rdfs:domain kgi:ResourceHostnameCommonalityDescription ;
    rdfs:isDefinedBy kgi: .

# Annotations

kgi:passed rdf:type owl:AnnotationProperty ;
    rdfs:subPropertyOf kgi:tested ;
    rdfs:label "passed"@en ;
    rdfs:comment "Annotation to indicate the success of a test or action."@en ;
    rdfs:isDefinedBy kgi: ;
    rdfs:range earl:ManifestEntry , earl:TestCase .

kgi:failed rdf:type owl:AnnotationProperty ;
    rdfs:subPropertyOf kgi:tested ;
    rdfs:label "failed"@en ;
    rdfs:comment "Annotation to indicate the failure of a test or action."@en ;
    rdfs:isDefinedBy kgi: ;
    rdfs:range earl:ManifestEntry , earl:TestCase .

kgi:tested rdf:type owl:AnnotationProperty ;
    rdfs:label "tested"@en ;
    rdfs:comment "Annotation to indicate that a test or action has been executed."@en ;
    rdfs:isDefinedBy kgi: ;
    rdfs:range earl:ManifestEntry , earl:TestCase ;
    owl:propertyChainAxiom ( kgi:subjectOfAssertion earl:test ) .

kgi:subjectOfAssertion rdf:type owl:AnnotationProperty ;
    rdfs:label "subject of assertion"@en ;
    rdfs:comment "Annotation to indicate the subject of an assertion."@en ;
    rdfs:isDefinedBy kgi: ;
    rdfs:range earl:Assertion ;
    rdfs:domain earl:TestSubject ;
    owl:inverseOf earl:subject .

## Availability of an endpoint

kgi:AvailableEndpoint rdf:type owl:Class ;
    rdfs:label "Available endpoint"@en ;
    rdfs:comment "Annotation to indicate the availability of an endpoint at the moment of the last indexing."@en ;
    rdfs:isDefinedBy kgi: ;
    rdfs:subClassOf dcat:DataService , sd:Service ;
    owl:equivalentClass [
        rdf:type owl:Restriction ;
        owl:onProperty kgi:subjectOfAssertion ;
        owl:allValuesFrom [
            rdf:type owl:Class ;
            owl:intersectionOf ( 
                [
                    rdf:type owl:Restriction ;
                    owl:onProperty earl:result ;
                    owl:someValuesFrom [
                        rdf:type owl:Restriction ;
                        owl:onProperty earl:outcome ;
                        owl:hasValue earl:passed
                    ]
                ]
                [
                    rdf:type owl:Restriction ;
                    owl:onProperty earl:test ;
                    owl:hasValue <https://raw.githubusercontent.com/Wimmics/IndeGx/intentionDeclaration/rules/intension/main/online.ttl>
                ]
            )
        ]
    ] ,
    [ 
        rdf:type owl:Restriction ;
        owl:onProperty kgi:passed ;
        owl:hasValue <https://raw.githubusercontent.com/Wimmics/IndeGx/intentionDeclaration/rules/intension/main/online.ttl>
    ] .

kgi:UnavailableEndpoint rdf:type owl:Class ;
    rdfs:subClassOf dcat:DataService ;
    rdfs:comment "Annotation to indicate the unavailability of an endpoint."@en ;
    rdfs:isDefinedBy kgi: ;
    rdfs:label "Unavailable endpoint"@en ;
    owl:equivalentClass [
        rdf:type owl:Restriction ;
        owl:onProperty kgi:subjectOfAssertion ;
        owl:allValuesFrom [
            rdf:type owl:Class ;
            owl:intersectionOf ( 
                [
                    rdf:type owl:Restriction ;
                    owl:onProperty earl:result ;
                    owl:someValuesFrom [
                        rdf:type owl:Restriction ;
                        owl:onProperty earl:outcome ;
                        owl:hasValue earl:failed
                    ]
                ]
                [
                    rdf:type owl:Restriction ;
                    owl:onProperty earl:test ;
                    owl:hasValue <https://raw.githubusercontent.com/Wimmics/IndeGx/intentionDeclaration/rules/intension/main/online.ttl>
                ]
            )
        ]
    ] ,
    [ 
        rdf:type owl:Restriction ;
        owl:onProperty kgi:failed ;
        owl:hasValue <https://raw.githubusercontent.com/Wimmics/IndeGx/intentionDeclaration/rules/intension/main/online.ttl>
    ] .


# Capacities of the endpoint

kgi:SPARQL10Compliant rdf:type owl:Class ;
    rdfs:label "SPARQL 1.0 compliant endpoint"@en ;
    rdfs:comment "Annotation to indicate that an endpoint is compliant with SPARQL 1.0."@en ;
    rdfs:isDefinedBy kgi: ;
    rdfs:subClassOf sd:Service , dcat:DataService ;
    owl:equivalentClass [
        rdf:type owl:Restriction ;
        owl:onProperty sd:feature ;
        owl:hasValue sd:SPARQL10Query
    ] ,
    [
        rdf:type owl:Class ;
        owl:intersectionOf (
            [
                rdf:type owl:Restriction ;
                owl:onProperty sd:feature ;
                owl:hasValue sparqles:ASK
            ]
            [
                rdf:type owl:Restriction ;
                owl:onProperty sd:feature ;
                owl:hasValue sparqles:CON
            ]
            [
                rdf:type owl:Restriction ;
                owl:onProperty sd:feature ;
                owl:hasValue sparqles:CONJOIN
            ]
            [
                rdf:type owl:Restriction ;
                owl:onProperty sd:feature ;
                owl:hasValue sparqles:CONOPT
            ]
            [
                rdf:type owl:Restriction ;
                owl:onProperty sd:feature ;
                owl:hasValue sparqles:SEL-DISTINCT
            ]
            [
                rdf:type owl:Restriction ;
                owl:onProperty sd:feature ;
                owl:hasValue sparqles:SEL-REDUCED
            ]
            [
                rdf:type owl:Restriction ;
                owl:onProperty sd:feature ;
                owl:hasValue sparqles:SEL
            ]
            [
                rdf:type owl:Restriction ;
                owl:onProperty sd:feature ;
                owl:hasValue sparqles:SELBNODE
            ]
            [
                rdf:type owl:Restriction ;
                owl:onProperty sd:feature ;
                owl:hasValue sparqles:SELEMPTY
            ]
            [
                rdf:type owl:Restriction ;
                owl:onProperty sd:feature ;
                owl:hasValue sparqles:SELFILBLANK
            ]
            [
                rdf:type owl:Restriction ;
                owl:onProperty sd:feature ;
                owl:hasValue sparqles:SELFILBOOL
            ]
            [
                rdf:type owl:Restriction ;
                owl:onProperty sd:feature ;
                owl:hasValue sparqles:SELFILIRI
            ]
            [
                rdf:type owl:Restriction ;
                owl:onProperty sd:feature ;
                owl:hasValue sparqles:SELFILNOTBOUND
            ]
            [
                rdf:type owl:Restriction ;
                owl:onProperty sd:feature ;
                owl:hasValue sparqles:SELFILNUM
            ]
            [
                rdf:type owl:Restriction ;
                owl:onProperty sd:feature ;
                owl:hasValue sparqles:SELFILREGEX-i
            ]
            [
                rdf:type owl:Restriction ;
                owl:onProperty sd:feature ;
                owl:hasValue sparqles:SELFILREGEX
            ]
            [
                rdf:type owl:Restriction ;
                owl:onProperty sd:feature ;
                owl:hasValue sparqles:SELFILSTR
            ]
            [
                rdf:type owl:Restriction ;
                owl:onProperty sd:feature ;
                owl:hasValue sparqles:SELFROM
            ]
            [
                rdf:type owl:Restriction ;
                owl:onProperty sd:feature ;
                owl:hasValue sparqles:SELGRAPH
            ]
            [
                rdf:type owl:Restriction ;
                owl:onProperty sd:feature ;
                owl:hasValue sparqles:SELGRAPHJOIN
            ]
            [
                rdf:type owl:Restriction ;
                owl:onProperty sd:feature ;
                owl:hasValue sparqles:SELGRAPHUNION
            ]
            [
                rdf:type owl:Restriction ;
                owl:onProperty sd:feature ;
                owl:hasValue sparqles:SELJOIN
            ]
            [
                rdf:type owl:Restriction ;
                owl:onProperty sd:feature ;
                owl:hasValue sparqles:SELOPT
            ]
            [
                rdf:type owl:Restriction ;
                owl:onProperty sd:feature ;
                owl:hasValue sparqles:SELUNION 
            ]
        )
    ] .

kgi:SPARQL11Compliant rdf:type owl:Class ;
    rdfs:label "SPARQL 1.1 compliant endpoint"@en ;
    rdfs:comment "Annotation to indicate that an endpoint is compliant with SPARQL 1.1."@en ;
    rdfs:isDefinedBy kgi: ;
    rdfs:subClassOf sd:Service , dcat:DataService ;
    owl:equivalentClass [
        rdf:type owl:Restriction ;
        owl:onProperty sd:feature ;
        owl:hasValue sd:SPARQL11Query
    ] ,
    [
        rdf:type owl:Class ;
        owl:intersectionOf (
            [
                rdf:type owl:Restriction ;
                owl:onProperty sd:feature ;
                owl:hasValue sparqles:ASKFILNOTIN
            ]
            [
                rdf:type owl:Restriction ;
                owl:onProperty sd:feature ;
                owl:hasValue sparqles:SELAVG
            ]
            [
                rdf:type owl:Restriction ;
                owl:onProperty sd:feature ;
                owl:hasValue sparqles:SELBIND
            ]
            [
                rdf:type owl:Restriction ;
                owl:onProperty sd:feature ;
                owl:hasValue sparqles:SELFILNOTEXISTS
            ]
            [
                rdf:type owl:Restriction ;
                owl:onProperty sd:feature ;
                owl:hasValue sparqles:SELFILABS
            ]
            [
                rdf:type owl:Restriction ;
                owl:onProperty sd:feature ;
                owl:hasValue sparqles:SELFILCONTAINS
            ]
            [
                rdf:type owl:Restriction ;
                owl:onProperty sd:feature ;
                owl:hasValue sparqles:SELFILNOTEXISTS
            ]
            [
                rdf:type owl:Restriction ;
                owl:onProperty sd:feature ;
                owl:hasValue sparqles:SELFILSTART
            ]
            [
                rdf:type owl:Restriction ;
                owl:onProperty sd:feature ;
                owl:hasValue sparqles:SELMAX
            ]
            [
                rdf:type owl:Restriction ;
                owl:onProperty sd:feature ;
                owl:hasValue sparqles:SELMIN
            ]
            [
                rdf:type owl:Restriction ;
                owl:onProperty sd:feature ;
                owl:hasValue sparqles:SELCOUNT
            ]
            [
                rdf:type owl:Restriction ;
                owl:onProperty sd:feature ;
                owl:hasValue sparqles:SELMINUS
            ]
            [
                rdf:type owl:Restriction ;
                owl:onProperty sd:feature ;
                owl:hasValue sparqles:SELPATHS
            ]
            [
                rdf:type owl:Restriction ;
                owl:onProperty sd:feature ;
                owl:hasValue sparqles:SELSERVICE
            ]
            [
                rdf:type owl:Restriction ;
                owl:onProperty sd:feature ;
                owl:hasValue sparqles:SELSUBQGRAPH
            ]
            [
                rdf:type owl:Restriction ;
                owl:onProperty sd:feature ;
                owl:hasValue sparqles:SELSUBQ
            ]
            [
                rdf:type owl:Restriction ;
                owl:onProperty sd:feature ;
                owl:hasValue sparqles:SELSUM
            ]
            [
                rdf:type owl:Restriction ;
                owl:onProperty sd:feature ;
                owl:hasValue sparqles:SELVALUES 
            ]
        )
    ] .

kgi:SPARQL11QueryWithoutFederation rdf:type owl:Class ;
    rdfs:label "SPARQL 1.1 compliant endpoint without federation"@en ;
    rdfs:comment "Annotation to indicate that an endpoint is compliant with SPARQL 1.1 without the federation features."@en ;
    rdfs:isDefinedBy kgi: ;
    rdfs:subClassOf sd:Service , dcat:DataService ;
    owl:equivalentClass [
        rdf:type owl:Class ;
        owl:intersectionOf (
            [
                rdf:type owl:Restriction ;
                owl:onProperty sd:feature ;
                owl:hasValue sparqles:ASKFILNOTIN
            ]
            [
                rdf:type owl:Restriction ;
                owl:onProperty sd:feature ;
                owl:hasValue sparqles:SELAVG
            ]
            [
                rdf:type owl:Restriction ;
                owl:onProperty sd:feature ;
                owl:hasValue sparqles:SELBIND
            ]
            [
                rdf:type owl:Restriction ;
                owl:onProperty sd:feature ;
                owl:hasValue sparqles:SELFILNOTEXISTS
            ]
            [
                rdf:type owl:Restriction ;
                owl:onProperty sd:feature ;
                owl:hasValue sparqles:SELFILABS
            ]
            [
                rdf:type owl:Restriction ;
                owl:onProperty sd:feature ;
                owl:hasValue sparqles:SELFILCONTAINS
            ]
            [
                rdf:type owl:Restriction ;
                owl:onProperty sd:feature ;
                owl:hasValue sparqles:SELFILNOTEXISTS
            ]
            [
                rdf:type owl:Restriction ;
                owl:onProperty sd:feature ;
                owl:hasValue sparqles:SELFILSTART
            ]
            [
                rdf:type owl:Restriction ;
                owl:onProperty sd:feature ;
                owl:hasValue sparqles:SELMAX
            ]
            [
                rdf:type owl:Restriction ;
                owl:onProperty sd:feature ;
                owl:hasValue sparqles:SELMIN
            ]
            [
                rdf:type owl:Restriction ;
                owl:onProperty sd:feature ;
                owl:hasValue sparqles:SELCOUNT
            ]
            [
                rdf:type owl:Restriction ;
                owl:onProperty sd:feature ;
                owl:hasValue sparqles:SELMINUS
            ]
            [
                rdf:type owl:Restriction ;
                owl:onProperty sd:feature ;
                owl:hasValue sparqles:SELPATHS
            ]
            [
                rdf:type owl:Restriction ;
                owl:onProperty sd:feature ;
                owl:hasValue sparqles:SELSUBQGRAPH
            ]
            [
                rdf:type owl:Restriction ;
                owl:onProperty sd:feature ;
                owl:hasValue sparqles:SELSUBQ
            ]
            [
                rdf:type owl:Restriction ;
                owl:onProperty sd:feature ;
                owl:hasValue sparqles:SELSUM
            ]
            [
                rdf:type owl:Restriction ;
                owl:onProperty sd:feature ;
                owl:hasValue sparqles:SELVALUES 
            ]
        )
    ] .

## Equivalences

dcat:Dataset owl:equivalentClass schema:Dataset ,
    dcmitype:Dataset ,
    void:Dataset ,        
    sd:Dataset .

dcterms:creator owl:equivalentProperty schema:creator ,
    schema:author ,
    foaf:maker ,
    dce:creator ,
    pav:authoredBy ,
    pav:createdBy .

dcterms:contributor owl:equivalentProperty schema:editor ,
    schema:contributor ,
    dce:contributor ,
    pav:contributedBy .

dcterms:issued owl:equivalentProperty dcterms:available ,
    schema:datePublished ,
    schema:sdDatePublished ,
    pav:authoredOn ,
    pav:createdOn  .

dcterms:publisher owl:equivalentProperty dce:publisher ,
    schema:publisher ,
    schema:sdPublisher ,
    pav:providedBy .

dcterms:created owl:equivalentProperty schema:dateCreated ,
    pav:createdOn ,
    prov:generatedAtTime .

schema:locationCreated owl:equivalentProperty pav:createdAt .

pav:createdWith owl:equivalentProperty pav:retrievedBy ,
    pav:importedBy  .

dcterms:modified owl:equivalentProperty schema:dateModified ,
    pav:lastUpdateOn ,
    pav:contributedOn .

prov:invalidatedAtTime owl:equivalentProperty schema:expires .

dcterms:valid owl:equivalentProperty schema:expires .

void:vocabulary owl:equivalentProperty dcterms:conformsTo .

dcterms:subject owl:equivalentProperty dcat:theme ,
    schema:about ,
    foaf:topic ,
    foaf:primaryTopic ,
    skos:subject .

dcat:keyword owl:equivalentProperty schema:keywords .

foaf:depiction owl:equivalentProperty schema:image .

dcat:endpointURL owl:equivalentProperty sd:endpoint .

dcat:distribution owl:equivalentProperty schema:distribution .

dcterms:format owl:equivalentProperty dce:format ,
    schema:encodingFormat .

dcat:version owl:equivalentProperty pav:version ,
    dcterms:hasVersion ,
    pav:hasCurrentVersion ,
    schema:version .

adms:versionNotes owl:equivalentProperty owl:versionInfo .

dcterms:isVersionOf owl:equivalentProperty pav:previousVersion ,
    owl:priorVersion .

dcterms:language owl:equivalentProperty dce:language ,
    schema:inLanguage .

dcterms:identifier owl:equivalentProperty schema:identifier ,
    dce:identifier ,
    dcterms:identifier ,
    adms:identifier .

schema:termCode owl:equivalentProperty <http://qudt.org/schema/qudt/acronym> .

dcat:landingPage owl:equivalentProperty foaf:homepage ,
    schema:url .


rdfs:seeAlso owl:equivalentProperty schema:relatedLink ,
    rdfs:seeAlso .

dcterms:references owl:equivalentProperty schema:publication .

void:exampleResource owl:equivalentProperty schema:workExample ,
    skos:example .

dcterms:license owl:equivalentProperty schema:license ,
    doap:license ,
    dbpo:license ,
    cc:license ,
    xhv:license ,
    sto:license ,
    nie:license .

dqv:hasQualityAnnotation owl:equivalentProperty schema:review .

dcterms:rights owl:equivalentProperty dcterms:accessRights ,
    dce:rights .

dcterms:source owl:equivalentProperty schema:isBasedOn ,
    dcterms:source ,
    dce:source ,
    dcterms:provenance ,
    prov:hadPrimarySource ,
    prov:wasDerivedFrom ,
    pav:derivedFrom ,
    pav:importedFrom ,
    pav:retrievedFrom .

dcterms:spatial owl:equivalentProperty schema:spatialCoverage .

dcterms:temporal owl:equivalentProperty schema:temporalCoverage .

# FAIR
## FAIR-Checker