@prefix adms: <http://www.w3.org/ns/adms#> .
@prefix cc: <http://creativecommons.org/ns#> .
@prefix dataid: <http://dataid.dbpedia.org/ns/core#> .
@prefix dcat: <http://www.w3.org/ns/dcat#> .
@prefix dce: <http://purl.org/dc/elements/1.1/> .
@prefix dcmitype: <http://purl.org/dc/dcmitype/> .
@prefix dcterms: <http://purl.org/dc/terms/> .
@prefix doap: <http://usefulinc.com/ns/doap#> .
@prefix dbpo: <http://dbpedia.org/ontology/> .
@prefix dqv: <http://www.w3.org/ns/dqv#> .
@prefix earl: <http://www.w3.org/ns/earl#> .
@prefix equiv: <https://ns.inria.fr/kg/equivalence#> .
@prefix fabio: <http://purl.org/spar/fabio/> .
@prefix foaf: <http://xmlns.com/foaf/0.1/> .
@prefix hydra: <http://www.w3.org/ns/hydra/core#> .
@prefix kgi: <http://ns.inria.fr/kg/index#> .
@prefix mf: <http://www.w3.org/2001/sw/DataAccess/tests/test-manifest#> .
@prefix mod: <https://w3id.org/mod#> .
@prefix nie: <http://www.semanticdesktop.org/ontologies/2007/01/19/nie#> .
@prefix owl: <http://www.w3.org/2002/07/owl#> .
@prefix pav: <http://purl.org/pav/> .
@prefix prov: <http://www.w3.org/ns/prov#> .
@prefix rdf: <http://www.w3.org/1999/02/22-rdf-syntax-ns#> .
@prefix rdfs: <http://www.w3.org/2000/01/rdf-schema#> .
@prefix sd: <http://www.w3.org/ns/sparql-service-description#> .
@prefix schema: <http://schema.org/> .
@prefix skos: <http://www.w3.org/2004/02/skos/core#> .
@prefix sto: <https://w3id.org/i40/sto#> .
@prefix vann: <http://purl.org/vocab/vann/> .
@prefix voaf: <http://purl.org/vocommons/voaf#>.
@prefix void: <http://rdfs.org/ns/void#> .
@prefix xhv: <http://www.w3.org/1999/xhtml/vocab#> .
@prefix xsd: <http://www.w3.org/2001/XMLSchema#> .

kgi: rdf:type owl:Ontology, voaf:Vocabulary ;
    rdfs:label "IndeGx vocabulary"@en ;
    dcterms:creator "Pierre Maillot", <https://orcid.org/0000-0002-9814-439X> ;
    dcterms:publisher "INRIA, Team WIMMICS", <https://www.inria.fr/fr/wimmics> ;
    dcterms:title  "IndeGx vocabulary"@en ;
    dcterms:description "Vocabulary extending the manifest and EARL vocabularies for the declaration of the IndeGx framework and the content of an index generated by the IndeGx framework"@en ;
    dcterms:date "2021-10" ;
    pav:lastUpdateOn "2023-06-20" ;
    dcterms:format "RDF" ;
    dcterms:identifier kgi: ;
    voaf:extends void: , mf: , earl: ;
    voaf:generalizes mf: , earl: ;
    owl:imports earl: , mf: .

# Index structuration vocabulary

kgi:IndeGxDataset rdf:type dcat:Dataset, schema:Dataset, void:Dataset, prov:Entity, sd:Dataset ;
    rdfs:label "IndeGx dataset root" ;
    rdfs:isDefinedBy kgi: ;
    rdfs:comment "Root of a dataset generated by IndeGx rules. Default resource used to represent the catalog at the root of the index."@en .

kgi:original rdf:type owl:ObjectProperty ;
    rdfs:label "original"@en ;
    rdfs:comment "Original description graph. Used to link the description of the indexation to the named graph containing the original data directly extracted from an endpoint by IndeGx"@en ;
    rdfs:isDefinedBy kgi: ;
    rdfs:domain prov:Activity ;
    rdfs:range sd:NamedGraph .

kgi:originalResource rdf:type owl:ObjectProperty ;
    rdfs:label "original resource"@en ;
    rdfs:comment "Original description resource. Resource describing a dataset of the endpoint directly extracted from the endpoint."@en ;
    rdfs:isDefinedBy kgi: ;
    rdfs:domain prov:Activity ;
    rdfs:range prov:Entity .

kgi:curated rdf:type owl:ObjectProperty ;
    rdfs:label "curated"@en ;
    rdfs:comment "Generated description graph. Used to link the description of the indexation to the named graph contaning the curated data generated by IndeGx."@en ;
    rdfs:isDefinedBy kgi: ;
    rdfs:domain prov:Activity ;
    rdfs:range sd:NamedGraph .

kgi:curatedResource rdf:type owl:ObjectProperty ;
    rdfs:label "curated resource"@en ;
    rdfs:comment "Generated description resource. Resource generated from the application of generation assets by IndeGx but not directly extracted from an endpoint."@en ;
    rdfs:isDefinedBy kgi: ;
    rdfs:domain prov:Activity ;
    rdfs:range prov:Entity .

kgi:summary rdf:type owl:ObjectProperty ;
    rdfs:label "summary"@en ;
    rdf:comment "Link between the indexation activity of an endpoint and the graph containing the summary of its content."@en ;
    rdfs:domain void:Dataset ;
    rdfs:range sd:NamedGraph .

kgi:trace rdf:type owl:ObjectProperty ;
    rdfs:label "trace"@en ;
    rdfs:comment "Trace report of the metadata generation. EARL report resulting in the execution of a query during the generation of the metadata."@en ;
    rdfs:isDefinedBy kgi: ;
    rdfs:domain prov:Entity ;
    rdfs:range earl:Assertion .

# Generation assets structuration vocabulary

kgi:endpoint rdf:type owl:ObjectProperty ;
    rdfs:label "endpoint"@en ;
    rdfs:comment "Indicates the endpoint to send a test or action."@en ;
    rdfs:domain [ owl:unionOf ( kgi:TestQuery kgi:Action ) ] ;
    rdfs:isDefinedBy kgi: .

kgi:TestQuery rdf:type rdfs:Class ;
    rdfs:label "Query test"@en ;
    rdfs:comment "Test based on a SPARQL query execution. Test the result of the execution of rdf:type query in the manner of rdf:type SHACL shape but allows declaration of constraints on the HTTP response and the result."@en ;
    rdfs:isDefinedBy kgi: ;
    rdfs:subClassOf earl:TestCase .

kgi:onSuccess rdf:type owl:ObjectProperty ;
    rdfs:label "on success"@en ;
    rdfs:comment "List of actions triggered by the success of the test present at the URI of the entry."@en ;
    rdfs:isDefinedBy kgi: ;
    rdfs:domain mf:ManifestEntry ;
    rdfs:range rdf:List .

kgi:onFailure rdf:type owl:ObjectProperty ;
    rdfs:label "on failure"@en ;
    rdfs:comment "List of actions triggered by the failure of the test present at the URI of the entry."@en ;
    rdfs:isDefinedBy kgi: ;
    rdfs:domain mf:ManifestEntry ;
    rdfs:range rdf:List .

kgi:DummyTest rdf:type rdfs:Class ;
    rdfs:label "Placeholder test"@en ;
    rdfs:isDefinedBy kgi: ;
    rdfs:comment "Placeholder class for the test of a rule only affecting the index data. Some tests and actions are 'meta' rules that do not need interaction with remote endpoints. This class is for a test that always succeed for these rules."@en ;
    rdfs:subClassOf earl:TestCase .

kgi:GenerationAsset rdf:type rdfs:Class ;
    rdfs:label "Generation asset."@en ;
    rdfs:isDefinedBy kgi: ;
    rdfs:comment "A generation asset is a test or an action that can be applied by IndeGx to a dataset to generate its description."@en .

kgi:requiredAssets rdf:type owl:ObjectProperty ;
    rdfs:label "required assets"@en ;
    rdfs:comment "Generation assets that must be applied for this generation asset to be applied."@en ;
    rdfs:isDefinedBy kgi: ;
    rdfs:domain kgi:GenerationAsset ;
    rdfs:range rdf:List .

kgi:Action rdf:type owl:Class ;
    rdfs:subClassOf kgi:GenerationAsset ;
    rdfs:label "Action"@en ;
    rdfs:comment "Action object. Must be linked with the property kgi:action to a SPARQL query"@en .

# Modifying existing vocabularies

earl:TestCase rdfs:subClassOf kgi:GenerationAsset .

mf:ManifestEntry rdfs:subClassOf kgi:GenerationAsset .

mf:Manifest rdfs:subClassOf kgi:GenerationAsset .

mf:action rdfs:domain kgi:Action .

# properties to set up the parameters of the indexation

kgi:timeout rdf:type owl:DatatypeProperty ;
    rdfs:label "timeout"@en ;
    rdfs:isDefinedBy kgi: ;
    rdfs:comment "Specify a timeout for a test or action. Queries sent during test and actions may need a specific timeout, generally longer than normal. This property specify the timeout for a test or an action."@en ;
    rdfs:domain kgi:Action ;
    rdfs:range xsd:duration .

kgi:recommendedPagination rdf:type owl:DatatypeProperty ;
    rdfs:label "recommended pagination"@en ;
    rdfs:comment "Recommended size for pagination during retrieval of the results of an action. This indicates the size of the page to use in the actions queries."@en ;
    rdfs:isDefinedBy kgi: ;
    rdfs:domain kgi:Action ;
    rdfs:range xsd:integer .

# Trace of indexation

kgi:sentQuery rdf:type owl:DatatypeProperty ;
    rdfs:comment "Query sent to the server. String representation of the SPARQL query sent to the server after transformation to adapt it to the endpoint, if necessary."@en ;
    rdfs:label "query sent"@en ;
    rdfs:domain earl:TestResult ;
    rdfs:range xsd:string .

# Pseudo-partitions and linksets

kgi:linkset rdf:type owl:ObjectProperty ;
    rdfs:label "linkset"@en ;
    rdfs:comment "Link a dataset description to the linkset that were retrieved during its indexation"@en ;
    rdfs:isDefinedBy kgi: ;
    rdfs:domain void:Dataset ;
    rdfs:range void:Linkset .

kgi:resourceHostname rdf:type owl:ObjectProperty ;
    rdfs:label "resource hostname"@en ;
    rdfs:comment "Hostname of the resources of the dataset. Linked to URIs representing the hostnames of the resources of the dataset."@en ;
    rdfs:isDefinedBy kgi: ;
    rdfs:domain void:Dataset .

kgi:hostnamePartition rdf:type owl:ObjectProperty ;
    rdfs:label "hostname partition"@en ;
    rdfs:comment "Partition of the dataset according to the hostname used the URIs of instances. This property is to be used on the same model as void:classPartition and void:propertyPartition."@en ;
    rdfs:subPropertyOf void:subset ;
    rdfs:isDefinedBy kgi: ;
    rdfs:domain void:Dataset .

kgi:vocabularyPartition rdf:type owl:ObjectProperty ;
    rdfs:label "vocabulary partition"@en ;
    rdfs:comment "Partition of the dataset according to the vocabulary used in triples. This property is to be used on the same model as void:classPartition and void:propertyPartition."@en ;
    rdfs:subPropertyOf void:subset ;
    rdfs:isDefinedBy kgi: ;
    rdfs:domain void:Dataset .

# Other dataset description properties

kgi:availableLiteralDatatypes rdf:type owl:ObjectProperty ;
    rdfs:label "available literal datatypes"@en ;
    rdfs:comment "Used to describe the datatype of the literals in the dataset."@en ;
    rdfs:isDefinedBy kgi: ;
    rdfs:domain void:Dataset ;
    rdfs:range xsd:string .

kgi:resourceHostname rdf:type owl:ObjectProperty ;
    rdfs:label "resource hostname"@en ;
    rdfs:comment "Used to describe the hostname of the resources of the dataset."@en ;
    rdfs:domain void:Dataset ;
    rdfs:isDefinedBy kgi: .

kgi:summary rdf:type owl:ObjectProperty ;
    rdfs:label "summary"@en ;
    rdfs:comment "Link between a dataset and a summary of its content."@en ;
    rdfs:domain void:Dataset ;
    rdfs:range sd:NamedGraph .

kgi:graph rdf:type owl:ObjectProperty ;
    rdfs:label "graph"@en ;
    rdfs:comment "Link between a dataset and a graph containing its content."@en ;
    rdfs:domain void:Dataset ;
    rdfs:range sd:NamedGraph .

# Description of the common elements between datasets

kgi:CommonalityDescription rdf:type rdfs:Class ;
    rdfs:label "Commonality description"@en;
    rdfs:comment "Description of the common elements between datasets. This is designed to give the elements that are common between the descriptions of groups of datasets"@en;
    rdfs:isDefinedBy kgi: .

kgi:dataset rdf:type owl:ObjectProperty ;
    rdfs:label "dataset"@en ;
    rdf:comment "Indicates the datasets whose commonalities are described by an instance of CommonalityDescription."@en ;
    rdfs:domain kgi:CommonalityDescription ;
    rdfs:range void:Dataset ;
    rdfs:isDefinedBy kgi: .

kgi:VocabularyCommonalityDescription rdf:subClassOf kgi:CommonalityDescription ;
    rdfs:label "Common vocabularies"@en ;
    rdfs:comment "Description of the common vocabularies used in different datasets. This shoud be used with kgi:vocabulary and kgi:dataset to list the vocabularies common to a group of datasets"@en ;
    rdfs:isDefinedBy kgi: .

kgi:ClassCommonalityDescription rdf:subClassOf kgi:CommonalityDescription ;
    rdfs:label "Common classes"@en ;
    rdfs:comment "Description of the common classes used in different datasets. This shoud be used with kgi:class and kgi:dataset to list the classes common to a group of datasets"@en ;
    rdfs:isDefinedBy kgi: .

kgi:PropertyCommonalityDescription rdf:subClassOf kgi:CommonalityDescription ;
    rdfs:label "Common properties"@en ;
    rdfs:comment "Description of the common properties used in different datasets. This shoud be used with kgi:property and kgi:dataset to list the properties common to a group of datasets"@en ;
    rdfs:isDefinedBy kgi: .

kgi:DatatypeCommonalityDescription rdf:subClassOf kgi:CommonalityDescription ;
    rdfs:label "Common datatypes"@en ;
    rdfs:comment "Description of the common datatypes used in different datasets. This shoud be used with kgi:datatype and kgi:dataset to list the datatypes common to a group of datasets"@en ;
    rdfs:isDefinedBy kgi: .

kgi:ResourceHostnameCommonalityDescription rdf:subClassOf kgi:CommonalityDescription ;
    rdfs:label "common resource hostnames"@en ;
    rdfs:comment "Description of the common resources hostnames used in different datasets. This shoud be used with kgi:hostname and kgi:dataset to list the resources hostnames common to a group of datasets"@en ;
    rdfs:isDefinedBy kgi: .

kgi:commonVocabularyDescription rdf:type owl:ObjectProperty ;
    rdfs:label "common vocabularies"@en ;
    rdfs:comment "Links a dataset to its vocabulary commonalities descriptions."@en ;
    rdfs:domain void:Dataset ;
    rdfs:range kgi:VocabularyCommonalityDescription ;
    rdfs:isDefinedBy kgi: .

kgi:vocabulary rdf:type owl:ObjectProperty ;
    rdfs:label "vocabulary"@en ;
    rdfs:comment "Indicates the vocabularies that are common to a group of datasets in an instance of CommonalityDescription."@en ;
    rdfs:domain kgi:VocabularyCommonalityDescription ;
    rdfs:isDefinedBy kgi: .

kgi:commonClassDescription rdf:type owl:ObjectProperty ;
    rdfs:label "common classes"@en ;
    rdfs:comment "Links a dataset to its class commonalities descriptions."@en ;
    rdfs:domain void:Dataset ;
    rdfs:range kgi:ClassCommonalityDescription ;
    rdfs:isDefinedBy kgi: .

kgi:class rdf:type owl:ObjectProperty ;
    rdfs:label "class"@en ;
    rdfs:comment "Indicates the classes that are common to a group of datasets in an instance of CommonalityDescription."@en ;
    rdfs:domain kgi:ClassCommonalityDescription ;
    rdfs:isDefinedBy kgi: .

kgi:commonPropertyDescription rdf:type owl:ObjectProperty ;
    rdfs:label "common properties"@en ;
    rdfs:comment "Links a dataset to its property commonalities descriptions."@en ;
    rdfs:domain void:Dataset ;
    rdfs:range kgi:PropertyCommonalityDescription ;
    rdfs:isDefinedBy kgi: .

kgi:property rdf:type owl:ObjectProperty ;
    rdfs:label "property"@en ;
    rdfs:comment "Indicates the properties that are common to a group of datasets in an instance of CommonalityDescription."@en ;
    rdfs:domain kgi:PropertyCommonalityDescription ;
    rdfs:isDefinedBy kgi: .

kgi:commonDatatypeDescription rdf:type owl:ObjectProperty ;
    rdfs:label "common datatypes"@en ;
    rdfs:comment "Links a dataset to its datatype commonalities descriptions."@en ;
    rdfs:domain void:Dataset ;
    rdfs:range kgi:DatatypeCommonalityDescription ;
    rdfs:isDefinedBy kgi: .

kgi:datatype rdf:type owl:ObjectProperty ;
    rdfs:label "datatype"@en ;
    rdfs:comment "Indicates the datatypes that are common to a group of datasets in an instance of CommonalityDescription."@en ;
    rdfs:domain kgi:DatatypeCommonalityDescription ;
    rdfs:isDefinedBy kgi: .

kgi:commonHostnameDescription rdf:type owl:ObjectProperty ;
    rdfs:label "common resource hostnames"@en ;
    rdfs:comment "Links a dataset to its hostname commonalities descriptions."@en ;
    rdfs:domain void:Dataset ;
    rdfs:range kgi:ResourceHostnameCommonalityDescription ;
    rdfs:isDefinedBy kgi: .

kgi:hostname rdf:type owl:ObjectProperty ;
    rdfs:label "resource hostname"@en ;
    rdfs:comment "Indicates the resource hostnames that are common to a group of datasets in an instance of CommonalityDescription."@en ;
    rdfs:comment "To not be confused with kgi:resourceHostname, which lists the resource hostnames appearing in a dataset."@en ;
    rdfs:domain kgi:ResourceHostnameCommonalityDescription ;
    rdfs:isDefinedBy kgi: .

# Annotations

## Availability

kgi:Endpoint rdf:type owl:Class .

kgi:AvailableEndpoint a owl:Class ;
    rdfs:label "Available endpoint"@en ;
    rdfs:comment "Annotation to indicate the availability of an endpoint."@en ;
    rdfs:isDefinedBy kgi: ;
    rdfs:subClassOf kgi:Endpoint .

kgi:UnavailableEndpoint a owl:Class ;
    rdfs:label "Unavailable endpoint"@en ;
    rdfs:comment "Annotation to indicate the unavailability of an endpoint."@en ;
    rdfs:isDefinedBy kgi: ;
    rdfs:subClassOf kgi:Endpoint ;
    owl:complementOf kgi:AvailableEndpoint .

[ rdf:type owl:Axiom ;
  owl:annotatedSource [ rdf:type owl:Restriction ;
                        owl:onProperty [ owl:inverseOf earl:subject
                                       ] ;
                        owl:someValuesFrom owl:Thing ;
                        rdfs:subClassOf kgi:AvailableEndpoint
                      ] ;
  owl:annotatedProperty rdfs:subClassOf ;
  owl:annotatedTarget kgi:AvailableEndpoint ;
  rdfs:comment "SWRL: earl:subject(?a, ?x) ^ earl:result(?a, ?r) ^ earl:outcome(?r, earl:passed) -> kgi:AvailableEndpoint(?x)"
] .

[ rdf:type owl:Axiom ;
  owl:annotatedSource [ rdf:type owl:Restriction ;
                        owl:onProperty [ owl:inverseOf earl:subject
                                       ] ;
                        owl:someValuesFrom owl:Thing ;
                        rdfs:subClassOf kgi:UnavailableEndpoint
                      ] ;
  owl:annotatedProperty rdfs:subClassOf ;
  owl:annotatedTarget kgi:UnavailableEndpoint ;
  rdfs:comment "SWRL: earl:subject(?a, ?x) ^ earl:result(?a, ?r) ^ earl:outcome(?r, earl:failed) -> kgi:UnavailableEndpoint(?x)"
] .

## Equivalences

:Dataset a equiv:AllEquivalentClasses ; 
    owl:members (
        schema:Dataset 
        dcmitype:Dataset 
        void:Dataset
        dcat:Dataset
        sd:Dataset 
    ) .

:identifier a equiv:AllEquivalentProperties ; 
    owl:members (
        dcterms:identifier
        skos:notation
        adms:identifier
        schema:identifier 
    ) .

:title a equiv:AllEquivalentProperties ; 
    owl:members (
        dcterms:title
        dce:title
        schema:name
        foaf:name
        rdfs:label
        skos:prefLabel
        cc:attributionName
    ) .

:description a equiv:AllEquivalentProperties ; 
    owl:members (
        dcterms:description
        dce:description
        schema:description
        owl:comment
        rdf:comment
        skos:note 
    ) .

:creator a equiv:AllEquivalentProperties ; 
    owl:members (
        dcterms:creator
        schema:creator
        schema:author
        foaf:maker
        dce:creator
        pav:authoredBy
        pav:createdBy 
    ) .

:contributor a equiv:AllEquivalentProperties ; 
    owl:members (
        schema:editor
        schema:contributor
        dcterms:contributor
        dce:contributor
        pav:contributedBy 
    ) .

:publicationDate a equiv:AllEquivalentProperties ; 
    owl:members (
        dcterms:issued
        dcterms:available
        schema:datePublished
        schema:sdDatePublished
        pav:authoredOn
        pav:createdOn 
    ) .

:publisher a equiv:AllEquivalentProperties ; 
    owl:members (
        dcterms:publisher
        dce:publisher
        schema:publisher
        schema:sdPublisher
        pav:providedBy 
    ) .

:creationDate a equiv:AllEquivalentProperties ; 
    owl:members (
        schema:dateCreated
        dcterms:created
        pav:createdOn
        prov:generatedAtTime 
    ) .

:creationLocation a equiv:AllEquivalentProperties ; 
    owl:members (
        schema:locationCreated
        pav:createdAt
    ) .

:creationMethod a equiv:AllEquivalentProperties ; 
    owl:members (
        pav:createdWith
        pav:retrievedBy
        pav:importedBy 
    ) .

:modificationDate a equiv:AllEquivalentProperties ; 
    owl:members (
        schema:dateModified
        dcterms:modified
        pav:lastUpdateOn
        pav:contributedOn 
    ) .

:endAvailability a equiv:AllEquivalentProperties ; 
    owl:members (
        schema:expires
        prov:invalidatedAtTime 
    ) .

:endValidity a equiv:AllEquivalentProperties ; 
    owl:members (
        dcterms:valid
        schema:expires
    ) .

:vocabulary a equiv:AllEquivalentProperties ; 
    owl:members (
        void:vocabulary
        dcterms:conformsTo
    ) .

:theme a equiv:AllEquivalentProperties ; 
    owl:members (
        dcat:theme
        schema:about
        dcterms:subject
        foaf:topic
        foaf:primaryTopic
        skos:subject
    ) .

:keyword a equiv:AllEquivalentProperties ; 
    owl:members (
        schema:keywords
        dcat:keyword
    ) .

:metaGraph a equiv:AllEquivalentProperties ; 
    owl:members (
        schema:image
        foaf:depiction
    ) .

:sparqlEndpoint a equiv:AllEquivalentProperties ; 
    owl:members (
        void:sparqlEndpoint
        schema:contentURL
    ) .

:serviceSparqlEndpoint a equiv:AllEquivalentProperties ; 
    owl:members (
        dcat:endpointURL
        sd:endpoint
    ) .

:distribution a equiv:AllEquivalentProperties ; 
    owl:members (
        dcat:distribution
        schema:distribution
    ) .

:RESTAPI a equiv:AllEquivalentProperties ; 
    owl:members (
        schema:mainEntityOfPage
        fabio:ApplicationProgrammingInterface
    ) .

:format a equiv:AllEquivalentProperties ; 
    owl:members (
        dce:format
        dcterms:format
        schema:encodingFormat
    ) .

:version a equiv:AllEquivalentProperties ; 
    owl:members (
        dcat:version
        pav:version
        dcterms:hasVersion
        pav:hasCurrentVersion
        schema:version
    ) .

:versionNotes a equiv:AllEquivalentProperties ; 
    owl:members (
        adms:versionNotes
        owl:versionInfo
    ) .

:otherVersion a equiv:AllEquivalentProperties ; 
    owl:members (
        dcterms:isVersionOf
        pav:previousVersion
        owl:priorVersion
    ) .

:language a equiv:AllEquivalentProperties ; 
    owl:members (
        dcterms:language
        dce:language
        schema:inLanguage
    ) .

:identifier a equiv:AllEquivalentProperties ; 
    owl:members (
        schema:identifier
        dce:identifier
        dcterms:identifier
        adms:identifier
    ) .

:alternativeTitle a equiv:AllEquivalentProperties ; 
    owl:members (
        dcterms:alternative
        schema:alternateName
        skos:altLabel
    ) .

:acronym a equiv:AllEquivalentProperties ; 
    owl:members (
        schema:termCode
        <http://qudt.org/schema/qudt/acronym>
    ) .

:homepage a equiv:AllEquivalentProperties ; 
    owl:members (
        foaf:homepage
        schema:url
        dcat:landingPage
    ) .

:otherPages a equiv:AllEquivalentProperties ; 
    owl:members (
        schema:relatedLink
        rdfs:seeAlso
    ) .

:publicationReferences a equiv:AllEquivalentProperties ; 
    owl:members (
        schema:publication
        dcterms:references
    ) .

:linkedresources a equiv:AllEquivalentProperties ; 
    owl:members (
        dcterms:relation
        void:target
    ) .

:example a equiv:AllEquivalentProperties ; 
    owl:members (
        void:exampleResource
        schema:workExample
        skos:example
    ) .

:license a equiv:AllEquivalentProperties ; 
    owl:members (
        schema:license
        dcterms:license
        doap:license
        dbpo:license
        cc:license
        xhv:license
        sto:license
        nie:license
    ) .

:qualityAnnotation a equiv:AllEquivalentProperties ; 
    owl:members (
        schema:review
        dqv:hasQualityAnnotation
    ) .

:accessStatement a equiv:AllEquivalentProperties ; 
    owl:members (
        dce:rights
        dcterms:rights 
        dcterms:accessRights
    ) .

:source a equiv:AllEquivalentProperties ; 
    owl:members (
        schema:isBasedOn
        dcterms:source
        dce:source
        dcterms:provenance
        prov:hadPrimarySource
        prov:wasDerivedFrom
        pav:derivedFrom
        pav:importedFrom
        pav:retrievedFrom
    ) .

:spatial a equiv:AllEquivalentProperties ; 
    owl:members (
        schema:spatialCoverage
        dcterms:spatial
    ) .

:temporal a equiv:AllEquivalentProperties ; 
    owl:members (
        schema:temporalCoverage
        dcterms:temporal
    ) .

mod:URI equiv:impliedProperty :identifier .